@prefix dc: <http://purl.org/dc/elements/1.1/> .
@prefix dcterms: <http://purl.org/dc/terms/> .
@prefix foaf: <http://xmlns.com/foaf/0.1/> .
@prefix ns1: <http://dbkwik.webdatacommons.org/marvelcinematicuniverse.wikia.com/property/> .
@prefix ns2: <http://dbkwik.webdatacommons.org/marvelcinematicuniverse.wikia.com/property/affiliation(s)> .
@prefix ns3: <http://dbkwik.webdatacommons.org/ontology/> .
@prefix ns6: <http://dbkwik.webdatacommons.org/marvelcinematicuniverse.wikia.com/property/%23> .
@prefix owl: <http://www.w3.org/2002/07/owl#> .
@prefix rdf: <http://www.w3.org/1999/02/22-rdf-syntax-ns#> .
@prefix rdfs: <http://www.w3.org/2000/01/rdf-schema#> .
@prefix skos: <http://www.w3.org/2004/02/skos/core#> .
@prefix xsd: <http://www.w3.org/2001/XMLSchema#> .

<http://dbkwik.webdatacommons.org/marvelcinematicuniverse.wikia.com/> a owl:Ontology .

ns6: a rdf:Property ;
    rdfs:label "#"@en .

ns1:actor a rdf:Property ;
    rdfs:label "actor"@en .

ns1:affiliation a rdf:Property ;
    rdfs:label "affiliation"@en .

ns2: a rdf:Property ;
    rdfs:label "affiliation(s)"@en .

ns1:after a rdf:Property ;
    rdfs:label "After"@en .

ns1:age a rdf:Property ;
    rdfs:label "age"@en .

ns1:alias a rdf:Property ;
    rdfs:label "alias"@en .

ns1:allies a rdf:Property ;
    rdfs:label "allies"@en .

ns1:appearances a rdf:Property ;
    rdfs:label "appearances"@en .

ns1:artista a rdf:Property ;
    rdfs:label "artista"@en .

ns1:artists a rdf:Property ;
    rdfs:label "artists"@en .

ns1:author a rdf:Property ;
    rdfs:label "author"@en .

ns1:battles a rdf:Property ;
    rdfs:label "battles"@en .

ns1:before a rdf:Property ;
    rdfs:label "Before"@en .

ns1:begin a rdf:Property ;
    rdfs:label "begin"@en .

ns1:body a rdf:Property ;
    rdfs:label "body"@en .

ns1:boxoffice a rdf:Property ;
    rdfs:label "boxoffice"@en .

ns1:builder a rdf:Property ;
    rdfs:label "builder"@en .

ns1:casualties a rdf:Property ;
    rdfs:label "casualties"@en .

ns1:channel a rdf:Property ;
    rdfs:label "channel"@en .

ns1:charaacter a rdf:Property ;
    rdfs:label "charaacter"@en .

ns1:character a rdf:Property ;
    rdfs:label "character"@en .

ns1:citizenship a rdf:Property ;
    rdfs:label "citizenship"@en .

ns1:clearance a rdf:Property ;
    rdfs:label "clearance"@en .

ns1:coat a rdf:Property ;
    rdfs:label "coat"@en .

ns1:combatants a rdf:Property ;
    rdfs:label "combatants"@en .

ns1:comic a rdf:Property ;
    rdfs:label "comic"@en .

ns1:commanders a rdf:Property ;
    rdfs:label "commanders"@en .

ns1:composer a rdf:Property ;
    rdfs:label "composer"@en .

ns1:conc a rdf:Property ;
    rdfs:label "conc"@en .

ns1:continent a rdf:Property ;
    rdfs:label "continent"@en .

ns1:contribution a rdf:Property ;
    rdfs:label "contribution"@en .

ns1:contributors a rdf:Property ;
    rdfs:label "contributors"@en .

ns1:cover a rdf:Property ;
    rdfs:label "cover"@en .

ns1:creator a rdf:Property ;
    rdfs:label "creator"@en .

ns1:current a rdf:Property ;
    rdfs:label "Current"@en .

ns1:date a rdf:Property ;
    rdfs:label "date"@en .

ns1:dates a rdf:Property ;
    rdfs:label "dates"@en .

ns1:defender a rdf:Property ;
    rdfs:label "defender"@en .

ns1:developers a rdf:Property ;
    rdfs:label "developers"@en .

ns1:directed a rdf:Property ;
    rdfs:label "directed"@en .

ns1:director a rdf:Property ;
    rdfs:label "director"@en .

ns1:directors a rdf:Property ;
    rdfs:label "directors"@en .

ns1:dob a rdf:Property ;
    rdfs:label "DOB"@en .

ns1:documentary a rdf:Property ;
    rdfs:label "documentary"@en .

ns1:dod a rdf:Property ;
    rdfs:label "DOD"@en .

ns1:duration a rdf:Property ;
    rdfs:label "duration"@en .

ns1:eason a rdf:Property ;
    rdfs:label "eason"@en .

ns1:editorinchief a rdf:Property ;
    rdfs:label "editorinchief"@en .

ns1:end a rdf:Property ;
    rdfs:label "end"@en .

ns1:episodes a rdf:Property ;
    rdfs:label "episodes"@en .

ns1:executor a rdf:Property ;
    rdfs:label "executor"@en .

ns1:film a rdf:Property ;
    rdfs:label "film"@en .

ns1:films a rdf:Property ;
    rdfs:label "films"@en .

ns1:first a rdf:Property ;
    rdfs:label "first"@en .

ns1:firstAired a rdf:Property ;
    rdfs:label "first aired"@en .

ns1:flag a rdf:Property ;
    rdfs:label "flag"@en .

ns1:followedBy a rdf:Property ;
    rdfs:label "followed by"@en .

ns1:formerLeader a rdf:Property ;
    rdfs:label "former leader"@en .

ns1:formerinhabitants a rdf:Property ;
    rdfs:label "formerinhabitants"@en .

ns1:formerleaders a rdf:Property ;
    rdfs:label "formerleaders"@en .

ns1:formermembers a rdf:Property ;
    rdfs:label "formermembers"@en .

ns1:formernotable a rdf:Property ;
    rdfs:label "formernotable"@en .

ns1:founder a rdf:Property ;
    rdfs:label "founder"@en .

ns1:game a rdf:Property ;
    rdfs:label "game"@en .

ns1:gender a rdf:Property ;
    rdfs:label "gender"@en .

ns1:heading a rdf:Property ;
    rdfs:label "heading"@en .

ns1:headquarters a rdf:Property ;
    rdfs:label "headquarters"@en .

ns1:height a rdf:Property ;
    rdfs:label "height"@en .

ns1:homeplanet a rdf:Property ;
    rdfs:label "homeplanet"@en .

ns1:idno a rdf:Property ;
    rdfs:label "IDno"@en .

ns1:imagebg a rdf:Property ;
    rdfs:label "imageBG"@en .

ns1:imagecaption a rdf:Property ;
    rdfs:label "imagecaption"@en .

ns1:inhabitants a rdf:Property ;
    rdfs:label "inhabitants"@en .

ns1:interest a rdf:Property ;
    rdfs:label "interest"@en .

ns1:isbn a rdf:Property ;
    rdfs:label "isbn"@en .

ns1:last a rdf:Property ;
    rdfs:label "last"@en .

ns1:leader a rdf:Property ;
    rdfs:label "leader"@en .

ns1:link a rdf:Property ;
    rdfs:label "link"@en .

ns1:location a rdf:Property ;
    rdfs:label "location"@en .

ns1:locations a rdf:Property ;
    rdfs:label "locations"@en .

ns1:made a rdf:Property ;
    rdfs:label "made"@en .

ns1:media a rdf:Property ;
    rdfs:label "media"@en .

ns1:members a rdf:Property ;
    rdfs:label "members"@en .

ns1:movie a rdf:Property ;
    rdfs:label "movie"@en .

ns1:movies a rdf:Property ;
    rdfs:label "movies"@en .

ns1:name a rdf:Property ;
    rdfs:label "name"@en .

ns1:namesake a rdf:Property ;
    rdfs:label "namesake"@en .

ns1:next a rdf:Property ;
    rdfs:label "next"@en .

ns1:nonlinktext a rdf:Property ;
    rdfs:label "nonlinktext"@en .

ns1:notable a rdf:Property ;
    rdfs:label "notable"@en .

ns1:notableformer a rdf:Property ;
    rdfs:label "notableformer"@en .

ns1:oneShot a rdf:Property ;
    rdfs:label "one-shot"@en .

ns1:oneshot a rdf:Property ;
    rdfs:label "oneshot"@en .

ns1:otherNames a rdf:Property ;
    rdfs:label "other names"@en .

ns1:owner a rdf:Property ;
    rdfs:label "owner"@en .

ns1:owners a rdf:Property ;
    rdfs:label "owners"@en .

ns1:pages a rdf:Property ;
    rdfs:label "pages"@en .

ns1:participants a rdf:Property ;
    rdfs:label "participants"@en .

ns1:passengers a rdf:Property ;
    rdfs:label "passengers"@en .

ns1:penciled a rdf:Property ;
    rdfs:label "penciled"@en .

ns1:performer a rdf:Property ;
    rdfs:label "performer"@en .

ns1:pilot a rdf:Property ;
    rdfs:label "pilot"@en .

ns1:place a rdf:Property ;
    rdfs:label "place"@en .

ns1:planet a rdf:Property ;
    rdfs:label "planet"@en .

ns1:planner a rdf:Property ;
    rdfs:label "planner"@en .

ns1:population a rdf:Property ;
    rdfs:label "population"@en .

ns1:precededBy a rdf:Property ;
    rdfs:label "preceded by"@en .

ns1:prev a rdf:Property ;
    rdfs:label "prev"@en .

ns1:previous a rdf:Property ;
    rdfs:label "previous"@en .

ns1:prisoners a rdf:Property ;
    rdfs:label "prisoners"@en .

ns1:produced a rdf:Property ;
    rdfs:label "produced"@en .

ns1:producer a rdf:Property ;
    rdfs:label "producer"@en .

ns1:publisher a rdf:Property ;
    rdfs:label "publisher"@en .

ns1:realName a rdf:Property ;
    rdfs:label "real name"@en .

ns1:release a rdf:Property ;
    rdfs:label "release"@en .

ns1:released a rdf:Property ;
    rdfs:label "released"@en .

ns1:result a rdf:Property ;
    rdfs:label "result"@en .

ns1:runntime a rdf:Property ;
    rdfs:label "runntime"@en .

ns1:runtime a rdf:Property ;
    rdfs:label "runtime"@en .

ns1:seal a rdf:Property ;
    rdfs:label "seal"@en .

ns1:season a rdf:Property ;
    rdfs:label "season"@en .

ns1:series a rdf:Property ;
    rdfs:label "series"@en .

ns1:showrunners a rdf:Property ;
    rdfs:label "showrunners"@en .

ns1:side a rdf:Property ;
    rdfs:label "side"@en .

ns1:species a rdf:Property ;
    rdfs:label "species"@en .

ns1:srclink a rdf:Property ;
    rdfs:label "srclink"@en .

ns1:status a rdf:Property ;
    rdfs:label "status"@en .

ns1:succeeded a rdf:Property ;
    rdfs:label "succeeded"@en .

ns1:succeededBy a rdf:Property ;
    rdfs:label "succeeded by"@en .

ns1:system a rdf:Property ;
    rdfs:label "system"@en .

ns1:target a rdf:Property ;
    rdfs:label "target"@en .

ns1:team a rdf:Property ;
    rdfs:label "team"@en .

ns1:text a rdf:Property ;
    rdfs:label "text"@en .

ns1:title a rdf:Property ;
    rdfs:label "title"@en .

ns1:tvSeries a rdf:Property ;
    rdfs:label "tv series"@en .

ns1:type a rdf:Property ;
    rdfs:label "type"@en .

ns1:users a rdf:Property ;
    rdfs:label "users"@en .

ns1:vehicles a rdf:Property ;
    rdfs:label "vehicles"@en .

ns1:voiceActor a rdf:Property ;
    rdfs:label "voice actor"@en .

ns1:war a rdf:Property ;
    rdfs:label "war"@en .

ns1:weapons a rdf:Property ;
    rdfs:label "weapons"@en .

ns1:webSeries a rdf:Property ;
    rdfs:label "web series"@en .

ns1:writer a rdf:Property ;
    rdfs:label "writer"@en .

ns1:writers a rdf:Property ;
    rdfs:label "writers"@en .

ns1:wrote a rdf:Property ;
    rdfs:label "wrote"@en .

ns1:years a rdf:Property ;
    rdfs:label "years"@en .

<http://dbkwik.webdatacommons.org/marvelcinematicuniverse.wikia.com/resource/%5BAKA_Start_at_the_Beginning> ns3:wikiPageWikiLinkText "[AKA Start at the Beginning"^^rdf:langString .

<http://dbkwik.webdatacommons.org/marvelcinematicuniverse.wikia.com/resource/%5BVladimir_Ranskahov> ns3:wikiPageWikiLinkText "Ranskahov"^^rdf:langString .

<http://dbkwik.webdatacommons.org/marvelcinematicuniverse.wikia.com/resource/...And_Finally:_Black_Bolt/Gallery> a owl:Thing ;
    rdfs:label "...And Finally: Black Bolt/Gallery"^^rdf:langString ;
    ns3:abstract """A gallery of images of, or related to, the Inhumans episode ...And Finally: Black Bolt.

"""@en ;
    ns3:thumbnail <http://marvelcinematicuniverse.wikia.com/wiki/Special:FilePath/...And_Finally_Black_Bolt_photo.jpg?width=300>,
        <http://marvelcinematicuniverse.wikia.com/wiki/Special:FilePath/And_Finally_Black_Bolt_1.jpg?width=300> ;
    ns3:wikiPageWikiLink <http://dbkwik.webdatacommons.org/marvelcinematicuniverse.wikia.com/resource/...And_Finally:_Black_Bolt>,
        <http://dbkwik.webdatacommons.org/marvelcinematicuniverse.wikia.com/resource/Category:Galleries> ;
    dcterms:subject <http://dbkwik.webdatacommons.org/marvelcinematicuniverse.wikia.com/resource/Category:Galleries> ;
    rdfs:comment """A gallery of images of, or related to, the Inhumans episode ...And Finally: Black Bolt.

"""@en ;
    skos:altLabel "...And Finally: Black Bolt/Gallery"^^rdf:langString ;
    foaf:depiction <http://marvelcinematicuniverse.wikia.com/wiki/Special:FilePath/...And_Finally_Black_Bolt_photo.jpg>,
        <http://marvelcinematicuniverse.wikia.com/wiki/Special:FilePath/And_Finally_Black_Bolt_1.jpg> .

<http://dbkwik.webdatacommons.org/marvelcinematicuniverse.wikia.com/resource/.380> a <http://dbkwik.webdatacommons.org/marvelcinematicuniverse.wikia.com/class/episode> ;
    rdfs:label ".380"^^rdf:langString ;
    ns1:director <http://dbkwik.webdatacommons.org/marvelcinematicuniverse.wikia.com/resource/Stephen_Surjik> ;
    ns1:firstAired "2016-03-18"^^xsd:date ;
    ns1:next <http://dbkwik.webdatacommons.org/marvelcinematicuniverse.wikia.com/resource/The_Dark_at_the_End_of_the_Tunnel> ;
    ns1:previous <http://dbkwik.webdatacommons.org/marvelcinematicuniverse.wikia.com/resource/The_Man_in_the_Box> ;
    ns1:season 2 ;
    ns1:writer <http://dbkwik.webdatacommons.org/marvelcinematicuniverse.wikia.com/resource/Mark_Verheiden> ;
    ns3:abstract """.380 is the eleventh episode of the second season of the Netflix exclusive television series Daredevil.

"""@en ;
    ns3:thumbnail <http://marvelcinematicuniverse.wikia.com/wiki/Special:FilePath/BMahoneyQuestioningKPage-S2E11.jpg?width=300>,
        <http://marvelcinematicuniverse.wikia.com/wiki/Special:FilePath/Daredevil-Episode-211-3-03212016.jpg?width=300> ;
    ns3:wikiPageExternalLink <http://marvel.wikia.com/wiki/Main_Page> ;
    ns3:wikiPageWikiLink <http://dbkwik.webdatacommons.org/marvelcinematicuniverse.wikia.com/resource/15th_Precinct_Police_Station> ;
    dcterms:subject <http://dbkwik.webdatacommons.org/marvelcinematicuniverse.wikia.com/resource/Category:Daredevil_(TV_series)_Episodes> ;
    rdfs:comment """.380 is the eleventh episode of the second season of the Netflix exclusive television series Daredevil.

"""@en ;
    skos:altLabel ".380"^^rdf:langString ;
    foaf:depiction <http://marvelcinematicuniverse.wikia.com/wiki/Special:FilePath/0-8-4_episode.png> .

<http://dbkwik.webdatacommons.org/marvelcinematicuniverse.wikia.com/resource/.380/Gallery> a owl:Thing ;
    rdfs:label ".380/Gallery"^^rdf:langString ;
    ns3:abstract """A gallery of images from, or related to, the Daredevil episode .380.

"""@en ;
    dcterms:subject <http://dbkwik.webdatacommons.org/marvelcinematicuniverse.wikia.com/resource/Category:Daredevil_(TV_series)>,
        <http://dbkwik.webdatacommons.org/marvelcinematicuniverse.wikia.com/resource/Category:Galleries> ;
    rdfs:comment """A gallery of images from, or related to, the Daredevil episode .380.

"""@en ;
    skos:altLabel ".380/Gallery"^^rdf:langString .

<http://dbkwik.webdatacommons.org/marvelcinematicuniverse.wikia.com/resource/0-8-4_(disambiguation)> a <http://dbkwik.webdatacommons.org/marvelcinematicuniverse.wikia.com/class/disambig> ;
    rdfs:label "0-8-4 (disambiguation)"^^rdf:langString ;
    ns3:wikiPageDisambiguates <http://dbkwik.webdatacommons.org/marvelcinematicuniverse.wikia.com/resource/0-8-4_(Code)>,
        <http://dbkwik.webdatacommons.org/marvelcinematicuniverse.wikia.com/resource/0-8-4_(episode)> .

<http://dbkwik.webdatacommons.org/marvelcinematicuniverse.wikia.com/resource/0-8-4_(episode)/Gallery> a owl:Thing ;
    rdfs:label "0-8-4 (episode)/Gallery"^^rdf:langString ;
    rdfs:comment """A gallery of images from, or related to, the Agents of S.H.I.E.L.D. episode 0-8-4.

"""@en .

<http://dbkwik.webdatacommons.org/marvelcinematicuniverse.wikia.com/resource/107th_Infantry_Regiment> a <http://dbkwik.webdatacommons.org/marvelcinematicuniverse.wikia.com/class/organization> ;
    rdfs:label "107th Infantry Regiment"^^rdf:langString ;
    ns1:formermembers <http://dbkwik.webdatacommons.org/marvelcinematicuniverse.wikia.com/resource/Joseph_Rogers>,
        <http://dbkwik.webdatacommons.org/marvelcinematicuniverse.wikia.com/resource/Winter_Soldier> ;
    ns1:headquarters <http://dbkwik.webdatacommons.org/marvelcinematicuniverse.wikia.com/resource/New_York> ;
    ns1:leader <http://dbkwik.webdatacommons.org/marvelcinematicuniverse.wikia.com/resource/Chester_Phillips> ;
    ns1:locations <http://dbkwik.webdatacommons.org/marvelcinematicuniverse.wikia.com/resource/Europe>,
        <http://dbkwik.webdatacommons.org/marvelcinematicuniverse.wikia.com/resource/United_States_of_America> ;
    ns1:members <http://dbkwik.webdatacommons.org/marvelcinematicuniverse.wikia.com/resource/Gilmore_Hodge> ;
    ns1:movie <http://dbkwik.webdatacommons.org/marvelcinematicuniverse.wikia.com/resource/Captain_America:_The_First_Avenger> ;
    ns1:tvSeries <http://dbkwik.webdatacommons.org/marvelcinematicuniverse.wikia.com/resource/Agent_Carter_(TV_series)>,
        <http://dbkwik.webdatacommons.org/marvelcinematicuniverse.wikia.com/resource/The_Iron_Ceiling> ;
    rdfs:comment """The 107th Infantry Regiment was a regiment of the New York Army National Guard. They fought for the United States Army for periods of time throughout the Twentieth Century, most notably during the Great War and World War II. They served with distinction, being instrumental in the destruction of Nazi Germany and the HYDRA threat.

"""@en .

<http://dbkwik.webdatacommons.org/marvelcinematicuniverse.wikia.com/resource/10cc> a <http://dbkwik.webdatacommons.org/marvelcinematicuniverse.wikia.com/class/music> ;
    rdfs:label "10cc"^^rdf:langString ;
    ns3:wikiPageExternalLink <http://play.spotify.com>,
        <https://play.spotify.com/artist/6i6WlGzQtXtz7GcC5H5st5/> ;
    rdfs:comment """10cc are an English art rock band.
Their song "I'm Not in Love" is featured in Guardians of the Galaxy.

"""@en .

<http://dbkwik.webdatacommons.org/marvelcinematicuniverse.wikia.com/resource/10th_Precinct_Police_Station> a <http://dbkwik.webdatacommons.org/marvelcinematicuniverse.wikia.com/class/location> ;
    rdfs:label "10th Precinct Police Station"^^rdf:langString ;
    ns1:continent <http://dbkwik.webdatacommons.org/marvelcinematicuniverse.wikia.com/resource/North_America> ;
    ns1:location <http://dbkwik.webdatacommons.org/marvelcinematicuniverse.wikia.com/resource/New_York>,
        <http://dbkwik.webdatacommons.org/marvelcinematicuniverse.wikia.com/resource/New_York_City> ;
    ns1:tvSeries <http://dbkwik.webdatacommons.org/marvelcinematicuniverse.wikia.com/resource/Front_Toward_Enemy>,
        <http://dbkwik.webdatacommons.org/marvelcinematicuniverse.wikia.com/resource/The_Punisher> ;
    rdfs:comment """The 10th Precinct Police Station is one of the police stations based in New York City.

"""@en .

<http://dbkwik.webdatacommons.org/marvelcinematicuniverse.wikia.com/resource/1900s> a <http://dbkwik.webdatacommons.org/marvelcinematicuniverse.wikia.com/class/timeline> ;
    rdfs:label "1900s"^^rdf:langString ;
    ns1:before <http://dbkwik.webdatacommons.org/marvelcinematicuniverse.wikia.com/resource/Before_20th_Century> ;
    rdfs:comment """This is a timeline of events that occurred during the 1900s.

"""@en .

<http://dbkwik.webdatacommons.org/marvelcinematicuniverse.wikia.com/resource/1910s> a <http://dbkwik.webdatacommons.org/marvelcinematicuniverse.wikia.com/class/timeline> ;
    rdfs:label "1910s"^^rdf:langString ;
    rdfs:comment """This is a timeline of events that occurred during the 1910s.

"""@en .

<http://dbkwik.webdatacommons.org/marvelcinematicuniverse.wikia.com/resource/1920s> a <http://dbkwik.webdatacommons.org/marvelcinematicuniverse.wikia.com/class/timeline> ;
    rdfs:label "1920s"^^rdf:langString ;
    rdfs:comment """This is a timeline of events that occurred during the 1920s.

"""@en .

<http://dbkwik.webdatacommons.org/marvelcinematicuniverse.wikia.com/resource/1930s> a <http://dbkwik.webdatacommons.org/marvelcinematicuniverse.wikia.com/class/timeline> ;
    rdfs:label "1930s"^^rdf:langString ;
    rdfs:comment """This is a timeline of events that occurred during the 1930s.

"""@en .

<http://dbkwik.webdatacommons.org/marvelcinematicuniverse.wikia.com/resource/1960s> a <http://dbkwik.webdatacommons.org/marvelcinematicuniverse.wikia.com/class/timeline> ;
    rdfs:label "1960s"^^rdf:langString ;
    rdfs:comment """This is a timeline of events that occurred during the 1960s.

"""@en .

<http://dbkwik.webdatacommons.org/marvelcinematicuniverse.wikia.com/resource/1970s> a <http://dbkwik.webdatacommons.org/marvelcinematicuniverse.wikia.com/class/timeline> ;
    rdfs:label "1970s"^^rdf:langString ;
    rdfs:comment """This is a timeline of events that occurred during the 1970s.

"""@en .

<http://dbkwik.webdatacommons.org/marvelcinematicuniverse.wikia.com/resource/2018> rdfs:label "2018"^^rdf:langString ;
    ns1:after <http://dbkwik.webdatacommons.org/marvelcinematicuniverse.wikia.com/resource/2091> ;
    rdfs:comment """This is a timeline of events that occurred during 2018.

"""@en .

<http://dbkwik.webdatacommons.org/marvelcinematicuniverse.wikia.com/resource/21_the_Producer> a <http://dbkwik.webdatacommons.org/marvelcinematicuniverse.wikia.com/class/music> ;
    rdfs:label "21 the Producer"^^rdf:langString ;
    rdfs:comment """21 the Producer is a musician and songwriter.
His collaboration with Xzibit, Demrick and Sylvester Jordan Jr., "Finders Keepers", is featured in Captain America: Civil War.
His song "Missionary" is featured in the Luke Cage episode Moment of Truth.

"""@en .

<http://dbkwik.webdatacommons.org/marvelcinematicuniverse.wikia.com/resource/29th_Precinct_Police_Station> a <http://dbkwik.webdatacommons.org/marvelcinematicuniverse.wikia.com/class/location> ;
    rdfs:label "29th Precinct Police Station"^^rdf:langString ;
    ns1:continent <http://dbkwik.webdatacommons.org/marvelcinematicuniverse.wikia.com/resource/North_America> ;
    ns1:location <http://dbkwik.webdatacommons.org/marvelcinematicuniverse.wikia.com/resource/New_York>,
        <http://dbkwik.webdatacommons.org/marvelcinematicuniverse.wikia.com/resource/New_York_City> ;
    rdfs:comment """The 29th Precinct Police Station is one of the major police stations based in Harlem, New York City.

"""@en .

<http://dbkwik.webdatacommons.org/marvelcinematicuniverse.wikia.com/resource/2_Chainz> a <http://dbkwik.webdatacommons.org/marvelcinematicuniverse.wikia.com/class/music> ;
    rdfs:label "2 Chainz"^^rdf:langString ;
    rdfs:comment """Tauheed Epps, known professionally as 2 Chainz, is an American rapper.
His collaboration with ScHoolboy Q and Saudi, "X", is featured on Black Panther: The Album.

"""@en .

<http://dbkwik.webdatacommons.org/marvelcinematicuniverse.wikia.com/resource/3OH!3> a <http://dbkwik.webdatacommons.org/marvelcinematicuniverse.wikia.com/class/music> ;
    rdfs:label "3OH!3"^^rdf:langString ;
    rdfs:comment """3OH!3 are an American electropop duo.
Their song "Bad Guy" is featured on Iron Man 3: Heroes Fall – Music Inspired by the Motion Picture, an album with music inspired by (but not used in) Iron Man 3.

"""@en .

<http://dbkwik.webdatacommons.org/marvelcinematicuniverse.wikia.com/resource/3_AM> a <http://dbkwik.webdatacommons.org/marvelcinematicuniverse.wikia.com/class/episode> ;
    rdfs:label "3 AM"^^rdf:langString ;
    ns1:director <http://dbkwik.webdatacommons.org/marvelcinematicuniverse.wikia.com/resource/Tom_Shankland> ;
    ns1:firstAired "2017-11-17"^^xsd:date ;
    ns1:next <http://dbkwik.webdatacommons.org/marvelcinematicuniverse.wikia.com/resource/Two_Dead_Men> ;
    ns1:season 1 ;
    rdfs:comment """3 AM is the first episode of the first season of the television series The Punisher.

"""@en .

<http://dbkwik.webdatacommons.org/marvelcinematicuniverse.wikia.com/resource/3_AM/Gallery> a owl:Thing ;
    rdfs:label "3 AM/Gallery"^^rdf:langString ;
    rdfs:comment """A gallery of images from, or related to, the The Punisher episode 3 AM.

"""@en .

<http://dbkwik.webdatacommons.org/marvelcinematicuniverse.wikia.com/resource/4,722_Hours> a <http://dbkwik.webdatacommons.org/marvelcinematicuniverse.wikia.com/class/episode> ;
    rdfs:label "4,722 Hours"^^rdf:langString ;
    ns1:director <http://dbkwik.webdatacommons.org/marvelcinematicuniverse.wikia.com/resource/Jesse_Bochco> ;
    ns1:firstAired "2015-10-27"^^xsd:date ;
    ns1:next <http://dbkwik.webdatacommons.org/marvelcinematicuniverse.wikia.com/resource/Among_Us_Hide...> ;
    ns1:previous <http://dbkwik.webdatacommons.org/marvelcinematicuniverse.wikia.com/resource/Devils_You_Know> ;
    ns1:season 3 ;
    rdfs:comment """4,722 Hours is the fifth episode of the third season of the television series Agents of S.H.I.E.L.D. and the forty-ninth episode overall.

"""@en .

<http://dbkwik.webdatacommons.org/marvelcinematicuniverse.wikia.com/resource/4,722_Hours/Gallery> a owl:Thing ;
    rdfs:label "4,722 Hours/Gallery"^^rdf:langString ;
    rdfs:comment """A gallery of images from, or related to, the Agents of S.H.I.E.L.D. episode 4,722 Hours.

"""@en .

<http://dbkwik.webdatacommons.org/marvelcinematicuniverse.wikia.com/resource/7kingZ> a <http://dbkwik.webdatacommons.org/marvelcinematicuniverse.wikia.com/class/music> ;
    rdfs:label "7kingZ"^^rdf:langString ;
    rdfs:comment """7kingZ are an American hip hop group.
Their song "Born For This" is featured in the Cloak & Dagger episode Princeton Offense.

"""@en .

<http://dbkwik.webdatacommons.org/marvelcinematicuniverse.wikia.com/resource/A$AP_Ferg> a <http://dbkwik.webdatacommons.org/marvelcinematicuniverse.wikia.com/class/wps> ;
    rdfs:label "A$AP Ferg"^^rdf:langString ;
    rdfs:comment """Darold Ferguson, Jr., professionally known as A$AP Ferg, is an American rapper.
His collaboration with Remy Ma, "East Coast", is featured in the Runaways episode Kingdom.
He contributed to the soundtrack of Luke Cage.

"""@en .

<http://dbkwik.webdatacommons.org/marvelcinematicuniverse.wikia.com/resource/A%27Lars> a <http://dbkwik.webdatacommons.org/marvelcinematicuniverse.wikia.com/class/character> ;
    rdfs:label "A'Lars"^^rdf:langString ;
    ns1:citizenship <http://dbkwik.webdatacommons.org/marvelcinematicuniverse.wikia.com/resource/Titan> ;
    ns1:gender "Male"^^rdf:langString ;
    ns1:movie <http://dbkwik.webdatacommons.org/marvelcinematicuniverse.wikia.com/resource/Avengers:_Infinity_War> ;
    ns1:species <http://dbkwik.webdatacommons.org/marvelcinematicuniverse.wikia.com/resource/Titans> ;
    rdfs:comment """A'Lars was a Titan and the father of the galactic warlord Thanos.

"""@en .

<http://dbkwik.webdatacommons.org/marvelcinematicuniverse.wikia.com/resource/A.I.M._Arc_Armiger> a <http://dbkwik.webdatacommons.org/marvelcinematicuniverse.wikia.com/class/item> ;
    rdfs:label "A.I.M. Arc Armiger"^^rdf:langString ;
    ns1:creator <http://dbkwik.webdatacommons.org/marvelcinematicuniverse.wikia.com/resource/A.I.M.> ;
    ns1:game <http://dbkwik.webdatacommons.org/marvelcinematicuniverse.wikia.com/resource/Iron_Man_2_(video_game)> ;
    ns1:owners <http://dbkwik.webdatacommons.org/marvelcinematicuniverse.wikia.com/resource/A.I.M.> ;
    ns1:users <http://dbkwik.webdatacommons.org/marvelcinematicuniverse.wikia.com/resource/A.I.M.>,
        <http://dbkwik.webdatacommons.org/marvelcinematicuniverse.wikia.com/resource/Iron_Man> ;
    rdfs:comment """The A.I.M. Arc Armiger was an enhanced version of the Roxxon Armiger created with implants from Project P.R.O.T.E.A.N..

"""@en .

<http://dbkwik.webdatacommons.org/marvelcinematicuniverse.wikia.com/resource/A.I.M._Drones> a <http://dbkwik.webdatacommons.org/marvelcinematicuniverse.wikia.com/class/item> ;
    rdfs:label "A.I.M. Drones"^^rdf:langString ;
    ns1:creator <http://dbkwik.webdatacommons.org/marvelcinematicuniverse.wikia.com/resource/A.I.M.> ;
    ns1:game <http://dbkwik.webdatacommons.org/marvelcinematicuniverse.wikia.com/resource/Iron_Man_2_(video_game)> ;
    ns1:owners <http://dbkwik.webdatacommons.org/marvelcinematicuniverse.wikia.com/resource/A.I.M.> ;
    ns1:users <http://dbkwik.webdatacommons.org/marvelcinematicuniverse.wikia.com/resource/A.I.M.> ;
    rdfs:comment """A.I.M. Drones were were robotic military drones designed by A.I.M.

"""@en .

<http://dbkwik.webdatacommons.org/marvelcinematicuniverse.wikia.com/resource/A.I.M._Gunship> a <http://dbkwik.webdatacommons.org/marvelcinematicuniverse.wikia.com/class/vehicle> ;
    rdfs:label "A.I.M. Gunship"^^rdf:langString ;
    ns1:builder <http://dbkwik.webdatacommons.org/marvelcinematicuniverse.wikia.com/resource/A.I.M.> ;
    ns1:game <http://dbkwik.webdatacommons.org/marvelcinematicuniverse.wikia.com/resource/Iron_Man_2_(video_game)> ;
    ns1:owner <http://dbkwik.webdatacommons.org/marvelcinematicuniverse.wikia.com/resource/A.I.M.> ;
    ns1:passengers <http://dbkwik.webdatacommons.org/marvelcinematicuniverse.wikia.com/resource/Iron_Man>,
        <http://dbkwik.webdatacommons.org/marvelcinematicuniverse.wikia.com/resource/War_Machine> ;
    ns1:users <http://dbkwik.webdatacommons.org/marvelcinematicuniverse.wikia.com/resource/A.I.M.>,
        <http://dbkwik.webdatacommons.org/marvelcinematicuniverse.wikia.com/resource/Black_Widow> ;
    rdfs:comment """A.I.M. Gunships were transport and combat vehicles developed by A.I.M..

"""@en .

<http://dbkwik.webdatacommons.org/marvelcinematicuniverse.wikia.com/resource/A.I.M._President> a <http://dbkwik.webdatacommons.org/marvelcinematicuniverse.wikia.com/class/character> ;
    rdfs:label "A.I.M. President"^^rdf:langString ;
    ns1:gender "Male"^^rdf:langString ;
    ns1:species <http://dbkwik.webdatacommons.org/marvelcinematicuniverse.wikia.com/resource/Humans> ;
    ns1:voiceActor <http://dbkwik.webdatacommons.org/marvelcinematicuniverse.wikia.com/resource/Fred_Tatasciore> ;
    rdfs:comment """The A.I.M. President was the CEO of Advanced Idea Mechanics.

"""@en .

<http://dbkwik.webdatacommons.org/marvelcinematicuniverse.wikia.com/resource/A.J._Franklin> a <http://dbkwik.webdatacommons.org/marvelcinematicuniverse.wikia.com/class/actor> ;
    rdfs:label "A.J. Franklin"^^rdf:langString ;
    rdfs:comment """A.J. Franklin portrayed Protester #4 in the Luke Cage episodes Take It Personal and Now You're Mine.

"""@en .

<http://dbkwik.webdatacommons.org/marvelcinematicuniverse.wikia.com/resource/A.R.M.O.R.> a <http://dbkwik.webdatacommons.org/marvelcinematicuniverse.wikia.com/class/organization> ;
    rdfs:label "A.R.M.O.R."^^rdf:langString ;
    ns1:locations <http://dbkwik.webdatacommons.org/marvelcinematicuniverse.wikia.com/resource/Hub_(S.H.I.E.L.D._Facility)> ;
    rdfs:comment """A.R.M.O.R. is an organization that had an office at the Hub.

"""@en .

<http://dbkwik.webdatacommons.org/marvelcinematicuniverse.wikia.com/resource/A._Todd_Holland> a <http://dbkwik.webdatacommons.org/marvelcinematicuniverse.wikia.com/class/wps> ;
    rdfs:label "A. Todd Holland"^^rdf:langString ;
    rdfs:comment """A. Todd Holland was an art director on Thor.

"""@en .

<http://dbkwik.webdatacommons.org/marvelcinematicuniverse.wikia.com/resource/AC/DC> a <http://dbkwik.webdatacommons.org/marvelcinematicuniverse.wikia.com/class/wps> ;
    rdfs:label "AC/DC"^^rdf:langString ;
    rdfs:comment """AC/DC are an Australian rock band.
Their songs "Back in Black" and "Shoot to Thrill" are featured in Iron Man and The Avengers, respectively.
The entire soundtrack of Iron Man 2 consists of AC/DC songs.

"""@en .

<http://dbkwik.webdatacommons.org/marvelcinematicuniverse.wikia.com/resource/AKA_1,000_Cuts> rdfs:label "AKA 1,000 Cuts"^^rdf:langString ;
    ns1:next <http://dbkwik.webdatacommons.org/marvelcinematicuniverse.wikia.com/resource/AKA_I%27ve_Got_the_Blues> ;
    ns1:previous <http://dbkwik.webdatacommons.org/marvelcinematicuniverse.wikia.com/resource/AKA_Sin_Bin> ;
    rdfs:comment """AKA 1,000 Cuts is the tenth episode of the first season of the Netflix exclusive television series Jessica Jones.

"""@en .

<http://dbkwik.webdatacommons.org/marvelcinematicuniverse.wikia.com/resource/A_Film_by_Peter_Parker> a <http://dbkwik.webdatacommons.org/marvelcinematicuniverse.wikia.com/class/item> ;
    rdfs:label "A Film by Peter Parker"^^rdf:langString ;
    ns1:creator <http://dbkwik.webdatacommons.org/marvelcinematicuniverse.wikia.com/resource/Spider-Man> ;
    ns1:owners <http://dbkwik.webdatacommons.org/marvelcinematicuniverse.wikia.com/resource/Spider-Man> ;
    rdfs:comment """A Film by Peter Parker is a recorded video diary of Peter Parker's trip to Berlin.

"""@en .

<http://dbkwik.webdatacommons.org/marvelcinematicuniverse.wikia.com/resource/A_Flock_of_Seagulls> a <http://dbkwik.webdatacommons.org/marvelcinematicuniverse.wikia.com/class/wps> ;
    rdfs:label "A Flock of Seagulls"^^rdf:langString ;
    rdfs:comment """A Flock of Seagulls are an English new wave and synthpop band.
Their song "Space Age Love Song" is featured in Spider-Man: Homecoming.

"""@en .

<http://dbkwik.webdatacommons.org/marvelcinematicuniverse.wikia.com/resource/A_Tribe_Called_Quest> a <http://dbkwik.webdatacommons.org/marvelcinematicuniverse.wikia.com/class/wps> ;
    rdfs:label "A Tribe Called Quest"^^rdf:langString ;
    rdfs:comment """A Tribe Called Quest are an American hip-hop group. Their song "Award Tour" is featured in the Iron Fist episode Snow Gives Way.

"""@en .

<http://dbkwik.webdatacommons.org/marvelcinematicuniverse.wikia.com/resource/Aaron_(disambiguation)> a <http://dbkwik.webdatacommons.org/marvelcinematicuniverse.wikia.com/class/disambig> ;
    rdfs:label "Aaron (disambiguation)"^^rdf:langString ;
    ns3:wikiPageDisambiguates <http://dbkwik.webdatacommons.org/marvelcinematicuniverse.wikia.com/resource/Aaron>,
        <http://dbkwik.webdatacommons.org/marvelcinematicuniverse.wikia.com/resource/Aaron_(Baby)> .

<http://dbkwik.webdatacommons.org/marvelcinematicuniverse.wikia.com/resource/Aaron_Behr> a <http://dbkwik.webdatacommons.org/marvelcinematicuniverse.wikia.com/class/actor> ;
    rdfs:label "Aaron Behr"^^rdf:langString ;
    ns1:character <http://dbkwik.webdatacommons.org/marvelcinematicuniverse.wikia.com/resource/List_of_Minor_Characters> ;
    rdfs:comment """Aaron Behr portrayed Angry Man in the Agents of S.H.I.E.L.D. episode Pilot.

"""@en .

<http://dbkwik.webdatacommons.org/marvelcinematicuniverse.wikia.com/resource/Aaron_Berg> a <http://dbkwik.webdatacommons.org/marvelcinematicuniverse.wikia.com/class/actor> ;
    rdfs:label "Aaron Berg"^^rdf:langString ;
    rdfs:comment """Aaron Berg portrayed Soldier in The Incredible Hulk.

"""@en .

<http://dbkwik.webdatacommons.org/marvelcinematicuniverse.wikia.com/resource/Aaron_Costa_Ganis> a <http://dbkwik.webdatacommons.org/marvelcinematicuniverse.wikia.com/class/actor> ;
    rdfs:label "Aaron Costa Ganis"^^rdf:langString ;
    ns1:character <http://dbkwik.webdatacommons.org/marvelcinematicuniverse.wikia.com/resource/Bobby> ;
    rdfs:comment """Aaron Costa Ganis portrayed Bobby in the Jessica Jones episode AKA The Sandwich Saved Me.

"""@en .

<http://dbkwik.webdatacommons.org/marvelcinematicuniverse.wikia.com/resource/Aaron_D._Alexander> a <http://dbkwik.webdatacommons.org/marvelcinematicuniverse.wikia.com/class/filmmaker> ;
    rdfs:label "Aaron D. Alexander"^^rdf:langString ;
    rdfs:comment """Aaron D. Alexander was a stunt performer in the Agents of S.H.I.E.L.D. episodes A Life Spent, A Life Earned and The Real Deal.
He was also a stunt double for Eme Ikwuakor in the Inhumans episodes Those Who Would Destroy Us, Divide -- And Conquer, Something Inhuman This Way Comes..., The Gentleman's Name is Gorgon and ...And Finally: Black Bolt.

"""@en .

<http://dbkwik.webdatacommons.org/marvelcinematicuniverse.wikia.com/resource/Aaron_Fili> a <http://dbkwik.webdatacommons.org/marvelcinematicuniverse.wikia.com/class/actor> ;
    rdfs:label "Aaron Fili"^^rdf:langString ;
    rdfs:comment """Aaron Fili portrayed Scientist in the Agents of S.H.I.E.L.D. episodes Inside Voices, The Honeymoon and All Roads Lead...

"""@en .

<http://dbkwik.webdatacommons.org/marvelcinematicuniverse.wikia.com/resource/Aaron_Gaffey> rdfs:label "Aaron Gaffey"^^rdf:langString ;
    ns1:character <http://dbkwik.webdatacommons.org/marvelcinematicuniverse.wikia.com/resource/List_of_Minor_Characters> ;
    rdfs:comment """Aaron Gaffey portrayed Mysterious Figure in the Agents of S.H.I.E.L.D. episode Uprising.

"""@en .

<http://dbkwik.webdatacommons.org/marvelcinematicuniverse.wikia.com/resource/Aaron_Goldenberg> a <http://dbkwik.webdatacommons.org/marvelcinematicuniverse.wikia.com/class/filmmaker> ;
    rdfs:label "Aaron Goldenberg"^^rdf:langString ;
    rdfs:comment """Aaron Goldenberg was a stand-in and a double in Iron Man 3.

"""@en .

<http://dbkwik.webdatacommons.org/marvelcinematicuniverse.wikia.com/resource/Aaron_Himelstein> rdfs:label "Aaron Himelstein"^^rdf:langString ;
    ns1:character <http://dbkwik.webdatacommons.org/marvelcinematicuniverse.wikia.com/resource/Cameron_Klein> ;
    rdfs:comment """Aaron Himelstein portrayed Cameron Klein in Captain America: The Winter Soldier and Avengers: Age of Ultron.

"""@en .

<http://dbkwik.webdatacommons.org/marvelcinematicuniverse.wikia.com/resource/Aaron_James> a <http://dbkwik.webdatacommons.org/marvelcinematicuniverse.wikia.com/class/character> ;
    rdfs:label "Aaron James"^^rdf:langString ;
    ns1:actor <http://dbkwik.webdatacommons.org/marvelcinematicuniverse.wikia.com/resource/Gabe_White> ;
    ns1:species <http://dbkwik.webdatacommons.org/marvelcinematicuniverse.wikia.com/resource/Humans> ;
    rdfs:comment """Aaraon James was a client of Matt Murdock, who potentially lost his ability to stand and walk after after the exposure to Endexoprene in a subway station built by Berkowitz's company.

"""@en .

<http://dbkwik.webdatacommons.org/marvelcinematicuniverse.wikia.com/resource/Aaron_Muir> a <http://dbkwik.webdatacommons.org/marvelcinematicuniverse.wikia.com/class/filmmaker> ;
    rdfs:label "Aaron Muir"^^rdf:langString ;
    rdfs:comment """Aaron Muir was a stunt rigger in Guardians of the Galaxy.

"""@en .

<http://dbkwik.webdatacommons.org/marvelcinematicuniverse.wikia.com/resource/Aaron_Norris> a <http://dbkwik.webdatacommons.org/marvelcinematicuniverse.wikia.com/class/filmmaker> ;
    rdfs:label "Aaron Norris"^^rdf:langString ;
    rdfs:comment """Aaron Norris was a utility stunts performer in Ant-Man.

"""@en .

<http://dbkwik.webdatacommons.org/marvelcinematicuniverse.wikia.com/resource/Aaron_Wilson> a <http://dbkwik.webdatacommons.org/marvelcinematicuniverse.wikia.com/class/filmmaker> ;
    rdfs:label "Aaron Wilson"^^rdf:langString ;
    rdfs:comment """Aaron Wilson was a digital artist for The Avengers.

"""@en .

<http://dbkwik.webdatacommons.org/marvelcinematicuniverse.wikia.com/resource/Abandoned_Building> rdfs:label "Abandoned Building"^^rdf:langString ;
    ns1:continent <http://dbkwik.webdatacommons.org/marvelcinematicuniverse.wikia.com/resource/North_America> ;
    ns1:location <http://dbkwik.webdatacommons.org/marvelcinematicuniverse.wikia.com/resource/New_York> ;
    rdfs:comment """The Abandoned Building is a former warehouse in Hell's Kitchen that had been abandoned.

"""@en .

<http://dbkwik.webdatacommons.org/marvelcinematicuniverse.wikia.com/resource/Abandoned_Warehouse> rdfs:label "Abandoned Warehouse"^^rdf:langString ;
    ns1:continent <http://dbkwik.webdatacommons.org/marvelcinematicuniverse.wikia.com/resource/North_America> ;
    rdfs:comment """The Abandoned Warehouse is a former storage building located in New York City that had been abandoned. The warehouse was used by Homeland Security for a sting operation against Anvil team led by Billy Russo.

"""@en .

<http://dbkwik.webdatacommons.org/marvelcinematicuniverse.wikia.com/resource/Abby> rdfs:label "Abby"^^rdf:langString ;
    ns1:actor <http://dbkwik.webdatacommons.org/marvelcinematicuniverse.wikia.com/resource/Ciara_Bravo> ;
    ns1:citizenship <http://dbkwik.webdatacommons.org/marvelcinematicuniverse.wikia.com/resource/Lighthouse> ;
    rdfs:comment """Abby is a young Inhuman living on the Lighthouse in an alternate future in which Earth was destroyed and the few Human survivors became slaves of the Kree.

"""@en .

<http://dbkwik.webdatacommons.org/marvelcinematicuniverse.wikia.com/resource/Abduction_at_Rae%27s_Restaurant> a <http://dbkwik.webdatacommons.org/marvelcinematicuniverse.wikia.com/class/conflict> ;
    rdfs:label "Abduction at Rae's Restaurant"^^rdf:langString ;
    ns1:commanders <http://dbkwik.webdatacommons.org/marvelcinematicuniverse.wikia.com/resource/Enoch>,
        <http://dbkwik.webdatacommons.org/marvelcinematicuniverse.wikia.com/resource/Phil_Coulson> ;
    ns1:date <http://dbkwik.webdatacommons.org/marvelcinematicuniverse.wikia.com/resource/2017> ;
    ns1:place <http://dbkwik.webdatacommons.org/marvelcinematicuniverse.wikia.com/resource/Chicago>,
        <http://dbkwik.webdatacommons.org/marvelcinematicuniverse.wikia.com/resource/Illinois> ;
    ns1:result <http://dbkwik.webdatacommons.org/marvelcinematicuniverse.wikia.com/resource/2091>,
        <http://dbkwik.webdatacommons.org/marvelcinematicuniverse.wikia.com/resource/Leo_Fitz> ;
    ns1:side <http://dbkwik.webdatacommons.org/marvelcinematicuniverse.wikia.com/resource/Enoch> ;
    rdfs:comment """The Abduction at Rae's Restaurant was a kidnapping operation led by the Chronicom Enoch, who intended to send Phil Coulson and his team to the year 2091 so that they could find a way to avert the prophesied Destruction of Earth.

"""@en .

<http://dbkwik.webdatacommons.org/marvelcinematicuniverse.wikia.com/resource/Abe_Brown> rdfs:label "Abe Brown"^^rdf:langString ;
    ns1:actor <http://dbkwik.webdatacommons.org/marvelcinematicuniverse.wikia.com/resource/Abraham_Attah> ;
    rdfs:comment """Abraham "Abe" Brown is a student at the Midtown School of Science and Technology, and a member of the decathlon team of the school.

"""@en .

<http://dbkwik.webdatacommons.org/marvelcinematicuniverse.wikia.com/resource/Abilisk> rdfs:label "Abilisk"^^rdf:langString ;
    ns1:dod <http://dbkwik.webdatacommons.org/marvelcinematicuniverse.wikia.com/resource/2014> ;
    rdfs:comment """The Abilisk was a multi-dimensional being who was devouring the power sources of the Sovereign planet. The Sovereign hired the Guardians of the Galaxy to fight it.

"""@en .

<http://dbkwik.webdatacommons.org/marvelcinematicuniverse.wikia.com/resource/Abomination/Quote> a <http://dbkwik.webdatacommons.org/marvelcinematicuniverse.wikia.com/class/quote> ;
    rdfs:label "Abomination/Quote"^^rdf:langString ;
    rdfs:comment """A collection of quotes from the former special-ops commando Emil Blonsky, also known as the Abomination.

"""@en .

<http://dbkwik.webdatacommons.org/marvelcinematicuniverse.wikia.com/resource/Abraham_Erskine> rdfs:label "Abraham Erskine"^^rdf:langString ;
    ns1:age 73 ;
    ns1:comic <http://dbkwik.webdatacommons.org/marvelcinematicuniverse.wikia.com/resource/Captain_America:_First_Vengeance> ;
    ns1:webSeries <http://dbkwik.webdatacommons.org/marvelcinematicuniverse.wikia.com/resource/WHiH_Newsfront_(web_series)> ;
    rdfs:comment """Dr. Abraham Erskine was a German scientist who created the Super Soldier Serum and was forced to use a preliminary version to transform Johann Schmidt into the Red Skull. Fleeing to the United States of America, Erskine joined the Strategic Scientific Reserve where he managed to perfect his serum, using it on Steve Rogers shortly before being assassinated by HYDRA.

"""@en .

<http://dbkwik.webdatacommons.org/marvelcinematicuniverse.wikia.com/resource/Abraham_Erskine/Quote> a <http://dbkwik.webdatacommons.org/marvelcinematicuniverse.wikia.com/class/quote> ;
    rdfs:label "Abraham Erskine/Quote"^^rdf:langString ;
    rdfs:comment """A collection of quotes from the German scientist and creator of the Super Soldier Serum, Abraham Erskine.

"""@en .

<http://dbkwik.webdatacommons.org/marvelcinematicuniverse.wikia.com/resource/Absolution_Virus> a <http://dbkwik.webdatacommons.org/marvelcinematicuniverse.wikia.com/class/item> ;
    rdfs:label "Absolution Virus"^^rdf:langString ;
    ns1:creator <http://dbkwik.webdatacommons.org/marvelcinematicuniverse.wikia.com/resource/Hive>,
        <http://dbkwik.webdatacommons.org/marvelcinematicuniverse.wikia.com/resource/Holden_Radcliffe> ;
    rdfs:comment """The Absolution Virus was a gaseous substance created by Holden Radcliffe. Whenever a human is exposed to this mist, they undergo a form of Terrigenesis that converts them into a Primitive creature that is instantaneously swayed by Hive.

"""@en .

<http://dbkwik.webdatacommons.org/marvelcinematicuniverse.wikia.com/resource/Absorbing_Man> rdfs:label "Absorbing Man"^^rdf:langString ;
    ns1:alias <http://dbkwik.webdatacommons.org/marvelcinematicuniverse.wikia.com/resource/George_Talbot> ;
    ns1:idno 23 ;
    rdfs:comment """Carl "Crusher" Creel was an enhanced individual with the ability to absorb the properties of anything he touches. Originally a boxer, Creel appeared on S.H.I.E.L.D.'s radar and had been deemed too dangerous, so John Garrett was sent to kill him. Garrett, who was secretly working for HYDRA, faked Creel's death and recruited him into HYDRA. Creel worked for Daniel Whitehall and was ordered to steal the Obelisk, but Creel was stopped by Phil Coulson's team and handed over to Glenn Talbot for custody. Having recovered from the effects of the Obelisk, Creel then underwent months of treatment to be rid of HYDRA's brainwashing. 
"""@en .

<http://dbkwik.webdatacommons.org/marvelcinematicuniverse.wikia.com/resource/Abstract> a <http://dbkwik.webdatacommons.org/marvelcinematicuniverse.wikia.com/class/item> ;
    rdfs:label "Abstract"^^rdf:langString ;
    ns1:owners <http://dbkwik.webdatacommons.org/marvelcinematicuniverse.wikia.com/resource/PRIDE> ;
    rdfs:comment """The Abstract is a book used during the Rite of Blood ceremonies.

"""@en .

<http://dbkwik.webdatacommons.org/marvelcinematicuniverse.wikia.com/resource/AccuTech> a <http://dbkwik.webdatacommons.org/marvelcinematicuniverse.wikia.com/class/organization> ;
    rdfs:label "AccuTech"^^rdf:langString ;
    ns1:founder <http://dbkwik.webdatacommons.org/marvelcinematicuniverse.wikia.com/resource/Gilbert_O%27Conner> ;
    ns1:headquarters <http://dbkwik.webdatacommons.org/marvelcinematicuniverse.wikia.com/resource/California>,
        <http://dbkwik.webdatacommons.org/marvelcinematicuniverse.wikia.com/resource/United_States_of_America> ;
    ns1:leader <http://dbkwik.webdatacommons.org/marvelcinematicuniverse.wikia.com/resource/Charles_Healey>,
        <http://dbkwik.webdatacommons.org/marvelcinematicuniverse.wikia.com/resource/Iron_Man> ;
    ns1:members <http://dbkwik.webdatacommons.org/marvelcinematicuniverse.wikia.com/resource/Klaus_Haas> ;
    rdfs:comment """AccuTech is a subsidiary of Stark Industries.

"""@en .

<http://dbkwik.webdatacommons.org/marvelcinematicuniverse.wikia.com/resource/Acura_2012_Stark_Industries_Super_Car> a <http://dbkwik.webdatacommons.org/marvelcinematicuniverse.wikia.com/class/vehicle> ;
    rdfs:label "Acura 2012 Stark Industries Super Car"^^rdf:langString ;
    ns1:owner <http://dbkwik.webdatacommons.org/marvelcinematicuniverse.wikia.com/resource/Iron_Man> ;
    ns1:passengers <http://dbkwik.webdatacommons.org/marvelcinematicuniverse.wikia.com/resource/Hulk> ;
    rdfs:comment """The Acura 2012 Stark Industries Super Car is a one-of-a-kind custom vehicle built by Acura and contracted by Tony Stark.

"""@en .

<http://dbkwik.webdatacommons.org/marvelcinematicuniverse.wikia.com/resource/Adam_Banks> rdfs:label "Adam Banks"^^rdf:langString ;
    ns1:produced <http://dbkwik.webdatacommons.org/marvelcinematicuniverse.wikia.com/resource/Luke_Cage_(TV_series)> ;
    rdfs:comment """Adam Banks was a post-production supervisor of the first season of Daredevil and the first season of Jessica Jones.
He was also an associate producer of the first season of Luke Cage tv series.

"""@en .

<http://dbkwik.webdatacommons.org/marvelcinematicuniverse.wikia.com/resource/Adam_Cooper> rdfs:label "Adam Cooper"^^rdf:langString ;
    ns1:age 19 ;
    rdfs:comment """Adam Cooper was the victim of PRIDE's second annual ceremony, as part of the Ultra Project.

"""@en .

<http://dbkwik.webdatacommons.org/marvelcinematicuniverse.wikia.com/resource/Adam_Cross> rdfs:label "Adam Cross"^^rdf:langString ;
    ns1:affiliation <http://dbkwik.webdatacommons.org/marvelcinematicuniverse.wikia.com/resource/Wrigley_Fire_Department> ;
    rdfs:comment """Adam Cross was a physical education teacher and varsity football coach at the local high-school, boy scout troop leader and volunteer firefighter from Wrigley, Pennsylvania.

"""@en .

<http://dbkwik.webdatacommons.org/marvelcinematicuniverse.wikia.com/resource/Adam_Goldstein> rdfs:label "Adam Goldstein"^^rdf:langString ;
    ns1:alias <http://dbkwik.webdatacommons.org/marvelcinematicuniverse.wikia.com/resource/DJ_AM> ;
    rdfs:comment """Adam Goldstein is a famous DJ.

"""@en .

<http://dbkwik.webdatacommons.org/marvelcinematicuniverse.wikia.com/resource/Adam_Harrington_(disambiguation)> a <http://dbkwik.webdatacommons.org/marvelcinematicuniverse.wikia.com/class/disambig> ;
    rdfs:label "Adam Harrington (disambiguation)"^^rdf:langString ;
    ns3:wikiPageDisambiguates <http://dbkwik.webdatacommons.org/marvelcinematicuniverse.wikia.com/resource/Adam_Harrington_(actor)> .

<http://dbkwik.webdatacommons.org/marvelcinematicuniverse.wikia.com/resource/Aden_Stay> rdfs:label "Aden Stay"^^rdf:langString ;
    ns1:webSeries <http://dbkwik.webdatacommons.org/marvelcinematicuniverse.wikia.com/resource/Agents_of_S.H.I.E.L.D.:_Double_Agent> ;
    rdfs:comment """Aden Stay was a stunt performer in the Agents of S.H.I.E.L.D. episode Making Friends and Influencing People and the Agents of S.H.I.E.L.D.: Double Agent episode The Mastermind is Revealed.
He was also a stunt double for Chris Sullivan in Guardians of the Galaxy Vol. 2 and Vincent D'Onofrio in upcoming episodes of Daredevil.

"""@en .

<http://dbkwik.webdatacommons.org/marvelcinematicuniverse.wikia.com/resource/Adolf_Hitler_(Fiction)> rdfs:label "Adolf Hitler (Fiction)"^^rdf:langString ;
    ns1:realName <http://dbkwik.webdatacommons.org/marvelcinematicuniverse.wikia.com/resource/Adolf_Hitler> ;
    rdfs:comment """Adolf Hitler was a fictional version of the real-life dictator of Nazi Germany. He appeared in several American propaganda tools during World War II as the nemesis of Captain America.

"""@en .

<http://dbkwik.webdatacommons.org/marvelcinematicuniverse.wikia.com/resource/Ador> rdfs:label "Ador"^^rdf:langString ;
    ns1:affiliation <http://dbkwik.webdatacommons.org/marvelcinematicuniverse.wikia.com/resource/Norse_Paganists> ;
    rdfs:comment """Ador is a member of a Norse Paganist hate group based in Norway.

"""@en .

<http://dbkwik.webdatacommons.org/marvelcinematicuniverse.wikia.com/resource/Adrian_Toomes%27_Campaign> a <http://dbkwik.webdatacommons.org/marvelcinematicuniverse.wikia.com/class/war> ;
    rdfs:label "Adrian Toomes' Campaign"^^rdf:langString ;
    ns1:battles <http://dbkwik.webdatacommons.org/marvelcinematicuniverse.wikia.com/resource/Ambush_at_the_Staten_Island_Ferry>,
        <http://dbkwik.webdatacommons.org/marvelcinematicuniverse.wikia.com/resource/Ambush_on_Peter_Parker> ;
    ns1:begin <http://dbkwik.webdatacommons.org/marvelcinematicuniverse.wikia.com/resource/2012> ;
    ns1:casualties <http://dbkwik.webdatacommons.org/marvelcinematicuniverse.wikia.com/resource/Jackson_Brice> ;
    ns1:commanders <http://dbkwik.webdatacommons.org/marvelcinematicuniverse.wikia.com/resource/Iron_Man>,
        <http://dbkwik.webdatacommons.org/marvelcinematicuniverse.wikia.com/resource/Shocker> ;
    ns1:conc <http://dbkwik.webdatacommons.org/marvelcinematicuniverse.wikia.com/resource/Chase_of_Quake>,
        <http://dbkwik.webdatacommons.org/marvelcinematicuniverse.wikia.com/resource/Erik_Killmonger%27s_Campaign> ;
    ns1:result <http://dbkwik.webdatacommons.org/marvelcinematicuniverse.wikia.com/resource/Avengers>,
        <http://dbkwik.webdatacommons.org/marvelcinematicuniverse.wikia.com/resource/Iron_Man> ;
    ns1:side <http://dbkwik.webdatacommons.org/marvelcinematicuniverse.wikia.com/resource/Adrian_Toomes%27_Crew>,
        <http://dbkwik.webdatacommons.org/marvelcinematicuniverse.wikia.com/resource/Iron_Man> ;
    rdfs:comment """Adrian Toomes' Campaign was a series of events in which Adrian Toomes, who began living a criminal lifestyle after the Department of Damage Control drove him out of business, came into conflict with the costumed superhero known as Spider-Man.

"""@en .

<http://dbkwik.webdatacommons.org/marvelcinematicuniverse.wikia.com/resource/Adrian_Toomes%27_Headquarters> rdfs:label "Adrian Toomes' Headquarters"^^rdf:langString ;
    ns1:notable <http://dbkwik.webdatacommons.org/marvelcinematicuniverse.wikia.com/resource/Jackson_Brice>,
        <http://dbkwik.webdatacommons.org/marvelcinematicuniverse.wikia.com/resource/Randy_Vale> ;
    rdfs:comment """Adrian Toomes' Headquarters is an arms-dealing business that reverse-engineers and weaponize alien technology for sale on the streets in order to earn profits.

"""@en .

<http://dbkwik.webdatacommons.org/marvelcinematicuniverse.wikia.com/resource/Adrian_Younge> rdfs:label "Adrian Younge"^^rdf:langString ;
    ns1:realName <http://dbkwik.webdatacommons.org/marvelcinematicuniverse.wikia.com/resource/Adrian_Younge_(actor)> ;
    rdfs:comment """Adrian Younge is a musician.

"""@en .

<http://dbkwik.webdatacommons.org/marvelcinematicuniverse.wikia.com/resource/Adrianne_Palicki> rdfs:label "Adrianne Palicki"^^rdf:langString ;
    ns1:webSeries <http://dbkwik.webdatacommons.org/marvelcinematicuniverse.wikia.com/resource/Agents_of_S.H.I.E.L.D.:_Double_Agent>,
        <http://dbkwik.webdatacommons.org/marvelcinematicuniverse.wikia.com/resource/Searching_for_Secrets> ;
    rdfs:comment """Adrianne Palicki portrayed Bobbi Morse in Agents of S.H.I.E.L.D., starting with the fifth episode of the second season A Hen in the Wolf House. She was credited as a guest star from the fifth to the tenth episode but was promoted to a series regular in episode 2.11 Aftershocks.
She was slated to be a main cast member on the Agents of S.H.I.E.L.D. spin-off series, Most Wanted.
She portrayed herself in the Agents of S.H.I.E.L.D.: Double Agent episode Searching for Secrets.

"""@en .

<http://dbkwik.webdatacommons.org/marvelcinematicuniverse.wikia.com/resource/Advanced_Threat_Containment_Unit> rdfs:label "Advanced Threat Containment Unit"^^rdf:langString ;
    ns1:affiliation <http://dbkwik.webdatacommons.org/marvelcinematicuniverse.wikia.com/resource/United_States_of_America> ;
    ns1:formerleaders <http://dbkwik.webdatacommons.org/marvelcinematicuniverse.wikia.com/resource/Glenn_Talbot>,
        <http://dbkwik.webdatacommons.org/marvelcinematicuniverse.wikia.com/resource/Rosalind_Price> ;
    ns1:founder <http://dbkwik.webdatacommons.org/marvelcinematicuniverse.wikia.com/resource/Matthew_Ellis> ;
    ns1:headquarters <http://dbkwik.webdatacommons.org/marvelcinematicuniverse.wikia.com/resource/Endotex_Labs> ;
    rdfs:comment """The Advanced Threat Containment Unit, also known by its acronym ATCU, is a new United States Government organization created to deal with the emergence of new Inhumans following the accidental release of the Terrigen Mist at the bottom of the ocean. However, since its foundation, the ATCU was manipulated by Gideon Malick's HYDRA cell to do HYDRA's bidding. After the death of its first director Rosalind Price, the ATCU was cleaned of HYDRA infiltrators and re-purposed to serve as the public face of the officially outlawed agency S.H.I.E.L.D. with the ATCU's new director Glenn Talbot being subordinate to S.H.I.E.L.D.'s director Phil Coulson.

"""@en .

<http://dbkwik.webdatacommons.org/marvelcinematicuniverse.wikia.com/resource/Aerodynamic_Marvel> a <http://dbkwik.webdatacommons.org/marvelcinematicuniverse.wikia.com/class/vehicle> ;
    rdfs:label "Aerodynamic Marvel"^^rdf:langString ;
    ns1:builder <http://dbkwik.webdatacommons.org/marvelcinematicuniverse.wikia.com/resource/Justin_Hammer> ;
    ns1:owner <http://dbkwik.webdatacommons.org/marvelcinematicuniverse.wikia.com/resource/Hammer_Industries> ;
    rdfs:comment """The Aerodynamic Marvel is a single-pilot attack aircraft designed by Justin Hammer.

"""@en .

<http://dbkwik.webdatacommons.org/marvelcinematicuniverse.wikia.com/resource/Afghan_National_Police> rdfs:label "Afghan National Police"^^rdf:langString ;
    ns1:locations <http://dbkwik.webdatacommons.org/marvelcinematicuniverse.wikia.com/resource/Afghanistan> ;
    rdfs:comment """The Afghan National Police, occasionally referred as ANP, is the national police force of Afghanistan, serving as a single law enforcement agency all across the country.

"""@en .

<http://dbkwik.webdatacommons.org/marvelcinematicuniverse.wikia.com/resource/Africa> rdfs:label "Africa"^^rdf:langString ;
    ns1:interest <http://dbkwik.webdatacommons.org/marvelcinematicuniverse.wikia.com/resource/Algeria>,
        <http://dbkwik.webdatacommons.org/marvelcinematicuniverse.wikia.com/resource/Benin> ;
    rdfs:comment """Africa is one of the seven continents.

"""@en .

<http://dbkwik.webdatacommons.org/marvelcinematicuniverse.wikia.com/resource/Afterlife_(episode)> rdfs:label "Afterlife (episode)"^^rdf:langString ;
    ns1:title <http://dbkwik.webdatacommons.org/marvelcinematicuniverse.wikia.com/resource/Afterlife> ;
    rdfs:comment """Afterlife is the sixteenth episode of the second season of the television series Agents of S.H.I.E.L.D. and the thirty-eighth episode overall.

"""@en .

<http://dbkwik.webdatacommons.org/marvelcinematicuniverse.wikia.com/resource/Agamotto> rdfs:label "Agamotto"^^rdf:langString ;
    ns1:alias <http://dbkwik.webdatacommons.org/marvelcinematicuniverse.wikia.com/resource/Magic> ;
    ns1:title <http://dbkwik.webdatacommons.org/marvelcinematicuniverse.wikia.com/resource/Category:Sorcerer_Supreme> ;
    rdfs:comment """Agamotto was the first Sorcerer Supreme of Earth, founder of the Masters of the Mystic Arts and the builder of the and the Eye of Agamotto.

"""@en .

<http://dbkwik.webdatacommons.org/marvelcinematicuniverse.wikia.com/resource/Agent_(Code_13)> rdfs:label "Agent (Code 13)"^^rdf:langString ;
    ns1:title <http://dbkwik.webdatacommons.org/marvelcinematicuniverse.wikia.com/resource/S.H.I.E.L.D.> ;
    rdfs:comment """The Agent was a S.H.I.E.L.D. undercover operative tasked with checking Steve Rogers following his awakening.

"""@en .

<http://dbkwik.webdatacommons.org/marvelcinematicuniverse.wikia.com/resource/Agent_13_(disambiguation)> a <http://dbkwik.webdatacommons.org/marvelcinematicuniverse.wikia.com/class/disambig> ;
    rdfs:label "Agent 13 (disambiguation)"^^rdf:langString .

<http://dbkwik.webdatacommons.org/marvelcinematicuniverse.wikia.com/resource/Agent_33> rdfs:label "Agent 33"^^rdf:langString ;
    ns1:alias <http://dbkwik.webdatacommons.org/marvelcinematicuniverse.wikia.com/resource/Brookton>,
        <http://dbkwik.webdatacommons.org/marvelcinematicuniverse.wikia.com/resource/Carla_Talbot> ;
    ns1:title <http://dbkwik.webdatacommons.org/marvelcinematicuniverse.wikia.com/resource/S.H.I.E.L.D.> ;
    rdfs:comment """Kara Palamas, better known as Agent 33, was a former S.H.I.E.L.D. agent who was brainwashed by Daniel Whitehall into serving HYDRA until his death, after which she allied herself with Grant Ward, who helped her to regain her identity and her freedom. She also gained limited shapeshifting abilities via a permanently implanted Photostatic Veil.
"""@en .

<http://dbkwik.webdatacommons.org/marvelcinematicuniverse.wikia.com/resource/Agent_Carter:_Season_One_Declassified> a <http://dbkwik.webdatacommons.org/marvelcinematicuniverse.wikia.com/class/book> ;
    rdfs:label "Agent Carter: Season One Declassified"^^rdf:langString ;
    ns1:isbn "ISBN-10: 0785197184"^^rdf:langString,
        "ISBN-13:978-0785197188"^^rdf:langString ;
    ns1:media "Behind-the-Scenes art book"^^rdf:langString ;
    ns1:pages 200 ;
    ns1:publisher "Marvel"^^rdf:langString ;
    ns1:released "2015-07-07"^^xsd:date ;
    rdfs:comment """Agent Carter: Season One Declassified is the official artbook and behind-the-scenes story about the first season of Agent Carter.

"""@en .

<http://dbkwik.webdatacommons.org/marvelcinematicuniverse.wikia.com/resource/Agent_Carter:_Season_Two_Declassified> a <http://dbkwik.webdatacommons.org/marvelcinematicuniverse.wikia.com/class/book> ;
    rdfs:label "Agent Carter: Season Two Declassified"^^rdf:langString ;
    ns1:isbn "ISBN-10: 0785195920"^^rdf:langString ;
    ns1:media "Behind-the-Scenes art book"^^rdf:langString ;
    ns1:pages 232 ;
    ns1:released "2016-10-18"^^xsd:date ;
    rdfs:comment """Agent Carter: Season Two Declassified is the official artbook and behind-the-scenes story about the second season of Agent Carter.

"""@en .

<http://dbkwik.webdatacommons.org/marvelcinematicuniverse.wikia.com/resource/Agent_Carter_(Season_One)/Home_Video> a <http://dbkwik.webdatacommons.org/marvelcinematicuniverse.wikia.com/class/dvd> ;
    rdfs:label "Agent Carter (Season One)/Home Video"^^rdf:langString ;
    ns1:prev <http://dbkwik.webdatacommons.org/marvelcinematicuniverse.wikia.com/resource/Agents_of_S.H.I.E.L.D._(Season_Two)/Home_Video> ;
    ns1:release "2015-09-18"^^xsd:date ;
    ns1:runtime "20100.0"^^<http://dbkwik.webdatacommons.org/datatype/second> ;
    ns1:series <http://dbkwik.webdatacommons.org/marvelcinematicuniverse.wikia.com/resource/Agent_Carter_(TV_series)> ;
    rdfs:comment """Agent Carter: The Complete First Season is the DVD and Blu-ray release for Agent Carter Season One.

"""@en .

<http://dbkwik.webdatacommons.org/marvelcinematicuniverse.wikia.com/resource/Agent_Carter_(Season_Two)/Home_Video> a <http://dbkwik.webdatacommons.org/marvelcinematicuniverse.wikia.com/class/dvd> ;
    rdfs:label "Agent Carter (Season Two)/Home Video"^^rdf:langString ;
    ns1:prev <http://dbkwik.webdatacommons.org/marvelcinematicuniverse.wikia.com/resource/Jessica_Jones_(Season_One)/Home_Video> ;
    ns1:release "2016-12-05"^^xsd:date ;
    ns1:series <http://dbkwik.webdatacommons.org/marvelcinematicuniverse.wikia.com/resource/Agent_Carter_(TV_series)> ;
    rdfs:comment """Agent Carter - The Complete Second Season is the Blu-ray release for Agent Carter Season Two.

"""@en .

<http://dbkwik.webdatacommons.org/marvelcinematicuniverse.wikia.com/resource/Agent_Carter_(TV_series)/Home_Video> a <http://dbkwik.webdatacommons.org/marvelcinematicuniverse.wikia.com/class/disambig> ;
    rdfs:label "Agent Carter (TV series)/Home Video"^^rdf:langString .

<http://dbkwik.webdatacommons.org/marvelcinematicuniverse.wikia.com/resource/Agent_Carter_(TV_series)/Season_Two> a <http://dbkwik.webdatacommons.org/marvelcinematicuniverse.wikia.com/class/season> ;
    rdfs:label "Agent Carter (TV series)/Season Two"^^rdf:langString ;
    ns1:channel <http://dbkwik.webdatacommons.org/marvelcinematicuniverse.wikia.com/resource/American_Broadcasting_Company> ;
    ns1:dates "--01-19"^^xsd:gMonthDay ;
    ns1:episodes 10 ;
    ns1:prev <http://dbkwik.webdatacommons.org/marvelcinematicuniverse.wikia.com/resource/Agent_Carter_(TV_series)/Season_One> ;
    rdfs:comment """The Second Season of Agent Carter was officially confirmed on May 7, 2015 by ABC. It premiered on January 19, 2016.

"""@en .

<http://dbkwik.webdatacommons.org/marvelcinematicuniverse.wikia.com/resource/Agents_of_S.H.I.E.L.D./Gallery> a <http://dbkwik.webdatacommons.org/marvelcinematicuniverse.wikia.com/class/col-end> ;
    rdfs:label "Agents of S.H.I.E.L.D./Gallery"^^rdf:langString ;
    rdfs:comment """The following is an index of galleries of screenshots and promotional material from the television show Agents of S.H.I.E.L.D..

"""@en .

<http://dbkwik.webdatacommons.org/marvelcinematicuniverse.wikia.com/resource/Agents_of_S.H.I.E.L.D./Season_Five> a <http://dbkwik.webdatacommons.org/marvelcinematicuniverse.wikia.com/class/season> ;
    rdfs:label "Agents of S.H.I.E.L.D./Season Five"^^rdf:langString ;
    ns1:channel <http://dbkwik.webdatacommons.org/marvelcinematicuniverse.wikia.com/resource/American_Broadcasting_Company> ;
    ns1:dates "--12-01"^^xsd:gMonthDay ;
    ns1:episodes 22 ;
    ns1:prev <http://dbkwik.webdatacommons.org/marvelcinematicuniverse.wikia.com/resource/Agents_of_S.H.I.E.L.D./Season_Four> ;
    rdfs:comment """The Fifth Season of Agents of S.H.I.E.L.D. was officially confirmed on May 11, 2017, by ABC.
The season premiered December 1, 2017, with a two-hour premiere.

"""@en .

<http://dbkwik.webdatacommons.org/marvelcinematicuniverse.wikia.com/resource/Agents_of_S.H.I.E.L.D./Season_One> a <http://dbkwik.webdatacommons.org/marvelcinematicuniverse.wikia.com/class/season> ;
    rdfs:label "Agents of S.H.I.E.L.D./Season One"^^rdf:langString ;
    ns1:episodes 22 ;
    rdfs:comment """The First Season of Agents of S.H.I.E.L.D. premiered on September 24, 2013 on ABC. It was previously aired to a small group of fans at San Diego Comic-Con on July 18, 2013.

"""@en .

<http://dbkwik.webdatacommons.org/marvelcinematicuniverse.wikia.com/resource/Agents_of_S.H.I.E.L.D.:_Academy> a <http://dbkwik.webdatacommons.org/marvelcinematicuniverse.wikia.com/class/web_series> ;
    rdfs:label "Agents of S.H.I.E.L.D.: Academy"^^rdf:langString ;
    rdfs:comment """Agents of S.H.I.E.L.D.: Academy is a five-part original web series designed as a behind-the-scenes feature for Agents of S.H.I.E.L.D. Contestants will compete in different challenges related to Agents of S.H.I.E.L.D. in order to win an appearance in the fourth season of the show.

"""@en .

<http://dbkwik.webdatacommons.org/marvelcinematicuniverse.wikia.com/resource/Agents_of_S.H.I.E.L.D.:_Agents_of_HYDRA> a <http://dbkwik.webdatacommons.org/marvelcinematicuniverse.wikia.com/class/reflist> ;
    rdfs:label "Agents of S.H.I.E.L.D.: Agents of HYDRA"^^rdf:langString ;
    rdfs:comment """Agents of S.H.I.E.L.D.: Agents of HYDRA is an event that serves as the third of the fourth season of Agents of S.H.I.E.L.D.. It focuses on the alternative lives the main characters have inside the Framework.

"""@en .

<http://dbkwik.webdatacommons.org/marvelcinematicuniverse.wikia.com/resource/Agents_of_S.H.I.E.L.D.:_Declassified> a <http://dbkwik.webdatacommons.org/marvelcinematicuniverse.wikia.com/class/web_series> ;
    rdfs:label "Agents of S.H.I.E.L.D.: Declassified"^^rdf:langString ;
    rdfs:comment """Agents of S.H.I.E.L.D.: Declassified is a companion series to the first season of Agents of S.H.I.E.L.D. hosted by Brett Erlich. It features recaps, sketches and featurettes to bring fans up to speed.

"""@en .

<http://dbkwik.webdatacommons.org/marvelcinematicuniverse.wikia.com/resource/Agents_of_S.H.I.E.L.D.:_Fallen_Agent> a <http://dbkwik.webdatacommons.org/marvelcinematicuniverse.wikia.com/class/marvel> ;
    rdfs:label "Agents of S.H.I.E.L.D.: Fallen Agent"^^rdf:langString ;
    rdfs:comment """Agents of S.H.I.E.L.D. Fallen Agent is an event that serves as the conclusion for the third season of Agents of S.H.I.E.L.D.. It focuses on the inevitable death of one of the S.H.I.E.L.D. agents.

"""@en .

<http://dbkwik.webdatacommons.org/marvelcinematicuniverse.wikia.com/resource/Agents_of_S.H.I.E.L.D.:_Ghost_Rider> a <http://dbkwik.webdatacommons.org/marvelcinematicuniverse.wikia.com/class/reflist> ;
    rdfs:label "Agents of S.H.I.E.L.D.: Ghost Rider"^^rdf:langString ;
    rdfs:comment """Agents of S.H.I.E.L.D. Ghost Rider is an event that serves as the first of the fourth season of Agents of S.H.I.E.L.D.. It focuses on Ghost Rider's introduction into the Marvel Cinematic Universe.

"""@en .

<http://dbkwik.webdatacommons.org/marvelcinematicuniverse.wikia.com/resource/Agents_of_S.H.I.E.L.D.:_LMD> a <http://dbkwik.webdatacommons.org/marvelcinematicuniverse.wikia.com/class/otheruses> ;
    rdfs:label "Agents of S.H.I.E.L.D.: LMD"^^rdf:langString ;
    rdfs:comment """Agents of S.H.I.E.L.D. LMD is an event that serves as the second of the fourth season of Agents of S.H.I.E.L.D.. It focuses on the proliferation of Life-Model Decoys.

"""@en .

<http://dbkwik.webdatacommons.org/marvelcinematicuniverse.wikia.com/resource/Agents_of_S.H.I.E.L.D.:_Season_Four_Declassified> a <http://dbkwik.webdatacommons.org/marvelcinematicuniverse.wikia.com/class/book> ;
    rdfs:label "Agents of S.H.I.E.L.D.: Season Four Declassified"^^rdf:langString ;
    ns1:author <http://dbkwik.webdatacommons.org/marvelcinematicuniverse.wikia.com/resource/Troy_Benjamin> ;
    ns1:media "Behind-the-Scenes art book"^^rdf:langString ;
    ns1:pages 240 ;
    ns1:released "2017-09-26"^^xsd:date ;
    rdfs:comment """Agents of S.H.I.E.L.D.: Season Four Declassified is the official artbook and behind-the-scenes story about the fourth season of Agents of S.H.I.E.L.D..

"""@en .

<http://dbkwik.webdatacommons.org/marvelcinematicuniverse.wikia.com/resource/Agents_of_S.H.I.E.L.D.:_Season_One_Declassified> a <http://dbkwik.webdatacommons.org/marvelcinematicuniverse.wikia.com/class/book> ;
    rdfs:label "Agents of S.H.I.E.L.D.: Season One Declassified"^^rdf:langString ;
    ns1:author <http://dbkwik.webdatacommons.org/marvelcinematicuniverse.wikia.com/resource/Troy_Benjamin> ;
    ns1:media "Behind-the-Scenes art book"^^rdf:langString ;
    ns1:pages 240 ;
    ns1:publisher <http://dbkwik.webdatacommons.org/marvelcinematicuniverse.wikia.com/resource/Dan_Buckley> ;
    ns1:released "2014-07-29"^^xsd:date ;
    rdfs:comment """Agents of S.H.I.E.L.D.: Season One Declassified is the official artbook and behind-the-scenes story about the first season of Agents of S.H.I.E.L.D..

"""@en .

<http://dbkwik.webdatacommons.org/marvelcinematicuniverse.wikia.com/resource/Agents_of_S.H.I.E.L.D.:_Season_Three_Declassified> a <http://dbkwik.webdatacommons.org/marvelcinematicuniverse.wikia.com/class/book> ;
    rdfs:label "Agents of S.H.I.E.L.D.: Season Three Declassified"^^rdf:langString ;
    ns1:author <http://dbkwik.webdatacommons.org/marvelcinematicuniverse.wikia.com/resource/Troy_Benjamin> ;
    ns1:media "Behind-the-Scenes art book"^^rdf:langString ;
    ns1:pages 248 ;
    ns1:released "Oktober 4, 2016"^^rdf:langString ;
    rdfs:comment """Agents of S.H.I.E.L.D.: Season Three Declassified is the official artbook and behind-the-scenes story about the third season of Agents of S.H.I.E.L.D..

"""@en .

<http://dbkwik.webdatacommons.org/marvelcinematicuniverse.wikia.com/resource/Agents_of_S.H.I.E.L.D.:_Season_Two_Declassified> rdfs:label "Agents of S.H.I.E.L.D.: Season Two Declassified"^^rdf:langString ;
    ns1:author <http://dbkwik.webdatacommons.org/marvelcinematicuniverse.wikia.com/resource/Troy_Benjamin> ;
    rdfs:comment """Agents of S.H.I.E.L.D.: Season Two Declassified is the official artbook and behind-the-scenes story about the second season of Agents of S.H.I.E.L.D..

"""@en .

<http://dbkwik.webdatacommons.org/marvelcinematicuniverse.wikia.com/resource/Agents_of_S.H.I.E.L.D.:_Slingshot> a <http://dbkwik.webdatacommons.org/marvelcinematicuniverse.wikia.com/class/web_series> ;
    rdfs:label "Agents of S.H.I.E.L.D.: Slingshot"^^rdf:langString ;
    rdfs:comment """Marvel’s Agents of S.H.I.E.L.D.: Slingshot or simply Agents of S.H.I.E.L.D.: Slingshot is a web series following Elena “Yo-Yo” Rodriguez, Inhuman agent of S.H.I.E.L.D.. The series is a spin-off to Agents of S.H.I.E.L.D. with its framing story taking place mid-fourth season, while the main story itself takes place slightly before it. It premiered on the ABC app, ABC.com,Marvel.com and YouTube on December 13, 2016.

"""@en .

<http://dbkwik.webdatacommons.org/marvelcinematicuniverse.wikia.com/resource/Agents_of_S.H.I.E.L.D.:_The_Chase> a <http://dbkwik.webdatacommons.org/marvelcinematicuniverse.wikia.com/class/comic> ;
    rdfs:label "Agents of S.H.I.E.L.D.: The Chase"^^rdf:langString ;
    ns6:_ 1 ;
    ns1:artists <http://dbkwik.webdatacommons.org/marvelcinematicuniverse.wikia.com/resource/Chris_Sotomayor>,
        <http://dbkwik.webdatacommons.org/marvelcinematicuniverse.wikia.com/resource/Frank_D%27Armata> ;
    ns1:editorinchief <http://dbkwik.webdatacommons.org/marvelcinematicuniverse.wikia.com/resource/Axel_Alonso> ;
    ns1:release "2014-07-24"^^xsd:date ;
    ns1:writers <http://dbkwik.webdatacommons.org/marvelcinematicuniverse.wikia.com/resource/George_Kitson> ;
    rdfs:comment """Agents of S.H.I.E.L.D.: The Chase is a comic sponsored by Lexus available exclusively at the 2014 San Diego Comic-Con or digitally to subscribers of the Marvel Unlimited program. The comic is based on the Agents of S.H.I.E.L.D. television series, and takes place soon after the first season episode Seeds.

"""@en .

<http://dbkwik.webdatacommons.org/marvelcinematicuniverse.wikia.com/resource/Agents_of_S.H.I.E.L.D.:_Uprising> a <http://dbkwik.webdatacommons.org/marvelcinematicuniverse.wikia.com/class/marvel> ;
    rdfs:label "Agents of S.H.I.E.L.D.: Uprising"^^rdf:langString ;
    rdfs:comment """Agents of S.H.I.E.L.D. Uprising is a that serves as a tie-in of the Agents of S.H.I.E.L.D. television series with the Captain America: The Winter Soldier movie.

"""@en .

<http://dbkwik.webdatacommons.org/marvelcinematicuniverse.wikia.com/resource/Agents_of_S.H.I.E.L.D._(Season_One)/Home_Video> a <http://dbkwik.webdatacommons.org/marvelcinematicuniverse.wikia.com/class/dvd> ;
    rdfs:label "Agents of S.H.I.E.L.D. (Season One)/Home Video"^^rdf:langString ;
    ns1:release "2014-09-09"^^xsd:date ;
    ns1:runtime "56760.0"^^<http://dbkwik.webdatacommons.org/datatype/second> ;
    ns1:series <http://dbkwik.webdatacommons.org/marvelcinematicuniverse.wikia.com/resource/Agents_of_S.H.I.E.L.D.> ;
    rdfs:comment """Agents of S.H.I.E.L.D. - The Complete First Season is the DVD and Blu-ray release for Agents of S.H.I.E.L.D. Season One.

"""@en .

<http://dbkwik.webdatacommons.org/marvelcinematicuniverse.wikia.com/resource/Agents_of_S.H.I.E.L.D._(Season_Three)/Home_Video> a <http://dbkwik.webdatacommons.org/marvelcinematicuniverse.wikia.com/class/dvd> ;
    rdfs:label "Agents of S.H.I.E.L.D. (Season Three)/Home Video"^^rdf:langString ;
    ns1:series <http://dbkwik.webdatacommons.org/marvelcinematicuniverse.wikia.com/resource/Agents_of_S.H.I.E.L.D.> ;
    rdfs:comment """Agents of S.H.I.E.L.D. - The Complete Third Season is the DVD and Blu-ray release for Agents of S.H.I.E.L.D. Season Three.

"""@en .

<http://dbkwik.webdatacommons.org/marvelcinematicuniverse.wikia.com/resource/Agents_of_S.H.I.E.L.D._(soundtrack)> a <http://dbkwik.webdatacommons.org/marvelcinematicuniverse.wikia.com/class/soundtrack> ;
    rdfs:label "Agents of S.H.I.E.L.D. (soundtrack)"^^rdf:langString ;
    ns1:composer <http://dbkwik.webdatacommons.org/marvelcinematicuniverse.wikia.com/resource/Bear_McCreary> ;
    ns1:producer <http://dbkwik.webdatacommons.org/marvelcinematicuniverse.wikia.com/resource/Bear_McCreary> ;
    ns1:runtime "4672.0"^^<http://dbkwik.webdatacommons.org/datatype/second> ;
    rdfs:comment """Marvel's Agents of S.H.I.E.L.D. (Original Soundtrack Album) is the soundtrack for the series of the same name. It was released on September 4, 2015.

"""@en .

<http://dbkwik.webdatacommons.org/marvelcinematicuniverse.wikia.com/resource/Agnes_Kitsworth> rdfs:label "Agnes Kitsworth"^^rdf:langString ;
    ns1:dod <http://dbkwik.webdatacommons.org/marvelcinematicuniverse.wikia.com/resource/2017> ;
    rdfs:comment """Agnes Kitsworth was an art collector and Holden Radcliffe's former romantic interest. After he left her to find a cure for her brain tumor, Radcliffe used Kitsworth's semblances to create a body for his assistant Aida while she went to live out her days in peace. Eventually Kitsworth was approached by S.H.I.E.L.D. who were attempting to arrest Radcliffe, but Kitsworth instead sided with her ex-partner and allowed him to log her into the Framework, where her mind could live in peace while her body died. Despite living with Radcliffe in the virtual world for a time, Kitsworth was confronted by HYDRA and Leo Fitz, who executed Kitsworth when Madame Hydra convinced Fitz that Kitsworth was a clone.

"""@en .

<http://dbkwik.webdatacommons.org/marvelcinematicuniverse.wikia.com/resource/Ahmed> rdfs:label "Ahmed"^^rdf:langString ;
    ns1:dod <http://dbkwik.webdatacommons.org/marvelcinematicuniverse.wikia.com/resource/2000s> ;
    rdfs:comment """Ahmed was a member of the Ten Rings. He was killed by Obadiah Stane.

"""@en .

<http://dbkwik.webdatacommons.org/marvelcinematicuniverse.wikia.com/resource/Aida> rdfs:label "Aida"^^rdf:langString ;
    ns1:dob <http://dbkwik.webdatacommons.org/marvelcinematicuniverse.wikia.com/resource/2016>,
        <http://dbkwik.webdatacommons.org/marvelcinematicuniverse.wikia.com/resource/2017> ;
    ns1:dod <http://dbkwik.webdatacommons.org/marvelcinematicuniverse.wikia.com/resource/2017> ;
    ns1:title <http://dbkwik.webdatacommons.org/marvelcinematicuniverse.wikia.com/resource/HYDRA_(Framework)> ;
    ns1:voiceActor <http://dbkwik.webdatacommons.org/marvelcinematicuniverse.wikia.com/resource/Amanda_Rea> ;
    rdfs:comment """Artificial Intelligent Digital Assistant (A.I.D.A.) was originally a Life-Model Decoy created by Holden Radcliffe from a defunct S.H.I.E.L.D. program. Physically modeled after Radcliffe's former love interest Agnes Kitsworth, Aida was initially kept secret from the public as her presence was in violation of the Sokovia Accords. Under Radcliffe's supervision, Aida became a valued S.H.I.E.L.D. asset, saving Melinda May, rescuing Phil Coulson and Leo Fitz from Hell, and stopping Eli Morrow from destroying Los Angeles.
"""@en .

<http://dbkwik.webdatacommons.org/marvelcinematicuniverse.wikia.com/resource/Aida_Mashaka_Croal> rdfs:label "Aida Mashaka Croal"^^rdf:langString ;
    ns1:produced <http://dbkwik.webdatacommons.org/marvelcinematicuniverse.wikia.com/resource/Luke_Cage_(TV_series)> ;
    ns1:wrote <http://dbkwik.webdatacommons.org/marvelcinematicuniverse.wikia.com/resource/AKA_Freak_Accident>,
        <http://dbkwik.webdatacommons.org/marvelcinematicuniverse.wikia.com/resource/AKA_Pork_Chop> ;
    rdfs:comment """Aida Mashaka Croal was a producer of Luke Cage.
She also wrote the Luke Cage episodes Blowin' Up the Spot, The Basement and Can't Front on Me and the Jessica Jones episodes AKA Freak Accident and AKA Pork Chop.
She also co-wrote the Luke Cage episode You Know My Steez with Cheo Hodari Coker.

"""@en .

<http://dbkwik.webdatacommons.org/marvelcinematicuniverse.wikia.com/resource/Air_Crash_in_the_Himalayas> a <http://dbkwik.webdatacommons.org/marvelcinematicuniverse.wikia.com/class/event> ;
    rdfs:label "Air Crash in the Himalayas"^^rdf:langString ;
    ns1:casualties <http://dbkwik.webdatacommons.org/marvelcinematicuniverse.wikia.com/resource/Heather_Rand>,
        <http://dbkwik.webdatacommons.org/marvelcinematicuniverse.wikia.com/resource/Wendell_Rand> ;
    ns1:executor <http://dbkwik.webdatacommons.org/marvelcinematicuniverse.wikia.com/resource/Harold_Meachum> ;
    ns1:planner <http://dbkwik.webdatacommons.org/marvelcinematicuniverse.wikia.com/resource/Hand>,
        <http://dbkwik.webdatacommons.org/marvelcinematicuniverse.wikia.com/resource/Harold_Meachum> ;
    ns1:result <http://dbkwik.webdatacommons.org/marvelcinematicuniverse.wikia.com/resource/Harold_Meachum> ;
    ns1:target <http://dbkwik.webdatacommons.org/marvelcinematicuniverse.wikia.com/resource/Wendell_Rand> ;
    ns1:type "Assassination attempt"^^rdf:langString ;
    rdfs:comment """The Air Crash in the Himalayas was an assassination orchestrated by Harold Meachum and Madame Gao and staged as an air crash accident, in order to prevent Wendell Rand from exposing the illegal activities being conducted within Rand Enterprises. Danny Rand became the lone survivor and was rescued by the monks of K'un-Lun.

"""@en .

<http://dbkwik.webdatacommons.org/marvelcinematicuniverse.wikia.com/resource/Air_Force_One> a <http://dbkwik.webdatacommons.org/marvelcinematicuniverse.wikia.com/class/vehicle> ;
    rdfs:label "Air Force One"^^rdf:langString ;
    ns1:passengers <http://dbkwik.webdatacommons.org/marvelcinematicuniverse.wikia.com/resource/Eric_Savin>,
        <http://dbkwik.webdatacommons.org/marvelcinematicuniverse.wikia.com/resource/Heather> ;
    rdfs:comment """Air Force One is the designation given to any United States Air Force aircraft transporting the President of the United States of America. "Air Force One" is typically used to refer to the two highly modified 747s that normally transport the president (tail numbers 28000 and 29000).

"""@en .

<http://dbkwik.webdatacommons.org/marvelcinematicuniverse.wikia.com/resource/Akela_Cooper> rdfs:label "Akela Cooper"^^rdf:langString ;
    ns1:produced <http://dbkwik.webdatacommons.org/marvelcinematicuniverse.wikia.com/resource/Luke_Cage_(TV_series)> ;
    ns1:wrote <http://dbkwik.webdatacommons.org/marvelcinematicuniverse.wikia.com/resource/Luke_Cage_(TV_series)>,
        <http://dbkwik.webdatacommons.org/marvelcinematicuniverse.wikia.com/resource/Manifest> ;
    rdfs:comment """Akela Cooper was a producer of Luke Cage. She also wrote the Luke Cage episodes Manifest, Straighten It Out and The Main Ingredient and co-wrote the Luke Cage episode Soliloquy of Chaos with Charles Murray.

"""@en .

<http://dbkwik.webdatacommons.org/marvelcinematicuniverse.wikia.com/resource/Alan_Taylor> rdfs:label "Alan Taylor"^^rdf:langString ;
    ns1:directed <http://dbkwik.webdatacommons.org/marvelcinematicuniverse.wikia.com/resource/Thor:_The_Dark_World> ;
    ns1:documentary <http://dbkwik.webdatacommons.org/marvelcinematicuniverse.wikia.com/resource/Marvel_Studios:_Assembling_a_Universe> ;
    rdfs:comment """Alan Taylor directed Thor: The Dark World.
He was interviewed for the documentary Marvel Studios: Assembling a Universe.

"""@en .

<http://dbkwik.webdatacommons.org/marvelcinematicuniverse.wikia.com/resource/Alaska> rdfs:label "Alaska"^^rdf:langString ;
    ns1:interest <http://dbkwik.webdatacommons.org/marvelcinematicuniverse.wikia.com/resource/Barrow> ;
    rdfs:comment """Alaska is a non-contiguous American state located in the northwestern region of North America.

"""@en .

<http://dbkwik.webdatacommons.org/marvelcinematicuniverse.wikia.com/resource/Aldrich_Killian%27s_War> a <http://dbkwik.webdatacommons.org/marvelcinematicuniverse.wikia.com/class/war> ;
    rdfs:label "Aldrich Killian's War"^^rdf:langString ;
    ns1:battles <http://dbkwik.webdatacommons.org/marvelcinematicuniverse.wikia.com/resource/Battle_of_Rose_Hill>,
        <http://dbkwik.webdatacommons.org/marvelcinematicuniverse.wikia.com/resource/Battle_on_the_Norco> ;
    ns1:casualties <http://dbkwik.webdatacommons.org/marvelcinematicuniverse.wikia.com/resource/Aldrich_Killian>,
        <http://dbkwik.webdatacommons.org/marvelcinematicuniverse.wikia.com/resource/Chad_Davis> ;
    ns1:commanders <http://dbkwik.webdatacommons.org/marvelcinematicuniverse.wikia.com/resource/Aldrich_Killian> ;
    ns1:conc <http://dbkwik.webdatacommons.org/marvelcinematicuniverse.wikia.com/resource/Chitauri_Invasion>,
        <http://dbkwik.webdatacommons.org/marvelcinematicuniverse.wikia.com/resource/Ego%27s_Expansion> ;
    ns1:place <http://dbkwik.webdatacommons.org/marvelcinematicuniverse.wikia.com/resource/United_States_of_America> ;
    ns1:side <http://dbkwik.webdatacommons.org/marvelcinematicuniverse.wikia.com/resource/Iron_Man> ;
    rdfs:comment """Aldrich Killian's War was a series of attacks executed by Aldrich Killian in his plan to gain control of the United States of America. Using Maya Hansen's research on the Extremis virus, Killian turned dozens of amputees and other disabled people into loyal super soldiers. 
When several of Killian's failed experiments resulted in the deaths of innocent civilians, he decided to masquerade them as terrorist attacks and hired actor Trevor Slattery to take responsibility by posing as the Mandarin, the leader of the Ten Rings.
"""@en .

<http://dbkwik.webdatacommons.org/marvelcinematicuniverse.wikia.com/resource/Aleta_Ravager_Clan> rdfs:label "Aleta Ravager Clan"^^rdf:langString ;
    ns1:founder <http://dbkwik.webdatacommons.org/marvelcinematicuniverse.wikia.com/resource/Aleta_Ogord> ;
    ns1:headquarters <http://dbkwik.webdatacommons.org/marvelcinematicuniverse.wikia.com/resource/Aleta_Ogord_Warship> ;
    ns1:leader <http://dbkwik.webdatacommons.org/marvelcinematicuniverse.wikia.com/resource/Aleta_Ogord> ;
    rdfs:comment """Aleta Ravager Clan is one of the hundred clans of the Ravagers. Distinguished by their dark green garbs, this clan is lead by Aleta Ogord.

"""@en .

<http://dbkwik.webdatacommons.org/marvelcinematicuniverse.wikia.com/resource/Alexander_Pierce> rdfs:label "Alexander Pierce"^^rdf:langString ;
    ns1:clearance <http://dbkwik.webdatacommons.org/marvelcinematicuniverse.wikia.com/resource/Clearance_Level> ;
    rdfs:comment """Alexander Goodwin Pierce was one of HYDRA's leaders and its top undercover operative inside the United States Government, S.H.I.E.L.D., and the World Security Council. He commanded the HYDRA forces within S.H.I.E.L.D., working to create a world so chaotic, that its people would give up their own freedoms willingly. To that end, he created Project Insight, a project that would have given HYDRA absolute control over the world, inciting the HYDRA Uprising. His plan was stopped by Captain America, Black Widow, Falcon, Maria Hill, and Nick Fury during the Battle at the Triskelion, in which he was killed by Director Fury.

"""@en .

<http://dbkwik.webdatacommons.org/marvelcinematicuniverse.wikia.com/resource/Alfheim> rdfs:label "Alfheim"^^rdf:langString ;
    ns1:population <http://dbkwik.webdatacommons.org/marvelcinematicuniverse.wikia.com/resource/Light_Elves> ;
    rdfs:comment """Alfheim is one of the Nine Realms and the home of the Light Elves.

"""@en .

<http://dbkwik.webdatacommons.org/marvelcinematicuniverse.wikia.com/resource/Algiers> rdfs:label "Algiers"^^rdf:langString ;
    ns1:coat 40 ;
    rdfs:comment """Algiers is the capital of Algeria.

"""@en .

<http://dbkwik.webdatacommons.org/marvelcinematicuniverse.wikia.com/resource/Alias_Investigations> rdfs:label "Alias Investigations"^^rdf:langString ;
    ns1:founder <http://dbkwik.webdatacommons.org/marvelcinematicuniverse.wikia.com/resource/Jessica_Jones> ;
    rdfs:comment """Alias Investigations is a detective agency owned by Jessica Jones. The detective agency used to have only one employee, Jones herself, and operates out of a run down office, that also serves as Jones' apartment. Following Kilgrave's death, Malcolm Ducasse joined the agency and received some training in becoming a private investigator himself before decidingly removing from the agency.

"""@en .

<http://dbkwik.webdatacommons.org/marvelcinematicuniverse.wikia.com/resource/Alisa_Jones> rdfs:label "Alisa Jones"^^rdf:langString ;
    ns1:dob <http://dbkwik.webdatacommons.org/marvelcinematicuniverse.wikia.com/resource/1950s> ;
    ns1:idno 46592 ;
    rdfs:comment """Alisa Jones (née Campbell) was Jessica and Phillip Jones' mother. She was seemingly killed in a car accident along her husband and son, with her daughter as the sole survivor. However, unknown to Jessica, she was brought back to life by Karl Malus' illegal experiments at IGH, which also gave her superhuman abilities. After escaping and accidentally killing Jessica's boyfriend, she stayed in the shadows with Malus, becoming life partners.
"""@en .

<http://dbkwik.webdatacommons.org/marvelcinematicuniverse.wikia.com/resource/All_the_Stars> a <http://dbkwik.webdatacommons.org/marvelcinematicuniverse.wikia.com/class/song> ;
    rdfs:label "All the Stars"^^rdf:langString ;
    ns1:composer <http://dbkwik.webdatacommons.org/marvelcinematicuniverse.wikia.com/resource/Kendrick_Lamar>,
        <http://dbkwik.webdatacommons.org/marvelcinematicuniverse.wikia.com/resource/SZA> ;
    ns1:performer <http://dbkwik.webdatacommons.org/marvelcinematicuniverse.wikia.com/resource/Kendrick_Lamar>,
        <http://dbkwik.webdatacommons.org/marvelcinematicuniverse.wikia.com/resource/SZA> ;
    ns1:runtime "236.0"^^<http://dbkwik.webdatacommons.org/datatype/second> ;
    rdfs:comment """"All the Stars" is a song recorded by Kendrick Lamar and SZA for Black Panther: The Album. It was released as a single on January 4, 2018.

"""@en .

<http://dbkwik.webdatacommons.org/marvelcinematicuniverse.wikia.com/resource/Allen_Maldonado> rdfs:label "Allen Maldonado"^^rdf:langString ;
    ns1:oneshot <http://dbkwik.webdatacommons.org/marvelcinematicuniverse.wikia.com/resource/Marvel_One-Shot:_All_Hail_the_King> ;
    rdfs:comment """Allen Maldonado portrayed Fletcher Heggs in Marvel One-Shot: All Hail the King.

"""@en .

<http://dbkwik.webdatacommons.org/marvelcinematicuniverse.wikia.com/resource/Allentown> rdfs:label "Allentown"^^rdf:langString ;
    ns1:oneshot <http://dbkwik.webdatacommons.org/marvelcinematicuniverse.wikia.com/resource/Marvel_One-Shot:_Item_47> ;
    rdfs:comment """Allentown is located in the state of Pennsylvania.

"""@en .

<http://dbkwik.webdatacommons.org/marvelcinematicuniverse.wikia.com/resource/Alphonso_Mackenzie> rdfs:label "Alphonso Mackenzie"^^rdf:langString ;
    ns1:before <http://dbkwik.webdatacommons.org/marvelcinematicuniverse.wikia.com/resource/Patriot> ;
    ns1:clearance <http://dbkwik.webdatacommons.org/marvelcinematicuniverse.wikia.com/resource/Clearance_Level> ;
    ns1:years 2018 ;
    rdfs:comment "Alphonso \"Mack\" Mackenzie is the Director of S.H.I.E.L.D. Despite the heavy casualties S.H.I.E.L.D. took during HYDRA's attack on it, he stayed loyal to his oath and continued his service in the remains of S.H.I.E.L.D. under Robert Gonzales. However, as another faction of S.H.I.E.L.D. led by Phil Coulson emerged, he was sent alongside Bobbi Morse and Isabelle Hartley to infiltrate it. Now working undercover, he pretended to be a simple mechanic while searching for Nick Fury's Toolbox. When the truth was revealed, Mackenzie's colleagues quickly attacked and occupied the Playground, taking control over most of S.H.I.E.L.D. However, the two factions eventually managed to put aside their differences and work together against HYDRA. When S.H.I.E.L.D."@en .

<http://dbkwik.webdatacommons.org/marvelcinematicuniverse.wikia.com/resource/Alphonso_Mackenzie_(Life-Model_Decoy)> rdfs:label "Alphonso Mackenzie (Life-Model Decoy)"^^rdf:langString ;
    ns1:dob <http://dbkwik.webdatacommons.org/marvelcinematicuniverse.wikia.com/resource/2017> ;
    rdfs:comment """Alphonso Mackenzie was the Life-Model Decoy of the real Alphonso Mackenzie who was sent on a secret mission by Holden Radcliffe to infiltrate S.H.I.E.L.D. and execute all the Inhumans for Anton Ivanov. The LMD's plan was revealed however and Mack's LMD hunted down Quake and Jemma Simmons, only to eventually be destroyed by a powerful shockwave caused by Quake.

"""@en .

<http://dbkwik.webdatacommons.org/marvelcinematicuniverse.wikia.com/resource/Ambush_at_Bay_Ridge_Rail_Yard> a <http://dbkwik.webdatacommons.org/marvelcinematicuniverse.wikia.com/class/conflict> ;
    rdfs:label "Ambush at Bay Ridge Rail Yard"^^rdf:langString ;
    ns1:place <http://dbkwik.webdatacommons.org/marvelcinematicuniverse.wikia.com/resource/Bay_Ridge_Rail_Yard>,
        <http://dbkwik.webdatacommons.org/marvelcinematicuniverse.wikia.com/resource/New_York> ;
    ns1:side <http://dbkwik.webdatacommons.org/marvelcinematicuniverse.wikia.com/resource/Daredevil> ;
    rdfs:comment """The Ambush at Bay Ridge Rail Yard was a trap planned by Yakuza in order to eluminate Daredevil and Elektra who investigated criminal activity in New York City.

"""@en .

<http://dbkwik.webdatacommons.org/marvelcinematicuniverse.wikia.com/resource/Ambush_at_Colleen_O%27Brien%27s_Apartment> a <http://dbkwik.webdatacommons.org/marvelcinematicuniverse.wikia.com/class/conflict> ;
    rdfs:label "Ambush at Colleen O'Brien's Apartment"^^rdf:langString ;
    rdfs:comment """The Ambush at Colleen O'Brien's Apartment was an attack on Peggy Carter by the Leviathan operative Sasha Demidov.

"""@en .

<http://dbkwik.webdatacommons.org/marvelcinematicuniverse.wikia.com/resource/Ambush_at_Declan_Research_Facility_Lab> a <http://dbkwik.webdatacommons.org/marvelcinematicuniverse.wikia.com/class/conflict> ;
    rdfs:label "Ambush at Declan Research Facility Lab"^^rdf:langString ;
    ns1:war <http://dbkwik.webdatacommons.org/marvelcinematicuniverse.wikia.com/resource/Uprising_in_Attilan> ;
    rdfs:comment """The Ambush at Declan Research Facility Lab was a confrontation between a group of Attilan rebels led by Auran and the former King of Attilan Black Bolt, who they had been sent to capture. Although Black Bolt was outnumbered, he managed to escape thanks to the interference of his wife Medusa and her friend Louise Fisher, who helped him to escape after capturing the rebel Locus.

"""@en .

<http://dbkwik.webdatacommons.org/marvelcinematicuniverse.wikia.com/resource/Ambush_at_Elektra_Natchios%27_Penthouse> a <http://dbkwik.webdatacommons.org/marvelcinematicuniverse.wikia.com/class/conflict> ;
    rdfs:label "Ambush at Elektra Natchios' Penthouse"^^rdf:langString ;
    ns1:date <http://dbkwik.webdatacommons.org/marvelcinematicuniverse.wikia.com/resource/2015> ;
    rdfs:comment """The Ambush at Elektra Natchios' Penthouse was a retaliation made by members of the of the Hand, led by Hirochi and disguised as Yakuza members, over the hacker that managed to obtain classified files from the Yakatomi Building.

"""@en .

<http://dbkwik.webdatacommons.org/marvelcinematicuniverse.wikia.com/resource/Ambush_at_Harold_Meachum%27s_Penthouse> rdfs:label "Ambush at Harold Meachum's Penthouse"^^rdf:langString ;
    ns1:date <http://dbkwik.webdatacommons.org/marvelcinematicuniverse.wikia.com/resource/2016> ;
    rdfs:comment """The Ambush at Harold Meachum's Penthouse was a confrontation on the Hand leader, Bakuto during his attempt to capture Iron Fist. After holding the Meachums hostage and wounding Joy Meachum, Bakuto lured Iron Fist to the penthouse to seize him. Once they have captured him, Bakuto and his men were ambushed by Colleen Wing and Davos, revealing that they already prepared a plan to fight him.

"""@en .

<http://dbkwik.webdatacommons.org/marvelcinematicuniverse.wikia.com/resource/Ambush_at_Matt_Murdock%27s_Apartment> a <http://dbkwik.webdatacommons.org/marvelcinematicuniverse.wikia.com/class/event> ;
    rdfs:label "Ambush at Matt Murdock's Apartment"^^rdf:langString ;
    ns1:date <http://dbkwik.webdatacommons.org/marvelcinematicuniverse.wikia.com/resource/2015> ;
    ns1:executor <http://dbkwik.webdatacommons.org/marvelcinematicuniverse.wikia.com/resource/Hand> ;
    ns1:planner <http://dbkwik.webdatacommons.org/marvelcinematicuniverse.wikia.com/resource/Hand> ;
    ns1:target <http://dbkwik.webdatacommons.org/marvelcinematicuniverse.wikia.com/resource/Daredevil>,
        <http://dbkwik.webdatacommons.org/marvelcinematicuniverse.wikia.com/resource/Elektra> ;
    ns1:type "Assassination attempt"^^rdf:langString ;
    rdfs:comment """The Ambush at Matt Murdock's Apartment was an failed assassination attempt on Matt Murdock and Elektra orchestrated by Hand.

"""@en .

<http://dbkwik.webdatacommons.org/marvelcinematicuniverse.wikia.com/resource/Ambush_at_Primed_and_Ready_Fireworks> rdfs:label "Ambush at Primed and Ready Fireworks"^^rdf:langString ;
    ns1:date <http://dbkwik.webdatacommons.org/marvelcinematicuniverse.wikia.com/resource/2017> ;
    rdfs:comment """The Ambush at Primed and Ready Fireworks was Hellfire's revenge on Quake for putting him through Terrigenesis.

"""@en .

<http://dbkwik.webdatacommons.org/marvelcinematicuniverse.wikia.com/resource/Ambush_at_the_Barbershop_Headquarters> rdfs:label "Ambush at the Barbershop Headquarters"^^rdf:langString ;
    ns1:war <http://dbkwik.webdatacommons.org/marvelcinematicuniverse.wikia.com/resource/HYDRA_Uprising> ;
    rdfs:comment """The Ambush at the Barbershop Headquarters was a trap staged by HYDRA to assassinate Phil Coulson and his S.H.I.E.L.D. team. A team of Centipede Soldiers remained in the Barbershop Headquarters waiting for S.H.I.E.L.D. to come while John Garrett and his operatives had abandoned the facility. However, the S.H.I.E.L.D. team survived the ambush.

"""@en .

<http://dbkwik.webdatacommons.org/marvelcinematicuniverse.wikia.com/resource/Ambush_at_the_Belgium_Safe_House> rdfs:label "Ambush at the Belgium Safe House"^^rdf:langString ;
    ns1:war <http://dbkwik.webdatacommons.org/marvelcinematicuniverse.wikia.com/resource/War_on_HYDRA> ;
    rdfs:comment """The Ambush at the Belgium Safe House was a failed attempt by HYDRA to exact vengeance against S.H.I.E.L.D. for infiltrating their organization.

"""@en .

<http://dbkwik.webdatacommons.org/marvelcinematicuniverse.wikia.com/resource/Ambush_at_the_Distant_Star_Facility> rdfs:label "Ambush at the Distant Star Facility"^^rdf:langString ;
    ns1:conc <http://dbkwik.webdatacommons.org/marvelcinematicuniverse.wikia.com/resource/Kidnapping_of_Thomas_Ward> ;
    ns1:war <http://dbkwik.webdatacommons.org/marvelcinematicuniverse.wikia.com/resource/Grant_Ward%27s_Campaign> ;
    rdfs:comment """The Ambush at the Distant Star Facility was a kidnapping orchestrated by HYDRA on S.H.I.E.L.D. agents Leo Fitz and Jemma Simmons, whom they believed could help HYDRA achieve their oldest goal, retrieving their leader from the distant planet where it was banished.

"""@en .

<http://dbkwik.webdatacommons.org/marvelcinematicuniverse.wikia.com/resource/Ambush_at_the_Hotel_La_Ona> rdfs:label "Ambush at the Hotel La Ona"^^rdf:langString ;
    ns1:srclink "Face My Enemy"^^rdf:langString ;
    ns1:war <http://dbkwik.webdatacommons.org/marvelcinematicuniverse.wikia.com/resource/War_on_HYDRA> ;
    rdfs:comment """The Ambush at the Hotel La Ona was a trap set by HYDRA in order to obtain a painting and prevent S.H.I.E.L.D. from further deciphering the Words of Creation.

"""@en .

<http://dbkwik.webdatacommons.org/marvelcinematicuniverse.wikia.com/resource/Ambush_in_Afterlife> rdfs:label "Ambush in Afterlife"^^rdf:langString ;
    ns1:executor <http://dbkwik.webdatacommons.org/marvelcinematicuniverse.wikia.com/resource/Jiaying> ;
    ns1:planner <http://dbkwik.webdatacommons.org/marvelcinematicuniverse.wikia.com/resource/Jiaying> ;
    rdfs:comment """The Ambush in Afterlife was a trap staged by Jiaying in order to make the Inhumans follow her into a war against S.H.I.E.L.D. by making apparent that they were the ones who attacked first.

"""@en .

<http://dbkwik.webdatacommons.org/marvelcinematicuniverse.wikia.com/resource/Ambush_on_Billy_Russo> a <http://dbkwik.webdatacommons.org/marvelcinematicuniverse.wikia.com/class/event> ;
    rdfs:label "Ambush on Billy Russo"^^rdf:langString ;
    ns1:planner <http://dbkwik.webdatacommons.org/marvelcinematicuniverse.wikia.com/resource/Dinah_Madani> ;
    ns1:target <http://dbkwik.webdatacommons.org/marvelcinematicuniverse.wikia.com/resource/Billy_Russo> ;
    rdfs:comment """The Ambush on Billy Russo was an attempt by Dinah Madani and her Homeland Security colleagues to apprehend Billy Russo.

"""@en .

<http://dbkwik.webdatacommons.org/marvelcinematicuniverse.wikia.com/resource/Ambush_on_Luke_Cage> a <http://dbkwik.webdatacommons.org/marvelcinematicuniverse.wikia.com/class/event> ;
    rdfs:label "Ambush on Luke Cage"^^rdf:langString ;
    ns1:executor <http://dbkwik.webdatacommons.org/marvelcinematicuniverse.wikia.com/resource/Bushmaster> ;
    ns1:target <http://dbkwik.webdatacommons.org/marvelcinematicuniverse.wikia.com/resource/Luke_Cage> ;
    rdfs:comment """The Ambush on Luke Cage was an unexpected attack on Luke Cage orchestrated by Bushmaster.

"""@en .

<http://dbkwik.webdatacommons.org/marvelcinematicuniverse.wikia.com/resource/Ambush_on_Turk_Barrett> a <http://dbkwik.webdatacommons.org/marvelcinematicuniverse.wikia.com/class/event> ;
    rdfs:label "Ambush on Turk Barrett"^^rdf:langString ;
    ns1:executor <http://dbkwik.webdatacommons.org/marvelcinematicuniverse.wikia.com/resource/Punisher> ;
    rdfs:comment """The Ambush on Turk Barrett was an attempt by Punisher to extract information regarding the Greek Mob from local arms dealer Turk Barrett.

"""@en .

<http://dbkwik.webdatacommons.org/marvelcinematicuniverse.wikia.com/resource/Amphibian_Alien> a <http://dbkwik.webdatacommons.org/marvelcinematicuniverse.wikia.com/class/race> ;
    rdfs:label "Amphibian Alien"^^rdf:langString ;
    rdfs:comment """The Amphibian Alien is an amphibian humanoid race that has orange scaled skin and membranes between its fingers.

"""@en .

<http://dbkwik.webdatacommons.org/marvelcinematicuniverse.wikia.com/resource/Amy_Vuckovich> rdfs:label "Amy Vuckovich"^^rdf:langString ;
    ns1:directed <http://dbkwik.webdatacommons.org/marvelcinematicuniverse.wikia.com/resource/Runaways_(TV_series)> ;
    rdfs:comment """Amy Vuckovich was a set decorator of Runaways.

"""@en .

<http://dbkwik.webdatacommons.org/marvelcinematicuniverse.wikia.com/resource/Anderson_(Agent)> rdfs:label "Anderson (Agent)"^^rdf:langString ;
    ns1:clearance <http://dbkwik.webdatacommons.org/marvelcinematicuniverse.wikia.com/resource/Clearance_Level> ;
    rdfs:comment """Anderson is a S.H.I.E.L.D. agent stationed at the Playground.

"""@en .

<http://dbkwik.webdatacommons.org/marvelcinematicuniverse.wikia.com/resource/Andi_Bushell> rdfs:label "Andi Bushell"^^rdf:langString ;
    ns1:wrote <http://dbkwik.webdatacommons.org/marvelcinematicuniverse.wikia.com/resource/Agent_Carter_(TV_series)> ;
    rdfs:comment """Andi Bushell was a co-executive producer on Agent Carter, and the writer of the episode Time and Tide.

"""@en .

<http://dbkwik.webdatacommons.org/marvelcinematicuniverse.wikia.com/resource/Andy_Nicholson> a <http://dbkwik.webdatacommons.org/marvelcinematicuniverse.wikia.com/class/wp> ;
    rdfs:label "Andy Nicholson"^^rdf:langString ;
    rdfs:comment """Andy Nicholson was a supervising art director for Captain America: The First Avenger, and the production designer of Captain Marvel.

"""@en .

<http://dbkwik.webdatacommons.org/marvelcinematicuniverse.wikia.com/resource/Angola> rdfs:label "Angola"^^rdf:langString ;
    ns1:coat 35 ;
    rdfs:comment """Angola is a country located in Western Africa.

"""@en .

<http://dbkwik.webdatacommons.org/marvelcinematicuniverse.wikia.com/resource/Ant-Man:_Larger_Than_Life> a <http://dbkwik.webdatacommons.org/marvelcinematicuniverse.wikia.com/class/comic> ;
    rdfs:label "Ant-Man: Larger Than Life"^^rdf:langString ;
    ns1:artists <http://dbkwik.webdatacommons.org/marvelcinematicuniverse.wikia.com/resource/Andrea_Di_Vito>,
        <http://dbkwik.webdatacommons.org/marvelcinematicuniverse.wikia.com/resource/Clayton_Cowles> ;
    ns1:writers <http://dbkwik.webdatacommons.org/marvelcinematicuniverse.wikia.com/resource/Will_Corona_Pilgrim> ;
    rdfs:comment """Ant-Man: Larger Than Life is a comic mini-series set in the Marvel Cinematic Universe. It is set before the events of Ant-Man.

"""@en .

<http://dbkwik.webdatacommons.org/marvelcinematicuniverse.wikia.com/resource/Ant-Man_(film)/Portal> a <http://dbkwik.webdatacommons.org/marvelcinematicuniverse.wikia.com/class/box> ;
    rdfs:label "Ant-Man (film)/Portal"^^rdf:langString ;
    ns1:link <http://dbkwik.webdatacommons.org/marvelcinematicuniverse.wikia.com/resource/Ant-Man_(film)>,
        "Yellowjacket"^^rdf:langString ;
    ns1:nonlinktext "Darren Cross"^^rdf:langString,
        "Scott Lang"^^rdf:langString ;
    ns1:text "Ant-Man"^^rdf:langString,
        "Yellowjacket"^^rdf:langString ;
    rdfs:comment """Characters from Ant-Man.
"""@en .

<http://dbkwik.webdatacommons.org/marvelcinematicuniverse.wikia.com/resource/Ant-Man_(film)/Promotional_Campaign> a <http://dbkwik.webdatacommons.org/marvelcinematicuniverse.wikia.com/class/reflist> ;
    rdfs:label "Ant-Man (film)/Promotional Campaign"^^rdf:langString ;
    rdfs:comment """The Ant-Man promotion campaign is a crossmedia campaign which was set up to promote Ant-Man. It started in July 2, 2015 and consists the social media platforms YouTube, Twitter, Google+ and LinkedIn.
The campaign started with a series videos of WHiH Newsfront on YouTube focusing on Scott Lang and his future release. These videos are supported by posts on Twitter and Google+. Items from the videos were further discussed in articles on the internet, like on the website Mashable.
"""@en .

<http://dbkwik.webdatacommons.org/marvelcinematicuniverse.wikia.com/resource/Ant-Man_(soundtrack)> a <http://dbkwik.webdatacommons.org/marvelcinematicuniverse.wikia.com/class/soundtrack> ;
    rdfs:label "Ant-Man (soundtrack)"^^rdf:langString ;
    ns1:producer <http://dbkwik.webdatacommons.org/marvelcinematicuniverse.wikia.com/resource/Dave_Jordan> ;
    rdfs:comment """Ant-Man: Original Motion Picture Soundtrack is the soundtrack for the film of the same name. It was released on August 7, 2015.

"""@en .

<http://dbkwik.webdatacommons.org/marvelcinematicuniverse.wikia.com/resource/Ant-Man_-_Scott_Lang:_Small_Time> a <http://dbkwik.webdatacommons.org/marvelcinematicuniverse.wikia.com/class/comic> ;
    rdfs:label "Ant-Man - Scott Lang: Small Time"^^rdf:langString ;
    ns6:_ 1 ;
    ns1:artists <http://dbkwik.webdatacommons.org/marvelcinematicuniverse.wikia.com/resource/Andres_Mossa> ;
    ns1:writers <http://dbkwik.webdatacommons.org/marvelcinematicuniverse.wikia.com/resource/Will_Corona_Pilgrim> ;
    rdfs:comment """Ant-Man - Scott Lang: Small Time is a comic set in the Marvel Cinematic Universe. It is set three years before the events of Ant-Man.

"""@en .

<http://dbkwik.webdatacommons.org/marvelcinematicuniverse.wikia.com/resource/Ant-Man_Prelude> a <http://dbkwik.webdatacommons.org/marvelcinematicuniverse.wikia.com/class/comic> ;
    rdfs:label "Ant-Man Prelude"^^rdf:langString ;
    ns6:_ 2 ;
    ns1:writers <http://dbkwik.webdatacommons.org/marvelcinematicuniverse.wikia.com/resource/Will_Corona_Pilgrim> ;
    rdfs:comment """Ant-Man Prelude is a two-issue comic mini-series set in the Marvel Cinematic Universe. It is set before the events of Ant-Man.

"""@en .

<http://dbkwik.webdatacommons.org/marvelcinematicuniverse.wikia.com/resource/Ant-Man_Prelude_(collection)> a <http://dbkwik.webdatacommons.org/marvelcinematicuniverse.wikia.com/class/comic> ;
    rdfs:label "Ant-Man Prelude (collection)"^^rdf:langString ;
    ns1:writers <http://dbkwik.webdatacommons.org/marvelcinematicuniverse.wikia.com/resource/Will_Corona_Pilgrim> ;
    rdfs:comment """Ant-Man Prelude is a collection of comics set in the Marvel Cinematic Universe and Earth-616.

"""@en .

<http://dbkwik.webdatacommons.org/marvelcinematicuniverse.wikia.com/resource/Ant-Man_Suit> rdfs:label "Ant-Man Suit"^^rdf:langString ;
    ns1:made <http://dbkwik.webdatacommons.org/marvelcinematicuniverse.wikia.com/resource/1980s>,
        <http://dbkwik.webdatacommons.org/marvelcinematicuniverse.wikia.com/resource/2016> ;
    ns1:owners <http://dbkwik.webdatacommons.org/marvelcinematicuniverse.wikia.com/resource/Ant-Man> ;
    rdfs:comment """The Ant-Man Suit is a suit created by Hank Pym to maximize the use of the Pym Particles while also protecting the wearer from the negative side-effects of using Pym Particles.

"""@en .

<http://dbkwik.webdatacommons.org/marvelcinematicuniverse.wikia.com/resource/Ant-Man_and_the_Wasp/Portal> a <http://dbkwik.webdatacommons.org/marvelcinematicuniverse.wikia.com/class/box> ;
    rdfs:label "Ant-Man and the Wasp/Portal"^^rdf:langString ;
    ns1:nonlinktext "Ava Starr"^^rdf:langString,
        "Hope van Dyne"^^rdf:langString,
        "Scott Lang"^^rdf:langString ;
    ns1:text "Ant-Man"^^rdf:langString,
        "Ghost"^^rdf:langString,
        "Wasp"^^rdf:langString ;
    rdfs:comment """Characters from Ant-Man and the Wasp.
"""@en .

<http://dbkwik.webdatacommons.org/marvelcinematicuniverse.wikia.com/resource/Ant-Man_and_the_Wasp/Trivia> a <http://dbkwik.webdatacommons.org/marvelcinematicuniverse.wikia.com/class/stub> ;
    rdfs:label "Ant-Man and the Wasp/Trivia"^^rdf:langString ;
    rdfs:comment """A list of trivia related to Ant-Man and the Wasp.

"""@en .

<http://dbkwik.webdatacommons.org/marvelcinematicuniverse.wikia.com/resource/Ant-Man_and_the_Wasp:_The_Heroes%27_Journey> rdfs:label "Ant-Man and the Wasp: The Heroes' Journey"^^rdf:langString ;
    ns1:author <http://dbkwik.webdatacommons.org/marvelcinematicuniverse.wikia.com/resource/Steve_Behling> ;
    rdfs:comment """Avengers: Infinity War: The Heroes' Journey is a audiobook based on Ant-Man and the Wasp.

"""@en .

<http://dbkwik.webdatacommons.org/marvelcinematicuniverse.wikia.com/resource/Ant-Man_and_the_Wasp_-_Original_Motion_Picture_Soundtrack> a <http://dbkwik.webdatacommons.org/marvelcinematicuniverse.wikia.com/class/soundtrack> ;
    rdfs:label "Ant-Man and the Wasp - Original Motion Picture Soundtrack"^^rdf:langString ;
    rdfs:comment """Ant-Man and the Wasp - Original Motion Picture Soundtrack contains Christophe Beck's score to Ant-Man and the Wasp.

"""@en .

<http://dbkwik.webdatacommons.org/marvelcinematicuniverse.wikia.com/resource/Ant-Man_and_the_Wasp_Prelude> rdfs:label "Ant-Man and the Wasp Prelude"^^rdf:langString ;
    ns6:_ 2 ;
    rdfs:comment """Ant-Man and the Wasp Prelude is a comic mini-series set in the Marvel Cinematic Universe. It is set before the events of Ant-Man and the Wasp.

"""@en .

<http://dbkwik.webdatacommons.org/marvelcinematicuniverse.wikia.com/resource/Anthony_Mackie> rdfs:label "Anthony Mackie"^^rdf:langString ;
    ns1:documentary <http://dbkwik.webdatacommons.org/marvelcinematicuniverse.wikia.com/resource/Marvel_Studios:_Assembling_a_Universe> ;
    rdfs:comment """Anthony Mackie portrayed Sam Wilson/Falcon in Captain America: The Winter Soldier, Avengers: Age of Ultron, Ant-Man, Captain America: Civil War, Avengers: Infinity War and Avengers 4.
He was interviewed for the documentary Marvel Studios: Assembling a Universe.

"""@en .

<http://dbkwik.webdatacommons.org/marvelcinematicuniverse.wikia.com/resource/Anthony_Molinari> rdfs:label "Anthony Molinari"^^rdf:langString ;
    ns1:oneshot <http://dbkwik.webdatacommons.org/marvelcinematicuniverse.wikia.com/resource/Marvel_One-Shot:_Agent_Carter> ;
    rdfs:comment """Anthony Molinari portrayed Guard #1 in Marvel One-Shot: Agent Carter and Police Officer in the Cloak & Dagger episode Colony Collapse.
He was also a stunt performer in Captain America: The Winter Soldier.
He was also a stunt double for Mark Ruffalo in The Avengers and Dylan Bruno in the Agents of S.H.I.E.L.D. episode Yes Men.

"""@en .

<http://dbkwik.webdatacommons.org/marvelcinematicuniverse.wikia.com/resource/Antoine_Triplett> rdfs:label "Antoine Triplett"^^rdf:langString ;
    ns1:clearance <http://dbkwik.webdatacommons.org/marvelcinematicuniverse.wikia.com/resource/Clearance_Level> ;
    rdfs:comment "Antoine \"Trip\" Triplett was a Level 6 S.H.I.E.L.D. agent who had formerly worked on Agent John Garrett's team. However Triplett soon discovered that Garrett was in fact a traitor and a part of HYDRA during the HYDRA Uprising, working as the terrorist known as the Clairvoyant who had killed several of Triplett's friends. In the wake of making this discovery, Triplett remained loyal to S.H.I.E.L.D. and then became a member of Agent Phil Coulson's team, despite having to prove himself in Coulson's eyes. He helped them stop Garrett's HYDRA cell at the Battle at Cybertek and then joined newly promoted Director Coulson and the rest of the team at the Playground to start finally rebuilding S.H.I.E.L.D.."@en .

<http://dbkwik.webdatacommons.org/marvelcinematicuniverse.wikia.com/resource/Antonio_Campos> a <http://dbkwik.webdatacommons.org/marvelcinematicuniverse.wikia.com/class/wp> ;
    rdfs:label "Antonio Campos"^^rdf:langString ;
    rdfs:comment """Antonio Campos directed The Punisher episode Cold Steel.

"""@en .

<http://dbkwik.webdatacommons.org/marvelcinematicuniverse.wikia.com/resource/Ants> a <http://dbkwik.webdatacommons.org/marvelcinematicuniverse.wikia.com/class/race> ;
    rdfs:label "Ants"^^rdf:langString ;
    ns1:homeplanet <http://dbkwik.webdatacommons.org/marvelcinematicuniverse.wikia.com/resource/Earth> ;
    rdfs:comment """Ants are eusocial insects native to Earth. They are among the most socially advanced species on the planet, being one of the few earthly creatures capable of operating as a unified entity. Ants form organized colonies that may occupy large territories and consist of millions of workers. Most colonies consist mostly of sterile, wingless females forming castes of specialized groups, while one fertile female and one fertile male. The queen and her drones are in charge of breeding other workers.
"""@en .

<http://dbkwik.webdatacommons.org/marvelcinematicuniverse.wikia.com/resource/Anvil> rdfs:label "Anvil"^^rdf:langString ;
    ns1:formerleaders <http://dbkwik.webdatacommons.org/marvelcinematicuniverse.wikia.com/resource/Billy_Russo> ;
    rdfs:comment """Anvil Security was a private military firm founded by Billy Russo with the purpose of providing military and security services.

"""@en .

<http://dbkwik.webdatacommons.org/marvelcinematicuniverse.wikia.com/resource/Arago-7> rdfs:label "Arago-7"^^rdf:langString ;
    ns1:population <http://dbkwik.webdatacommons.org/marvelcinematicuniverse.wikia.com/resource/Hurctarians> ;
    rdfs:comment """Arago-7 is a dry planet inhabited by the Hurctarians.

"""@en .

<http://dbkwik.webdatacommons.org/marvelcinematicuniverse.wikia.com/resource/Aranda_de_Duero> rdfs:label "Aranda de Duero"^^rdf:langString ;
    ns1:coat <http://dbkwik.webdatacommons.org/marvelcinematicuniverse.wikia.com/resource/File:Coat_of_Arms_of_Aranda_de_Duero.png> ;
    ns1:flag <http://dbkwik.webdatacommons.org/marvelcinematicuniverse.wikia.com/resource/File:Banderadearanda.png> ;
    rdfs:comment """Aranda de Duero is a town located in Spain.

"""@en .

<http://dbkwik.webdatacommons.org/marvelcinematicuniverse.wikia.com/resource/Argentina> rdfs:label "Argentina"^^rdf:langString ;
    ns1:coat 40 ;
    rdfs:comment """Argentina, officially the Argentine Republic, is a country located in the southeastern South America.

"""@en .

<http://dbkwik.webdatacommons.org/marvelcinematicuniverse.wikia.com/resource/Ark> a <http://dbkwik.webdatacommons.org/marvelcinematicuniverse.wikia.com/class/vehicle> ;
    rdfs:label "Ark"^^rdf:langString ;
    ns1:builder <http://dbkwik.webdatacommons.org/marvelcinematicuniverse.wikia.com/resource/Dark_Elves> ;
    ns1:owner <http://dbkwik.webdatacommons.org/marvelcinematicuniverse.wikia.com/resource/Malekith> ;
    rdfs:comment """The Arks were among the most numerous warships used by the Dark Elves of Svartalfheim. The Arks were capable of ferrying smaller Dark Elf Harrow fighters, and were powered by black holes.

"""@en .

<http://dbkwik.webdatacommons.org/marvelcinematicuniverse.wikia.com/resource/Arnim_Zola> rdfs:label "Arnim Zola"^^rdf:langString ;
    ns1:idno 33327 ;
    ns1:voiceActor <http://dbkwik.webdatacommons.org/marvelcinematicuniverse.wikia.com/resource/André_Sogliuzzo> ;
    rdfs:comment """Doctor Arnim Zola was a Swiss scientist working for HYDRA before, during, and after World War II. Originally an employee of the Nazi Sturmabteilung, in 1934 he was recruited by Johann Schmidt to become a lead scientist for Schmidt's HYDRA organization. During the war, he designed many advanced weapons to aid HYDRA in its quest for world domination. Despite being captured by the Allies shortly before Schmidt's defeat in 1945, he was offered a position in S.H.I.E.L.D., the newly formed peacekeeping organization, and he used that opportunity to secretly rebuild HYDRA.
"""@en .

<http://dbkwik.webdatacommons.org/marvelcinematicuniverse.wikia.com/resource/Arnim_Zola%27s_Film_Reels> rdfs:label "Arnim Zola's Film Reels"^^rdf:langString ;
    ns1:made <http://dbkwik.webdatacommons.org/marvelcinematicuniverse.wikia.com/resource/1940s> ;
    rdfs:comment """Arnim Zola's Film Reels were the recordings made by the HYDRA scientist Arnim Zola during World War II.

"""@en .

<http://dbkwik.webdatacommons.org/marvelcinematicuniverse.wikia.com/resource/Arrest_of_Connors> rdfs:label "Arrest of Connors"^^rdf:langString ;
    ns1:type "Arrest"^^rdf:langString ;
    rdfs:comment """The Arrest of Connors is the outcome of an operation planned by Tyrone Johnson and Brigid O'Reilly to make corrupt Detective Connors the Assassination of Billy Johnson.

"""@en .

<http://dbkwik.webdatacommons.org/marvelcinematicuniverse.wikia.com/resource/Arrest_of_Liam_Walsh> rdfs:label "Arrest of Liam Walsh"^^rdf:langString ;
    ns1:type "Arrest"^^rdf:langString ;
    rdfs:comment """The Arrest of Liam Walsh was the detention of one of the first suspects in Brigid O'Reilly's investigation on the crime scene involving Rick Cotton.

"""@en .

<http://dbkwik.webdatacommons.org/marvelcinematicuniverse.wikia.com/resource/Asano_Robotics> rdfs:label "Asano Robotics"^^rdf:langString ;
    ns1:formerleaders <http://dbkwik.webdatacommons.org/marvelcinematicuniverse.wikia.com/resource/Hirochi> ;
    rdfs:comment """Asano Robotics (アサノ ロボティクス Asano robotikusu) is a robotics corporation and the Japanese branch of Roxxon Corporation.

"""@en .

<http://dbkwik.webdatacommons.org/marvelcinematicuniverse.wikia.com/resource/Asgard-Jotunheim_War> a <http://dbkwik.webdatacommons.org/marvelcinematicuniverse.wikia.com/class/war> ;
    rdfs:label "Asgard-Jotunheim War"^^rdf:langString ;
    ns1:battles <http://dbkwik.webdatacommons.org/marvelcinematicuniverse.wikia.com/resource/Attack_on_Jotunheim> ;
    rdfs:comment """The Asgard-Jotunheim War was a conflict between the Asgardians and Frost Giants that took place from 965 A.D. to 2010.

"""@en .

<http://dbkwik.webdatacommons.org/marvelcinematicuniverse.wikia.com/resource/Asgardian_Skiff> rdfs:label "Asgardian Skiff"^^rdf:langString ;
    ns1:builder <http://dbkwik.webdatacommons.org/marvelcinematicuniverse.wikia.com/resource/Asgardians> ;
    ns1:pilot <http://dbkwik.webdatacommons.org/marvelcinematicuniverse.wikia.com/resource/Asgardians>,
        <http://dbkwik.webdatacommons.org/marvelcinematicuniverse.wikia.com/resource/Fandral> ;
    rdfs:comment """Asgardian Skiffs were a type of hovercraft used by the Asgardians for transportation. They are armed with rapid-firing rotary plasma cannons and missiles.

"""@en .

<http://dbkwik.webdatacommons.org/marvelcinematicuniverse.wikia.com/resource/Asgardian_Wolves> a <http://dbkwik.webdatacommons.org/marvelcinematicuniverse.wikia.com/class/race> ;
    rdfs:label "Asgardian Wolves"^^rdf:langString ;
    ns1:homeplanet <http://dbkwik.webdatacommons.org/marvelcinematicuniverse.wikia.com/resource/Asgard> ;
    rdfs:comment """The Asgardian Wolves were an immensely powerful and ferocious breed of giant wolves, one notable among them being Fenris.

"""@en .

<http://dbkwik.webdatacommons.org/marvelcinematicuniverse.wikia.com/resource/Assassination_of_Christian_Blake> rdfs:label "Assassination of Christian Blake"^^rdf:langString ;
    ns1:defender <http://dbkwik.webdatacommons.org/marvelcinematicuniverse.wikia.com/resource/Daredevil> ;
    rdfs:comment """The Assassination of Christian Blake was an attempt by Carl Hoffman to execute his partner Christian Blake.

"""@en .

<http://dbkwik.webdatacommons.org/marvelcinematicuniverse.wikia.com/resource/Athens> rdfs:label "Athens"^^rdf:langString ;
    ns1:seal 35 ;
    rdfs:comment """Athens is the capital and largest city of Greece.

"""@en .

<http://dbkwik.webdatacommons.org/marvelcinematicuniverse.wikia.com/resource/Atlas_Academy> rdfs:label "Atlas Academy"^^rdf:langString ;
    ns1:seal 40 ;
    rdfs:comment """Atlas Academy is a high school in Los Angeles that the Runaways attended.

"""@en .

<http://dbkwik.webdatacommons.org/marvelcinematicuniverse.wikia.com/resource/Atreus_Plastics> rdfs:label "Atreus Plastics"^^rdf:langString ;
    ns1:status <http://dbkwik.webdatacommons.org/marvelcinematicuniverse.wikia.com/resource/Glenn_Industries> ;
    rdfs:comment """Atreus Plastics is a plastics company operating in New York City founded by Mark Higgins.

"""@en .

<http://dbkwik.webdatacommons.org/marvelcinematicuniverse.wikia.com/resource/Attack_on_Grotto> rdfs:label "Attack on Grotto"^^rdf:langString ;
    ns1:defender <http://dbkwik.webdatacommons.org/marvelcinematicuniverse.wikia.com/resource/Daredevil>,
        <http://dbkwik.webdatacommons.org/marvelcinematicuniverse.wikia.com/resource/Karen_Page> ;
    rdfs:comment """The Attack on Grotto was an assault on Metro-General Hospital orchestrated by Punisher, in order to assassinate Grotto. However, Grotto's death was prevented as Karen Page escaped with him while Daredevil confronted Punisher.

"""@en .

<http://dbkwik.webdatacommons.org/marvelcinematicuniverse.wikia.com/resource/Attack_on_Harold_Meachum> rdfs:label "Attack on Harold Meachum"^^rdf:langString ;
    ns1:defender <http://dbkwik.webdatacommons.org/marvelcinematicuniverse.wikia.com/resource/Iron_Fist> ;
    rdfs:comment """The Attack on Harold Meachum was a prevented punishment of Harold Meachum through body mutilation executed by Hand.

"""@en .

<http://dbkwik.webdatacommons.org/marvelcinematicuniverse.wikia.com/resource/Attack_on_Hive> rdfs:label "Attack on Hive"^^rdf:langString ;
    ns1:defender <http://dbkwik.webdatacommons.org/marvelcinematicuniverse.wikia.com/resource/Hellfire> ;
    rdfs:comment """The Attack on Hive was an attempt by S.H.I.E.L.D. to eliminate the dark Inhuman Hive.

"""@en .

<http://dbkwik.webdatacommons.org/marvelcinematicuniverse.wikia.com/resource/Attack_on_the_Sanctums> a <http://dbkwik.webdatacommons.org/marvelcinematicuniverse.wikia.com/class/war> ;
    rdfs:label "Attack on the Sanctums"^^rdf:langString ;
    ns1:begin <http://dbkwik.webdatacommons.org/marvelcinematicuniverse.wikia.com/resource/2017> ;
    ns1:end <http://dbkwik.webdatacommons.org/marvelcinematicuniverse.wikia.com/resource/2017> ;
    rdfs:comment """The Attack on the Sanctums was a series of attacks executed by the Zealots in their quest to destroy the Masters of the Mystic Arts, summon Dormammu and merge Earth with the Dark Dimension.

"""@en .

<http://dbkwik.webdatacommons.org/marvelcinematicuniverse.wikia.com/resource/Austra> a <http://dbkwik.webdatacommons.org/marvelcinematicuniverse.wikia.com/class/wp> ;
    rdfs:label "Austra"^^rdf:langString ;
    rdfs:comment """Austra are a Canadian electronic music project.
Their song "Beyond a Mortal" is featured in the Runaways episode Reunion and on the original soundtrack of the series.

"""@en .

<http://dbkwik.webdatacommons.org/marvelcinematicuniverse.wikia.com/resource/Ava> rdfs:label "Ava"^^rdf:langString ;
    ns1:citizenship <http://dbkwik.webdatacommons.org/marvelcinematicuniverse.wikia.com/resource/Lighthouse> ;
    rdfs:comment """Ava is a resident of the Lighthouse and one of Kasius' many slave servitors.

"""@en .

<http://dbkwik.webdatacommons.org/marvelcinematicuniverse.wikia.com/resource/Avengers:_Age_of_Ultron> a <http://dbkwik.webdatacommons.org/marvelcinematicuniverse.wikia.com/class/movie> ;
    rdfs:label "Avengers: Age of Ultron"^^rdf:langString ;
    ns1:boxoffice "1.405E9"^^<http://dbkwik.webdatacommons.org/datatype/usDollar> ;
    rdfs:comment """Avengers: Age of Ultron is a 2015 superhero film, based on the Marvel Comics superhero team of the same name. It is a sequel to The Avengers and a crossover between/sequel to Iron Man 3, Thor: The Dark World and Captain America: The Winter Soldier, as well as the eleventh installment in the Marvel Cinematic Universe and the fifth installment of Phase Two. The film was released on April 22, 2015 internationally and on May 1, 2015 in the United States.
"""@en .

<http://dbkwik.webdatacommons.org/marvelcinematicuniverse.wikia.com/resource/Avengers:_Age_of_Ultron/Portal> a <http://dbkwik.webdatacommons.org/marvelcinematicuniverse.wikia.com/class/box> ;
    rdfs:label "Avengers: Age of Ultron/Portal"^^rdf:langString ;
    rdfs:comment """Characters from Avengers: Age of Ultron.
"""@en .

<http://dbkwik.webdatacommons.org/marvelcinematicuniverse.wikia.com/resource/Avengers:_Age_of_Ultron_(soundtrack)> a <http://dbkwik.webdatacommons.org/marvelcinematicuniverse.wikia.com/class/soundtrack> ;
    rdfs:label "Avengers: Age of Ultron (soundtrack)"^^rdf:langString ;
    rdfs:comment """Avengers: Age of Ultron: Original Motion Picture Soundtrack is the soundtrack for the film of the same name.

"""@en .

<http://dbkwik.webdatacommons.org/marvelcinematicuniverse.wikia.com/resource/Avengers:_Age_of_Ultron_Episode_0> rdfs:label "Avengers: Age of Ultron Episode 0"^^rdf:langString ;
    ns6:_ 1 ;
    rdfs:comment """This year's 30th issue of Kodansha's Shonen Magazine is revealing on Wednesday that Yūsaku Komiyama (Ixion Saga manga) will publish an "Avengers: Age of Ultron Episode 0" one-shot manga in the magazine's 31st issue, which will ship on July 1.

"""@en .

<http://dbkwik.webdatacommons.org/marvelcinematicuniverse.wikia.com/resource/Avengers:_Infinity_War/Credits> a <http://dbkwik.webdatacommons.org/marvelcinematicuniverse.wikia.com/class/reflist> ;
    rdfs:label "Avengers: Infinity War/Credits"^^rdf:langString ;
    rdfs:comment """Full Credits for Avengers: Infinity War.

"""@en .

<http://dbkwik.webdatacommons.org/marvelcinematicuniverse.wikia.com/resource/Avengers:_Infinity_War/Portal> a <http://dbkwik.webdatacommons.org/marvelcinematicuniverse.wikia.com/class/box> ;
    rdfs:label "Avengers: Infinity War/Portal"^^rdf:langString ;
    rdfs:comment """Characters in Avengers: Infinity War.
"""@en .

<http://dbkwik.webdatacommons.org/marvelcinematicuniverse.wikia.com/resource/Avengers:_Infinity_War:_The_Heroes%27_Journey> rdfs:label "Avengers: Infinity War: The Heroes' Journey"^^rdf:langString ;
    ns1:publisher <http://dbkwik.webdatacommons.org/marvelcinematicuniverse.wikia.com/resource/Little,_Brown_Books_for_Young_Readers> ;
    rdfs:comment """Avengers: Infinity War: The Heroes' Journey is a book based on Avengers: Infinity War featuring the stories of various characters leading up to the film.

"""@en .

<http://dbkwik.webdatacommons.org/marvelcinematicuniverse.wikia.com/resource/Avengers:_Infinity_War_-_Original_Motion_Picture_Soundtrack> a <http://dbkwik.webdatacommons.org/marvelcinematicuniverse.wikia.com/class/soundtrack> ;
    rdfs:label "Avengers: Infinity War - Original Motion Picture Soundtrack"^^rdf:langString ;
    rdfs:comment """Avengers: Infinity War - Original Motion Picture Soundtrack contains Alan Silvestri's score to Avengers: Infinity War.

"""@en .

<http://dbkwik.webdatacommons.org/marvelcinematicuniverse.wikia.com/resource/Avengers:_Operation_HYDRA> rdfs:label "Avengers: Operation HYDRA"^^rdf:langString ;
    ns1:editorinchief <http://dbkwik.webdatacommons.org/marvelcinematicuniverse.wikia.com/resource/Axel_Alonso> ;
    rdfs:comment """Avengers: Operation HYDRA is a comic set in the Marvel Cinematic Universe. It is set after the events of Captain America: The Winter Soldier and before the events of Avengers: Age of Ultron.

"""@en .

<http://dbkwik.webdatacommons.org/marvelcinematicuniverse.wikia.com/resource/Avengers_4> a <http://dbkwik.webdatacommons.org/marvelcinematicuniverse.wikia.com/class/movie> ;
    rdfs:label "Avengers 4"^^rdf:langString ;
    rdfs:comment """Avengers 4 is an upcoming 2019 superhero film, based on the Marvel Comics superhero team of the same name. It is a sequel to The Avengers, Avengers: Age of Ultron and Avengers: Infinity War, and a crossover/sequel to Ant-Man and the Wasp and Captain Marvel. The film will be the twenty-second main installment in the Marvel Cinematic Universe as well as the tenth and final installment of Phase Three. The movie is set to be released on April 26, 2019.

"""@en .

<http://dbkwik.webdatacommons.org/marvelcinematicuniverse.wikia.com/resource/Avengers_Civil_War> a <http://dbkwik.webdatacommons.org/marvelcinematicuniverse.wikia.com/class/war> ;
    rdfs:label "Avengers Civil War"^^rdf:langString ;
    rdfs:comment """The Avengers Civil War was a conflict between members of the Avengers that was semi-orchestrated by terrorist Helmut Zemo, who sought to exact revenge for his family's deaths during the Battle of Sokovia.

"""@en .

<http://dbkwik.webdatacommons.org/marvelcinematicuniverse.wikia.com/resource/Avengers_Initiative> a <http://dbkwik.webdatacommons.org/marvelcinematicuniverse.wikia.com/class/project> ;
    rdfs:label "Avengers Initiative"^^rdf:langString ;
    ns1:participants <http://dbkwik.webdatacommons.org/marvelcinematicuniverse.wikia.com/resource/Abomination>,
        <http://dbkwik.webdatacommons.org/marvelcinematicuniverse.wikia.com/resource/Captain_America> ;
    rdfs:comment """The Avengers Initiative (a.k.a Phase 1) was a secret project created by S.H.I.E.L.D. to create the Avengers, a collection of the most able individuals to defend Earth from imminent global threats; these individuals functioning as a response team to said threats which are too great for the forces of mankind to handle.
The Initiative was scrapped by the World Security Council after the alien incursion in New Mexico in favor of a weapons development program known as Phase 2. It was eventually reactivated in 2012 during the Chitauri Invasion.

"""@en .

<http://dbkwik.webdatacommons.org/marvelcinematicuniverse.wikia.com/resource/Avengers_Tower> rdfs:label "Avengers Tower"^^rdf:langString ;
    ns1:notableformer <http://dbkwik.webdatacommons.org/marvelcinematicuniverse.wikia.com/resource/Hulk>,
        <http://dbkwik.webdatacommons.org/marvelcinematicuniverse.wikia.com/resource/Iron_Man> ;
    rdfs:comment """Avengers Tower, also known as Stark Tower, was a high-rise building complex located in Manhattan, New York City. Owned and constructed by Tony Stark, the tower is powered by an Arc Reactor that makes it capable of running itself for over a year. The top ten floors were originally all devoted to research and development.
"""@en .

<http://dbkwik.webdatacommons.org/marvelcinematicuniverse.wikia.com/resource/Ayesha> rdfs:label "Ayesha"^^rdf:langString ;
    ns2:_ <http://dbkwik.webdatacommons.org/marvelcinematicuniverse.wikia.com/resource/Adam_Warlock>,
        <http://dbkwik.webdatacommons.org/marvelcinematicuniverse.wikia.com/resource/Priestesses_of_the_Sovereign> ;
    ns1:citizenship <http://dbkwik.webdatacommons.org/marvelcinematicuniverse.wikia.com/resource/Sovereign_(Planet)> ;
    rdfs:comment """Ayesha is the Golden High Priestess of the Sovereign. She was brought into conflict with the Guardians of the Galaxy as a result of Rocket Raccoon stealing from her people. Having failed to destroy the Guardians herself, Ayesha hired Yondu Udonta and his own band of Ravagers to complete the task, only to be betrayed. With information gained from Taserface, Ayesha's army tried again to kill the Guardians during their battle against Ego, only to fail once again, forcing Ayesha to create Adam Warlock as their greatest weapon to finally get their revenge against the Guardians.

"""@en .

<http://dbkwik.webdatacommons.org/marvelcinematicuniverse.wikia.com/resource/Azzuri> rdfs:label "Azzuri"^^rdf:langString ;
    ns1:after <http://dbkwik.webdatacommons.org/marvelcinematicuniverse.wikia.com/resource/T%27Chaka> ;
    ns1:years -1981 ;
    rdfs:comment """Azzuri was the ruler of the Kingdom of Wakanda and the father of T'Chaka and N'Jobu.

"""@en .

<http://dbkwik.webdatacommons.org/marvelcinematicuniverse.wikia.com/resource/Baby_Monitor_Protocol> a <http://dbkwik.webdatacommons.org/marvelcinematicuniverse.wikia.com/class/project> ;
    rdfs:label "Baby Monitor Protocol"^^rdf:langString ;
    rdfs:comment """The Baby Monitor Protocol is a security feature installed by Tony Stark within the Spider-Man Suit to observe and record everything Spider-Man sees through his eye-lenses.

"""@en .

<http://dbkwik.webdatacommons.org/marvelcinematicuniverse.wikia.com/resource/Basha%27s_Ship> rdfs:label "Basha's Ship"^^rdf:langString ;
    ns1:owner <http://dbkwik.webdatacommons.org/marvelcinematicuniverse.wikia.com/resource/Basha> ;
    rdfs:comment """Basha's Ship is a personal starship used by Lady Basha after the destruction of Earth.

"""@en .

<http://dbkwik.webdatacommons.org/marvelcinematicuniverse.wikia.com/resource/Bastille> a <http://dbkwik.webdatacommons.org/marvelcinematicuniverse.wikia.com/class/wp> ;
    rdfs:label "Bastille"^^rdf:langString ;
    rdfs:comment """Bastille are a British indie band.
Their song "Blame" is featured in the Runaways episode Fifteen.

"""@en .

<http://dbkwik.webdatacommons.org/marvelcinematicuniverse.wikia.com/resource/Battle_Tank> rdfs:label "Battle Tank"^^rdf:langString ;
    ns1:builder <http://dbkwik.webdatacommons.org/marvelcinematicuniverse.wikia.com/resource/Justin_Hammer> ;
    rdfs:comment """The Battle Tank was built by Hammer Industries. It was stolen by the terrorist organization Ten Rings whose members later used it against War Machine in the battle of Hong Kong.

"""@en .

<http://dbkwik.webdatacommons.org/marvelcinematicuniverse.wikia.com/resource/Ben_Collins> a <http://dbkwik.webdatacommons.org/marvelcinematicuniverse.wikia.com/class/wp> ;
    rdfs:label "Ben Collins"^^rdf:langString ;
    rdfs:comment """Ben Lievesley Collins, previously known as The Stig, was a stunt performer in Doctor Strange.

"""@en .

<http://dbkwik.webdatacommons.org/marvelcinematicuniverse.wikia.com/resource/Bern_2000> rdfs:label "Bern 2000"^^rdf:langString ;
    ns1:participants <http://dbkwik.webdatacommons.org/marvelcinematicuniverse.wikia.com/resource/Aldrich_Killian>,
        <http://dbkwik.webdatacommons.org/marvelcinematicuniverse.wikia.com/resource/Ho_Yinsen> ;
    rdfs:comment """Bern 2000 was a science conference in Bern, Switzerland that began on New Year's Eve 1999 and ended on New Year's Day 2000.

"""@en .

<http://dbkwik.webdatacommons.org/marvelcinematicuniverse.wikia.com/resource/Berserker_Staff> rdfs:label "Berserker Staff"^^rdf:langString ;
    ns1:status <http://dbkwik.webdatacommons.org/marvelcinematicuniverse.wikia.com/resource/Barbershop_Headquarters> ;
    rdfs:comment """The Berserker Staff is an ancient Asgardian weapon left behind on Earth centuries ago by an Asgardian soldier. The Soldier broke the staff into three pieces and hid them across Europe. It was recovered by a group of Norse Paganists who wanted to use the staff to aid in their terrorism. The staff was later taken into possession by S.H.I.E.L.D., then HYDRA, then S.H.I.E.L.D. again.

"""@en .

<http://dbkwik.webdatacommons.org/marvelcinematicuniverse.wikia.com/resource/Big_Shot> a <http://dbkwik.webdatacommons.org/marvelcinematicuniverse.wikia.com/class/song> ;
    rdfs:label "Big Shot"^^rdf:langString ;
    ns1:performer <http://dbkwik.webdatacommons.org/marvelcinematicuniverse.wikia.com/resource/Kendrick_Lamar>,
        <http://dbkwik.webdatacommons.org/marvelcinematicuniverse.wikia.com/resource/Travis_Scott> ;
    rdfs:comment """"Big Shot" is a song recorded by Kendrick Lamar & Travis Scott for Black Panther: The Album.

"""@en .

<http://dbkwik.webdatacommons.org/marvelcinematicuniverse.wikia.com/resource/Bio-Tech_Force_Enhancement_Project> a <http://dbkwik.webdatacommons.org/marvelcinematicuniverse.wikia.com/class/project> ;
    rdfs:label "Bio-Tech Force Enhancement Project"^^rdf:langString ;
    ns1:contributors <http://dbkwik.webdatacommons.org/marvelcinematicuniverse.wikia.com/resource/Betty_Ross>,
        <http://dbkwik.webdatacommons.org/marvelcinematicuniverse.wikia.com/resource/Hulk> ;
    ns1:participants <http://dbkwik.webdatacommons.org/marvelcinematicuniverse.wikia.com/resource/Hulk> ;
    rdfs:comment """The Bio-Tech Force Enhancement Project was an attempt to recreate the results of Project Rebirth, started after the 9/11 attacks in order to make Super Soldiers like Captain America. The project was a failure and started Bruce Banner's initial transformation as Hulk.

"""@en .

<http://dbkwik.webdatacommons.org/marvelcinematicuniverse.wikia.com/resource/Birth_Pods> rdfs:label "Birth Pods"^^rdf:langString ;
    ns1:made <http://dbkwik.webdatacommons.org/marvelcinematicuniverse.wikia.com/resource/Sovereign> ;
    rdfs:comment """The Birth Pods, previously called Cosmic Cocoons, are incubators used by the Sovereign to procreate. One of the Cosmic Coccoons is in possession of Taneleer Tivan stored in his museum.

"""@en .

<http://dbkwik.webdatacommons.org/marvelcinematicuniverse.wikia.com/resource/Black_Order> rdfs:label "Black Order"^^rdf:langString ;
    ns1:vehicles <http://dbkwik.webdatacommons.org/marvelcinematicuniverse.wikia.com/resource/Q-Ship>,
        <http://dbkwik.webdatacommons.org/marvelcinematicuniverse.wikia.com/resource/Sanctuary_II> ;
    rdfs:comment """The Black Order, also known as the Children of Thanos, was a group comprised of Thanos' adopted children. They served as Thanos' vicious lieutenants and assisted him in his mission to find and harness the power of the Infinity Stones.

"""@en .

<http://dbkwik.webdatacommons.org/marvelcinematicuniverse.wikia.com/resource/Black_Panther> rdfs:label "Black Panther"^^rdf:langString ;
    ns1:after <http://dbkwik.webdatacommons.org/marvelcinematicuniverse.wikia.com/resource/Erik_Killmonger> ;
    ns1:before <http://dbkwik.webdatacommons.org/marvelcinematicuniverse.wikia.com/resource/Erik_Killmonger>,
        <http://dbkwik.webdatacommons.org/marvelcinematicuniverse.wikia.com/resource/T%27Chaka> ;
    rdfs:comment """T'Challa was the monarch of the African nation of Wakanda. As the Wakandan monarch, he was also the former holder of the Black Panther mantle. After his father was killed in a bombing attack orchestrated by Helmut Zemo, the new monarch set out to kill the Winter Soldier, who was widely believed to be responsible for the attack. After being drawn into the Avengers Civil War and siding with Iron Man, T'Challa learned the truth about Zemo's deception and decided to help the Winter Soldier by granting him asylum in Wakanda and also help him get a cure for his mental programming.
"""@en .

<http://dbkwik.webdatacommons.org/marvelcinematicuniverse.wikia.com/resource/Black_Panther_(film)/Portal> a <http://dbkwik.webdatacommons.org/marvelcinematicuniverse.wikia.com/class/box> ;
    rdfs:label "Black Panther (film)/Portal"^^rdf:langString ;
    ns1:link <http://dbkwik.webdatacommons.org/marvelcinematicuniverse.wikia.com/resource/Black_Panther_(film)> ;
    rdfs:comment """Characters from Black Panther.
"""@en .

<http://dbkwik.webdatacommons.org/marvelcinematicuniverse.wikia.com/resource/Black_Panther_(song)> a <http://dbkwik.webdatacommons.org/marvelcinematicuniverse.wikia.com/class/song> ;
    rdfs:label "Black Panther (song)"^^rdf:langString ;
    ns1:performer <http://dbkwik.webdatacommons.org/marvelcinematicuniverse.wikia.com/resource/Kendrick_Lamar> ;
    rdfs:comment """"Black Panther" is a song recorded by Kendrick Lamar for Black Panther: The Album.

"""@en .

<http://dbkwik.webdatacommons.org/marvelcinematicuniverse.wikia.com/resource/Blackout> rdfs:label "Blackout"^^rdf:langString ;
    ns1:idno "FPN 084-22-1836"^^rdf:langString ;
    rdfs:comment """Marcus Daniels, also known as Blackout, was a man with the ability to manipulate Darkforce. He was apparently killed by Phil Coulson and Antoine Triplett while stalking his "only light in the darkness", Audrey Nathan.

"""@en .

<http://dbkwik.webdatacommons.org/marvelcinematicuniverse.wikia.com/resource/Bloody_Waters> a <http://dbkwik.webdatacommons.org/marvelcinematicuniverse.wikia.com/class/song> ;
    rdfs:label "Bloody Waters"^^rdf:langString ;
    rdfs:comment """"Bloody Waters" is a song recorded by Ab-Soul, Anderson. Paak & James Blake for Black Panther: The Album.

"""@en .

<http://dbkwik.webdatacommons.org/marvelcinematicuniverse.wikia.com/resource/Bombing_of_the_Vienna_International_Centre> rdfs:label "Bombing of the Vienna International Centre"^^rdf:langString ;
    ns1:type <http://dbkwik.webdatacommons.org/marvelcinematicuniverse.wikia.com/resource/Attack_on_the_IFID_Headquarters> ;
    rdfs:comment """The Bombing of the Vienna International Centre was a terrorist attack on a United Nations ceremony in Austria, orchestrated by Helmut Zemo in his campaign to divide and destroy the Avengers. It resulted in the death of 12 people including T'Chaka, the King of Wakanda.

"""@en .

<http://dbkwik.webdatacommons.org/marvelcinematicuniverse.wikia.com/resource/Brad_Ricker> a <http://dbkwik.webdatacommons.org/marvelcinematicuniverse.wikia.com/class/imdb> ;
    rdfs:label "Brad Ricker"^^rdf:langString ;
    rdfs:comment """Brad Ricker was a supervising art director on Spider-Man: Homecoming.

"""@en .

<http://dbkwik.webdatacommons.org/marvelcinematicuniverse.wikia.com/resource/Brady_Romberg> rdfs:label "Brady Romberg"^^rdf:langString ;
    ns1:film <http://dbkwik.webdatacommons.org/marvelcinematicuniverse.wikia.com/resource/Captain_America:_The_First_Avenger> ;
    rdfs:comment """Brady Romberg was a utility stunts performer in Captain America: The First Avenger and a stunt performer in the Agents of S.H.I.E.L.D. episode S.O.S. Part One and the Daredevil episode Shadows in the Glass.
He was also a stunt double for Bill Paxton in the Agents of S.H.I.E.L.D. episode T.A.H.I.T.I. and Danny Lopes in the Agents of S.H.I.E.L.D. episode Who You Really Are.

"""@en .

<http://dbkwik.webdatacommons.org/marvelcinematicuniverse.wikia.com/resource/Brett_Morgen> rdfs:label "Brett Morgen"^^rdf:langString ;
    ns1:directed <http://dbkwik.webdatacommons.org/marvelcinematicuniverse.wikia.com/resource/Reunion_(Runaways)> ;
    rdfs:comment """Brett Morgen is a co-producer of the first season of Runaways.
He also directed the episode Reunion.

"""@en .

<http://dbkwik.webdatacommons.org/marvelcinematicuniverse.wikia.com/resource/Brisbane> rdfs:label "Brisbane"^^rdf:langString ;
    ns1:flag <http://dbkwik.webdatacommons.org/marvelcinematicuniverse.wikia.com/resource/File:Flag_of_Brisbane.png> ;
    rdfs:comment """Brisbane is the third most popolous city in Australia.

"""@en .

<http://dbkwik.webdatacommons.org/marvelcinematicuniverse.wikia.com/resource/Bulletproof_Love> a <http://dbkwik.webdatacommons.org/marvelcinematicuniverse.wikia.com/class/song> ;
    rdfs:label "Bulletproof Love"^^rdf:langString ;
    rdfs:comment """"Bulletproof Love" is a song composed and recorded by Adrian Younge, Ali Shaheed Muhammad and Method Man for the Luke Cage episode Soliloquy of Chaos. It was released on September 30, 2016 and featured on the album Luke Cage.

"""@en .

<http://dbkwik.webdatacommons.org/marvelcinematicuniverse.wikia.com/resource/Buri> rdfs:label "Buri"^^rdf:langString ;
    ns1:after <http://dbkwik.webdatacommons.org/marvelcinematicuniverse.wikia.com/resource/Bor> ;
    rdfs:comment """Buri was the first King of Asgard, father of Bor, grandfather of Odin and great grandfather of Thor. Since his reign, Asgard has protected the Nine Realms.

"""@en .

<http://dbkwik.webdatacommons.org/marvelcinematicuniverse.wikia.com/resource/Bus> rdfs:label "Bus"^^rdf:langString ;
    ns1:prisoners <http://dbkwik.webdatacommons.org/marvelcinematicuniverse.wikia.com/resource/Akela_Amador>,
        <http://dbkwik.webdatacommons.org/marvelcinematicuniverse.wikia.com/resource/Blizzard> ;
    rdfs:comment "The Bus (formally known as the CXD 23215 Airborne Mobile Command Station officially designated as \"S.H.I.E.L.D. 6-1-6\".) was a specialized Boeing C-17 Globemaster III owned and modified by S.H.I.E.L.D.. The planes were in heavy rotation from the 1980s to the 1990s until S.H.I.E.L.D. built the Helicarrier. Following the Battle of New York on Director Nick Fury's and Agent Phil Coulson's orders, the Bus underwent a complete overhaul. It served as a flying command center for Agent Phil Coulson and his team before being stolen by Grant Ward. Coulson's team reclaimed it during the Battle at Cybertek. It continued its role as Coulson's mobile command center when he became Director of S.H.I.E.L.D, although Coulson's team became primarily based at the Playground."@en .

<http://dbkwik.webdatacommons.org/marvelcinematicuniverse.wikia.com/resource/Callisto_Aerospace> rdfs:label "Callisto Aerospace"^^rdf:langString ;
    ns1:vehicles <http://dbkwik.webdatacommons.org/marvelcinematicuniverse.wikia.com/resource/Callisto_Aerospace_Rover> ;
    rdfs:comment """Callisto Aerospace is an aerospace technology company located in the United States of America.

"""@en .

<http://dbkwik.webdatacommons.org/marvelcinematicuniverse.wikia.com/resource/Captain_America%27s_Shield> rdfs:label "Captain America's Shield"^^rdf:langString ;
    ns1:made <http://dbkwik.webdatacommons.org/marvelcinematicuniverse.wikia.com/resource/1940s> ;
    rdfs:comment """Captain America's Shield was the primary defensive and offensive weapon used and owned by Steve Rogers. The original shield that Rogers carried into battle was made of steel and was shaped like a traditional heater shield. Later, Rogers adopted his more well-known, discus-shaped shield which was made out of vibranium.

"""@en .

<http://dbkwik.webdatacommons.org/marvelcinematicuniverse.wikia.com/resource/Captain_America:_75_Heroic_Years> a <http://dbkwik.webdatacommons.org/marvelcinematicuniverse.wikia.com/class/documentary> ;
    rdfs:label "Captain America: 75 Heroic Years"^^rdf:langString ;
    rdfs:comment """Captain America: 75 Heroic Years is a one-hour special documentary that aired on ABC on January 19, 2016.

"""@en .

<http://dbkwik.webdatacommons.org/marvelcinematicuniverse.wikia.com/resource/Captain_America:_Evil_Lurks_Everywhere> rdfs:label "Captain America: Evil Lurks Everywhere"^^rdf:langString ;
    ns1:editorinchief <http://dbkwik.webdatacommons.org/marvelcinematicuniverse.wikia.com/resource/Axel_Alonso> ;
    rdfs:comment """Captain America: Evil Lurks Everywhere is a comic book one-shot written by Stan Lee and drawn by Jason Armstrong that ties in to the movie Captain America: The First Avenger. The comic could only be obtained by buying a Norton Internet Security 2011 or Norton AntiVirus 2011 software package.
The comic was made in 3D and it came with a set of Captain America-themed 3D glasses.

"""@en .

<http://dbkwik.webdatacommons.org/marvelcinematicuniverse.wikia.com/resource/Captain_America:_The_First_Avenger_Movie_Special> a <http://dbkwik.webdatacommons.org/marvelcinematicuniverse.wikia.com/class/magazine> ;
    rdfs:label "Captain America: The First Avenger Movie Special"^^rdf:langString ;
    rdfs:comment """Captain America: The First Avenger Official Movie Special was a magazine. It featured a 22 page comic, cast interviews and photos from the movie.

"""@en .

<http://dbkwik.webdatacommons.org/marvelcinematicuniverse.wikia.com/resource/Captain_America:_The_Winter_Soldier_-_The_Official_Game> a <http://dbkwik.webdatacommons.org/marvelcinematicuniverse.wikia.com/class/game> ;
    rdfs:label "Captain America: The Winter Soldier - The Official Game"^^rdf:langString ;
    ns1:system ", ,"^^rdf:langString ;
    rdfs:comment """Captain America: The Winter Soldier - The Official Game is a 2014 video game loosely based on the film of the same name.
This game is a Hack and Slash, where the player can face R.A.I.D., U.L.T.I.M.A.T.U.M., and other foes.

"""@en .

<http://dbkwik.webdatacommons.org/marvelcinematicuniverse.wikia.com/resource/Carrick_O%27Quinn> rdfs:label "Carrick O'Quinn"^^rdf:langString ;
    ns1:movies <http://dbkwik.webdatacommons.org/marvelcinematicuniverse.wikia.com/resource/Thor_(film)> ;
    rdfs:comment """Carrick O'Quinn portrayed Frost Giant in Thor and Tall Bouncer in the Agent Carter episode Now is Not the End.
He was also a utility stunts performer in Thor, Captain America: The First Avenger and Thor: The Dark World and a stunt performer in the Agent Carter episode Now is Not the End.

"""@en .

<http://dbkwik.webdatacommons.org/marvelcinematicuniverse.wikia.com/resource/Cassie_Lang> rdfs:label "Cassie Lang"^^rdf:langString ;
    ns1:dob <http://dbkwik.webdatacommons.org/marvelcinematicuniverse.wikia.com/resource/2000s> ;
    rdfs:comment """Cassandra "Cassie" Lang is the daughter of Scott and Maggie Lang.

"""@en .

<http://dbkwik.webdatacommons.org/marvelcinematicuniverse.wikia.com/resource/Category:0-8-4> a skos:Concept ;
    rdfs:label "0-8-4"^^rdf:langString ;
    skos:broader <http://dbkwik.webdatacommons.org/marvelcinematicuniverse.wikia.com/resource/Category:Items>,
        <http://dbkwik.webdatacommons.org/marvelcinematicuniverse.wikia.com/resource/Category:S.H.I.E.L.D.> ;
    skos:prefLabel "0-8-4"^^rdf:langString .

<http://dbkwik.webdatacommons.org/marvelcinematicuniverse.wikia.com/resource/Category:A.I.M._Employees> a skos:Concept ;
    rdfs:label "A.I.M. Employees"^^rdf:langString ;
    skos:broader <http://dbkwik.webdatacommons.org/marvelcinematicuniverse.wikia.com/resource/Category:A.I.M.>,
        <http://dbkwik.webdatacommons.org/marvelcinematicuniverse.wikia.com/resource/Category:Characters_by_Affiliation> ;
    skos:prefLabel "A.I.M. Employees"^^rdf:langString .

<http://dbkwik.webdatacommons.org/marvelcinematicuniverse.wikia.com/resource/Category:A.I.M._Leaders> a skos:Concept ;
    rdfs:label "A.I.M. Leaders"^^rdf:langString ;
    skos:prefLabel "A.I.M. Leaders"^^rdf:langString .

<http://dbkwik.webdatacommons.org/marvelcinematicuniverse.wikia.com/resource/Category:A.I.M._Operatives> a skos:Concept ;
    rdfs:label "A.I.M. Operatives"^^rdf:langString ;
    skos:prefLabel "A.I.M. Operatives"^^rdf:langString .

<http://dbkwik.webdatacommons.org/marvelcinematicuniverse.wikia.com/resource/Category:Copyright> rdfs:label "Copyright"^^rdf:langString ;
    skos:related <http://dbkwik.webdatacommons.org/marvelcinematicuniverse.wikia.com/resource/Category:Policy> .

<http://dbkwik.webdatacommons.org/marvelcinematicuniverse.wikia.com/resource/Category:Help_desk> rdfs:label "Help desk"^^rdf:langString ;
    skos:related <http://dbkwik.webdatacommons.org/marvelcinematicuniverse.wikia.com/resource/Category:Help> .

<http://dbkwik.webdatacommons.org/marvelcinematicuniverse.wikia.com/resource/Category:Iron_Legion> rdfs:label "Iron Legion"^^rdf:langString ;
    skos:related <http://dbkwik.webdatacommons.org/marvelcinematicuniverse.wikia.com/resource/Category:Iron_Man_Armors> .

<http://dbkwik.webdatacommons.org/marvelcinematicuniverse.wikia.com/resource/Caterpillars> a <http://dbkwik.webdatacommons.org/marvelcinematicuniverse.wikia.com/class/project> ;
    rdfs:label "Caterpillars"^^rdf:langString ;
    ns1:contributors <http://dbkwik.webdatacommons.org/marvelcinematicuniverse.wikia.com/resource/Lash> ;
    ns1:end <http://dbkwik.webdatacommons.org/marvelcinematicuniverse.wikia.com/resource/2016> ;
    rdfs:comment """Caterpillars was a S.H.I.E.L.D. program led by Director Phil Coulson, which consisted in recruiting gifted individuals and helping them gain control over their powers. Graduates of the program joined the team Secret Warriors.

"""@en .

<http://dbkwik.webdatacommons.org/marvelcinematicuniverse.wikia.com/resource/Centipede_Project> a <http://dbkwik.webdatacommons.org/marvelcinematicuniverse.wikia.com/class/project> ;
    rdfs:label "Centipede Project"^^rdf:langString ;
    ns1:contributors <http://dbkwik.webdatacommons.org/marvelcinematicuniverse.wikia.com/resource/Debbie>,
        <http://dbkwik.webdatacommons.org/marvelcinematicuniverse.wikia.com/resource/Edison_Po> ;
    rdfs:comment """The Centipede Project is the name of a program organized and funded by John Garrett.

"""@en .

<http://dbkwik.webdatacommons.org/marvelcinematicuniverse.wikia.com/resource/Charlotta_Mohlin> rdfs:label "Charlotta Mohlin"^^rdf:langString ;
    ns1:charaacter "Greeter"^^rdf:langString ;
    rdfs:comment """Charlotta Mohlin portrayed Greeter in Agents of S.H.I.E.L.D..

"""@en .

<http://dbkwik.webdatacommons.org/marvelcinematicuniverse.wikia.com/resource/Chikara_Dojo/Promotional_Campaign> a <http://dbkwik.webdatacommons.org/marvelcinematicuniverse.wikia.com/class/clear> ;
    rdfs:label "Chikara Dojo/Promotional Campaign"^^rdf:langString ;
    rdfs:comment """After the premiere of the first season of Iron Fist, a promotional website was released on 23 March, 2017. This in-universe website is a introduction page for the Chikara Dojo. The website also contains a promotional video to learn Kenjutsu at the Dojo.
The webpage includes a advertisement by Rand Enterprises, which is redirected to a Linkedin page for Ward Meachum.

"""@en .

<http://dbkwik.webdatacommons.org/marvelcinematicuniverse.wikia.com/resource/Cloak_&_Dagger> a <http://dbkwik.webdatacommons.org/marvelcinematicuniverse.wikia.com/class/tv> ;
    rdfs:label "Cloak & Dagger"^^rdf:langString ;
    ns1:first <http://dbkwik.webdatacommons.org/marvelcinematicuniverse.wikia.com/resource/First_Light> ;
    ns1:showrunners <http://dbkwik.webdatacommons.org/marvelcinematicuniverse.wikia.com/resource/Joe_Pokaski> ;
    rdfs:comment """Marvel's Cloak & Dagger, or simply Cloak & Dagger, is an American television series based on the Marvel Comics superheroes of the same names. It is produced by Marvel Television and airs on Freeform.
The first season premiered on June 7, 2018.
On July 20, 2018, it was renewed for a second season. The second season will premiere in the Spring of 2019.

"""@en .

<http://dbkwik.webdatacommons.org/marvelcinematicuniverse.wikia.com/resource/Cloak_&_Dagger/Trivia> a <http://dbkwik.webdatacommons.org/marvelcinematicuniverse.wikia.com/class/stub> ;
    rdfs:label "Cloak & Dagger/Trivia"^^rdf:langString ;
    rdfs:comment """A list of trivia related to Cloak & Dagger.

"""@en .

<http://dbkwik.webdatacommons.org/marvelcinematicuniverse.wikia.com/resource/Cloak_&_Dagger_(Original_Television_Series_Soundtrack)> rdfs:label "Cloak & Dagger (Original Television Series Soundtrack)"^^rdf:langString ;
    ns1:runntime "2485.0"^^<http://dbkwik.webdatacommons.org/datatype/second> ;
    rdfs:comment """Cloak & Dagger (Original Television Series Soundtrack) contains songs featured in the first season of Cloak & Dagger. It was released digitally on June 8, 2018.

"""@en .

<http://dbkwik.webdatacommons.org/marvelcinematicuniverse.wikia.com/resource/Comics> a <http://dbkwik.webdatacommons.org/marvelcinematicuniverse.wikia.com/class/reflist> ;
    rdfs:label "Comics"^^rdf:langString ;
    rdfs:comment """The following is a list of Marvel-licensed comics set in the Marvel Cinematic Universe.

"""@en .

<http://dbkwik.webdatacommons.org/marvelcinematicuniverse.wikia.com/resource/Confederacy> rdfs:label "Confederacy"^^rdf:langString ;
    ns1:vehicles <http://dbkwik.webdatacommons.org/marvelcinematicuniverse.wikia.com/resource/Qovas%27_Ship> ;
    rdfs:comment """The Confederacy is an intergalactic alliance formed by members of six extraterrestrial species that have approached Earth demanding Gravitonium and Inhumans, in exchange for protection from Thanos. They initially struck a deal with HYDRA leader Hale, but they were ultimately forced to collaborate with a Gravitonium empowered Glenn Talbot, who seized a seat in the Confederacy.

"""@en .

<http://dbkwik.webdatacommons.org/marvelcinematicuniverse.wikia.com/resource/Contest_of_Champions> rdfs:label "Contest of Champions"^^rdf:langString ;
    ns1:begin <http://dbkwik.webdatacommons.org/marvelcinematicuniverse.wikia.com/resource/Before_20th_Century> ;
    ns1:combatants <http://dbkwik.webdatacommons.org/marvelcinematicuniverse.wikia.com/resource/Ares>,
        <http://dbkwik.webdatacommons.org/marvelcinematicuniverse.wikia.com/resource/Beta_Ray_Bill> ;
    rdfs:comment """The Contest of Champions is a tournament organized by the Grandmaster to entertain the citizens of Sakaar.

"""@en .

<http://dbkwik.webdatacommons.org/marvelcinematicuniverse.wikia.com/resource/Coulson%27s_Team> rdfs:label "Coulson's Team"^^rdf:langString ;
    ns1:status <http://dbkwik.webdatacommons.org/marvelcinematicuniverse.wikia.com/resource/S.H.I.E.L.D.> ;
    rdfs:comment """After Phil Coulson recovered from his injuries sustained before the Battle of New York, Melinda May put together a team to investigate the cases S.H.I.E.L.D. had not yet classified. When HYDRA came out of the shadows and into the light during the events of the HYDRA Uprising, they enacted Odyssey Protocol and erased all online proof of their existence, vanishing. The team was effectively dissolved when Coulson become the new Director of S.H.I.E.L.D., as they relocated to their new base of operations, the Playground, to begin rebuilding S.H.I.E.L.D. as the core members of the organization. The team was temporarily reassembled when Coulson needed Grant Ward's help to take down a HYDRA base in the Arctic, only to be permanently dissolved when Ward deserted them after the mission.

"""@en .

<http://dbkwik.webdatacommons.org/marvelcinematicuniverse.wikia.com/resource/Craig_Kyle> a <http://dbkwik.webdatacommons.org/marvelcinematicuniverse.wikia.com/class/imdb> ;
    rdfs:label "Craig Kyle"^^rdf:langString ;
    rdfs:comment """Craig Kyle co-produced Thor and executive produced Thor: The Dark World.
He also co-wrote the screenplay for Thor: Ragnarok along with frequent writing partner Christopher Yost, with whom he also co-wrote the Thor: The Dark World Prelude comic.

"""@en .

<http://dbkwik.webdatacommons.org/marvelcinematicuniverse.wikia.com/resource/Crimson_Dynamo_Armor> a <http://dbkwik.webdatacommons.org/marvelcinematicuniverse.wikia.com/class/armor> ;
    rdfs:label "Crimson Dynamo Armor"^^rdf:langString ;
    rdfs:comment """Two different versions of the Crimson Dynamo Armor have appeared in video games inspired by the Marvel Cinematic Universe:
							
The Crimson Dynamo Armor was an armored suit created by A.I.M.. It was worn by General Valentin Shatalov.

"""@en .

<http://dbkwik.webdatacommons.org/marvelcinematicuniverse.wikia.com/resource/Damage_Control_(TV_series)> a <http://dbkwik.webdatacommons.org/marvelcinematicuniverse.wikia.com/class/tv> ;
    rdfs:label "Damage Control (TV series)"^^rdf:langString ;
    rdfs:comment """Marvel's Damage Control, or simply Damage Control, is an American television series currently in development on the ABC network based on the Marvel Comics team of the same name.

"""@en .

<http://dbkwik.webdatacommons.org/marvelcinematicuniverse.wikia.com/resource/Damien_Moreno> rdfs:label "Damien Moreno"^^rdf:langString ;
    ns1:movies <http://dbkwik.webdatacommons.org/marvelcinematicuniverse.wikia.com/resource/Iron_Man_(film)> ;
    rdfs:comment """Damien Moreno portrayed Terrorist Soldier in Iron Man and Cybertek Agent in the Agents of S.H.I.E.L.D. episode T.R.A.C.K.S..
He was also a stunt performer in Iron Man and the Agents of S.H.I.E.L.D. episodes Seeds and T.R.A.C.K.S..

"""@en .

<http://dbkwik.webdatacommons.org/marvelcinematicuniverse.wikia.com/resource/Daniel_Drumm> rdfs:label "Daniel Drumm"^^rdf:langString ;
    ns1:succeeded "-"^^rdf:langString ;
    rdfs:comment """Daniel Drumm was a Master of the Mystic Arts of Kamar-Taj who was charged as the protector of the New York Sanctum. However when a former member of the Masters of the Mystic Arts named Kaecilius betrayed them, he targeted the Sanctorum with his Zealots. Although Drumm attempted to protect the building, he was soon defeated and executed by Kaecilius.

"""@en .

<http://dbkwik.webdatacommons.org/marvelcinematicuniverse.wikia.com/resource/Danielle_Daly> rdfs:label "Danielle Daly"^^rdf:langString ;
    ns1:oneShot <http://dbkwik.webdatacommons.org/marvelcinematicuniverse.wikia.com/resource/Marvel_One-Shot:_All_Hail_the_King> ;
    rdfs:comment """Danielle Daly was the post production supervisor of Iron Man 3, All Hail the King, Captain America: The Winter Soldier, Avengers: Age of Ultron and Captain America: Civil War.
She was also an addictional production coordinator in Iron Man 2, a senior post-production coordinator in Captain America: The First Avenger and a supervising post-production coordinator in The Avengers.

"""@en .

<http://dbkwik.webdatacommons.org/marvelcinematicuniverse.wikia.com/resource/Daredevil:_Defender_of_Hell%27s_Kitchen:_Season_One> rdfs:label "Daredevil: Defender of Hell's Kitchen: Season One"^^rdf:langString ;
    ns1:isbn <http://dbkwik.webdatacommons.org/marvelcinematicuniverse.wikia.com/resource/Special:BookSources/0785194010>,
        <http://dbkwik.webdatacommons.org/marvelcinematicuniverse.wikia.com/resource/Special:BookSources/9780785194019> ;
    rdfs:comment """Daredevil: Defender of Hell's Kitchen: Season One is the official artbook and behind-the-scenes story of the first season of the Netflix television series Daredevil.

"""@en .

<http://dbkwik.webdatacommons.org/marvelcinematicuniverse.wikia.com/resource/David_Hasselhoff> rdfs:label "David Hasselhoff"^^rdf:langString ;
    ns1:contribution <http://dbkwik.webdatacommons.org/marvelcinematicuniverse.wikia.com/resource/Guardians_Inferno>,
        <http://dbkwik.webdatacommons.org/marvelcinematicuniverse.wikia.com/resource/Guardians_of_the_Galaxy_Vol._2> ;
    rdfs:comment """David Michael Hasselhoff is an American actor, singer, producer, and businessman. He recorded the song "Guardians Inferno" (written by James Gunn) with The Sneepers in Guardians of the Galaxy Vol. 2.
He also portrayed an alternate form of Ego in Guardians of the Galaxy Vol. 2 as well as himself in the credits.

"""@en .

<http://dbkwik.webdatacommons.org/marvelcinematicuniverse.wikia.com/resource/Destroyer> rdfs:label "Destroyer"^^rdf:langString ;
    ns1:status <http://dbkwik.webdatacommons.org/marvelcinematicuniverse.wikia.com/resource/Destroyer_Armor_Prototype_Gun> ;
    rdfs:comment """The Destroyer (a.k.a. The Destroyer Automaton) was an enchanted Asgardian automaton used primarily to guard the Weapon's Vault of Asgard, though it could also be used as a weapon against its master's enemies. The Destroyer unquestionably obeyed the ruler of Asgard and wielder of Gungnir, no matter who the ruler may be at any given time. Thus, the Destroyer could be used both for good and evil intentions.

"""@en .

<http://dbkwik.webdatacommons.org/marvelcinematicuniverse.wikia.com/resource/Diviner> rdfs:label "Diviner"^^rdf:langString ;
    ns1:otherNames "The Obelisk"^^rdf:langString ;
    rdfs:comment """The Diviners are items constructed by the Kree thousands of years ago as a containment device for the Terrigen Crystals. A number of Diviners were left on Earth several millennia ago, buried until World War II, when at least one of them was procured by HYDRA who dubbed it the Obelisk. In 1945 the Obelisk was confiscated by the Strategic Scientific Reserve where it became the first 0-8-4. The Diviners regained prominence in 2014, when the "Obelisk" became central in a conflict between HYDRA and S.H.I.E.L.D. (the Strategic Scientific Reserve's modern successor). Eventually that Diviner was activated, leading to the emergence of two new Inhumans, Raina and Skye.

"""@en .

<http://dbkwik.webdatacommons.org/marvelcinematicuniverse.wikia.com/resource/Doctor_Strange> rdfs:label "Doctor Strange"^^rdf:langString ;
    ns1:current <http://dbkwik.webdatacommons.org/marvelcinematicuniverse.wikia.com/resource/Doctor_Strange_(film)> ;
    ns1:succeeded "-"^^rdf:langString ;
    rdfs:comment "Stephen Vincent Strange M.D., Ph.D was a powerful sorcerer and a leading member of the Masters of the Mystic Arts. Originally a brilliant yet arrogant neurosurgeon, Strange had suffered a car accident, resulting in his hands becoming crippled. When Western medicine failed him, Strange embarked on a journey that led him to Kamar-Taj where Strange had made the discovery of magic and alternate dimensions, being trained by the Ancient One. Though focused on healing his hands, Strange learned more of the mystic arts and helped the Masters prevent Kaecilius from merging Earth with their Dark Dimension, but not before witnessing the Ancient One's death."@en .

<http://dbkwik.webdatacommons.org/marvelcinematicuniverse.wikia.com/resource/Doctor_Strange_(film)/Portal> rdfs:label "Doctor Strange (film)/Portal"^^rdf:langString ;
    ns1:link <http://dbkwik.webdatacommons.org/marvelcinematicuniverse.wikia.com/resource/Doctor_Strange_(film)> ;
    rdfs:comment "Characters from Doctor Strange."@en .

<http://dbkwik.webdatacommons.org/marvelcinematicuniverse.wikia.com/resource/Eternal_Flame> rdfs:label "Eternal Flame"^^rdf:langString ;
    ns1:status <http://dbkwik.webdatacommons.org/marvelcinematicuniverse.wikia.com/resource/Surtur> ;
    rdfs:comment """The Eternal Flame was a mystical, inextinguishable flame that contained the true power of the Fire Demon Surtur, and is capable of resurrecting deceased individuals.

"""@en .

<http://dbkwik.webdatacommons.org/marvelcinematicuniverse.wikia.com/resource/Executioner> rdfs:label "Executioner"^^rdf:langString ;
    ns1:succeeded <http://dbkwik.webdatacommons.org/marvelcinematicuniverse.wikia.com/resource/Volstagg> ;
    rdfs:comment """Skurge was an Asgardian warrior who was tasked with becoming the guardian of the Bifrost Bridge by Loki following the banishment of Heimdall. When Loki was revealed to have been ruling Asgard in secret, Skurge was demoted and made the janitor, however he was later recruited by Hela to become her personal Executioner. However, Skurge's disillusion and inner conflict of his new position upon seeing her brutality against her own people and the threat she posed to the Nine Realms ultimately made him turn against the Goddess of Death. During his final moments, Skurge fought Hela's entire army of the Berserkers and then allowed all of his people to survive the Destruction of Asgard at the cost of his own life. These actions also finally made Skurge a hero of Asgard.

"""@en .

<http://dbkwik.webdatacommons.org/marvelcinematicuniverse.wikia.com/resource/Eyad_Elbitar> rdfs:label "Eyad Elbitar"^^rdf:langString ;
    ns1:movies <http://dbkwik.webdatacommons.org/marvelcinematicuniverse.wikia.com/resource/Iron_Man_(film)> ;
    rdfs:comment """Eyad Elbitar portrayed Terrorist in Iron Man and Nahui in the Agents of S.H.I.E.L.D. episode 0-8-4.
He was also a stunt performer in Iron Man, Captain America: The Winter Soldier and the Agents of S.H.I.E.L.D. episode 0-8-4, a utility stunts performer in Iron Man 2 and a stunt driver in Iron Man 3 and Captain Marvel.
He was also a stunt double for Maximiliano Hernández in Captain America: The Winter Soldier.

"""@en .

<http://dbkwik.webdatacommons.org/marvelcinematicuniverse.wikia.com/resource/Firepower_Armor> a <http://dbkwik.webdatacommons.org/marvelcinematicuniverse.wikia.com/class/armor> ;
    rdfs:label "Firepower Armor"^^rdf:langString ;
    rdfs:comment """The Firepower Armor was an armored suit created by A.I.M.. It was worn by the mercenary known as Firepower. 

"""@en .

<http://dbkwik.webdatacommons.org/marvelcinematicuniverse.wikia.com/resource/First_Dark_Elf_Conflict> rdfs:label "First Dark Elf Conflict"^^rdf:langString ;
    ns1:imagebg "Dark Elves at War.jpg"^^rdf:langString ;
    rdfs:comment """The Dark Elf conflict is a conflict that lasted for thousands of years. Dating back to 2988 B.C., the crisis was instigated when Malekith, the insane, genocidal leader of the Dark Elves, attempted to use the Infinity Stone known as the Aether, which controls reality, to eradicate the Nine Realms. The Dark Elves were defeated and nearly exterminated by an opposing army of Asgardians led by the then-king Bor, and Malekith and several others of his species went into hibernation and until the next Convergence.

"""@en .

<http://dbkwik.webdatacommons.org/marvelcinematicuniverse.wikia.com/resource/Gaithersburg> rdfs:label "Gaithersburg"^^rdf:langString ;
    ns1:flag <http://dbkwik.webdatacommons.org/marvelcinematicuniverse.wikia.com/resource/File:Flag_of_Gaithersburg.png> ;
    ns1:seal <http://dbkwik.webdatacommons.org/marvelcinematicuniverse.wikia.com/resource/File:Seal_of_Gaithersburg.png> ;
    rdfs:comment """Gaithersburg, officially the City of Gaithersburg, is a city located in Maryland.

"""@en .

<http://dbkwik.webdatacommons.org/marvelcinematicuniverse.wikia.com/resource/Gary_Kosko> a <http://dbkwik.webdatacommons.org/marvelcinematicuniverse.wikia.com/class/imdb> ;
    rdfs:label "Gary Kosko"^^rdf:langString ;
    rdfs:comment """Gary Kosko was an art director for Captain America: The Winter Soldier.

"""@en .

<http://dbkwik.webdatacommons.org/marvelcinematicuniverse.wikia.com/resource/Geneva> rdfs:label "Geneva"^^rdf:langString ;
    ns1:inhabitants <http://dbkwik.webdatacommons.org/marvelcinematicuniverse.wikia.com/resource/Theo_Broussard> ;
    rdfs:comment """Geneva is a city in Switzerland.

"""@en .

<http://dbkwik.webdatacommons.org/marvelcinematicuniverse.wikia.com/resource/Geo_Corvera> rdfs:label "Geo Corvera"^^rdf:langString ;
    ns1:movies <http://dbkwik.webdatacommons.org/marvelcinematicuniverse.wikia.com/resource/Iron_Man_(film)> ;
    rdfs:comment """Geo Corvera portrayed Terrorist in Iron Man and Francis Noche in the Agents of S.H.I.E.L.D. episode One of Us.
He was also a stunt performer in Ant-Man and the Agents of S.H.I.E.L.D. episode 0-8-4.
He was also a utility stunts performer in Iron Man and Ant-Man.

"""@en .

<http://dbkwik.webdatacommons.org/marvelcinematicuniverse.wikia.com/resource/Ghost_Suit> rdfs:label "Ghost Suit"^^rdf:langString ;
    ns1:movies <http://dbkwik.webdatacommons.org/marvelcinematicuniverse.wikia.com/resource/Ant-Man_and_the_Wasp> ;
    rdfs:comment """The Ghost Suit is a full-body suit designed by S.H.I.E.L.D. in order to help Ava Starr to better control her phasing powers.

"""@en .

<http://dbkwik.webdatacommons.org/marvelcinematicuniverse.wikia.com/resource/Gladiator_(Sakaaran_Rebellion)> a <http://dbkwik.webdatacommons.org/marvelcinematicuniverse.wikia.com/class/delete> ;
    rdfs:label "Gladiator (Sakaaran Rebellion)"^^rdf:langString .

<http://dbkwik.webdatacommons.org/marvelcinematicuniverse.wikia.com/resource/Google+_Profile/Darren_Cross> a <http://dbkwik.webdatacommons.org/marvelcinematicuniverse.wikia.com/class/linkedin> ;
    rdfs:label "Google+ Profile/Darren Cross"^^rdf:langString ;
    rdfs:comment """The Google+ profile of Darren Cross was part of the 2015 Ant-Man promotional campaign. It supported the WIRED Insider: Darren Cross interview. This is a page which includes all the Google+ posts of Darren Cross.

"""@en .

<http://dbkwik.webdatacommons.org/marvelcinematicuniverse.wikia.com/resource/Google+_Profile/Pym_Technologies> a <http://dbkwik.webdatacommons.org/marvelcinematicuniverse.wikia.com/class/google+> ;
    rdfs:label "Google+ Profile/Pym Technologies"^^rdf:langString ;
    rdfs:comment """The Google+ profile of Pym Technologies was part of the 2015 Ant-Man promotional campaign. It supported the WIRED Insider: Darren Cross interview. This is a page which includes all the Google+ posts of Pym Technologies.

"""@en .

<http://dbkwik.webdatacommons.org/marvelcinematicuniverse.wikia.com/resource/Google+_Profile/WHiH_Newsfront> a <http://dbkwik.webdatacommons.org/marvelcinematicuniverse.wikia.com/class/google+> ;
    rdfs:label "Google+ Profile/WHiH Newsfront"^^rdf:langString ;
    rdfs:comment """The Google+ profile of WHiH Newsfront was part of the 2015 Ant-Man promotional campaign. It supported the videos of the WHiH Newsfront web series. This is a page which includes all the Google+ posts of WHiH Newsfront.

"""@en .

<http://dbkwik.webdatacommons.org/marvelcinematicuniverse.wikia.com/resource/Guidebook_to_the_Marvel_Cinematic_Universe> a <http://dbkwik.webdatacommons.org/marvelcinematicuniverse.wikia.com/class/guidebook> ;
    rdfs:label "Guidebook to the Marvel Cinematic Universe"^^rdf:langString ;
    rdfs:comment """The following is a list of Marvel-licensed comics set in the Marvel Cinematic Universe.

"""@en .

<http://dbkwik.webdatacommons.org/marvelcinematicuniverse.wikia.com/resource/Guidebook_to_the_Marvel_Cinematic_Universe_-_Ant-Man> a <http://dbkwik.webdatacommons.org/marvelcinematicuniverse.wikia.com/class/guidebook> ;
    rdfs:label "Guidebook to the Marvel Cinematic Universe - Ant-Man"^^rdf:langString ;
    ns1:cover <http://dbkwik.webdatacommons.org/marvelcinematicuniverse.wikia.com/resource/Mike_del_Mundo> ;
    rdfs:comment """Guidebook to the Marvel Cinematic Universe - Ant-Man is the tenth issue of a series of guidebooks that explores the Marvel Cinematic Universe. It covers Ant-Man, Ant-Man Prelude and Ant-Man - Scott Lang: Small Time.

"""@en .

<http://dbkwik.webdatacommons.org/marvelcinematicuniverse.wikia.com/resource/Guidebook_to_the_Marvel_Cinematic_Universe_-_Avengers:_Age_of_Ultron> a <http://dbkwik.webdatacommons.org/marvelcinematicuniverse.wikia.com/class/guidebook> ;
    rdfs:label "Guidebook to the Marvel Cinematic Universe - Avengers: Age of Ultron"^^rdf:langString ;
    ns1:cover <http://dbkwik.webdatacommons.org/marvelcinematicuniverse.wikia.com/resource/Mike_del_Mundo> ;
    rdfs:comment """Guidebook to the Marvel Cinematic Universe - Avengers: Age of Ultron is the thirteenth issue of a series of guidebooks that explores the Marvel Cinematic Universe. It covers Avengers: Age of Ultron and Avengers: Age of Ultron Prelude - This Scepter'd Isle.

"""@en .

<http://dbkwik.webdatacommons.org/marvelcinematicuniverse.wikia.com/resource/Guidebook_to_the_Marvel_Cinematic_Universe_-_Avengers_Initiative> a <http://dbkwik.webdatacommons.org/marvelcinematicuniverse.wikia.com/class/guidebook> ;
    rdfs:label "Guidebook to the Marvel Cinematic Universe - Avengers Initiative"^^rdf:langString ;
    ns1:cover <http://dbkwik.webdatacommons.org/marvelcinematicuniverse.wikia.com/resource/Marcos_Martín> ;
    rdfs:comment """Official Guidebook To The Marvel Cinematic Universe - Avengers Initiative is the collection of a series of guidebooks that explores the Marvel Cinematic Universe.

"""@en .

<http://dbkwik.webdatacommons.org/marvelcinematicuniverse.wikia.com/resource/Guidebook_to_the_Marvel_Cinematic_Universe_-_Captain_America:_Civil_War> a <http://dbkwik.webdatacommons.org/marvelcinematicuniverse.wikia.com/class/guidebook> ;
    rdfs:label "Guidebook to the Marvel Cinematic Universe - Captain America: Civil War"^^rdf:langString ;
    ns1:cover <http://dbkwik.webdatacommons.org/marvelcinematicuniverse.wikia.com/resource/Mike_del_Mundo> ;
    rdfs:comment """Official Guidebook To The Marvel Cinematic Universe - Captain America: Civil War is the eighteenth issue of a series of guidebooks that explores the Marvel Cinematic Universe. It covers Captain America: Civil War.

"""@en .

<http://dbkwik.webdatacommons.org/marvelcinematicuniverse.wikia.com/resource/Guidebook_to_the_Marvel_Cinematic_Universe_-_Captain_America:_The_First_Avenger> rdfs:label "Guidebook to the Marvel Cinematic Universe - Captain America: The First Avenger"^^rdf:langString ;
    ns1:cover <http://dbkwik.webdatacommons.org/marvelcinematicuniverse.wikia.com/resource/Mike_del_Mundo> ;
    rdfs:comment """Guidebook to the Marvel Cinematic Universe - Captain America: The First Avenger is the fifth issue of a series of guidebooks that explores the Marvel Cinematic Universe. It covers Captain America: The First Avenger, Captain America: First Vengeance Issues 1 to 4 and Captain America: The First Avenger Adaptation.

"""@en .

<http://dbkwik.webdatacommons.org/marvelcinematicuniverse.wikia.com/resource/HYDRA_Mini_Tank> rdfs:label "HYDRA Mini Tank"^^rdf:langString ;
    ns1:weapons <http://dbkwik.webdatacommons.org/marvelcinematicuniverse.wikia.com/resource/HYDRA_Cannon>,
        <http://dbkwik.webdatacommons.org/marvelcinematicuniverse.wikia.com/resource/HYDRA_Flamethrower> ;
    rdfs:comment """The HYDRA Mini Tank was an armored vehicle used by HYDRA during the Spanish Civil War and World War II.

"""@en .

<http://dbkwik.webdatacommons.org/marvelcinematicuniverse.wikia.com/resource/HYDRA_QuadCopter> rdfs:label "HYDRA QuadCopter"^^rdf:langString ;
    ns1:prisoners <http://dbkwik.webdatacommons.org/marvelcinematicuniverse.wikia.com/resource/Charles_Hinton>,
        <http://dbkwik.webdatacommons.org/marvelcinematicuniverse.wikia.com/resource/Lucio> ;
    rdfs:comment """The HYDRA Quadcopter is a large vehicle dedicated to the extraction and capture of Inhumans. Equipped with an Extraction Claw, the QuadCopter was capable of securing and transporting Inhumans quickly.

"""@en .

<http://dbkwik.webdatacommons.org/marvelcinematicuniverse.wikia.com/resource/Heart-Shaped_Herb> rdfs:label "Heart-Shaped Herb"^^rdf:langString ;
    ns1:imagecaption "Children prepare the Heart-Shaped Herb."^^rdf:langString ;
    rdfs:comment """The Heart-Shaped Herb was a plant native to Wakanda that was traditionally consumed by the new King and the heir to the mantle of the Black Panther in order to obtain enhanced physical abilities, as well as entering the Ancestral Plane through a ritual process.

"""@en .

<http://dbkwik.webdatacommons.org/marvelcinematicuniverse.wikia.com/resource/Heimdall> rdfs:label "Heimdall"^^rdf:langString ;
    ns1:years <http://dbkwik.webdatacommons.org/marvelcinematicuniverse.wikia.com/resource/2017> ;
    rdfs:comment """Heimdall was the all-seeing and all-hearing Asgardian and former guard of the Bifrost Bridge. He could see and hear nearly everything that happens in the Nine Realms. Despite vowing to obey the orders of Odin, Heimdall was prepared to commit treason if it meant protecting the Realms, as he allowed the Warriors Three to return Thor from Midgard to defeat Loki. 
"""@en .

<http://dbkwik.webdatacommons.org/marvelcinematicuniverse.wikia.com/resource/Helicarrier> rdfs:label "Helicarrier"^^rdf:langString ;
    ns1:prisoners <http://dbkwik.webdatacommons.org/marvelcinematicuniverse.wikia.com/resource/Loki> ;
    rdfs:comment """The Helicarrier is an advanced aerial vehicle with a design and function closely resembling that of a modern aircraft carrier. Specifically, the Helicarrier is designed to be capable of sustained, independently-powered flight, via four, massive engines that provide the lift needed to keep it in the air. After the Attack on the Helicarrier, Tony Stark upgraded the Helicarriers so that they relied on repulsor technology rather than turbines, allowing them to stay in the air indefinitely.
"""@en .

<http://dbkwik.webdatacommons.org/marvelcinematicuniverse.wikia.com/resource/Herefordshire> rdfs:label "Herefordshire"^^rdf:langString ;
    ns1:flag <http://dbkwik.webdatacommons.org/marvelcinematicuniverse.wikia.com/resource/File:Flag_of_Herefordshire.png> ;
    rdfs:comment """Herefordshire is a county located in the west of England.

"""@en .

<http://dbkwik.webdatacommons.org/marvelcinematicuniverse.wikia.com/resource/Hulu> a <http://dbkwik.webdatacommons.org/marvelcinematicuniverse.wikia.com/class/linkedin> ;
    rdfs:label "Hulu"^^rdf:langString ;
    rdfs:comment """Hulu is an American subscription video on demand service owned by Hulu LLC, a joint venture between multiple companies. It is offered only to users in Japan and the United States and its overseas territories.

"""@en .

<http://dbkwik.webdatacommons.org/marvelcinematicuniverse.wikia.com/resource/IMAX_Corporation> a <http://dbkwik.webdatacommons.org/marvelcinematicuniverse.wikia.com/class/youtube> ;
    rdfs:label "IMAX Corporation"^^rdf:langString ;
    rdfs:comment """IMAX Corporation is a theatre company based in Ontario, California that designs and manufactures IMAX cameras and projection systems. A number of Marvel Studios projects were filmed using IMAX cameras, including The Avengers and Avengers: Infinity War, as well as Marvel Television's Inhumans.

"""@en .

<http://dbkwik.webdatacommons.org/marvelcinematicuniverse.wikia.com/resource/Ibiza> rdfs:label "Ibiza"^^rdf:langString ;
    ns1:flag <http://dbkwik.webdatacommons.org/marvelcinematicuniverse.wikia.com/resource/File:Flag_of_Ibiza.png> ;
    rdfs:comment """Ibiza is an island and tourist attraction located near the southeastern coast of Spain.

"""@en .

<http://dbkwik.webdatacommons.org/marvelcinematicuniverse.wikia.com/resource/Inhumans_(TV_series)> rdfs:label "Inhumans (TV series)"^^rdf:langString ;
    ns1:last <http://dbkwik.webdatacommons.org/marvelcinematicuniverse.wikia.com/resource/...And_Finally:_Black_Bolt> ;
    rdfs:comment """Marvel's Inhumans is an American eight-episode live-action television series, based on the Royal Family of the Inhumans. It is produced by Marvel Television and distributed by ABC, and the first television series distributed by IMAX. The first two episodes of the series was shot with IMAX digital cameras and available in IMAX cinemas. It premiered September 29, 2017 on ABC.
On May 11, 2018, the series was cancelled by ABC.

"""@en .

<http://dbkwik.webdatacommons.org/marvelcinematicuniverse.wikia.com/resource/Instagram_Profile/Danny_Rand> a <http://dbkwik.webdatacommons.org/marvelcinematicuniverse.wikia.com/class/instagram> ;
    rdfs:label "Instagram Profile/Danny Rand"^^rdf:langString ;
    rdfs:comment """The Instagram profile of Danny Rand was part of a marketing campaign for Season 1 of Iron Fist. This profile could be accessed via an Instagram link on the Chikara Dojo website.
CharactersDanny RandJeri Hogarth (mentioned)
ItemsM&M'siPod ClassicKatana
OrganizationsStark Industries (mentioned)


"""@en .

<http://dbkwik.webdatacommons.org/marvelcinematicuniverse.wikia.com/resource/Inventory_of_Rare_and_Endangered_Tracheophyta_of_Amazônia> rdfs:label "Inventory of Rare and Endangered Tracheophyta of Amazônia"^^rdf:langString ;
    ns1:name "Inventory of Rare and Endangered Tracheophyta of Amazônia"^^rdf:langString ;
    rdfs:comment """Inventory of Rare and Endangered Tracheophyta of Amazonia is a botanical manual providing information on rare, threatened, and endangered Amazonia native plants. The book was written by Amanda Kirchhoff and printed by Rathburn University.

"""@en .

<http://dbkwik.webdatacommons.org/marvelcinematicuniverse.wikia.com/resource/Iron_Fist_(TV_series)/Trivia> a <http://dbkwik.webdatacommons.org/marvelcinematicuniverse.wikia.com/class/expand> ;
    rdfs:label "Iron Fist (TV series)/Trivia"^^rdf:langString ;
    rdfs:comment """A list of trivia related to Iron Fist.

"""@en .

<http://dbkwik.webdatacommons.org/marvelcinematicuniverse.wikia.com/resource/Iron_Legion> a <http://dbkwik.webdatacommons.org/marvelcinematicuniverse.wikia.com/class/armor> ;
    rdfs:label "Iron Legion"^^rdf:langString ;
    rdfs:comment """The Iron Legion was a group of Iron Man armors and droids used primarily to guard and protect civilians when the Avengers are fighting perilous battles in populated areas. The Iron Legion was originally a group of controlled by J.A.R.V.I.S., ranging from Marks VIII to XLI, that served as Iron Man's main combat support team when he was in need of reinforcements in battle.
"""@en .

<http://dbkwik.webdatacommons.org/marvelcinematicuniverse.wikia.com/resource/Iron_Man:_Limited_Edition> rdfs:label "Iron Man: Limited Edition"^^rdf:langString ;
    ns1:release <http://www.newsarama.com/5512-iron-man-2-augmented-reality-app-coming-to-lg-phones.html> ;
    rdfs:comment """Iron Man: Limited Edition is a tie-in for Iron Man 2 sponsored by LG, as an element of a partnership between Marvel and LG to combine augmented reality and exclusive content for the film.

"""@en .

<http://dbkwik.webdatacommons.org/marvelcinematicuniverse.wikia.com/resource/Iron_Man_(film)/Portal> rdfs:label "Iron Man (film)/Portal"^^rdf:langString ;
    ns1:link <http://dbkwik.webdatacommons.org/marvelcinematicuniverse.wikia.com/resource/Iron_Man_(film)> ;
    rdfs:comment """Characters from Iron Man.
"""@en .

<http://dbkwik.webdatacommons.org/marvelcinematicuniverse.wikia.com/resource/Iron_Man_2:_Phil_Coulson:_Agent_of_S.H.I.E.L.D.> rdfs:label "Iron Man 2: Phil Coulson: Agent of S.H.I.E.L.D."^^rdf:langString ;
    ns1:artista <http://dbkwik.webdatacommons.org/marvelcinematicuniverse.wikia.com/resource/Felix_Ruiz>,
        <http://dbkwik.webdatacommons.org/marvelcinematicuniverse.wikia.com/resource/Ian_Hannin> ;
    rdfs:comment """Iron Man 2: Phil Coulson: Agent of S.H.I.E.L.D. is a comic book published by Marvel Digital Comics Unlimited.

"""@en .

<http://dbkwik.webdatacommons.org/marvelcinematicuniverse.wikia.com/resource/Iron_Man_3_-_The_Official_Game> a <http://dbkwik.webdatacommons.org/marvelcinematicuniverse.wikia.com/class/game> ;
    rdfs:label "Iron Man 3 - The Official Game"^^rdf:langString ;
    ns1:system ", ,"^^rdf:langString ;
    rdfs:comment """Iron Man 3 - The Official Game is a 2013 video game loosely based on the film of the same name. This game was released on April, 25, 2013 and allows players to suit up as Iron Man using over 18 of his most famous armors.
The game acts in a Temple Run-like manner as the player attempts to dodge various objects to score points and try to complete the level while still defeating Aldrich Killian and his evil forces.

"""@en .

<http://dbkwik.webdatacommons.org/marvelcinematicuniverse.wikia.com/resource/Iron_Man_Armor:_Mark_IX> rdfs:label "Iron Man Armor: Mark IX"^^rdf:langString ;
    ns1:precededBy <http://dbkwik.webdatacommons.org/marvelcinematicuniverse.wikia.com/resource/Iron_Man_Armor:_Mark_VIII> ;
    ns1:succeededBy <http://dbkwik.webdatacommons.org/marvelcinematicuniverse.wikia.com/resource/Iron_Man_Armor:_Mark_X> ;
    rdfs:comment """The Mark IX Armor was Tony Stark's ninth Iron Man suit and the second suit created after the Battle of New York. The Mark IX was one of the first in a series of Iron Man suits created during a period of rapid development that led to the creation of the Iron Legion. It was destroyed by Pepper Potts.

"""@en .

<http://dbkwik.webdatacommons.org/marvelcinematicuniverse.wikia.com/resource/Iron_Man_Armor:_Mark_L> rdfs:label "Iron Man Armor: Mark L"^^rdf:langString ;
    ns1:precededBy <http://dbkwik.webdatacommons.org/marvelcinematicuniverse.wikia.com/resource/Iron_Man_Armor:_Mark_XLIX> ;
    rdfs:comment """The Mark L Armor is Tony Stark's fiftieth Iron Man suit. It was built after the Iron Man Armor: Mark XLVII, XLVIII, and XLIX. It is used to battle Thanos along with his allies. This armor is more advanced than any other proceeding armor, as it possesses many capabilities and useful functions for Stark to use at his disposal. It is the first armor to utilize nanotechnology.

"""@en .

<http://dbkwik.webdatacommons.org/marvelcinematicuniverse.wikia.com/resource/Iron_Man_Armor:_Mark_XIX> rdfs:label "Iron Man Armor: Mark XIX"^^rdf:langString ;
    ns1:name "Tiger Armor"^^rdf:langString ;
    rdfs:comment """The Mark XIX Armor (codenamed Tiger) was Tony Stark's ninteenth Iron Man suit and was specialized for high velocity flight.  It is part of the Iron Legion. It was destroyed following the Clean Slate Protocol.

"""@en .

<http://dbkwik.webdatacommons.org/marvelcinematicuniverse.wikia.com/resource/Jasper_Sitwell> rdfs:label "Jasper Sitwell"^^rdf:langString ;
    ns1:height 5 ;
    rdfs:comment "Jasper Sitwell was a Level 7 S.H.I.E.L.D. operative and member of HYDRA. Sitwell was indoctrinated into the ranks of HYDRA from being trained at the HYDRA Preparatory Academy, for whom he took on a role as a double agent within S.H.I.E.L.D. Several of his missions involved extraterrestrials and demigods. During the years of service working undercover, Sitwell became a good friend with his fellow agent Phil Coulson. Overtly, he conducted all his duties with efficiency, while covertly he aided a deep-rooted conspiracy to reshape the world in HYDRA's image. Eventually, Sitwell's true allegiance toward HYDRA had been uncovered by the S.H.I.E.L.D."@en .

<http://dbkwik.webdatacommons.org/marvelcinematicuniverse.wikia.com/resource/Javi_Fernandez> a <http://dbkwik.webdatacommons.org/marvelcinematicuniverse.wikia.com/class/marvel> ;
    rdfs:label "Javi Fernandez"^^rdf:langString ;
    rdfs:comment """Javier "Javi" Fernandez was an artist for Captain America: First Vengeance.

"""@en .

<http://dbkwik.webdatacommons.org/marvelcinematicuniverse.wikia.com/resource/Jefferson_Lewis> a <http://dbkwik.webdatacommons.org/marvelcinematicuniverse.wikia.com/class/imdb> ;
    rdfs:label "Jefferson Lewis"^^rdf:langString ;
    rdfs:comment """Jefferson Lewis III was a stunt performer in Black Panther, Avengers: Infinity War and Avengers 4.

"""@en .

<http://dbkwik.webdatacommons.org/marvelcinematicuniverse.wikia.com/resource/Joe_Caramagna> rdfs:label "Joe Caramagna"^^rdf:langString ;
    ns1:penciled <http://dbkwik.webdatacommons.org/marvelcinematicuniverse.wikia.com/resource/Captain_America:_Homecoming>,
        <http://dbkwik.webdatacommons.org/marvelcinematicuniverse.wikia.com/resource/Iron_Man:_I_Am_Iron_Man!> ;
    rdfs:comment """Joe Caramagna wrote the comics Nick Fury: Spies Like Us and Iron Man 2: Security Breach.
He was also an artist for Iron Man: Security Measures, Iron Man: I Am Iron Man!, Iron Man 2: Agents of S.H.I.E.L.D., The Avengers Prelude: Fury's Big Week, Iron Man: The Coming of the Melter, Thor: The Dark World Prelude and Captain America: Homecoming.

"""@en .

<http://dbkwik.webdatacommons.org/marvelcinematicuniverse.wikia.com/resource/John_Cassaday> rdfs:label "John Cassaday"^^rdf:langString ;
    ns1:penciled <http://dbkwik.webdatacommons.org/marvelcinematicuniverse.wikia.com/resource/Captain_America:_First_Vengeance> ;
    rdfs:comment """John Cassaday was an artist for Captain America: First Vengeance.
He was interviewed for the documentary Captain America: 75 Heroic Years.

"""@en .

<http://dbkwik.webdatacommons.org/marvelcinematicuniverse.wikia.com/resource/Joint_Counter_Terrorist_Centre_Building> rdfs:label "Joint Counter Terrorist Centre Building"^^rdf:langString ;
    ns1:formernotable <http://dbkwik.webdatacommons.org/marvelcinematicuniverse.wikia.com/resource/Avengers>,
        <http://dbkwik.webdatacommons.org/marvelcinematicuniverse.wikia.com/resource/Sharon_Carter> ;
    rdfs:comment """The Joint Counter Terrorist Centre Building is the headquarters of the Joint Counter Terrorist Centre located in Berlin, Germany.

"""@en .

<http://dbkwik.webdatacommons.org/marvelcinematicuniverse.wikia.com/resource/Jupiter> a <http://dbkwik.webdatacommons.org/marvelcinematicuniverse.wikia.com/class/marvel> ;
    rdfs:label "Jupiter"^^rdf:langString ;
    rdfs:comment """Jupiter is the fifth and largest planet of the Solar system, located 365 million miles away from Earth.

"""@en .

<http://dbkwik.webdatacommons.org/marvelcinematicuniverse.wikia.com/resource/Kandi_Marks> rdfs:label "Kandi Marks"^^rdf:langString ;
    ns1:contribution <http://dbkwik.webdatacommons.org/marvelcinematicuniverse.wikia.com/resource/AKA_I_Want_Your_Cray_Cray>,
        <http://dbkwik.webdatacommons.org/marvelcinematicuniverse.wikia.com/resource/I_Want_Your_Cray_Cray> ;
    rdfs:comment """Kandi Marks recorded the song "I Want Your Cray Cray" with Rachael Taylor for the Jessica Jones episode AKA I Want Your Cray Cray.

"""@en .

<http://dbkwik.webdatacommons.org/marvelcinematicuniverse.wikia.com/resource/Kevin_Ishioka> a <http://dbkwik.webdatacommons.org/marvelcinematicuniverse.wikia.com/class/imdb> ;
    rdfs:label "Kevin Ishioka"^^rdf:langString ;
    rdfs:comment """Kevin Ishioka was an art director for Captain America: The Winter Soldier.

"""@en .

<http://dbkwik.webdatacommons.org/marvelcinematicuniverse.wikia.com/resource/Landman_and_Zack> rdfs:label "Landman and Zack"^^rdf:langString ;
    ns1:formerLeader <http://dbkwik.webdatacommons.org/marvelcinematicuniverse.wikia.com/resource/Parish_Landman> ;
    rdfs:comment """Landman and Zack LLP is a law firm in New York City.

"""@en .

<http://dbkwik.webdatacommons.org/marvelcinematicuniverse.wikia.com/resource/Linkedin_Profile/Ward_Meachum> a <http://dbkwik.webdatacommons.org/marvelcinematicuniverse.wikia.com/class/linkedin> ;
    rdfs:label "Linkedin Profile/Ward Meachum"^^rdf:langString ;
    rdfs:comment """The LinkedIn profile of Ward Meachum was part of a marketing campaign for Season 1 of Iron Fist. This profile could be accessed via an advertisement on the Chikara Dojo website. On Meachum's profile there's also a video, where Joy Meachum and Ward Meachum are being interviewed by the New York Bulletin. This is a page which includes all the Linkedin posts and information of Ward Meachum.

"""@en .

<http://dbkwik.webdatacommons.org/marvelcinematicuniverse.wikia.com/resource/List_of_Powers_and_Abilities> a <http://dbkwik.webdatacommons.org/marvelcinematicuniverse.wikia.com/class/rewrite> ;
    rdfs:label "List of Powers and Abilities"^^rdf:langString ;
    rdfs:comment """The following is a list of the Powers and Abilities displayed by different characters in the Marvel Cinematic Universe.

"""@en .

<http://dbkwik.webdatacommons.org/marvelcinematicuniverse.wikia.com/resource/Maria_Stark> rdfs:label "Maria Stark"^^rdf:langString ;
    ns1:team <http://dbkwik.webdatacommons.org/marvelcinematicuniverse.wikia.com/resource/Stark_Industries> ;
    rdfs:comment """Maria Collins Carbonell Stark was Tony Stark's mother and Howard Stark's wife. She was assasinated along with her husband by the Winter Soldier under HYDRA orders, making it appear as an accidental car crash.

"""@en .

<http://dbkwik.webdatacommons.org/marvelcinematicuniverse.wikia.com/resource/Marvel_Cinematic_Universe> a <http://dbkwik.webdatacommons.org/marvelcinematicuniverse.wikia.com/class/marvel> ;
    rdfs:label "Marvel Cinematic Universe"^^rdf:langString ;
    rdfs:comment """The Marvel Cinematic Universe is a shared universe created by Marvel Studios, designated as Earth-199999 within Marvel's multiverse system. The universe is comprised mainly of films independently made by Marvel Studios, that are always set within this same universe, much like Marvel has done with their comics.
The universe includes a series of short films, called Marvel One-Shots, launched with each film's Blu-ray release starting with Thor and finishing with Thor: The Dark World. These short films were, however, eventually discontinued.
"""@en .

<http://dbkwik.webdatacommons.org/marvelcinematicuniverse.wikia.com/resource/Marvel_Cinematic_Universe_Wiki> a <http://dbkwik.webdatacommons.org/marvelcinematicuniverse.wikia.com/class/section> ;
    rdfs:label "Marvel Cinematic Universe Wiki"^^rdf:langString ;
    ns1:body <http://dbkwik.webdatacommons.org/marvelcinematicuniverse.wikia.com/resource/File:Marvel_Studios%27_Captain_Marvel_-_Official_Trailer>,
        <http://dbkwik.webdatacommons.org/marvelcinematicuniverse.wikia.com/resource/File:Marvel’s_Iron_Fist_Season_2_Official_Trailer_HD_Netflix>,
        270 ;
    ns1:heading "COUNTDOWN"^^rdf:langString,
        "FEATURED CHARACTERS"^^rdf:langString,
        "FEATURED VIDEO"^^rdf:langString,
        "MEDIA"^^rdf:langString,
        "News"^^rdf:langString ;
    rdfs:comment "es:fr:ru:pl:zh:"@en .

<http://dbkwik.webdatacommons.org/marvelcinematicuniverse.wikia.com/resource/Marvel_One-Shot:_A_Funny_Thing_Happened_on_the_Way_to_Thor%27s_Hammer> a <http://dbkwik.webdatacommons.org/marvelcinematicuniverse.wikia.com/class/one-shot> ;
    rdfs:label "Marvel One-Shot: A Funny Thing Happened on the Way to Thor's Hammer"^^rdf:langString ;
    rdfs:comment """A Funny Thing Happened on the Way to Thor's Hammer is the second in a series of Marvel One-Shots, released on the Captain America: The First Avenger Blu-ray on October 25, 2011. It takes place during the events of The Incredible Hulk, and in between the events of Iron Man 2 and Thor.

"""@en .

<http://dbkwik.webdatacommons.org/marvelcinematicuniverse.wikia.com/resource/Most_Wanted/Gallery> a <http://dbkwik.webdatacommons.org/marvelcinematicuniverse.wikia.com/class/cancelled> ;
    rdfs:label "Most Wanted/Gallery"^^rdf:langString ;
    rdfs:comment """The following is an index of galleries of screenshots and promotional material from the television show Most Wanted.

"""@en .

<http://dbkwik.webdatacommons.org/marvelcinematicuniverse.wikia.com/resource/Most_Wanted/Portal> a <http://dbkwik.webdatacommons.org/marvelcinematicuniverse.wikia.com/class/cancelled> ;
    rdfs:label "Most Wanted/Portal"^^rdf:langString ;
    rdfs:comment """Characters from Most Wanted.
"""@en .

<http://dbkwik.webdatacommons.org/marvelcinematicuniverse.wikia.com/resource/Netflix> a <http://dbkwik.webdatacommons.org/marvelcinematicuniverse.wikia.com/class/linkedin> ;
    rdfs:label "Netflix"^^rdf:langString ;
    rdfs:comment """Netflix, Inc. is an American provider of on-demand Internet streaming media available to viewers in America, Europe (except Crimea), Asia (except China , North Korea and Syria), Africa and Oceania.

"""@en .

<http://dbkwik.webdatacommons.org/marvelcinematicuniverse.wikia.com/resource/New_Warriors_(TV_series)/Trivia> a <http://dbkwik.webdatacommons.org/marvelcinematicuniverse.wikia.com/class/imageless> ;
    rdfs:label "New Warriors (TV series)/Trivia"^^rdf:langString ;
    rdfs:comment """Characters from the comics adapted for the series are Doreen Green / Squirrel Girl, Craig Hollis / Mister Immortal, Dwayne Taylor / Night Thrasher, Microbe, and Deborah Fields / Debrii. It also marks the debut of the titular New Warriors group.The Marvel Cinematic Universe's version of the New Warriors included team members and peculiar aspects of the Great Lake Avengers, a mid-western iteration of the Avengers.
"""@en .

<http://dbkwik.webdatacommons.org/marvelcinematicuniverse.wikia.com/resource/New_York_Bulletin/Promotional_Campaign> a <http://dbkwik.webdatacommons.org/marvelcinematicuniverse.wikia.com/class/clear> ;
    rdfs:label "New York Bulletin/Promotional Campaign"^^rdf:langString ;
    rdfs:comment """After the premiere of Iron Fist a promotional website was released on 4 April, 2017. This in-universe website archives news covers and interviews from the New York Bulletin. The website also includes an advertisement, which links to an in-universe advertisement at the Chikara Dojo website.

"""@en .

<http://dbkwik.webdatacommons.org/marvelcinematicuniverse.wikia.com/resource/Paramount_Pictures> a <http://dbkwik.webdatacommons.org/marvelcinematicuniverse.wikia.com/class/youtube> ;
    rdfs:label "Paramount Pictures"^^rdf:langString ;
    rdfs:comment """Paramount Pictures is a film studio and subsidiary of Viacom in Hollywood, California that distributed Iron Man, Iron Man 2, Thor, and Captain America: The First Avenger until the rights were acquired by Walt Disney Studios.

"""@en .

<http://dbkwik.webdatacommons.org/marvelcinematicuniverse.wikia.com/resource/Peggy_Carter> rdfs:label "Peggy Carter"^^rdf:langString ;
    ns1:gender <http://dbkwik.webdatacommons.org/marvelcinematicuniverse.wikia.com/resource/Dottie_Underwood> ;
    rdfs:comment """Margaret Elizabeth "Peggy" Carter was one of the most prominent agents of the Strategic Scientific Reserve (SSR) during and after World War II and one of the founders of S.H.I.E.L.D.. Originally a code-breaker working at Bletchley Park, she joined the Special Operations Executive following her brother's death. Carter later joined the Strategic Scientific Reserve, an Allied deep science agency formed to fight HYDRA, the Nazi weapons division. On the mission in Germany she saved Professor Abraham Erskine from Johann Schmidt. The success of her mission enabled the SSR to start Project Rebirth and develop their Super Soldier Serum to make the army of Super Soldiers. During the project she had befriended Steve Rogers, one of the project's candidates.
"""@en .

<http://dbkwik.webdatacommons.org/marvelcinematicuniverse.wikia.com/resource/Phase_One> a <http://dbkwik.webdatacommons.org/marvelcinematicuniverse.wikia.com/class/phase_one> ;
    rdfs:label "Phase One"^^rdf:langString ;
    rdfs:comment """Phase One is the first part of the Marvel Cinematic Universe. It has also been called Avengers Assembled. From 2008 to 2012, the Phase One films grossed $3.8 billion ($3,811,026,406) worldwide. The next group of films is called Phase Two.

"""@en .

<http://dbkwik.webdatacommons.org/marvelcinematicuniverse.wikia.com/resource/Phase_Three> a <http://dbkwik.webdatacommons.org/marvelcinematicuniverse.wikia.com/class/phase> ;
    rdfs:label "Phase Three"^^rdf:langString ;
    ns1:directors <http://dbkwik.webdatacommons.org/marvelcinematicuniverse.wikia.com/resource/Anna_Boden>,
        <http://dbkwik.webdatacommons.org/marvelcinematicuniverse.wikia.com/resource/Anthony_Russo> ;
    ns1:duration 2016 ;
    ns1:films <http://dbkwik.webdatacommons.org/marvelcinematicuniverse.wikia.com/resource/Ant-Man_and_the_Wasp>,
        <http://dbkwik.webdatacommons.org/marvelcinematicuniverse.wikia.com/resource/Avengers:_Infinity_War> ;
    ns1:followedBy <http://dbkwik.webdatacommons.org/marvelcinematicuniverse.wikia.com/resource/Phase_Four> ;
    rdfs:comment """Phase Three is the third part of the Marvel Cinematic Universe after Phase Two and is to be followed by Phase Four.

"""@en .

<http://dbkwik.webdatacommons.org/marvelcinematicuniverse.wikia.com/resource/Playground_(Framework)> rdfs:label "Playground (Framework)"^^rdf:langString ;
    ns1:formerinhabitants <http://dbkwik.webdatacommons.org/marvelcinematicuniverse.wikia.com/resource/Patriot> ;
    rdfs:comment """The Playground is a virtual recreation of the real-world S.H.I.E.L.D. headquarters of the same name that serves as the headquarters for the Resistance inside the Framework.

"""@en .

<http://dbkwik.webdatacommons.org/marvelcinematicuniverse.wikia.com/resource/Quantum_Tunnel> rdfs:label "Quantum Tunnel"^^rdf:langString ;
    ns1:film <http://dbkwik.webdatacommons.org/marvelcinematicuniverse.wikia.com/resource/Ant-Man_and_the_Wasp> ;
    rdfs:comment """The Quantum Tunnel is a inter-dimensional gateway created by Hank Pym, Elihas Starr and Bill Foster that is capable of creating a portal to the Quantum Realm. 

"""@en .

<http://dbkwik.webdatacommons.org/marvelcinematicuniverse.wikia.com/resource/Richard_Day> rdfs:label "Richard Day"^^rdf:langString ;
    ns1:allies "Potential Juror Number 17"^^rdf:langString ;
    rdfs:comment """Richard Day is a New York City citizen and potential juror at "The People vs. Frank Castle".

"""@en .

<http://dbkwik.webdatacommons.org/marvelcinematicuniverse.wikia.com/resource/Rising_Tide/Promotional_Campaign> a <http://dbkwik.webdatacommons.org/marvelcinematicuniverse.wikia.com/class/clear> ;
    rdfs:label "Rising Tide/Promotional Campaign"^^rdf:langString ;
    rdfs:comment """Prior to the premiere of the first season of Agents of S.H.I.E.L.D., a promotional website was released on 12 May, 2013. This in-universe website was created by a group of hackers called the Rising Tide. Containing secretive videos and information about superheroes and S.H.I.E.L.D., they were determined to reveal the truth.
"""@en .

<http://dbkwik.webdatacommons.org/marvelcinematicuniverse.wikia.com/resource/Riyadh> rdfs:label "Riyadh"^^rdf:langString ;
    ns1:seal <http://dbkwik.webdatacommons.org/marvelcinematicuniverse.wikia.com/resource/File:Seal_of_Riyadh.svg> ;
    rdfs:comment """Riyadh is the capital and largest city of Saudi Arabia.

"""@en .

<http://dbkwik.webdatacommons.org/marvelcinematicuniverse.wikia.com/resource/Schoonebeek> rdfs:label "Schoonebeek"^^rdf:langString ;
    ns1:coat <http://dbkwik.webdatacommons.org/marvelcinematicuniverse.wikia.com/resource/File:Coat_of_Arms_of_Schoonebeek.png> ;
    rdfs:comment """Schoonebeek is a city located in Netherlands, where HYDRA leader Gideon Malick had a base of operations.

"""@en .

<http://dbkwik.webdatacommons.org/marvelcinematicuniverse.wikia.com/resource/Second_Dark_Elf_Conflict> rdfs:label "Second Dark Elf Conflict"^^rdf:langString ;
    ns1:imagebg "Dark Elves at War.jpg"^^rdf:langString ;
    rdfs:comment """The Dark Elf conflict is a conflict that lasted for thousands of years. Dating back to 2988 B.C., when Malekith, the insane, genocidal leader of the Dark Elves, attempted to use the Infinity Stone known as the Aether to eradicate the Nine Realms. After the the Dark Elves were defeated by the Asgardians led by the then-king Bor, Malekith and several others of his species went into hibernation. In 2013, during the Convergence, Jane Foster located the Aether and unintentionally attracted the attention of Malekith. A series of confrontations followed, spanning across all the Nine Realms, ending with Thor defeating Malekith at the Battle of Greenwich.

"""@en .

<http://dbkwik.webdatacommons.org/marvelcinematicuniverse.wikia.com/resource/Short_Bus> rdfs:label "Short Bus"^^rdf:langString ;
    ns1:pilot <http://dbkwik.webdatacommons.org/marvelcinematicuniverse.wikia.com/resource/Grant_Ward>,
        <http://dbkwik.webdatacommons.org/marvelcinematicuniverse.wikia.com/resource/Quake> ;
    rdfs:comment """The Short Bus was the nickname Coulson's Team gave to the van they used in Belarus while tracking Akela Amador.

"""@en .

<http://dbkwik.webdatacommons.org/marvelcinematicuniverse.wikia.com/resource/Sneepers> rdfs:label "Sneepers"^^rdf:langString ;
    ns1:planet "Sneep"^^rdf:langString ;
    rdfs:comment """The Sneepers are a race of olive-skinned aliens that populates the Galaxy.

"""@en .

<http://dbkwik.webdatacommons.org/marvelcinematicuniverse.wikia.com/resource/South_Dakota> rdfs:label "South Dakota"^^rdf:langString ;
    ns1:inhabitants <http://dbkwik.webdatacommons.org/marvelcinematicuniverse.wikia.com/resource/Hellfire> ;
    rdfs:comment """South Dakota is a state located in the nortwestern region of the United States of America.

"""@en .

<http://dbkwik.webdatacommons.org/marvelcinematicuniverse.wikia.com/resource/St._Louis> rdfs:label "St. Louis"^^rdf:langString ;
    ns1:seal <http://dbkwik.webdatacommons.org/marvelcinematicuniverse.wikia.com/resource/File:Seal_of_St._Louis.png> ;
    rdfs:comment """St. Louis is the second largest city of the state of Missouri.

"""@en .

<http://dbkwik.webdatacommons.org/marvelcinematicuniverse.wikia.com/resource/Stephany_Folsom> a <http://dbkwik.webdatacommons.org/marvelcinematicuniverse.wikia.com/class/twitter> ;
    rdfs:label "Stephany Folsom"^^rdf:langString ;
    rdfs:comment """Stephany Folsom was a screenwriter on Thor: Ragnarok.

"""@en .

<http://dbkwik.webdatacommons.org/marvelcinematicuniverse.wikia.com/resource/The_Avengers:_The_Movie> a <http://dbkwik.webdatacommons.org/marvelcinematicuniverse.wikia.com/class/game> ;
    rdfs:label "The Avengers: The Movie"^^rdf:langString ;
    rdfs:comment """The Avengers: The Movie is a cancelled video game loosely based on the film of the same name.

"""@en .

<http://dbkwik.webdatacommons.org/marvelcinematicuniverse.wikia.com/resource/The_Avengers:_The_Movie/Gallery> a <http://dbkwik.webdatacommons.org/marvelcinematicuniverse.wikia.com/class/cancelled> ;
    rdfs:label "The Avengers: The Movie/Gallery"^^rdf:langString ;
    rdfs:comment """A gallery of images from or related to the cancelled video game The Avengers: The Movie.

"""@en .

<http://dbkwik.webdatacommons.org/marvelcinematicuniverse.wikia.com/resource/The_Cosmic_Quest_Volume_One:_Beginning> rdfs:label "The Cosmic Quest Volume One: Beginning"^^rdf:langString ;
    ns1:publisher <http://dbkwik.webdatacommons.org/marvelcinematicuniverse.wikia.com/resource/Little,_Brown_Books_for_Young_Readers> ;
    rdfs:comment """The Cosmic Quest Volume One: Beginning is a book based on Avengers: Infinity War featuring The Collector and The Grandmaster.

"""@en .

<http://dbkwik.webdatacommons.org/marvelcinematicuniverse.wikia.com/resource/The_Cosmic_Quest_Volume_Two> rdfs:label "The Cosmic Quest Volume Two"^^rdf:langString ;
    ns1:publisher <http://dbkwik.webdatacommons.org/marvelcinematicuniverse.wikia.com/resource/Little,_Brown_Books_for_Young_Readers> ;
    rdfs:comment """The Cosmic Quest Volume Two is a book based on Avengers: Infinity War featuring Erik Selvig.

"""@en .

<http://dbkwik.webdatacommons.org/marvelcinematicuniverse.wikia.com/resource/The_Defenders> rdfs:label "The Defenders"^^rdf:langString ;
    ns1:last <http://dbkwik.webdatacommons.org/marvelcinematicuniverse.wikia.com/resource/The_Defenders_(episode)> ;
    rdfs:comment """Marvel's The Defenders, or simply The Defenders, is a Netflix television miniseries that features Daredevil, Jessica Jones, Luke Cage and Iron Fist joining together to form the Defenders.
It premiered on August 18, 2017.

"""@en .

<http://dbkwik.webdatacommons.org/marvelcinematicuniverse.wikia.com/resource/The_Defenders/Trivia> a <http://dbkwik.webdatacommons.org/marvelcinematicuniverse.wikia.com/class/stub> ;
    rdfs:label "The Defenders/Trivia"^^rdf:langString ;
    rdfs:comment """A list of trivia related to The Defenders.

"""@en .

<http://dbkwik.webdatacommons.org/marvelcinematicuniverse.wikia.com/resource/The_Punisher/Trivia> a <http://dbkwik.webdatacommons.org/marvelcinematicuniverse.wikia.com/class/stub> ;
    rdfs:label "The Punisher/Trivia"^^rdf:langString ;
    rdfs:comment """A list of trivia related to The Punisher.

"""@en .

<http://dbkwik.webdatacommons.org/marvelcinematicuniverse.wikia.com/resource/The_Well> rdfs:label "The Well"^^rdf:langString ;
    ns1:eason 1 ;
    rdfs:comment """The Well is the eighth episode of the first season of the television series Agents of S.H.I.E.L.D.

"""@en .

<http://dbkwik.webdatacommons.org/marvelcinematicuniverse.wikia.com/resource/Thor:_The_Dark_World_-_The_Official_Game> a <http://dbkwik.webdatacommons.org/marvelcinematicuniverse.wikia.com/class/game> ;
    rdfs:label "Thor: The Dark World - The Official Game"^^rdf:langString ;
    ns1:system ", ,"^^rdf:langString ;
    rdfs:comment """Thor: The Dark World - The Official Game is a 2013 video game loosely based on the film of the same name. This game was released on October, 31, 2013 and allows players to control Thor.
This game acts in a Hack and Slash kind of game, where the player can face the Dark Elves and other Nine Realms' foes.

"""@en .

<http://dbkwik.webdatacommons.org/marvelcinematicuniverse.wikia.com/resource/Tom_Morello> rdfs:label "Tom Morello"^^rdf:langString ;
    ns1:contribution <http://dbkwik.webdatacommons.org/marvelcinematicuniverse.wikia.com/resource/Iron_Man_(film)> ;
    rdfs:comment """Thomas Baptise "Tom" Morello is an American guitarist best known for his tenure with the bands Rage Against the Machine, Audioslave, his acoustic solo act The Nightwatchman and his newest group, Street Sweeper Social Club. He played guitar on the soundtracks of Iron Man and Iron Man 2, and had a cameo in the first film as a member of the Ten Rings.
His collaboration with Raury, "Friends" is featured in the Runaways episode Reunion.

"""@en .

<http://dbkwik.webdatacommons.org/marvelcinematicuniverse.wikia.com/resource/Twitter_Profile/Pym_Technologies> a <http://dbkwik.webdatacommons.org/marvelcinematicuniverse.wikia.com/class/google+> ;
    rdfs:label "Twitter Profile/Pym Technologies"^^rdf:langString ;
    rdfs:comment """The Twitter profile of Pym Technologies was part of the 2015 Ant-Man promotional campaign. It supported the WIRED Insider: Darren Cross interview.

"""@en .

<http://dbkwik.webdatacommons.org/marvelcinematicuniverse.wikia.com/resource/Twitter_Profile/WHiH_Newsfront> a <http://dbkwik.webdatacommons.org/marvelcinematicuniverse.wikia.com/class/google+> ;
    rdfs:label "Twitter Profile/WHiH Newsfront"^^rdf:langString ;
    rdfs:comment """The Twitter profile of WHiH Newsfront is part of promotional campaign of the movies Ant-Man and Captain America: Civil War. It started with the Ant-Man promotional campaign in July 2015. It supported the videos of the WHiH Newsfront web series. This is a page which includes all the Twitter posts of WHiH Newsfront.

"""@en .

<http://dbkwik.webdatacommons.org/marvelcinematicuniverse.wikia.com/resource/Universal_Pictures> a <http://dbkwik.webdatacommons.org/marvelcinematicuniverse.wikia.com/class/youtube> ;
    rdfs:label "Universal Pictures"^^rdf:langString ;
    rdfs:comment """Universal Pictures is a major film studio in Hollywood, and the current holder of distribution rights for solo Hulk movies. In 2005, Marvel Studios regained the film rights from Universal for the Hulk after the mixed critical reception of the 2003 Hulk film. In 2008, Marvel Studios and Universal collaborated on the movie The Incredible Hulk. 

"""@en .

<http://dbkwik.webdatacommons.org/marvelcinematicuniverse.wikia.com/resource/Valkyrie_(Vehicle)> rdfs:label "Valkyrie (Vehicle)"^^rdf:langString ;
    ns1:weapons <http://dbkwik.webdatacommons.org/marvelcinematicuniverse.wikia.com/resource/HYDRA_Cannon>,
        <http://dbkwik.webdatacommons.org/marvelcinematicuniverse.wikia.com/resource/HYDRA_Parasit> ;
    rdfs:comment """The Valkyrie was an advanced bomber plane used by HYDRA during World War II.

"""@en .

<http://dbkwik.webdatacommons.org/marvelcinematicuniverse.wikia.com/resource/Walt_Disney_Studios> a <http://dbkwik.webdatacommons.org/marvelcinematicuniverse.wikia.com/class/google+> ;
    rdfs:label "Walt Disney Studios"^^rdf:langString ;
    rdfs:comment """Walt Disney Studios is a film studio and a division of The Walt Disney Company in Burbank, California that owns the film rights to and distributes almost all the Marvel Cinematic Universe movies.

"""@en .

<http://dbkwik.webdatacommons.org/marvelcinematicuniverse.wikia.com/resource/Yellowjacket/Gallery> a <http://dbkwik.webdatacommons.org/marvelcinematicuniverse.wikia.com/class/clear> ;
    rdfs:label "Yellowjacket/Gallery"^^rdf:langString ;
    rdfs:comment """A gallery of images of the Cross Technologies CEO Darren Cross.

"""@en .

<http://dbkwik.webdatacommons.org/marvelcinematicuniverse.wikia.com/resource/Yorkes_Residence> rdfs:label "Yorkes Residence"^^rdf:langString ;
    ns1:appearances <http://dbkwik.webdatacommons.org/marvelcinematicuniverse.wikia.com/resource/Runaways_(TV_series)> ;
    rdfs:comment """The Yorkes Residence was the place of living of Dale, Stacey and Gert Yorkes as well as Molly Hernandez.

"""@en .

<http://marvelcinematicuniverse.wikia.com/wiki/Special:FilePath/$.jpeg> a ns3:Image ;
    dc:rights <http://marvelcinematicuniverse.wikia.com/wiki/File:$.jpeg> ;
    foaf:thumbnail <http://marvelcinematicuniverse.wikia.com/wiki/Special:FilePath/$.jpeg?width=300> .

<http://marvelcinematicuniverse.wikia.com/wiki/Special:FilePath/%0A0-8-4.png> a ns3:Image ;
    dc:rights <http://marvelcinematicuniverse.wikia.com/wiki/File:%0A0-8-4.png> ;
    foaf:thumbnail <http://marvelcinematicuniverse.wikia.com/wiki/Special:FilePath/%0A0-8-4.png?width=300> .

<http://marvelcinematicuniverse.wikia.com/wiki/Special:FilePath/%0A14322773_1183458818385631_8153783337637045775_n.jpg> a ns3:Image ;
    dc:rights <http://marvelcinematicuniverse.wikia.com/wiki/File:%0A14322773_1183458818385631_8153783337637045775_n.jpg> ;
    foaf:thumbnail <http://marvelcinematicuniverse.wikia.com/wiki/Special:FilePath/%0A14322773_1183458818385631_8153783337637045775_n.jpg?width=300> .

<http://marvelcinematicuniverse.wikia.com/wiki/Special:FilePath/%0A33_Brookton.png> foaf:thumbnail <http://marvelcinematicuniverse.wikia.com/wiki/Special:FilePath/%0A33_Brookton.png?width=300> .

<http://marvelcinematicuniverse.wikia.com/wiki/Special:FilePath/%0A33_Carla.png> foaf:thumbnail <http://marvelcinematicuniverse.wikia.com/wiki/Special:FilePath/%0A33_Carla.png?width=300> .

<http://dbkwik.webdatacommons.org/marvelcinematicuniverse.wikia.com/class/col-end> a owl:Class ;
    rdfs:label "Col-end"@en .

<http://dbkwik.webdatacommons.org/marvelcinematicuniverse.wikia.com/class/delete> a owl:Class ;
    rdfs:label "Delete"@en .

<http://dbkwik.webdatacommons.org/marvelcinematicuniverse.wikia.com/class/expand> a owl:Class ;
    rdfs:label "Expand"@en .

<http://dbkwik.webdatacommons.org/marvelcinematicuniverse.wikia.com/class/imageless> a owl:Class ;
    rdfs:label "Imageless"@en .

<http://dbkwik.webdatacommons.org/marvelcinematicuniverse.wikia.com/class/instagram> a owl:Class ;
    rdfs:label "Instagram"@en .

<http://dbkwik.webdatacommons.org/marvelcinematicuniverse.wikia.com/class/magazine> a owl:Class ;
    rdfs:label "Magazine"@en .

<http://dbkwik.webdatacommons.org/marvelcinematicuniverse.wikia.com/class/otheruses> a owl:Class ;
    rdfs:label "Otheruses"@en .

<http://dbkwik.webdatacommons.org/marvelcinematicuniverse.wikia.com/class/phase_one> a owl:Class ;
    rdfs:label "Phase One"@en .

<http://dbkwik.webdatacommons.org/marvelcinematicuniverse.wikia.com/class/rewrite> a owl:Class ;
    rdfs:label "Rewrite"@en .

<http://dbkwik.webdatacommons.org/marvelcinematicuniverse.wikia.com/class/section> a owl:Class ;
    rdfs:label "Section"@en .

<http://dbkwik.webdatacommons.org/marvelcinematicuniverse.wikia.com/class/twitter> a owl:Class ;
    rdfs:label "Twitter"@en .

<http://dbkwik.webdatacommons.org/marvelcinematicuniverse.wikia.com/resource/0-8-4_(Code)> a <http://dbkwik.webdatacommons.org/marvelcinematicuniverse.wikia.com/class/quote> ;
    rdfs:label "0-8-4 (Code)"^^rdf:langString ;
    ns3:abstract """An 0-8-4 is an object of unknown origin detected by S.H.I.E.L.D.. Depending on the situation, either a small or large group of agents are sent to determine what the 0-8-4 is, and how it could be used.
The code "0-8-4" derives from the identification number used on the case containing the first object of unknown origin encountered by the Strategic Scientific Reserve, the precursor of S.H.I.E.L.D. The object was a Diviner obtained by Peggy Carter during the raid of the HYDRA Research Facility in Austria in 1945. It was most likely the eighty-fourth item catalogued during the raid.
Leo Fitz explained to Skye that he had never experienced an 0-8-4 being a person, though it was possible. He elaborated by saying that he has read about weapons, spacecrafts, and energy sources labeled as 0-8-4s, citing that the only characteristic they had in common is that all were dangerous.

"""@en ;
    rdfs:comment """An 0-8-4 is an object of unknown origin detected by S.H.I.E.L.D.. Depending on the situation, either a small or large group of agents are sent to determine what the 0-8-4 is, and how it could be used.
The code "0-8-4" derives from the identification number used on the case containing the first object of unknown origin encountered by the Strategic Scientific Reserve, the precursor of S.H.I.E.L.D. The object was a Diviner obtained by Peggy Carter during the raid of the HYDRA Research Facility in Austria in 1945. It was most likely the eighty-fourth item catalogued during the raid.
"""@en ;
    skos:altLabel "0-8-4 (Code)"^^rdf:langString .

<http://dbkwik.webdatacommons.org/marvelcinematicuniverse.wikia.com/resource/0-8-4_(episode)> a <http://dbkwik.webdatacommons.org/marvelcinematicuniverse.wikia.com/class/episode> ;
    rdfs:label "0-8-4 (episode)"^^rdf:langString ;
    ns1:director <http://dbkwik.webdatacommons.org/marvelcinematicuniverse.wikia.com/resource/David_Straiton> ;
    ns1:firstAired "2013-10-01"^^xsd:date ;
    ns1:next <http://dbkwik.webdatacommons.org/marvelcinematicuniverse.wikia.com/resource/The_Asset> ;
    ns1:previous <http://dbkwik.webdatacommons.org/marvelcinematicuniverse.wikia.com/resource/Pilot> ;
    ns1:season 1 ;
    ns1:writer <http://dbkwik.webdatacommons.org/marvelcinematicuniverse.wikia.com/resource/Jed_Whedon>,
        <http://dbkwik.webdatacommons.org/marvelcinematicuniverse.wikia.com/resource/Jeffrey_Bell> ;
    ns3:wikiPageExternalLink <http://marvel.wikia.com/wiki/Main_Page> ;
    rdfs:comment """0-8-4 is the second episode of the first season of the television series Agents of S.H.I.E.L.D.

"""@en .

<http://dbkwik.webdatacommons.org/marvelcinematicuniverse.wikia.com/resource/15th_Precinct_Police_Station> a <http://dbkwik.webdatacommons.org/marvelcinematicuniverse.wikia.com/class/location> ;
    rdfs:label "15th Precinct Police Station"^^rdf:langString ;
    ns1:continent <http://dbkwik.webdatacommons.org/marvelcinematicuniverse.wikia.com/resource/North_America> ;
    ns1:tvSeries <http://dbkwik.webdatacommons.org/marvelcinematicuniverse.wikia.com/resource/Daredevil_(TV_series)> ;
    rdfs:comment """The 15th Precinct Police Station is one of the main police stations in the neighborhood of Hell's Kitchen, New York City.

"""@en .

<http://dbkwik.webdatacommons.org/marvelcinematicuniverse.wikia.com/resource/1950s> a <http://dbkwik.webdatacommons.org/marvelcinematicuniverse.wikia.com/class/timeline> ;
    rdfs:label "1950s"^^rdf:langString ;
    rdfs:comment """This is a timeline of events that occurred during the 1950s.

"""@en .

<http://dbkwik.webdatacommons.org/marvelcinematicuniverse.wikia.com/resource/1980s> a <http://dbkwik.webdatacommons.org/marvelcinematicuniverse.wikia.com/class/timeline> ;
    rdfs:label "1980s"^^rdf:langString ;
    rdfs:comment """This is a timeline of events that occurred during the 1980s.

"""@en .

<http://dbkwik.webdatacommons.org/marvelcinematicuniverse.wikia.com/resource/1990s> a <http://dbkwik.webdatacommons.org/marvelcinematicuniverse.wikia.com/class/timeline> ;
    rdfs:label "1990s"^^rdf:langString ;
    rdfs:comment """This is a timeline of events that occurred during the 1990s.

"""@en .

<http://dbkwik.webdatacommons.org/marvelcinematicuniverse.wikia.com/resource/2012> rdfs:label "2012"^^rdf:langString ;
    rdfs:comment """This is a timeline of events that occurred in 2012.

"""@en .

<http://dbkwik.webdatacommons.org/marvelcinematicuniverse.wikia.com/resource/A%27askavariia> a <http://dbkwik.webdatacommons.org/marvelcinematicuniverse.wikia.com/class/location> ;
    rdfs:label "A'askavariia"^^rdf:langString ;
    ns1:movie <http://dbkwik.webdatacommons.org/marvelcinematicuniverse.wikia.com/resource/Guardians_of_the_Galaxy_Vol._2> ;
    ns1:population <http://dbkwik.webdatacommons.org/marvelcinematicuniverse.wikia.com/resource/A%27askavariians> ;
    rdfs:comment """A'askavariia is the home planet of the A'askavariians.

"""@en .

<http://dbkwik.webdatacommons.org/marvelcinematicuniverse.wikia.com/resource/A%27askavariians> a <http://dbkwik.webdatacommons.org/marvelcinematicuniverse.wikia.com/class/quote> ;
    rdfs:label "A'askavariians"^^rdf:langString ;
    ns1:homeplanet <http://dbkwik.webdatacommons.org/marvelcinematicuniverse.wikia.com/resource/A%27askavariia> ;
    ns1:movie <http://dbkwik.webdatacommons.org/marvelcinematicuniverse.wikia.com/resource/Guardians_of_the_Galaxy_(film)> ;
    rdfs:comment """A'askvariians are an alien race encountered by Peter Quill.

"""@en .

<http://dbkwik.webdatacommons.org/marvelcinematicuniverse.wikia.com/resource/AKA_Freak_Accident> rdfs:label "AKA Freak Accident"^^rdf:langString ;
    rdfs:comment """AKA Freak Accident is the second episode of the second season of the television series Jessica Jones, and the fifteenth episode overall.

"""@en .

<http://dbkwik.webdatacommons.org/marvelcinematicuniverse.wikia.com/resource/AKA_I%27ve_Got_the_Blues> rdfs:label "AKA I've Got the Blues"^^rdf:langString ;
    rdfs:comment """AKA I've Got the Blues is the eleventh episode of the first season of the Netflix exclusive television series Jessica Jones.

"""@en .

<http://dbkwik.webdatacommons.org/marvelcinematicuniverse.wikia.com/resource/AKA_I_Want_Your_Cray_Cray> rdfs:label "AKA I Want Your Cray Cray"^^rdf:langString ;
    rdfs:comment """AKA I Want Your Cray Cray is the seventh episode of the second season of the television series Jessica Jones, and the twentieth episode overall.

"""@en .

<http://dbkwik.webdatacommons.org/marvelcinematicuniverse.wikia.com/resource/AKA_Pork_Chop> rdfs:label "AKA Pork Chop"^^rdf:langString ;
    rdfs:comment """AKA Pork Chop is the tenth episode of the second season of the television series Jessica Jones, and the twenty-third episode overall.

"""@en .

<http://dbkwik.webdatacommons.org/marvelcinematicuniverse.wikia.com/resource/AKA_Sin_Bin> rdfs:label "AKA Sin Bin"^^rdf:langString ;
    rdfs:comment """AKA Sin Bin is the ninth episode of the first season of the Netflix exclusive television series Jessica Jones.

"""@en .

<http://dbkwik.webdatacommons.org/marvelcinematicuniverse.wikia.com/resource/Aakon> a <http://dbkwik.webdatacommons.org/marvelcinematicuniverse.wikia.com/class/location> ;
    rdfs:label "Aakon"^^rdf:langString ;
    ns1:population <http://dbkwik.webdatacommons.org/marvelcinematicuniverse.wikia.com/resource/Aakons> ;
    rdfs:comment """Aakon is the homeworld of the Aakons.

"""@en .

<http://dbkwik.webdatacommons.org/marvelcinematicuniverse.wikia.com/resource/Aakons> a <http://dbkwik.webdatacommons.org/marvelcinematicuniverse.wikia.com/class/race> ;
    rdfs:label "Aakons"^^rdf:langString ;
    ns1:homeplanet <http://dbkwik.webdatacommons.org/marvelcinematicuniverse.wikia.com/resource/Aakon> ;
    rdfs:comment """The Aakons are race of hairless yellow-skinned aliens that are spread throughout the galaxy.

"""@en .

<http://dbkwik.webdatacommons.org/marvelcinematicuniverse.wikia.com/resource/Aaron> a <http://dbkwik.webdatacommons.org/marvelcinematicuniverse.wikia.com/class/character> ;
    rdfs:label "Aaron"^^rdf:langString ;
    ns1:actor <http://dbkwik.webdatacommons.org/marvelcinematicuniverse.wikia.com/resource/D.C._Pierson> ;
    ns1:gender "Male"^^rdf:langString ;
    ns1:species <http://dbkwik.webdatacommons.org/marvelcinematicuniverse.wikia.com/resource/Humans> ;
    rdfs:comment """Aaron is an employee who worked at Apple Inc. in a shopping mall in Washington, D.C..

"""@en .

<http://dbkwik.webdatacommons.org/marvelcinematicuniverse.wikia.com/resource/Aaron_(Baby)> a <http://dbkwik.webdatacommons.org/marvelcinematicuniverse.wikia.com/class/character> ;
    rdfs:label "Aaron (Baby)"^^rdf:langString ;
    ns1:gender "Male"^^rdf:langString ;
    ns1:species <http://dbkwik.webdatacommons.org/marvelcinematicuniverse.wikia.com/resource/Humans> ;
    rdfs:comment """Aaron is the newborn son of Sophie and Marcus.

"""@en .

<http://dbkwik.webdatacommons.org/marvelcinematicuniverse.wikia.com/resource/Aaron_Hendry> rdfs:label "Aaron Hendry"^^rdf:langString ;
    ns1:character <http://dbkwik.webdatacommons.org/marvelcinematicuniverse.wikia.com/resource/Loyolis> ;
    rdfs:comment """Aaron Hendry portrayed Loyolis in the Inhumans episodes Behold…The Inhumans!, Those Who Would Destroy Us, The Gentleman's Name is Gorgon, Havoc in the Hidden Land and ...And Finally: Black Bolt.

"""@en .

<http://dbkwik.webdatacommons.org/marvelcinematicuniverse.wikia.com/resource/Abomination> rdfs:label "Abomination"^^rdf:langString ;
    ns1:actor <http://dbkwik.webdatacommons.org/marvelcinematicuniverse.wikia.com/resource/Tim_Roth> ;
    ns1:affiliation <http://dbkwik.webdatacommons.org/marvelcinematicuniverse.wikia.com/resource/Strategic_Operations_Command_Center> ;
    ns1:age 47 ;
    ns1:comic <http://dbkwik.webdatacommons.org/marvelcinematicuniverse.wikia.com/resource/The_Avengers_Prelude:_Fury%27s_Big_Week>,
        <http://dbkwik.webdatacommons.org/marvelcinematicuniverse.wikia.com/resource/The_Incredible_Hulk:_The_Big_Picture> ;
    ns1:oneshot <http://dbkwik.webdatacommons.org/marvelcinematicuniverse.wikia.com/resource/Marvel_One-Shot:_The_Consultant> ;
    ns1:voiceActor <http://dbkwik.webdatacommons.org/marvelcinematicuniverse.wikia.com/resource/Fred_Tatasciore>,
        <http://dbkwik.webdatacommons.org/marvelcinematicuniverse.wikia.com/resource/J.B._Blanc> ;
    ns1:webSeries <http://dbkwik.webdatacommons.org/marvelcinematicuniverse.wikia.com/resource/WHiH_Newsfront_(web_series)> ;
    rdfs:comment """Emil Blonsky is a former special-ops commando with the British Royal Marines on loan to General Thaddeus Ross in his efforts to capture Bruce Banner better known as Hulk. Blonsky was injected with a small dose of the mothballed original Super Soldier Serum and later was injected with Bruce Banner's blood causing him to transform into the Hulk-sized Abomination. He then proceeded to go on a rampage in Harlem until he was defeated by Hulk and captured by the United States Armed Forces.

"""@en .

<http://dbkwik.webdatacommons.org/marvelcinematicuniverse.wikia.com/resource/Abraham_Attah> rdfs:label "Abraham Attah"^^rdf:langString ;
    rdfs:comment """Abraham Attah portrayed Abe Brown in Spider-Man: Homecoming and Spider-Man: Far From Home.

"""@en .

<http://dbkwik.webdatacommons.org/marvelcinematicuniverse.wikia.com/resource/Adam_Harrington_(actor)> rdfs:label "Adam Harrington (actor)"^^rdf:langString ;
    rdfs:comment """Adam Harrington portrayed Reporter in Iron Man.

"""@en .

<http://dbkwik.webdatacommons.org/marvelcinematicuniverse.wikia.com/resource/Adam_Warlock> rdfs:label "Adam Warlock"^^rdf:langString ;
    ns1:citizenship <http://dbkwik.webdatacommons.org/marvelcinematicuniverse.wikia.com/resource/Sovereign_(Planet)> ;
    rdfs:comment """Adam is an android created by Ayesha in order to help her destroy the Guardians of the Galaxy.

"""@en .

<http://dbkwik.webdatacommons.org/marvelcinematicuniverse.wikia.com/resource/Adolf_Hitler> rdfs:label "Adolf Hitler"^^rdf:langString ;
    ns1:age 56 ;
    rdfs:comment """Adolf Hitler was the Führer und Reichskanzler of Nazi Germany, the Third Reich, before and during World War II. He started the war with the intention to create the German Empire that would dominate Europe. He was responsible for a genocide in which about six million European Jews and other people were murdered. His reign of terror also gave rise to another great war criminal, Johann Schmidt, the infamous Red Skull.

"""@en .

<http://dbkwik.webdatacommons.org/marvelcinematicuniverse.wikia.com/resource/Adria> rdfs:label "Adria"^^rdf:langString ;
    ns1:dod <http://dbkwik.webdatacommons.org/marvelcinematicuniverse.wikia.com/resource/1990s> ;
    ns1:realName <http://dbkwik.webdatacommons.org/marvelcinematicuniverse.wikia.com/resource/Adria> ;
    rdfs:comment """Adria was the wife of Kaecilius, who died because of a brain aneurysm.

"""@en .

<http://dbkwik.webdatacommons.org/marvelcinematicuniverse.wikia.com/resource/Adrian_Toomes%27_Crew> a <http://dbkwik.webdatacommons.org/marvelcinematicuniverse.wikia.com/class/organization> ;
    rdfs:label "Adrian Toomes' Crew"^^rdf:langString ;
    ns1:formermembers <http://dbkwik.webdatacommons.org/marvelcinematicuniverse.wikia.com/resource/Jackson_Brice> ;
    ns1:leader <http://dbkwik.webdatacommons.org/marvelcinematicuniverse.wikia.com/resource/Vulture> ;
    ns1:locations <http://dbkwik.webdatacommons.org/marvelcinematicuniverse.wikia.com/resource/New_York_City> ;
    ns1:members <http://dbkwik.webdatacommons.org/marvelcinematicuniverse.wikia.com/resource/Randy_Vale> ;
    rdfs:comment """Adrian Toomes' Crew, formerly known as Bestman Salvage, was a cleanup crew that held a contract to salvage any incidents occurring in New York City. Following the Battle of New York, the crew were replaced by the Department of Damage Control, causing Toomes, still in possession of Chitauri technology from their initial clean-up, to commission a specialized exo-suit created for him. Over the next few years, Toomes used the suit to steal artifacts collected by Damage Control from Avengers battles, which he had the Tinkerer modify. The crew then sold weapons made from Chitauri, Dark Elf, S.H.I.E.L.D., Ultron and HYDRA technology and sold them to buyers on the black market.

"""@en .

<http://dbkwik.webdatacommons.org/marvelcinematicuniverse.wikia.com/resource/Adrian_Younge_(actor)> rdfs:label "Adrian Younge (actor)"^^rdf:langString ;
    rdfs:comment """Adrian Younge scored Luke Cage with Ali Shaheed Muhammad.
He portrayed himself in the Luke Cage episodes All Souled Out and They Reminisce Over You (T.R.O.Y.).

"""@en .

<http://dbkwik.webdatacommons.org/marvelcinematicuniverse.wikia.com/resource/Afghanistan> rdfs:label "Afghanistan"^^rdf:langString ;
    ns1:interest <http://dbkwik.webdatacommons.org/marvelcinematicuniverse.wikia.com/resource/Bagram>,
        <http://dbkwik.webdatacommons.org/marvelcinematicuniverse.wikia.com/resource/Bakhmala> ;
    ns1:notable <http://dbkwik.webdatacommons.org/marvelcinematicuniverse.wikia.com/resource/Ahmad_Zubair>,
        <http://dbkwik.webdatacommons.org/marvelcinematicuniverse.wikia.com/resource/Ho_Yinsen> ;
    rdfs:comment """Afghanistan, officially the Islamic Republic of Afghanistan, is a landlocked country in Asia.

"""@en .

<http://dbkwik.webdatacommons.org/marvelcinematicuniverse.wikia.com/resource/Afterlife> rdfs:label "Afterlife"^^rdf:langString ;
    ns1:notable <http://dbkwik.webdatacommons.org/marvelcinematicuniverse.wikia.com/resource/Alisha_Whitley> ;
    ns1:population <http://dbkwik.webdatacommons.org/marvelcinematicuniverse.wikia.com/resource/Inhumans> ;
    rdfs:comment """Afterlife (來世 Lai Shi, translated as "Next Life") was an Inhuman settlement.

"""@en .

<http://dbkwik.webdatacommons.org/marvelcinematicuniverse.wikia.com/resource/Agent_Carter_(TV_series)/Season_One> a <http://dbkwik.webdatacommons.org/marvelcinematicuniverse.wikia.com/class/season> ;
    rdfs:label "Agent Carter (TV series)/Season One"^^rdf:langString ;
    ns1:channel <http://dbkwik.webdatacommons.org/marvelcinematicuniverse.wikia.com/resource/American_Broadcasting_Company> ;
    ns1:dates "--01-06"^^xsd:gMonthDay ;
    ns1:episodes 8 ;
    rdfs:comment """The First Season of Agent Carter premiered on January 6, 2015 on ABC.

"""@en .

<http://dbkwik.webdatacommons.org/marvelcinematicuniverse.wikia.com/resource/Agents_of_S.H.I.E.L.D./Season_Four> a <http://dbkwik.webdatacommons.org/marvelcinematicuniverse.wikia.com/class/season> ;
    rdfs:label "Agents of S.H.I.E.L.D./Season Four"^^rdf:langString ;
    ns1:episodes 22 ;
    rdfs:comment """The Fourth Season of Agents of S.H.I.E.L.D. was officially confirmed on March 3, 2016 by ABC. The season premiered on September 20, 2016.

"""@en .

<http://dbkwik.webdatacommons.org/marvelcinematicuniverse.wikia.com/resource/Agents_of_S.H.I.E.L.D._(Season_Two)/Home_Video> a <http://dbkwik.webdatacommons.org/marvelcinematicuniverse.wikia.com/class/dvd> ;
    rdfs:label "Agents of S.H.I.E.L.D. (Season Two)/Home Video"^^rdf:langString ;
    ns1:runtime "56760.0"^^<http://dbkwik.webdatacommons.org/datatype/second> ;
    ns1:series <http://dbkwik.webdatacommons.org/marvelcinematicuniverse.wikia.com/resource/Agents_of_S.H.I.E.L.D.> ;
    rdfs:comment """Agents of S.H.I.E.L.D. - The Complete Second Season is the DVD and Blu-ray release for Agents of S.H.I.E.L.D. Season Two.

"""@en .

<http://dbkwik.webdatacommons.org/marvelcinematicuniverse.wikia.com/resource/Agon> rdfs:label "Agon"^^rdf:langString ;
    ns1:affiliation <http://dbkwik.webdatacommons.org/marvelcinematicuniverse.wikia.com/resource/Inhuman_Royal_Family> ;
    rdfs:comment """Agon was the former King of the Inhumans and father of Black Bolt and Maximus.

"""@en .

<http://dbkwik.webdatacommons.org/marvelcinematicuniverse.wikia.com/resource/Ahmad_Zubair> rdfs:label "Ahmad Zubair"^^rdf:langString ;
    rdfs:comment """Ahmad Zubair was a member of the Afghan National Police and had cooperated with Dinah Madani in an investigation into Afghan heroin smuggling. When Zubair uncovered some of the illegal actions of Operation Cerberus, as well as the operation's ties to the smuggling, he was painted a "terrorist" by William Rawlins and captured by Cerberus Squad. While Rawlins did not disclosed the real reasons for capturing and detaining Zubair, he personally took charge of torturing him. Despite Zubair insisting upon his innocence, Rawlins had then ordered Lieutenant Frank Castle to illegally execute him.

"""@en .

<http://dbkwik.webdatacommons.org/marvelcinematicuniverse.wikia.com/resource/Akela_Amador> rdfs:label "Akela Amador"^^rdf:langString ;
    ns1:clearance <http://dbkwik.webdatacommons.org/marvelcinematicuniverse.wikia.com/resource/Clearance_Level> ;
    ns1:idno "A 9632284"^^rdf:langString ;
    rdfs:comment """Akela Amador is a former S.H.I.E.L.D. agent who was presumed dead, and reappeared on the grid committing diamond heists. A former protégé of Agent Phil Coulson, Amador was an unwilling servant of HYDRA for several years.

"""@en .

<http://dbkwik.webdatacommons.org/marvelcinematicuniverse.wikia.com/resource/Alan_Fine> rdfs:label "Alan Fine"^^rdf:langString ;
    ns1:documentary <http://dbkwik.webdatacommons.org/marvelcinematicuniverse.wikia.com/resource/Marvel_75_Years:_From_Pulp_to_Pop>,
        <http://dbkwik.webdatacommons.org/marvelcinematicuniverse.wikia.com/resource/Marvel_Studios:_Assembling_a_Universe> ;
    ns1:produced <http://dbkwik.webdatacommons.org/marvelcinematicuniverse.wikia.com/resource/Agent_Carter_(TV_series)>,
        <http://dbkwik.webdatacommons.org/marvelcinematicuniverse.wikia.com/resource/Agents_of_S.H.I.E.L.D.> ;
    rdfs:comment """Alan Fine is an executive producer on Iron Man 2, Thor, Marvel One-Shot: The Consultant, Captain America: The First Avenger, Marvel One-Shot: A Funny Thing Happened on the Way to Thor's Hammer, The Avengers, Marvel One-Shot: Item 47, Iron Man 3, Marvel One-Shot: Agent Carter, Agents of S.H.I.E.L.D., Thor: The Dark World, Marvel One-Shot: All Hail the King, Captain America: The Winter Soldier, Guardians of the Galaxy, Agent Carter, Daredevil, Avengers: Age of Ultron, Ant-Man, Jessica Jones, Luke Cage, Doctor Strange, The Defenders, Cloak & Dagger and Avengers: Infinity War.
"""@en .

<http://dbkwik.webdatacommons.org/marvelcinematicuniverse.wikia.com/resource/Algeria> rdfs:label "Algeria"^^rdf:langString ;
    rdfs:comment """Algeria is a country located in Africa.

"""@en .

<http://dbkwik.webdatacommons.org/marvelcinematicuniverse.wikia.com/resource/Alisha_Whitley> rdfs:label "Alisha Whitley"^^rdf:langString ;
    rdfs:comment """Alisha Whitley was an Inhuman who lived in Afterlife and acted as Jiaying's one-woman army when she waged open war against S.H.I.E.L.D.. In the aftermath of the war, Whitley focused her efforts on protecting Inhumans targeted by Lash, entering an alliance with S.H.I.E.L.D. to accomplish this. However, Whitley was targeted by Hive and infected by the parasitic Inhuman, serving him and his plans for world domination until her eventual violent death at the hands of the Kree Reapers while attempting to protect Hive.

"""@en .

<http://dbkwik.webdatacommons.org/marvelcinematicuniverse.wikia.com/resource/Amanda_Rea> rdfs:label "Amanda Rea"^^rdf:langString ;
    rdfs:comment """Amanda Rea voiced Aida in the Agents of S.H.I.E.L.D. episode Ascension.
She also portrayed Girlfriend in Runaways.

"""@en .

<http://dbkwik.webdatacommons.org/marvelcinematicuniverse.wikia.com/resource/Ambush_at_the_Staten_Island_Ferry> rdfs:label "Ambush at the Staten Island Ferry"^^rdf:langString ;
    rdfs:comment """The Ambush at the Staten Island Ferry was a conflict between Spider-Man, Vulture, Mac Gargan, and FBI that began when the web-slinger attempted to hijack an illegal arms deal between Gargan and Adrian Toomes' Crew.

"""@en .

<http://dbkwik.webdatacommons.org/marvelcinematicuniverse.wikia.com/resource/Ambush_on_Peter_Parker> rdfs:label "Ambush on Peter Parker"^^rdf:langString ;
    rdfs:comment """The Ambush on Peter Parker was a failed attack instigated by Shocker to prevent Spider-Man from interfering with Vulture's plan to hijack the Stark Cargo Plane.

"""@en .

<http://dbkwik.webdatacommons.org/marvelcinematicuniverse.wikia.com/resource/Among_Us_Hide...> rdfs:label "Among Us Hide..."^^rdf:langString ;
    rdfs:comment """Among Us Hide... is the sixth episode of the third season of the television series Agents of S.H.I.E.L.D. and the fiftieth episode overall.

"""@en .

<http://dbkwik.webdatacommons.org/marvelcinematicuniverse.wikia.com/resource/Andrea_Di_Vito> rdfs:label "Andrea Di Vito"^^rdf:langString ;
    rdfs:comment """Andrea Di Vito was an artist for Guardians of the Galaxy Prequel Infinite Comic, Guardians of the Galaxy: Galaxy's Most Wanted, Ant-Man: Larger Than Life, Avengers: Operation HYDRA, Captain America: Road to War. and Doctor Strange: Mystic Apprentice.

"""@en .

<http://dbkwik.webdatacommons.org/marvelcinematicuniverse.wikia.com/resource/Andres_Mossa> rdfs:label "Andres Mossa"^^rdf:langString ;
    rdfs:comment """Andres Mossa was an artist for Thor: The Dark World Prelude and Ant-Man - Scott Lang: Small Time.

"""@en .

<http://dbkwik.webdatacommons.org/marvelcinematicuniverse.wikia.com/resource/André_Sogliuzzo> rdfs:label "André Sogliuzzo"^^rdf:langString ;
    rdfs:comment """André Sogliuzzo voiced Arnim Zola in Captain America: Super Soldier.

"""@en .

<http://dbkwik.webdatacommons.org/marvelcinematicuniverse.wikia.com/resource/Anna_Boden> rdfs:label "Anna Boden"^^rdf:langString ;
    rdfs:comment """Anna Boden will co-direct Captain Marvel with Ryan Fleck.

"""@en .

<http://dbkwik.webdatacommons.org/marvelcinematicuniverse.wikia.com/resource/Anon> rdfs:label "Anon"^^rdf:langString ;
    ns1:realName <http://dbkwik.webdatacommons.org/marvelcinematicuniverse.wikia.com/resource/Anon> ;
    rdfs:comment """Anon is a Transhumanists follower and a former assistant of Doctor Holden Radcliffe.

"""@en .

<http://dbkwik.webdatacommons.org/marvelcinematicuniverse.wikia.com/resource/Ant-Man> rdfs:label "Ant-Man"^^rdf:langString ;
    rdfs:comment """Scott Edward Harris Lang is a former criminal who was convinced by Pym Technologies CEO Hank Pym to take up his mantle as the new Ant-Man. As Ant-Man, Lang fought against Darren Cross, Pym's protégé who became obsessed with Pym Particles and intended to recreate and sell the technology to terrorist organizations such as HYDRA and the Ten Rings. After his daughter, Cassie Lang, was taken hostage by Cross, Lang was able to send both of them into the Quantum Realm, where he saw Pym's wife Janet van Dyne, before successfully returning. Cross was presumably killed. Lang then began a romantic relationship with Pym's daughter, Hope van Dyne.
"""@en .

<http://dbkwik.webdatacommons.org/marvelcinematicuniverse.wikia.com/resource/Anthony_Russo> rdfs:label "Anthony Russo"^^rdf:langString ;
    ns1:directed <http://dbkwik.webdatacommons.org/marvelcinematicuniverse.wikia.com/resource/Ant-Man_(film)>,
        <http://dbkwik.webdatacommons.org/marvelcinematicuniverse.wikia.com/resource/Avengers:_Infinity_War> ;
    ns1:documentary <http://dbkwik.webdatacommons.org/marvelcinematicuniverse.wikia.com/resource/Marvel_Studios:_Assembling_a_Universe> ;
    rdfs:comment """Anthony Russo co-directed Captain America: The Winter Soldier, Captain America: Civil War, Avengers: Infinity War and Avengers 4 with his brother Joe.
He also directed the post-credits scene of Ant-Man with Joe.
He was interviewed for the documentary Marvel Studios: Assembling a Universe. 

"""@en .

<http://dbkwik.webdatacommons.org/marvelcinematicuniverse.wikia.com/resource/Ares> rdfs:label "Ares"^^rdf:langString ;
    rdfs:comment """Ares was a powerful fighter and was one of the warriors who gained the title of Champion of the Contest of Champions of Sakaar.

"""@en .

<http://dbkwik.webdatacommons.org/marvelcinematicuniverse.wikia.com/resource/Attack_on_Jotunheim> rdfs:label "Attack on Jotunheim"^^rdf:langString ;
    rdfs:comment """The Attack on Jotunheim was a failed attempt undertaken by Thor to attack Laufey after Frost Giants broke into Odin's Vault and tried to steal the Casket of Ancient Winters.

"""@en .

<http://dbkwik.webdatacommons.org/marvelcinematicuniverse.wikia.com/resource/Attack_on_the_IFID_Headquarters> rdfs:label "Attack on the IFID Headquarters"^^rdf:langString ;
    rdfs:comment """The Attack on the IFID Headquarters, also known as the Lagos Catastrophe, was an open confrontation between the Avengers and former HYDRA agent Brock Rumlow in Lagos, Nigeria. 

"""@en .

<http://dbkwik.webdatacommons.org/marvelcinematicuniverse.wikia.com/resource/Bagram> rdfs:label "Bagram"^^rdf:langString ;
    rdfs:comment """Bagram is a small town in Afghanistan and home of Bagram Air Base.

"""@en .

<http://dbkwik.webdatacommons.org/marvelcinematicuniverse.wikia.com/resource/Bakhmala> rdfs:label "Bakhmala"^^rdf:langString ;
    rdfs:comment """Bakhmala is a small city in Afghanistan.

"""@en .

<http://dbkwik.webdatacommons.org/marvelcinematicuniverse.wikia.com/resource/Barbershop_Headquarters> rdfs:label "Barbershop Headquarters"^^rdf:langString ;
    rdfs:comment """The Barbershop Headquarters was a secret S.H.I.E.L.D. facility located in Havana, Cuba, concealed under a barbershop named the "Habana Vieja Barbería".
HYDRA took over the facility during the HYDRA Uprising and used it as the main headquarters for the Centipede Project.

"""@en .

<http://dbkwik.webdatacommons.org/marvelcinematicuniverse.wikia.com/resource/Barrow> rdfs:label "Barrow"^^rdf:langString ;
    rdfs:comment """Barrow is a city in the state of Alaska.

"""@en .

<http://dbkwik.webdatacommons.org/marvelcinematicuniverse.wikia.com/resource/Basha> rdfs:label "Basha"^^rdf:langString ;
    rdfs:comment """Basha is an alien noblewoman that purchased Inhuman fighters from Kasius.

"""@en .

<http://dbkwik.webdatacommons.org/marvelcinematicuniverse.wikia.com/resource/Battle_of_Rose_Hill> rdfs:label "Battle of Rose Hill"^^rdf:langString ;
    rdfs:comment """The Battle of Rose Hill was a failed assassination plot by Eric Savin and Ellen Brandt to kill Tony Stark.

"""@en .

<http://dbkwik.webdatacommons.org/marvelcinematicuniverse.wikia.com/resource/Battle_on_the_Norco> rdfs:label "Battle on the Norco"^^rdf:langString ;
    rdfs:comment """The Battle on the Norco took place on the impounded tanker Roxxon Norco, where Extremis scientist and visionary Aldrich Killian made his base of operations, and had held Matthew Ellis, President of the United States of America hostage following an attack on Air Force One. Previously, he instigated a terrorist campaign across the United States, using the Mandarin and the involvement of the Ten Rings as a front.
"""@en .

<http://dbkwik.webdatacommons.org/marvelcinematicuniverse.wikia.com/resource/Benin> rdfs:label "Benin"^^rdf:langString ;
    rdfs:comment """Benin, officially known as Republic of Benin and formerly known as Dahomey, is a country located in western Africa.

"""@en .

<http://dbkwik.webdatacommons.org/marvelcinematicuniverse.wikia.com/resource/Beta_Ray_Bill> rdfs:label "Beta Ray Bill"^^rdf:langString ;
    rdfs:comment """Beta Ray Bill was a powerful fighter and was one of the warriors who gained the title of Champion of the Contest of Champions of Sakaar.

"""@en .

<http://dbkwik.webdatacommons.org/marvelcinematicuniverse.wikia.com/resource/Betty_Ross> rdfs:label "Betty Ross"^^rdf:langString ;
    rdfs:comment """Doctor Elizabeth "Betty" Ross was a scientist and professor at Culver University. She dated Bruce Banner and helped him after a horrible accident involving Gamma Radiation turned him into the Hulk.
When Thanos completed the Infinity Gauntlet and his goal of killing half the universe came into effect, Ross was among those who were killed.

"""@en .

<http://dbkwik.webdatacommons.org/marvelcinematicuniverse.wikia.com/resource/Billy_Gierhart> rdfs:label "Billy Gierhart"^^rdf:langString ;
    rdfs:comment """Billy Gierhart directed the Agents of S.H.I.E.L.D. episodes Repairs, Nothing Personal, Ye Who Enter Here, Aftershocks, S.O.S. Part Two, Absolution, The Ghost, The Good Samaritan, BOOM, All the Madame's Men and World's End, the Jessica Jones episode AKA Take a Bloody Number and the Inhumans episode ...And Finally: Black Bolt.
He also directed the unaired pilot of Most Wanted.

"""@en .

<http://dbkwik.webdatacommons.org/marvelcinematicuniverse.wikia.com/resource/Black_Mariah> rdfs:label "Black Mariah"^^rdf:langString ;
    ns1:realName <http://dbkwik.webdatacommons.org/marvelcinematicuniverse.wikia.com/resource/Black_Mariah> ;
    rdfs:comment """Mariah Dillard (née Stokes), was a powerful woman working in Harlem politics looking to bring a new era of change to the streets she grew up on. Her personal life and professional career are thrown into turmoil by both Luke Cage as well as her cousin Cottonmouth's nefarious acts. As her political career was falling apart, Dillard reached her breaking point and murdered her cousin, forcing her to work with Shades to protect herself as she slowly became indoctrinated into the crime world, working with Diamondback while Misty Knight attempted to bring her to justice. Dillard was spared jail by ordering the murder of the only witness Candace Miller and accepted her new role of crime lord of Harlem.
"""@en .

<http://dbkwik.webdatacommons.org/marvelcinematicuniverse.wikia.com/resource/Black_Panther_(film)> rdfs:label "Black Panther (film)"^^rdf:langString ;
    ns1:boxoffice "1.347E9"^^<http://dbkwik.webdatacommons.org/datatype/usDollar> ;
    rdfs:comment """Black Panther is a 2018 superhero film, based on the Marvel Comics superhero of the same name. It is a sequel to Avengers: Age of Ultron and Captain America: Civil War, and is the eighteenth installment in the Marvel Cinematic Universe as well as the sixth installment of Phase Three. The film was released on February 15, 2018 internationally and on February 16, 2018 in the United States.
"""@en .

<http://dbkwik.webdatacommons.org/marvelcinematicuniverse.wikia.com/resource/Black_Widow> rdfs:label "Black Widow"^^rdf:langString ;
    ns1:namesake <http://dbkwik.webdatacommons.org/marvelcinematicuniverse.wikia.com/resource/Nathaniel_Barton> ;
    rdfs:comment """Natalia Alianovna "Natasha" Romanoff, better known as Black Widow, is one of the most talented spies and assassins in the entire world and a founding member of the Avengers. Originally an agent of the Soviet agency for foreign intelligence, the KGB, she later became a member of S.H.I.E.L.D., the international counter-intelligence agency. Having extensive mastery in martial arts and armed with her Widow's Bite, Black Widow became one of S.H.I.E.L.D.'s most efficient agents. During one mission, she was sent undercover into Stark Industries to watch Tony Stark due to fears that he was dying. During this mission, Romanoff had assisted Stark with defeating Ivan Vanko's terrorist plots against him.
"""@en .

<http://dbkwik.webdatacommons.org/marvelcinematicuniverse.wikia.com/resource/Black_Widow_(film)> rdfs:label "Black Widow (film)"^^rdf:langString ;
    rdfs:comment """Black Widow is an upcoming superhero film, based on the Marvel Comics superheroine of the same name.

"""@en .

<http://dbkwik.webdatacommons.org/marvelcinematicuniverse.wikia.com/resource/Blizzard> rdfs:label "Blizzard"^^rdf:langString ;
    rdfs:comment """Donald "Donnie" Gill was a former student at the S.H.I.E.L.D. Academy of Science and Technology who was brainwashed into working for HYDRA during the HYDRA Uprising after gaining the power of instantly freezing any item around him. After the Battle at the Sandbox, Gill broke free of his brainwashing and went into hiding in Morocco. Sunil Bakshi tracked him down and attempted to bring him back to HYDRA, managing once again to trigger his brainwashing despite Gill's rebellion on the organization. On a clash against S.H.I.E.L.D. on the Maribel del Mar, Gill was shot by Skye and was left to sink down to the bottom of the ocean.

"""@en .

<http://dbkwik.webdatacommons.org/marvelcinematicuniverse.wikia.com/resource/Bobby> rdfs:label "Bobby"^^rdf:langString ;
    rdfs:comment """Bobby is a patron who attempted to flirt with Trish Walker and was challenged by Jessica Jones in a local bar.

"""@en .

<http://dbkwik.webdatacommons.org/marvelcinematicuniverse.wikia.com/resource/Bor> rdfs:label "Bor"^^rdf:langString ;
    ns1:after <http://dbkwik.webdatacommons.org/marvelcinematicuniverse.wikia.com/resource/Odin> ;
    rdfs:comment """Bor Burison was the King of Asgard, son of Buri, father of Odin, and grandfather of Hela and Thor. He was responsible for the defeat of Malekith's and the Dark Elves' army during the First Battle of Svartalfheim.
He was succeeded to the Asgardian Throne by his son Odin following his death in a war.

"""@en .

<http://dbkwik.webdatacommons.org/marvelcinematicuniverse.wikia.com/resource/Brad_Winderbaum> rdfs:label "Brad Winderbaum"^^rdf:langString ;
    rdfs:comment """Brad Winderbaum is the Vice President of Production & Development at Marvel Studios.
He was a China unit producer on Iron Man 3, a co-producer on Ant-Man and an executive producer on Thor: Ragnarok.
He also served as executive producer in Marvel One-Shot: The Consultant, Marvel One-Shot: A Funny Thing Happened on the Way to Thor's Hammer, Marvel One-Shot: Item 47, Marvel One-Shot: Agent Carter, Marvel One-Shot: All Hail the King, Team Thor, Team Thor: Part 2 and Team Darryl.
"""@en .

<http://dbkwik.webdatacommons.org/marvelcinematicuniverse.wikia.com/resource/Brookton> rdfs:label "Brookton"^^rdf:langString ;
    rdfs:comment """Staff Sergeant Brookton was a non-commissioned officer of the United States Air Force.

"""@en .

<http://dbkwik.webdatacommons.org/marvelcinematicuniverse.wikia.com/resource/Bushmaster> rdfs:label "Bushmaster"^^rdf:langString ;
    rdfs:comment """John McIver, also known as Bushmaster, is the charismatic enhanced individual who had previously witnessed his family being murdered by Mama Mabel as he vowed revenge on the Stokes family. With a mission of vengeance, Bushmaster soon arrived in Harlem to kill Mariah Stokes, the last member of the Stokes family, only to be challenged by Luke Cage who stood in the way of Bushmaster's revenge mission. 
"""@en .

<http://dbkwik.webdatacommons.org/marvelcinematicuniverse.wikia.com/resource/California> rdfs:label "California"^^rdf:langString ;
    rdfs:comment """California is a state located on the West Coast of the United States of America.

"""@en .

<http://dbkwik.webdatacommons.org/marvelcinematicuniverse.wikia.com/resource/Callisto_Aerospace_Rover> rdfs:label "Callisto Aerospace Rover"^^rdf:langString ;
    rdfs:comment """The Callisto Aerospace Rover was a Moon rover sent by the American company Callisto Aerospace to explore the surface of the satellite.

"""@en .

<http://dbkwik.webdatacommons.org/marvelcinematicuniverse.wikia.com/resource/Cameron_Klein> rdfs:label "Cameron Klein"^^rdf:langString ;
    rdfs:comment """Cameron Klein is a former S.H.I.E.L.D. technician who stayed loyal to Captain America during the Battle at the Triskelion and stood against Brock Rumlow in the face of death. He was later recruited by Nick Fury to assist in the Battle of Sokovia.

"""@en .

<http://dbkwik.webdatacommons.org/marvelcinematicuniverse.wikia.com/resource/Captain_America> rdfs:label "Captain America"^^rdf:langString ;
    rdfs:comment """Steven Grant "Steve" Rogers is a World War II veteran, and is known as the world's first superhero. Born within Brooklyn, New York City, the young Rogers had suffered from numerous health problems, and upon America's entry into World War II, was rejected from military service despite several attempts to enlist. Determined to serve, he ultimately volunteered for the top-secret Super Soldier program, and the frail Rogers was then enhanced to the peak of human perfection. Rogers soon joined the war effort as the mascot, given the new moniker of Captain America, and later joined the war with a combat role after he single-handedly liberated captured Allied POWs. 
"""@en .

<http://dbkwik.webdatacommons.org/marvelcinematicuniverse.wikia.com/resource/Captain_America:_Civil_War_Prelude> rdfs:label "Captain America: Civil War Prelude"^^rdf:langString ;
    ns1:editorinchief <http://dbkwik.webdatacommons.org/marvelcinematicuniverse.wikia.com/resource/Axel_Alonso> ;
    rdfs:comment """Captain America: Civil War Prelude is a 4-issue comic mini-series set in the Marvel Cinematic Universe. It is set before the events of Captain America: Civil War.

"""@en .

<http://dbkwik.webdatacommons.org/marvelcinematicuniverse.wikia.com/resource/Captain_America:_Homecoming> rdfs:label "Captain America: Homecoming"^^rdf:langString ;
    rdfs:comment """Captain America: Homecoming is a comic set between the events of The Avengers and Captain America: The Winter Soldier written by Fred Van Lente.

"""@en .

<http://dbkwik.webdatacommons.org/marvelcinematicuniverse.wikia.com/resource/Carla_Talbot> rdfs:label "Carla Talbot"^^rdf:langString ;
    rdfs:comment """Carla Talbot is the wife of Brigadier General Glenn Talbot.

"""@en .

<http://dbkwik.webdatacommons.org/marvelcinematicuniverse.wikia.com/resource/Cate_Shortland> rdfs:label "Cate Shortland"^^rdf:langString ;
    rdfs:comment """Cate Shortland will direct Black Widow.

"""@en .

<http://dbkwik.webdatacommons.org/marvelcinematicuniverse.wikia.com/resource/Category:A.I.M.> a skos:Concept ;
    rdfs:label "A.I.M."^^rdf:langString ;
    skos:broader <http://dbkwik.webdatacommons.org/marvelcinematicuniverse.wikia.com/resource/Category:Organizations> ;
    skos:prefLabel "A.I.M."^^rdf:langString .

<http://dbkwik.webdatacommons.org/marvelcinematicuniverse.wikia.com/resource/Category:Characters_by_Affiliation> rdfs:label "Characters by Affiliation"^^rdf:langString .

<http://dbkwik.webdatacommons.org/marvelcinematicuniverse.wikia.com/resource/Category:Daredevil_(TV_series)> rdfs:label "Daredevil (TV series)"^^rdf:langString .

<http://dbkwik.webdatacommons.org/marvelcinematicuniverse.wikia.com/resource/Category:Daredevil_(TV_series)_Episodes> rdfs:label "Daredevil (TV series) Episodes"^^rdf:langString .

<http://dbkwik.webdatacommons.org/marvelcinematicuniverse.wikia.com/resource/Category:Inhumans_(TV_series)_Episodes> rdfs:label "Inhumans (TV series) Episodes"^^rdf:langString .

<http://dbkwik.webdatacommons.org/marvelcinematicuniverse.wikia.com/resource/Category:Iron_Man_Armors> rdfs:label "Iron Man Armors"^^rdf:langString .

<http://dbkwik.webdatacommons.org/marvelcinematicuniverse.wikia.com/resource/Category:Items> rdfs:label "Items"^^rdf:langString .

<http://dbkwik.webdatacommons.org/marvelcinematicuniverse.wikia.com/resource/Category:Organizations> rdfs:label "Organizations"^^rdf:langString .

<http://dbkwik.webdatacommons.org/marvelcinematicuniverse.wikia.com/resource/Category:Policy> rdfs:label "Policy"^^rdf:langString ;
    skos:related <http://dbkwik.webdatacommons.org/marvelcinematicuniverse.wikia.com/resource/Category:Help> .

<http://dbkwik.webdatacommons.org/marvelcinematicuniverse.wikia.com/resource/Category:S.H.I.E.L.D.> rdfs:label "S.H.I.E.L.D."^^rdf:langString .

<http://dbkwik.webdatacommons.org/marvelcinematicuniverse.wikia.com/resource/Category:Sorcerer_Supreme> rdfs:label "Sorcerer Supreme"^^rdf:langString .

<http://dbkwik.webdatacommons.org/marvelcinematicuniverse.wikia.com/resource/Chad_Davis> rdfs:label "Chad Davis"^^rdf:langString ;
    rdfs:comment """Sergeant Chad Davis was a former non-commissioned officer of the United States Army injected with Extremis, which eventually killed him.

"""@en .

<http://dbkwik.webdatacommons.org/marvelcinematicuniverse.wikia.com/resource/Charles_Healey> rdfs:label "Charles Healey"^^rdf:langString ;
    rdfs:comment """Charles Healey is the CEO of AccuTech.

"""@en .

<http://dbkwik.webdatacommons.org/marvelcinematicuniverse.wikia.com/resource/Charles_Hinton> rdfs:label "Charles Hinton"^^rdf:langString ;
    rdfs:comment """Charles Hinton was an Inhuman who was able to give people a glimpse of the death of a single individual upon physical contact; this terrible power forced him to abandon his wife and daughter and live as a homeless man. He was kidnapped by HYDRA so that his gifts could be used by Hive; however, when S.H.I.E.L.D. came to rescue him from his own captors, Hinton fought against Gideon Malick and sacrificed his life to protect Daisy Johnson.

"""@en .

<http://dbkwik.webdatacommons.org/marvelcinematicuniverse.wikia.com/resource/Charles_Newirth> rdfs:label "Charles Newirth"^^rdf:langString ;
    rdfs:comment """Charles Newirth was an executive producer on Iron Man 3, Doctor Strange and Ant-Man and the Wasp.

"""@en .

<http://dbkwik.webdatacommons.org/marvelcinematicuniverse.wikia.com/resource/Chase_of_Quake> rdfs:label "Chase of Quake"^^rdf:langString ;
    ns1:begin <http://dbkwik.webdatacommons.org/marvelcinematicuniverse.wikia.com/resource/2016> ;
    ns1:end <http://dbkwik.webdatacommons.org/marvelcinematicuniverse.wikia.com/resource/2017> ;
    rdfs:comment """The Chase of Quake was an organized search issued by the newly legitimized peacekeeping organization S.H.I.E.L.D. for former Inhuman agent Daisy Johnson. 

"""@en .

<http://dbkwik.webdatacommons.org/marvelcinematicuniverse.wikia.com/resource/Chester_Phillips> rdfs:label "Chester Phillips"^^rdf:langString ;
    rdfs:comment """Colonel Chester Phillips was an officer of the United States Army, the first and only director of the Strategic Scientific Reserve, Steve Rogers' commanding officer, and one of the founding members of S.H.I.E.L.D. During World War II, Philips was a key factor in the creation of the world's first Super Soldier and the defeat of HYDRA.

"""@en .

<http://dbkwik.webdatacommons.org/marvelcinematicuniverse.wikia.com/resource/Chicago> rdfs:label "Chicago"^^rdf:langString ;
    rdfs:comment """Chicago is the largest city of the state of Illinois.

"""@en .

<http://dbkwik.webdatacommons.org/marvelcinematicuniverse.wikia.com/resource/Chitauri_Invasion> rdfs:label "Chitauri Invasion"^^rdf:langString ;
    rdfs:comment """The Chitauri Invasion was one of the first wars between humanity and beings from other worlds. The war lasted for less than a week, but the impact it left was great. Taking place on Earth, the war was fought by the exiled Asgardian prince Loki and his Chitauri allies against the applicants of the Avengers Initiative and the espionage agency known as S.H.I.E.L.D. At first the members of the team refused to cooperate with each other, but after Phil Coulson's demise at the hands of Loki, they were able to work together and defeated the Chitauri at the Battle of New York.

"""@en .

<http://dbkwik.webdatacommons.org/marvelcinematicuniverse.wikia.com/resource/Chloé_Zhao> rdfs:label "Chloé Zhao"^^rdf:langString ;
    rdfs:comment """Chloé Zhao will direct The Eternals.

"""@en .

<http://dbkwik.webdatacommons.org/marvelcinematicuniverse.wikia.com/resource/Chris_Dingess> rdfs:label "Chris Dingess"^^rdf:langString ;
    rdfs:comment """Chris Dingess is an executive producer on Agent Carter.
He wrote the Agent Carter episode Snafu, the teleplay for A Little Song and Dance, and the story for Hollywood Ending. He also co-wrote the episode Absolution of Agents of S.H.I.E.L.D. with Drew Z. Greenberg.

"""@en .

<http://dbkwik.webdatacommons.org/marvelcinematicuniverse.wikia.com/resource/Chris_Sotomayor> rdfs:label "Chris Sotomayor"^^rdf:langString ;
    rdfs:comment """Chris Sotomayor was an artist for Iron Man: Fast Friends, The Incredible Hulk: The Fury Files, Nick Fury: Spies Like Us, Iron Man: I Am Iron Man!, Iron Man 2: Fist of Iron, Iron Man 2: Security Breach, Iron Man Royal Purple Custom Comic, Iron Man 2 Adaptation, The Avengers Prelude: Fury's Big Week, The Avengers: The Avengers Initiative, The Avengers Prelude: Black Widow Strikes, Iron Man 3 Prelude, Iron Man: The Coming of the Melter, Thor: The Dark World Prelude, Captain America: The First Avenger Adaptation, Captain America: Homecoming and Agents of S.H.I.E.L.D.: The Chase.

"""@en .

<http://dbkwik.webdatacommons.org/marvelcinematicuniverse.wikia.com/resource/Christopher_Lennertz> rdfs:label "Christopher Lennertz"^^rdf:langString ;
    rdfs:comment """Christopher Joseph Lennertz scored Marvel One-Shot: Item 47, Marvel One-Shot: Agent Carter and Agent Carter.

"""@en .

<http://dbkwik.webdatacommons.org/marvelcinematicuniverse.wikia.com/resource/Ciara_Bravo> rdfs:label "Ciara Bravo"^^rdf:langString ;
    rdfs:comment """Ciara Quinn Bravo portrayed Abby in the Agents of S.H.I.E.L.D. episode A Life Spent.

"""@en .

<http://dbkwik.webdatacommons.org/marvelcinematicuniverse.wikia.com/resource/Clayton_Cowles> rdfs:label "Clayton Cowles"^^rdf:langString ;
    rdfs:comment """Clayton Cowles was an artist for Iron Man 2: Public Identity, Iron Man 2: Agents of S.H.I.E.L.D., Iron Man 2: Fist of Iron, Captain America: First Vengeance, Iron Man 2 Adaptation, The Avengers Prelude: Black Widow Strikes, Thor Adaptation, Captain America: The First Avenger Adaptation, Captain America: The Winter Soldier Infinite Comic, Guardians of the Galaxy Prelude, Guardians of the Galaxy: Galaxy's Most Wanted, The Avengers Adaptation, Avengers: Age of Ultron Prelude - This Scepter'd Isle, Ant-Man Prelude, Ant-Man - Scott Lang: Small Time, Avengers: Operation HYDRA and Ant-Man: Larger Than Life.

"""@en .

<http://dbkwik.webdatacommons.org/marvelcinematicuniverse.wikia.com/resource/D.C._Pierson> rdfs:label "D.C. Pierson"^^rdf:langString ;
    rdfs:comment """D.C. Pierson portrayed Aaron in Captain America: The Winter Soldier.

"""@en .

<http://dbkwik.webdatacommons.org/marvelcinematicuniverse.wikia.com/resource/DJ_AM> rdfs:label "DJ AM"^^rdf:langString ;
    rdfs:comment """Adam Michael Goldstein was an American DJ, remixer, record producer and musician better known as DJ AM. He made a cameo appearance as himself in Iron Man 2.

"""@en .

<http://dbkwik.webdatacommons.org/marvelcinematicuniverse.wikia.com/resource/Dan_Buckley> rdfs:label "Dan Buckley"^^rdf:langString ;
    rdfs:comment """Dan Buckley is the President of Marvel Entertainment. He published Agents of S.H.I.E.L.D.: Season One Declassified.
He is an executive producer for Daredevil, Jessica Jones, Luke Cage and The Defenders.
He was also interviewed for the documentaries Marvel Studios: Assembling a Universe, Marvel 75 Years: From Pulp to Pop and Captain America: 75 Heroic Years.

"""@en .

<http://dbkwik.webdatacommons.org/marvelcinematicuniverse.wikia.com/resource/Daredevil_(TV_series)> a <http://dbkwik.webdatacommons.org/marvelcinematicuniverse.wikia.com/class/tv> ;
    rdfs:label "Daredevil (TV series)"^^rdf:langString ;
    ns1:first <http://dbkwik.webdatacommons.org/marvelcinematicuniverse.wikia.com/resource/Into_the_Ring> ;
    rdfs:comment """Marvel's Daredevil, or simply Daredevil, is an American web television series that stars the superhero character of the same name. It is produced by Marvel Television and airs on Netflix.
On November 7, 2013, Marvel announced the 13-episode series as a joint project with Netflix. On December 6, 2013, Marvel announced that Drew Goddard would join the series as Showrunner and Executive Producer and write the first episode Into the Ring. On May 24, 2014, Drew Goddard left the project handing his position to Steven S. DeKnight. The whole first season premiered on April 10, 2015.
"""@en .

<http://dbkwik.webdatacommons.org/marvelcinematicuniverse.wikia.com/resource/Dark_Elves> rdfs:label "Dark Elves"^^rdf:langString ;
    rdfs:comment """The Dark Elves (known as Svartálfar by the Ancient Norse, Älfeneel or Harudheeniksel by the Dark Elves themselves) are the oldest known species in existence, hailing from the obscure realm of Svartalfheim. They are mortal enemies of the Asgardians. Some members of their race have been shown to have the fortitude to wield the power of an Infinity Stone. They are now presumed to be critically endangered as a species or even extinct.

"""@en .

<http://dbkwik.webdatacommons.org/marvelcinematicuniverse.wikia.com/resource/Dave_Jordan> rdfs:label "Dave Jordan"^^rdf:langString ;
    rdfs:comment """Dave Jordan is a music supervisor for all films set in the Marvel Cinematic Universe.

"""@en .

<http://dbkwik.webdatacommons.org/marvelcinematicuniverse.wikia.com/resource/David_Straiton> rdfs:label "David Straiton"^^rdf:langString ;
    rdfs:comment """David Straiton directed the Agents of S.H.I.E.L.D. episodes 0-8-4 and Beginning of the End and the Inhumans episode Make Way For... Medusa.

"""@en .

<http://dbkwik.webdatacommons.org/marvelcinematicuniverse.wikia.com/resource/Debbie> rdfs:label "Debbie"^^rdf:langString ;
    rdfs:comment """Debbie was a doctor that was testing the Centipede Device for the Centipede Project. She was killed by Scorch after he went rogue.

"""@en .

<http://dbkwik.webdatacommons.org/marvelcinematicuniverse.wikia.com/resource/Destroyer_Armor_Prototype_Gun> rdfs:label "Destroyer Armor Prototype Gun"^^rdf:langString ;
    rdfs:comment """The Destroyer Armor Prototype Gun, codenamed as "Bambino", is a weapon made out of the Destroyer's body and designed by a group of S.H.I.E.L.D. scientists. It is the final weapon used by Phil Coulson before his death, which inspired the Avengers to fight in the Battle of New York. It was taken into possession by Nick Fury who gave it back to Coulson during the HYDRA Uprising.

"""@en .

<http://dbkwik.webdatacommons.org/marvelcinematicuniverse.wikia.com/resource/Devils_You_Know> rdfs:label "Devils You Know"^^rdf:langString ;
    rdfs:comment """Devils You Know is the fourth episode of the third season of the television series Agents of S.H.I.E.L.D. and the forty-eighth episode overall.

"""@en .

<http://dbkwik.webdatacommons.org/marvelcinematicuniverse.wikia.com/resource/Dinah_Madani> rdfs:label "Dinah Madani"^^rdf:langString ;
    rdfs:comment """Dinah Madani is a highly-trained, sophisticated Homeland Security agent who, upon returning from active duty in Kandahar is vexed by the Punisher during her own investigation into the death of her partner Ahmad Zubair. Upon gaining a leadership position after the sudden murder of Carson Wolf, Madani soon learned that Frank Castle was still alive and uncovered a conspiracy involving William Rawlins and Billy Russo linking to Zubair's death and, siding with Castle, assisted in the death of Rawlins and the capture of Russo, exposing Operation Cerberus and all their illegal actions to the world.

"""@en .

<http://dbkwik.webdatacommons.org/marvelcinematicuniverse.wikia.com/resource/Dottie_Underwood> rdfs:label "Dottie Underwood"^^rdf:langString ;
    rdfs:comment """The woman known as Dorothy "Dottie" Underwood is a Soviet assassin trained in the Red Room Academy. As an operative of a Soviet espionage agency Leviathan, she participated in Johann Fennhoff's revenge plot against the American industrialist Howard Stark. She subsequently adopted the persona of a small-town girl from Iowa and infiltrated the Griffith Hotel in New York City. While assisting Fennhoff, she came in conflict with Peggy Carter, an SSR agent. During Fennhoff's attempt to kill the entire population of New York City on V-E Day, she was wounded but eventually managed to escape her pursuers. After the failure of her mission, she chose to stay in the USA and became a mercenary. 
"""@en .

<http://dbkwik.webdatacommons.org/marvelcinematicuniverse.wikia.com/resource/Edison_Po> rdfs:label "Edison Po"^^rdf:langString ;
    rdfs:comment """Edison Po was a former Marine and member of the Centipede Project. He was the Group's contact with the mysterious Clairvoyant. After the group succeeded in capturing S.H.I.E.L.D. agent Phil Coulson, he was killed by the Clairvoyant who believed his usefulness had ended.

"""@en .

<http://dbkwik.webdatacommons.org/marvelcinematicuniverse.wikia.com/resource/Ego%27s_Expansion> rdfs:label "Ego's Expansion"^^rdf:langString ;
    ns1:begin <http://dbkwik.webdatacommons.org/marvelcinematicuniverse.wikia.com/resource/Before_20th_Century> ;
    ns1:end <http://dbkwik.webdatacommons.org/marvelcinematicuniverse.wikia.com/resource/2014> ;
    rdfs:comment """Ego's Expansion was an attempt by the Celestial Ego to assimilate and conquer the universe.

"""@en .

<http://dbkwik.webdatacommons.org/marvelcinematicuniverse.wikia.com/resource/Elektra> rdfs:label "Elektra"^^rdf:langString ;
    rdfs:comment """Elektra, also known as Elektra Natchios, is an assassin who was trained under Stick, the same member from the Chaste who later trained Matt Murdock. She fell in love with Murdock during a mission for Stick to bring Murdock into the organization. She returned to his life after years of absence, putting her beliefs and methods at conflict with his own. Later, she was revealed to potentially be the Black Sky, the one who is supposed to lead the organization of assassins known as the Hand. However, Elektra chose to help Murdock defeat the malevolent organization, and was killed in the final confrontation with Nobu Yoshioka. The Hand then retrieved Elektra's corpse from the grave and placed it in a stone chamber to be exposed to the Resurrection Elixir.
"""@en .

<http://dbkwik.webdatacommons.org/marvelcinematicuniverse.wikia.com/resource/Ellen_Brandt> rdfs:label "Ellen Brandt"^^rdf:langString ;
    rdfs:comment """Ellen Brandt was an agent of A.I.M. and an enemy of Iron Man who had been injected with the Extremis virus, making her a highly dangerous warrior. She was killed by Stark while attempting to capture him.

"""@en .

<http://dbkwik.webdatacommons.org/marvelcinematicuniverse.wikia.com/resource/Endotex_Labs> rdfs:label "Endotex Labs"^^rdf:langString ;
    rdfs:comment """Endotex Labs is a front company for the Advanced Threat Containment Unit.

"""@en .

<http://dbkwik.webdatacommons.org/marvelcinematicuniverse.wikia.com/resource/Erik_Killmonger%27s_Campaign> rdfs:label "Erik Killmonger's Campaign"^^rdf:langString ;
    ns1:end <http://dbkwik.webdatacommons.org/marvelcinematicuniverse.wikia.com/resource/2016> ;
    rdfs:comment """Erik Killmonger's Campaign was a series of battles between Erik Killmonger's faction, whose goals were to overthrow the governments of the world and replace them with a Wakandan Empire, and those still loyal to T'Challa, who wanted to avoid war with the rest of the world.

"""@en .

<http://dbkwik.webdatacommons.org/marvelcinematicuniverse.wikia.com/resource/Europe> rdfs:label "Europe"^^rdf:langString ;
    rdfs:comment """Europe is the second smallest continent out of seven. It is known for its varied nature.

"""@en .

<http://dbkwik.webdatacommons.org/marvelcinematicuniverse.wikia.com/resource/Fandral> rdfs:label "Fandral"^^rdf:langString ;
    rdfs:comment """Fandral was a highly respected Asgardian warrior, an ally as well as friend of Thor, and a member of the Warriors Three, known for his charm. Alongside all his fellow warriors, Fandral took part in a poorly considered strike against all the Frost Giants of Jotunheim, which soon resulted in King Odin deciding to directly punish Thor by banishing him to the Earth without his powers. When Loki then took the throne of Asgard during Thor's banishment, Fandral and his allies played a key role saving Thor from the Destroyer before bringing him back to Asgard where he successfully stopped Loki from stealing the throne of Asgard and restoring the peace.
"""@en .

<http://dbkwik.webdatacommons.org/marvelcinematicuniverse.wikia.com/resource/Felix_Ruiz> rdfs:label "Felix Ruiz"^^rdf:langString ;
    rdfs:comment """Felix Ruiz was an artist for Iron Man 2: Agents of S.H.I.E.L.D..

"""@en .

<http://dbkwik.webdatacommons.org/marvelcinematicuniverse.wikia.com/resource/First_Light> rdfs:label "First Light"^^rdf:langString ;
    rdfs:comment """First Light is the first episode of the first season of the television series Cloak & Dagger.

"""@en .

<http://dbkwik.webdatacommons.org/marvelcinematicuniverse.wikia.com/resource/Frank_D%27Armata> rdfs:label "Frank D'Armata"^^rdf:langString ;
    rdfs:comment """Frank D'Armata was an artist for Iron Man 2: Agents of S.H.I.E.L.D. and Agents of S.H.I.E.L.D.: The Chase.

"""@en .

<http://dbkwik.webdatacommons.org/marvelcinematicuniverse.wikia.com/resource/Front_Toward_Enemy> rdfs:label "Front Toward Enemy"^^rdf:langString ;
    rdfs:comment """Front Toward Enemy is the ninth episode of the first season of the television series The Punisher.

"""@en .

<http://dbkwik.webdatacommons.org/marvelcinematicuniverse.wikia.com/resource/Gabe_White> rdfs:label "Gabe White"^^rdf:langString ;
    rdfs:comment """Gabe White portrayed Aaron James in The Defenders episode The H Word.

"""@en .

<http://dbkwik.webdatacommons.org/marvelcinematicuniverse.wikia.com/resource/George_Kitson> rdfs:label "George Kitson"^^rdf:langString ;
    rdfs:comment """George Kitson wrote the comic Agents of S.H.I.E.L.D.: The Chase and co-wrote the Agents of S.H.I.E.L.D. episode Paradise Lost and the web series Agents of S.H.I.E.L.D.: Double Agent with Sharla Oliver. He also wrote the Agents of S.H.I.E.L.D. episodes Best Laid Plans and All Roads Lead... and the Agents of S.H.I.E.L.D.: Slingshot episode Progress.
He also works on Agents of S.H.I.E.L.D. as a personal assistant to Jeffrey Bell.

"""@en .

<http://dbkwik.webdatacommons.org/marvelcinematicuniverse.wikia.com/resource/George_Talbot> rdfs:label "George Talbot"^^rdf:langString ;
    rdfs:comment """George Talbot is the son of Glenn and Carla Talbot.

"""@en .

<http://dbkwik.webdatacommons.org/marvelcinematicuniverse.wikia.com/resource/Gilbert_O%27Conner> rdfs:label "Gilbert O'Conner"^^rdf:langString ;
    rdfs:comment """Gilbert O'Conner was the founder of AccuTech.

"""@en .

<http://dbkwik.webdatacommons.org/marvelcinematicuniverse.wikia.com/resource/Gilmore_Hodge> rdfs:label "Gilmore Hodge"^^rdf:langString ;
    rdfs:comment """Private Gilmore Hodge was a member of the United States Army during World War II, assigned to the Strategic Scientific Reserve.

"""@en .

<http://dbkwik.webdatacommons.org/marvelcinematicuniverse.wikia.com/resource/Glenn_Industries> rdfs:label "Glenn Industries"^^rdf:langString ;
    rdfs:comment """Glenn Industries is an industrial corporation operating in New York City.

"""@en .

<http://dbkwik.webdatacommons.org/marvelcinematicuniverse.wikia.com/resource/Glenn_Talbot> rdfs:label "Glenn Talbot"^^rdf:langString ;
    rdfs:comment "Brigadier General Glenn Talbot was a high-ranking officer of the United States Air Force. Following all the terrorist attacks connected to the HYDRA Uprising, Talbot was then personally tasked with capturing the remaining S.H.I.E.L.D. facilities, for which he was promoted. Despite their long standing feud and constant attempts to better each other, Talbot soon grew to respect S.H.I.E.L.D. new Director, Phil Coulson, accepting his help in the War on HYDRA. All his experiences in dealing with S.H.I.E.L.D. had soon led to President Matthew Ellis putting Talbot in charge of the ATCU, which was re-purposed to serve as the public face of S.H.I.E.L.D. after Rosalind Price's death, as Talbot used his possession to assist S.H.I.E.L.D."@en .

<http://dbkwik.webdatacommons.org/marvelcinematicuniverse.wikia.com/resource/Grant_Ward> rdfs:label "Grant Ward"^^rdf:langString ;
    rdfs:comment """Grant Douglas Ward was one of the leaders of HYDRA and the most personal adversary of Phil Coulson and S.H.I.E.L.D.. A former HYDRA infiltrator in S.H.I.E.L.D., disguised as a Level 7 operative, he was abused as a child by his family. As a teenager, he tried to burn down his family home. Ward was imprisoned until he was freed by John Garrett, who trained Ward to become a cold-blooded killer. Ward eventually became more loyal to him than to HYDRA. As an agent of S.H.I.E.L.D., he was recruited onto Coulson's Team, working with them on all their missions, pretending to be gruff and anti-social and to become emotionally attached to the team.
"""@en .

<http://dbkwik.webdatacommons.org/marvelcinematicuniverse.wikia.com/resource/Grant_Ward%27s_Campaign> rdfs:label "Grant Ward's Campaign"^^rdf:langString ;
    rdfs:comment """Grant Ward's Campaign was an attempt by former S.H.I.E.L.D. agent Grant Ward to rebuild the terrorist organization HYDRA following its severe defeat. 

"""@en .

<http://dbkwik.webdatacommons.org/marvelcinematicuniverse.wikia.com/resource/Guardians_Inferno> rdfs:label "Guardians Inferno"^^rdf:langString ;
    rdfs:comment """"Guardians Inferno" is a song composed by Tyler Bates and James Gunn and recorded by The Sneepers and David Hasselhoff for Guardians of the Galaxy Vol. 2. It was featured on the album Guardians of the Galaxy Vol. 2: Awesome Mix Vol. 2. The video of the song was directed by David Yarovesky.

"""@en .

<http://dbkwik.webdatacommons.org/marvelcinematicuniverse.wikia.com/resource/Guardians_of_the_Galaxy_(film)> rdfs:label "Guardians of the Galaxy (film)"^^rdf:langString ;
    rdfs:comment """Guardians of the Galaxy is a 2014 superhero film, based on the Marvel Comics superhero team of the same name. It is in the tenth installment in the Marvel Cinematic Universe and the fourth of Phase Two. The film was released on July 31, 2014 internationally and on August 1, 2014 in the United States.
"""@en .

<http://dbkwik.webdatacommons.org/marvelcinematicuniverse.wikia.com/resource/HYDRA_(Framework)> rdfs:label "HYDRA (Framework)"^^rdf:langString ;
    rdfs:comment """HYDRA was a virtual recreation of the real-world organization of the same name inside the Framework.

"""@en .

<http://dbkwik.webdatacommons.org/marvelcinematicuniverse.wikia.com/resource/HYDRA_Flamethrower> rdfs:label "HYDRA Flamethrower"^^rdf:langString ;
    rdfs:comment """The HYDRA Flamethrower is one of the advanced weapons developed and used by HYDRA during World War II, before harnessing the power of the Tesseract.

"""@en .

<http://dbkwik.webdatacommons.org/marvelcinematicuniverse.wikia.com/resource/HYDRA_Parasit> rdfs:label "HYDRA Parasit"^^rdf:langString ;
    rdfs:comment """The HYDRA Parasit was a flying Atomic Bomb produced by HYDRA during World War II.

"""@en .

<http://dbkwik.webdatacommons.org/marvelcinematicuniverse.wikia.com/resource/HYDRA_Uprising> rdfs:label "HYDRA Uprising"^^rdf:langString ;
    rdfs:comment """The HYDRA Uprising, also known as the HYDRA Infiltration and the Fall of S.H.I.E.L.D., was a major conflict that went back as early as the 1940s. After World War II, the security agency S.H.I.E.L.D. was founded, but was soon infiltrated by HYDRA, the rogue Nazi science group originally formed by the Red Skull prior to his disappearance.
"""@en .

<http://dbkwik.webdatacommons.org/marvelcinematicuniverse.wikia.com/resource/Hammer_Industries> rdfs:label "Hammer Industries"^^rdf:langString ;
    rdfs:comment """Hammer Industries is a weapons manufacturer company led by Justin Hammer.

"""@en .

<http://dbkwik.webdatacommons.org/marvelcinematicuniverse.wikia.com/resource/Havoc_in_the_Hidden_Land> rdfs:label "Havoc in the Hidden Land"^^rdf:langString ;
    rdfs:comment """Havoc in the Hidden Land is the seventh episode of the first season of the television series Inhumans.

"""@en .

<http://dbkwik.webdatacommons.org/marvelcinematicuniverse.wikia.com/resource/Heather> rdfs:label "Heather"^^rdf:langString ;
    rdfs:comment """Heather was among the crew on Air Force One when it got destroyed during the Kidnapping of President Ellis.

"""@en .

<http://dbkwik.webdatacommons.org/marvelcinematicuniverse.wikia.com/resource/Heather_Rand> rdfs:label "Heather Rand"^^rdf:langString ;
    rdfs:comment """Heather Rand was the wife of Wendell Rand and the mother of Danny Rand.

"""@en .

<http://dbkwik.webdatacommons.org/marvelcinematicuniverse.wikia.com/resource/Hela> rdfs:label "Hela"^^rdf:langString ;
    ns1:succeeded <http://dbkwik.webdatacommons.org/marvelcinematicuniverse.wikia.com/resource/Thor> ;
    ns1:years <http://dbkwik.webdatacommons.org/marvelcinematicuniverse.wikia.com/resource/Before_20th_Century> ;
    rdfs:comment "Hela Odinsdottir was the Asgardian Goddess of Death and the former Executioner of Asgard. Imprisoned in Hel for millennia by her father Odin, Hela was released from her prison following his death and went to restore her power over Asgard, while simultaneously engaging in a series of encounters with her younger brothers Thor and Loki. Gaining power from Asgard, Hela planned to rule Asgard and create an Asgardian Empire. When the people of Asgard refused to bow to her, Hela set about massacring Odin's armies and enslaving the people, while recruiting Skurge to be her own Executioner in the process."@en .

<http://dbkwik.webdatacommons.org/marvelcinematicuniverse.wikia.com/resource/Hirochi> rdfs:label "Hirochi"^^rdf:langString ;
    rdfs:comment """Hirochi was a representative of Asano Robotics, and secretly one of the high-ranking members of the Hand. He lead the Hand's front business operations within New York City, having to deal with both the Chaste's and Daredevil's interference, until he was killed by Stick as part of his escape from the Hand's custody.

"""@en .

<http://dbkwik.webdatacommons.org/marvelcinematicuniverse.wikia.com/resource/Hive> rdfs:label "Hive"^^rdf:langString ;
    rdfs:comment """Alveus, also known as Hive, was a parasitic Inhuman capable of infesting and possessing the bodies of dead humans and controlling other Inhumans through a hive mind. Because of his great powers, Alveus was banished to a barren planet. Alveus' worshipers founded a secret society with the sole purpose of bringing Hive back to Earth to conquer it. Over the centuries, that society evolved into HYDRA. Eventually, Alveus possessed Grant Ward's dead body when he was killed by Phil Coulson with his prosthetic hand on Maveth, and was able to return to Earth once more. Working with Gideon Malick, Alveus soon took the reins of HYDRA from him.
"""@en .

<http://dbkwik.webdatacommons.org/marvelcinematicuniverse.wikia.com/resource/Holden_Radcliffe> rdfs:label "Holden Radcliffe"^^rdf:langString ;
    rdfs:comment """Holden Radcliffe was a transhumanist whose theories got him fired from GT Agrochemical. He was kidnapped and recruited by Hive in order to recreate the Kree experiment which had created the Inhumans. Despite Radcliffe's enthusiasm, he struggled to perfect the experiment, inadvertently creating the Primitives. He was saved by S.H.I.E.L.D. and reached a new deal where he was cleared of all charges, but with the condition that all of his research was submitted for approval and oversight. However, Radcliffe had secretly begun working on Life-Model Decoys with Leo Fitz.
"""@en .

<http://dbkwik.webdatacommons.org/marvelcinematicuniverse.wikia.com/resource/Hollywood_Ending> rdfs:label "Hollywood Ending"^^rdf:langString ;
    rdfs:comment """Hollywood Ending is the tenth and final episode of the second season of the television series Agent Carter, and the last episode of the series overall.

"""@en .

<http://dbkwik.webdatacommons.org/marvelcinematicuniverse.wikia.com/resource/Hub_(S.H.I.E.L.D._Facility)> rdfs:label "Hub (S.H.I.E.L.D. Facility)"^^rdf:langString ;
    rdfs:comment """The Hub was one of the largest S.H.I.E.L.D. facilities. It served as a secondary headquarters for S.H.I.E.L.D. and one of its primary staging grounds and provider of back-end support for on-going operations. After the HYDRA Uprising, it was occupied by the United States Armed Forces.

"""@en .

<http://dbkwik.webdatacommons.org/marvelcinematicuniverse.wikia.com/resource/Hurctarians> rdfs:label "Hurctarians"^^rdf:langString ;
    rdfs:comment """The Hurctarians are a species of bipedal humanoids that inhabit the galaxy.

"""@en .

<http://dbkwik.webdatacommons.org/marvelcinematicuniverse.wikia.com/resource/I_Want_Your_Cray_Cray> rdfs:label "I Want Your Cray Cray"^^rdf:langString ;
    rdfs:comment """"I Want Your Cray Cray" is a song recorded by Rachael Taylor and Kandi Marks for the Jessica Jones episode AKA I Want Your Cray Cray. It was released on March 16, 2018.

"""@en .

<http://dbkwik.webdatacommons.org/marvelcinematicuniverse.wikia.com/resource/Ian_Hannin> rdfs:label "Ian Hannin"^^rdf:langString ;
    rdfs:comment """Ian Hannin was an artist for Iron Man 2: Agents of S.H.I.E.L.D..

"""@en .

<http://dbkwik.webdatacommons.org/marvelcinematicuniverse.wikia.com/resource/Illinois> rdfs:label "Illinois"^^rdf:langString ;
    rdfs:comment """Illinois is a state located on the widwestern region of the United States of America.

"""@en .

<http://dbkwik.webdatacommons.org/marvelcinematicuniverse.wikia.com/resource/Infiltrating_the_Set> rdfs:label "Infiltrating the Set"^^rdf:langString ;
    rdfs:comment """Infiltrating the Set is the first episode of the web series Agents of S.H.I.E.L.D.: Double Agent.

"""@en .

<http://dbkwik.webdatacommons.org/marvelcinematicuniverse.wikia.com/resource/Inhuman_Royal_Family> rdfs:label "Inhuman Royal Family"^^rdf:langString ;
    rdfs:comment """The Inhuman Royal Family is a group of Inhumans who, under the rule of Black Bolt, serve as the governing body of Attilan.

"""@en .

<http://dbkwik.webdatacommons.org/marvelcinematicuniverse.wikia.com/resource/Inhumans> rdfs:label "Inhumans"^^rdf:langString ;
    rdfs:comment """The Inhumans are a race of altered human beings that were the result of experiments on ancient humans by the extraterrestrial race, the Kree, embedding into their genetic code the potential to transform and acquire superhuman abilities through a process known as Terrigenesis.

"""@en .

<http://dbkwik.webdatacommons.org/marvelcinematicuniverse.wikia.com/resource/Into_the_Ring> rdfs:label "Into the Ring"^^rdf:langString ;
    rdfs:comment """Into the Ring is the first episode of the first season of the Netflix exclusive television series Daredevil.

"""@en .

<http://dbkwik.webdatacommons.org/marvelcinematicuniverse.wikia.com/resource/Ionizer_Missiles> rdfs:label "Ionizer Missiles"^^rdf:langString ;
    rdfs:comment """The Ionizer Missiles are missiles that one of the Confederacy leaders, Qovas, used on his ship.

"""@en .

<http://dbkwik.webdatacommons.org/marvelcinematicuniverse.wikia.com/resource/Iron_Man:_I_Am_Iron_Man!> rdfs:label "Iron Man: I Am Iron Man!"^^rdf:langString ;
    rdfs:comment """Iron Man: I Am Iron Man! is a two-part comic which retells the events of Iron Man. It also shows a few pannels that were omitted from the film.

"""@en .

<http://dbkwik.webdatacommons.org/marvelcinematicuniverse.wikia.com/resource/Iron_Man:_The_Price_of_Doing_Business> rdfs:label "Iron Man: The Price of Doing Business"^^rdf:langString ;
    rdfs:comment """Iron Man: The Price of Doing Business is a comic given away free with a pre-order of the first Iron Man video game from Sega.

"""@en .

<http://dbkwik.webdatacommons.org/marvelcinematicuniverse.wikia.com/resource/Iron_Man_(video_game)> rdfs:label "Iron Man (video game)"^^rdf:langString ;
    rdfs:comment """Iron Man is a 2008 video game based on the film of the same name. It was released on May 2, 2008 to coincide with the release of the film in cinemas. The game is published by Sega, and was released on PlayStation 3, Xbox 360 (developed by Secret Level), PlayStation 2, PlayStation Portable, Nintendo DS, Wii, Microsoft Windows (developed by Artificial Mind and Movement) and Mobile Platforms.
The enemies are Advanced Idea Mechanics, the Maggia and the Ten Rings terrorist group. The super-villains in the game include Blacklash, Madame Masque, Controller, Titanium Man, Melter, and Iron Monger.
"""@en .

<http://dbkwik.webdatacommons.org/marvelcinematicuniverse.wikia.com/resource/Iron_Man_3> rdfs:label "Iron Man 3"^^rdf:langString ;
    rdfs:comment """Iron Man 3 is a 2013 superhero film, based on the Marvel Comics superhero of the same name. It is a sequel to Iron Man, Iron Man 2, and The Avengers, and is the seventh installment in the Marvel Cinematic Universe and the first installment of Phase Two. The film was released internationally on April 24, 2013 and on May 3, 2013 in the United States.
"""@en .

<http://dbkwik.webdatacommons.org/marvelcinematicuniverse.wikia.com/resource/Iron_Man_Armor:_Mark_I> a <http://dbkwik.webdatacommons.org/marvelcinematicuniverse.wikia.com/class/armor> ;
    rdfs:label "Iron Man Armor: Mark I"^^rdf:langString ;
    ns1:name "Makeshift Armor"^^rdf:langString ;
    ns1:succeededBy <http://dbkwik.webdatacommons.org/marvelcinematicuniverse.wikia.com/resource/Iron_Man_Armor:_Mark_II> ;
    rdfs:comment """The Mark I Armor was Tony Stark's first Iron Man suit, built to help him escape from forced captivity by the Ten Rings. The suit was crafted from the limited resources around him, including salvaged pieces of scrap metal and machine parts.

"""@en .

<http://dbkwik.webdatacommons.org/marvelcinematicuniverse.wikia.com/resource/Iron_Man_Armor:_Mark_IV> rdfs:label "Iron Man Armor: Mark IV"^^rdf:langString ;
    ns1:precededBy <http://dbkwik.webdatacommons.org/marvelcinematicuniverse.wikia.com/resource/Iron_Man_Armor:_Mark_III> ;
    ns1:succeededBy <http://dbkwik.webdatacommons.org/marvelcinematicuniverse.wikia.com/resource/Iron_Man_Armor:_Mark_V> ;
    rdfs:comment """The Mark IV Armor was Tony Stark's fourth Iron Man suit and was built to replace the Mark III after it was heavily damaged in Stark's fight with Obadiah Stane. Because it was built to be a direct replacement, the Mark IV is very similar to the Mark III with only a few minor changes.

"""@en .

<http://dbkwik.webdatacommons.org/marvelcinematicuniverse.wikia.com/resource/Iron_Man_Armor:_Mark_V> rdfs:label "Iron Man Armor: Mark V"^^rdf:langString ;
    ns1:name "Portable Armor"^^rdf:langString ;
    rdfs:comment """The Mark V Armor was Tony Stark's fifth Iron Man suit and the first specialized suit to focus on portability and easy access. When not in use the suit can be collapsed and concealed in a form that resembles a standard briefcase. When activated the suit will open, allowing the user to take hold of it as it assembles around their body.

"""@en .

<http://dbkwik.webdatacommons.org/marvelcinematicuniverse.wikia.com/resource/Iron_Man_Armor:_Mark_VIII> rdfs:label "Iron Man Armor: Mark VIII"^^rdf:langString ;
    rdfs:comment """The Mark VIII Armor was Tony Stark's eighth Iron Man suit and the first suit created after the Battle of New York. The Mark VIII was the first in a series of Iron Man suits created during a period of rapid development that led to the creation of the Iron Legion. It was destroyed when the Clean Slate Protocol was activated by Tony Stark.

"""@en .

<http://dbkwik.webdatacommons.org/marvelcinematicuniverse.wikia.com/resource/Iron_Man_Armor:_Mark_X> rdfs:label "Iron Man Armor: Mark X"^^rdf:langString ;
    rdfs:comment """The Mark X Armor was Tony Stark's tenth Iron Man suit and the third suit created after the Battle of New York. The Mark X was one of the first in a series of Iron Man suits created during a period of rapid development that led to the creation of the Iron Legion. It was destroyed when the Clean Slate Protocol was activated by Tony Stark.

"""@en .

<http://dbkwik.webdatacommons.org/marvelcinematicuniverse.wikia.com/resource/Iron_Man_Armor:_Mark_XLIX> rdfs:label "Iron Man Armor: Mark XLIX"^^rdf:langString ;
    rdfs:comment """The Mark XLIX Armor, also known as the Hulkbuster 2.0, is Tony Stark's forty-ninth Iron Man suit. It was initially created for the purpose of restraining the Hulk, however, it was later repurposed by Bruce Banner to fight in the Battle of Wakanda against an army of Outriders, the Black Order and Thanos with the remaining Avengers on Earth.

"""@en .

<http://dbkwik.webdatacommons.org/marvelcinematicuniverse.wikia.com/resource/J.B._Blanc> rdfs:label "J.B. Blanc"^^rdf:langString ;
    rdfs:comment """Jean-Benoît "J. B." Blanc voiced Hulk and Abomination in The Incredible Hulk.

"""@en .

<http://dbkwik.webdatacommons.org/marvelcinematicuniverse.wikia.com/resource/Jesse_Bochco> rdfs:label "Jesse Bochco"^^rdf:langString ;
    rdfs:comment """Jesse Bochco directed the Agents of S.H.I.E.L.D. episodes Girl in the Flower Dress, Heavy is the Head, Love in the Time of HYDRA, 4,722 Hours, Watchdogs, Deals With Our Devils, Wake Up, Orientation Part One, Rewind and Rise and Shine.

"""@en .

<http://dbkwik.webdatacommons.org/marvelcinematicuniverse.wikia.com/resource/Jessica_Jones> rdfs:label "Jessica Jones"^^rdf:langString ;
    rdfs:comment """Jessica Campbell Jones is a private investigator from New York City. After becoming orphaned at a young age, Jones was taken in by Dorothy Walker, and developed a deep friendship bond with her adoptive sister, Trish. Shortly after being adopted, Jones discovered she possessed superhuman abilities due to the fatal car crash that took the lives of her parents and eventually decided to pursue a career as a superhero. However, a fateful encounter with Kilgrave, a vicious man with mind controlling powers, derailed her superhero career and she spent a torturous tenure as Kilgrave's sex slave before finally breaking free of his control. The experience left Jones suffering from post-traumatic stress disorder, prompting her to hang up her secret identity and open her own detective agency.
"""@en .

<http://dbkwik.webdatacommons.org/marvelcinematicuniverse.wikia.com/resource/Jessica_Jones_(Season_One)/Home_Video> rdfs:label "Jessica Jones (Season One)/Home Video"^^rdf:langString ;
    rdfs:comment """Jessica Jones - The Complete First Season is the Blu-ray release for Jessica Jones Season One.

"""@en .

<http://dbkwik.webdatacommons.org/marvelcinematicuniverse.wikia.com/resource/Joe_Pokaski> rdfs:label "Joe Pokaski"^^rdf:langString ;
    rdfs:comment """Joe Pokaski is a co-executive producer for Daredevil and showrunner for Cloak & Dagger.
He also wrote the Daredevil episodes In the Blood and Condemned. He also wrote the Cloak & Dagger episodes First Light, Suicide Sprints and Colony Collapse alone, Princeton Offense with Niceole R. Levy and Lotus Eaters with Peter Calloway.

"""@en .

<http://dbkwik.webdatacommons.org/marvelcinematicuniverse.wikia.com/resource/Joseph_Rogers> rdfs:label "Joseph Rogers"^^rdf:langString ;
    rdfs:comment """Joseph Rogers was the father of Steve Rogers, and a soldier with the 107th Infantry Regiment of the United States Army. He was killed during World War I.

"""@en .

<http://dbkwik.webdatacommons.org/marvelcinematicuniverse.wikia.com/resource/Karen_Page> rdfs:label "Karen Page"^^rdf:langString ;
    rdfs:comment """Karen Page is the former secretary for Nelson and Murdock and, along with Foggy Nelson, Matt Murdock and Ben Urich, was instrumental in the effort to bring Wilson Fisk to justice. While working for Nelson and Murdock, Page came into contact with Frank Castle, who she helped defend in court. When Nelson and Murdock fell apart, Page joined the New York Bulletin with the intention of writing Castle's true story, however during her investigation she was kidnapped by Ray Schoonover and saved by Castle. Later the Hand also kidnapped Page and she was rescued by Daredevil before Murdock revealed to her that he was Daredevil.

"""@en .

<http://dbkwik.webdatacommons.org/marvelcinematicuniverse.wikia.com/resource/Kidnapping_of_Thomas_Ward> rdfs:label "Kidnapping of Thomas Ward"^^rdf:langString ;
    rdfs:comment """The Kidnapping of Thomas Ward was the abduction of Thomas Ward by S.H.I.E.L.D. in retaliation for the role his brother Grant played in the death of Rosalind Price.

"""@en .

<http://dbkwik.webdatacommons.org/marvelcinematicuniverse.wikia.com/resource/Klaus_Haas> rdfs:label "Klaus Haas"^^rdf:langString ;
    rdfs:comment """Klaus Haas is the head of Research and Development at AccuTech.

"""@en .

<http://dbkwik.webdatacommons.org/marvelcinematicuniverse.wikia.com/resource/Lash> rdfs:label "Lash"^^rdf:langString ;
    rdfs:comment """Andrew Garner was a Neurologist and Forensic Psychologist who specialized in working with the gifted individuals from the Index. During his career within S.H.I.E.L.D., he met and married Agent Melinda May, though they eventually got divorced. Garner later returned to S.H.I.E.L.D. to do a profile on Skye, who had recently developed superpowers from undergoing Terrigenesis. Garner's own latent Inhuman genes were activated when he accidentally broke the Terrigen Crystal hidden in a ledger originally belonging to Jiaying, and he was transformed into the monstrous Lash.
"""@en .

<http://dbkwik.webdatacommons.org/marvelcinematicuniverse.wikia.com/resource/Leo_Fitz> rdfs:label "Leo Fitz"^^rdf:langString ;
    rdfs:comment "Leopold James \"Leo\" Fitz was a Scottish-born former S.H.I.E.L.D. agent and scientist. A genius engineer, he is one of the youngest and most prominent members of S.H.I.E.L.D.'s Sci-Tech division, and inseparable from his research partner and friend (and later wife), Jemma Simmons. He, along with Simmons, was recruited to Coulson's Team and worked with them on all of their missions. While on the team, Fitz became good friends with teammates Grant Ward and Skye. During the HYDRA Uprising, Fitz was an active participant in hunting for John Garrett and the rest of the Centipede Project. He was shocked by the revelation that Ward had been a member of HYDRA all along, and refused to believe it. When Ward was ordered to kill him and Simmons, they were trapped on the ocean floor."@en .

<http://dbkwik.webdatacommons.org/marvelcinematicuniverse.wikia.com/resource/Light_Elves> rdfs:label "Light Elves"^^rdf:langString ;
    rdfs:comment """The Light Elves are a race native to the Realm of Alfheim.

"""@en .

<http://dbkwik.webdatacommons.org/marvelcinematicuniverse.wikia.com/resource/Loki> rdfs:label "Loki"^^rdf:langString ;
    ns1:succeeded <http://dbkwik.webdatacommons.org/marvelcinematicuniverse.wikia.com/resource/Hela> ;
    rdfs:comment "Loki Laufeyson was the biological son of King Laufey, the ruler of the Frost Giants in Jotunheim. Shortly after his birth, Loki was then abandoned and left to die. Found by the Asgardian King Odin, he was taken to Asgard and raised by Odin and his wife Frigga as an Asgardian prince, along with their true biological son Thor. When he grew up, he became known as the \"God of Mischief\". When Thor was to be crowned King, Loki had sabotaged the coronation by letting the Frost Giants attack Asgard, thus leading Thor to seek vengeance on Jotunheim, which resulted in Thor's banishment to Earth and Loki finding out the truth about his heritage."@en .

<http://dbkwik.webdatacommons.org/marvelcinematicuniverse.wikia.com/resource/Loyolis> rdfs:label "Loyolis"^^rdf:langString ;
    rdfs:comment """Loyolis is an lower-caste Inhuman of Attilan, who works in the mines of the city because of his genetic heritage. He is the husband of Paripan and the father of Iridia and Bronaja.

"""@en .

<http://dbkwik.webdatacommons.org/marvelcinematicuniverse.wikia.com/resource/Lucio> rdfs:label "Lucio"^^rdf:langString ;
    rdfs:comment """Lucio was a Colombian Inhuman who worked with the National Police of Colombia. Due to his powers, he was abducted by HYDRA under Gideon Malick's orders, as the first step into rebuilding an Inhuman army for Hive. Soon, he became enthralled by Hive and actively worked to serve HYDRA before meeting his end at the hands of Joey Gutierrez.

"""@en .

<http://dbkwik.webdatacommons.org/marvelcinematicuniverse.wikia.com/resource/Luke_Cage> rdfs:label "Luke Cage"^^rdf:langString ;
    rdfs:comment "Carl Lucas is the son of James Lucas as well as a childhood friend of Willis Stryker who, while he was still serving as a policeman from Savannah, Georgia, was wrongfully convicted for a crime he did not commit and sent into Seagate Prison, where he met and fell in love with therapist Reva Connors who tried to make his time in jail easier. During his time inside prison, Lucas was then subjected to an experiment by Noah Burstein to save his life after Albert Rackham tried to kill him, leaving Lucas physically enhanced with superhuman strength and seemingly unbreakable skin."@en .

<http://dbkwik.webdatacommons.org/marvelcinematicuniverse.wikia.com/resource/Magic> rdfs:label "Magic"^^rdf:langString ;
    rdfs:comment """Magic is the practice of harnessing dimensional energies to manipulate one or more aspects of the infinite realities that are present within the Multiverse. It encompasses many different activities, including astral projection, divination, spell casting and teleportation, and includes the practices of many cultures and religions, as well as many books and writings from ancient times. Depending upon the individual, some sorcerers practice their power by certain belief systems, such as Shamanism, Voodoo, Wicca, or any number of other practices from cultures around the world.

"""@en .

<http://dbkwik.webdatacommons.org/marvelcinematicuniverse.wikia.com/resource/Malekith> rdfs:label "Malekith"^^rdf:langString ;
    rdfs:comment "Malekith (Mälekith in Shiväisith) was the utterly cruel and malevolent leader of the Dark Elves, a race of beings said to be older than the universe itself. Born in a realm of complete darkness, Malekith had led his people in a War against the Asgardians, using an ancient weapon known as the Aether, but they were thought to have been destroyed thousands of years ago during a final battle against the Asgardian King Bor. Malekith had survived, however, and after going into hiding for thousands of years, he returned during the Convergence and sought to retake the Aether and use its power to transform the universe by plunging it back into eternal darkness."@en .

<http://dbkwik.webdatacommons.org/marvelcinematicuniverse.wikia.com/resource/Manifest> rdfs:label "Manifest"^^rdf:langString ;
    rdfs:comment """Manifest is the seventh episode of the first season of the Netflix exclusive television series Luke Cage.

"""@en .

<http://dbkwik.webdatacommons.org/marvelcinematicuniverse.wikia.com/resource/Marcos_Martín> rdfs:label "Marcos Martín"^^rdf:langString ;
    rdfs:comment """Marcos Martín was an artist for Guidebook to the Marvel Cinematic Universe - Iron Man 3, Guidebook to the Marvel Cinematic Universe - Thor: The Dark World and Guidebook to the Marvel Cinematic Universe - Doctor Strange.

"""@en .

<http://dbkwik.webdatacommons.org/marvelcinematicuniverse.wikia.com/resource/Mark_Verheiden> rdfs:label "Mark Verheiden"^^rdf:langString ;
    rdfs:comment """Mark Verheiden wrote the Daredevil episodes New York's Finest and .380.

"""@en .

<http://dbkwik.webdatacommons.org/marvelcinematicuniverse.wikia.com/resource/Marvel_75_Years:_From_Pulp_to_Pop> a <http://dbkwik.webdatacommons.org/marvelcinematicuniverse.wikia.com/class/documentary> ;
    rdfs:label "Marvel 75 Years: From Pulp to Pop"^^rdf:langString ;
    rdfs:comment """Marvel 75 Years: From Pulp to Pop is a one-hour special documentary that aired on ABC on November 4, 2015.

"""@en .

<http://dbkwik.webdatacommons.org/marvelcinematicuniverse.wikia.com/resource/Marvel_One-Shot:_Agent_Carter> a <http://dbkwik.webdatacommons.org/marvelcinematicuniverse.wikia.com/class/one-shot> ;
    rdfs:label "Marvel One-Shot: Agent Carter"^^rdf:langString ;
    rdfs:comment """Agent Carter is the fourth Marvel One-Shot and was released on the Iron Man 3 Blu-ray. It takes place after the main events of Captain America: The First Avenger.

"""@en .

<http://dbkwik.webdatacommons.org/marvelcinematicuniverse.wikia.com/resource/Marvel_One-Shot:_Item_47> a <http://dbkwik.webdatacommons.org/marvelcinematicuniverse.wikia.com/class/one-shot> ;
    rdfs:label "Marvel One-Shot: Item 47"^^rdf:langString ;
    rdfs:comment """Item 47 is the third in a series of Marvel One-Shots, released on the The Avengers Blu-ray on September 25, 2012. It is set right after the Battle of New York, and features many references to The Avengers.

"""@en .

<http://dbkwik.webdatacommons.org/marvelcinematicuniverse.wikia.com/resource/Marvel_One-Shot:_The_Consultant> a <http://dbkwik.webdatacommons.org/marvelcinematicuniverse.wikia.com/class/one-shot> ;
    rdfs:label "Marvel One-Shot: The Consultant"^^rdf:langString ;
    rdfs:comment """The Consultant is the first in a series of Marvel One-Shots, released on the Thor Blu-ray on September 13, 2011. It is set after the main events of Thor and during the final events of The Incredible Hulk. It focuses on Phil Coulson and Jasper Sitwell's attempts to out-manuever the World Security Council's orders.

"""@en .

<http://dbkwik.webdatacommons.org/marvelcinematicuniverse.wikia.com/resource/Matthew_Ellis> rdfs:label "Matthew Ellis"^^rdf:langString ;
    rdfs:comment """Matthew Ellis is the President of the United States. While vowing to stop the attacks from the so-called Mandarin, the President was kidnapped and nearly assassinated by Aldrich Killian, but was rescued by Iron Man, allowing Ellis to continue his Presidency. During the HYDRA Uprising, Ellis was targeted again by HYDRA's Project Insight, but was saved by Captain America. 
"""@en .

<http://dbkwik.webdatacommons.org/marvelcinematicuniverse.wikia.com/resource/Michele_Fazekas> rdfs:label "Michele Fazekas"^^rdf:langString ;
    rdfs:comment """Michele Fazekas and her writing partner, Tara Butters, are executive producers for Agent Carter.
With Butters, she also wrote the Agent Carter episode Valediction, the story for A Little Song and Dance, and the teleplay for Hollywood Ending.
She was interviewed for the documentary Captain America: 75 Heroic Years.

"""@en .

<http://dbkwik.webdatacommons.org/marvelcinematicuniverse.wikia.com/resource/Nathaniel_Barton> rdfs:label "Nathaniel Barton"^^rdf:langString ;
    rdfs:comment """Nathaniel Pietro Barton is the third child of Clint and Laura Barton. His first name is the masculine form of Natasha, after Natasha Romanoff, while his middle name is a homage to Pietro Maximoff.

"""@en .

<http://dbkwik.webdatacommons.org/marvelcinematicuniverse.wikia.com/resource/Norse_Paganists> rdfs:label "Norse Paganists"^^rdf:langString ;
    rdfs:comment """The Norse Paganists were a hate group based out of Norway led by Jakob Nystrom and his girlfriend, Petra Larsen that was obsessed with anything to do with Asgardian mythology.

"""@en .

<http://dbkwik.webdatacommons.org/marvelcinematicuniverse.wikia.com/resource/Now_is_Not_the_End> rdfs:label "Now is Not the End"^^rdf:langString ;
    rdfs:comment """Now is Not the End is the first episode of the first season of the television series Agent Carter.

"""@en .

<http://dbkwik.webdatacommons.org/marvelcinematicuniverse.wikia.com/resource/Odin> rdfs:label "Odin"^^rdf:langString ;
    rdfs:comment "Odin Borson was the former King of Asgard, protector of the Nine Realms, father of Hela and Thor, the adoptive father of Loki, and husband of Frigga. During the ancient times, he was worshiped as the god of wisdom by the inhabitants of Earth. Once the greatest warrior in all the Nine Realms, over the centuries he learned how to appreciate peace, eventually banishing his own daughter to Hel when she attempted to subjugate the entire universe. When Thor almost provoked a new war with the Frost Giants of Jotunheim, Odin stripped him of his powers and exiled him to Earth, leaving Loki to take the throne."@en .

<http://dbkwik.webdatacommons.org/marvelcinematicuniverse.wikia.com/resource/PRIDE> rdfs:label "PRIDE"^^rdf:langString ;
    rdfs:comment """PRIDE (Promoting Resilience, Independence, Dedication & Excellence) is a Los Angeles-based charity organization whose members are some of the most rich and prominent families in Los Angeles. However, it serves as a front for their true agenda, tied to the ceremonial sacrifices of the Church of Gibborim in order to restore Jonah, their benefactor. Despite that, they eventually chose to turn against Jonah due to his numerous threats towards the children of the members of the PRIDE, the Runaways.

"""@en .

<http://dbkwik.webdatacommons.org/marvelcinematicuniverse.wikia.com/resource/Parish_Landman> rdfs:label "Parish Landman"^^rdf:langString ;
    rdfs:comment """Parish Landman is the co-founder of the large law-firm Landman and Zack. He was arrested for aiding Wilson Fisk with his illicit activities.

"""@en .

<http://dbkwik.webdatacommons.org/marvelcinematicuniverse.wikia.com/resource/Phase_Four> a <http://dbkwik.webdatacommons.org/marvelcinematicuniverse.wikia.com/class/phase> ;
    rdfs:label "Phase Four"^^rdf:langString ;
    ns1:directors <http://dbkwik.webdatacommons.org/marvelcinematicuniverse.wikia.com/resource/Cate_Shortland>,
        <http://dbkwik.webdatacommons.org/marvelcinematicuniverse.wikia.com/resource/Chloé_Zhao> ;
    ns1:duration 2019 ;
    ns1:films <http://dbkwik.webdatacommons.org/marvelcinematicuniverse.wikia.com/resource/Black_Widow_(film)>,
        <http://dbkwik.webdatacommons.org/marvelcinematicuniverse.wikia.com/resource/Guardians_of_the_Galaxy_Vol._3> ;
    rdfs:comment """Phase Four will be the fourth part of the Marvel Cinematic Universe after Phase Three.

"""@en .

<http://dbkwik.webdatacommons.org/marvelcinematicuniverse.wikia.com/resource/Priestesses_of_the_Sovereign> rdfs:label "Priestesses of the Sovereign"^^rdf:langString ;
    rdfs:comment """The Priestesses of the Sovereign is a religious group among the Sovereign, having Ayesha as their leader.

"""@en .

<http://dbkwik.webdatacommons.org/marvelcinematicuniverse.wikia.com/resource/Punisher> rdfs:label "Punisher"^^rdf:langString ;
    rdfs:comment """Francis "Frank" David Castle Sr. is a violent vigilante and former member of the United States Marine Corps, who had joined Cerberus Squad while he was serving in Afghanistan. Fearing he was slowly losing his honor under the command of Agent Orange, Castle returned to his family, only to lose them all during a brutal shooting. Castle became the Punisher, as he aimed to clean up New York City of crime by any means necessary. While seeking to avenge his own family's deaths, Castle came into conflict with Daredevil. Castle was soon arrested and, despite the efforts of Nelson and Murdock, was sentenced to life within prison. However, Castle was freed with the help of Wilson Fisk, and discovered the Blacksmith was the one who was responsible for his family's murder. 
"""@en .

<http://dbkwik.webdatacommons.org/marvelcinematicuniverse.wikia.com/resource/Q-Ship> rdfs:label "Q-Ship"^^rdf:langString ;
    rdfs:comment """Q-Ships are massive spaceships used by Thanos and the Black Order. These ring-shaped vessels were stored inside the even larger Sanctuary II, and Thanos deployed them during his invasions of Zen-Whoberi and Earth.

"""@en .

<http://dbkwik.webdatacommons.org/marvelcinematicuniverse.wikia.com/resource/Qovas%27_Ship> rdfs:label "Qovas' Ship"^^rdf:langString ;
    ns1:weapons <http://dbkwik.webdatacommons.org/marvelcinematicuniverse.wikia.com/resource/Ionizer_Missiles> ;
    rdfs:comment """Qovas' Ship is a Confederacy warship used by the Remorath Qovas, and later Glenn Talbot.

"""@en .

<http://dbkwik.webdatacommons.org/marvelcinematicuniverse.wikia.com/resource/Quake> rdfs:label "Quake"^^rdf:langString ;
    rdfs:comment """Daisy Johnson, formerly known as Skye, is an Inhuman, a genius-level hacker and a S.H.I.E.L.D. operative. She was born to Calvin L. Johnson, a doctor working in China, and Jiaying, but was taken away when her mother was seemingly killed by HYDRA. Growing up an orphan, she adopted the name Skye and worked for the Rising Tide, putting her on S.H.I.E.L.D.'s radar. However Phil Coulson recruited her into his team and appointed her as a consultant where she became a valued agent during the hunt for the Clairvoyant. After the events of the HYDRA Uprising, she joined the rest of her team in going off the grid. Skye was devastated when she learned that fellow agent Grant Ward was a HYDRA operative, and she joined the team in defeating the Centipede Project and John Garrett.
"""@en .

<http://dbkwik.webdatacommons.org/marvelcinematicuniverse.wikia.com/resource/Quinjet> rdfs:label "Quinjet"^^rdf:langString ;
    rdfs:comment """The Quinjet is a technologically advanced S.H.I.E.L.D. jet frequently used by the Avengers and STRIKE teams for transportation. Quinjets possess unique flight capabilities thanks to their unique wings which contain turbine fans. While most early Quinjets were lightly armed, the former S.H.I.E.L.D. initiative known as Project Insight introduced a series of Quinjets with a wider range of weapons.

"""@en .

<http://dbkwik.webdatacommons.org/marvelcinematicuniverse.wikia.com/resource/Reunion_(Runaways)> rdfs:label "Reunion (Runaways)"^^rdf:langString ;
    rdfs:comment """Reunion is the first episode of the first season of the television series Runaways.

"""@en .

<http://dbkwik.webdatacommons.org/marvelcinematicuniverse.wikia.com/resource/Rick_Cleveland> rdfs:label "Rick Cleveland"^^rdf:langString ;
    rdfs:comment """Rick Cleveland wrote the Inhumans episode Divide -- And Conquer and co-wrote the Inhumans episode ...And Finally: Black Bolt with Scott Reynolds.

"""@en .

<http://dbkwik.webdatacommons.org/marvelcinematicuniverse.wikia.com/resource/Rodriguez> rdfs:label "Rodriguez"^^rdf:langString ;
    rdfs:comment """Vice President Rodriguez was the former Vice President of the United States until he was caught and arrested for associating with A.I.M. under the leadership of Aldrich Killian.

"""@en .

<http://dbkwik.webdatacommons.org/marvelcinematicuniverse.wikia.com/resource/Rosalind_Price> rdfs:label "Rosalind Price"^^rdf:langString ;
    rdfs:comment """"Rosalind Price" was the head of the Advanced Threat Containment Unit, charged by President Matthew Ellis to control the increasing numbers of Inhumans appearing across the world. Since her organization was formed as a replacement for the outlawed agency S.H.I.E.L.D., she treated Phil Coulson and his agents as enemies, but later accepted them as reluctant allies in the fight against the rogue Inhuman Lash. She continued to build up a rapport with S.H.I.E.L.D., even growing romantically attached to Coulson, until she was tragically assassinated by Grant Ward.

"""@en .

<http://dbkwik.webdatacommons.org/marvelcinematicuniverse.wikia.com/resource/Sanctuary_II> rdfs:label "Sanctuary II"^^rdf:langString ;
    rdfs:comment """The Sanctuary II is a massive warship commanded by Thanos.

"""@en .

<http://dbkwik.webdatacommons.org/marvelcinematicuniverse.wikia.com/resource/Scott_Reynolds> rdfs:label "Scott Reynolds"^^rdf:langString ;
    rdfs:comment """Scott Reynolds is a co-executive producer for Jessica Jones and Iron Fist.
He also wrote the Jessica Jones episodes AKA It's Called Whiskey, AKA WWJD?, AKA I've Got the Blues and AKA Smile, the Iron Fist episodes Eight Diagram Dragon Palm and Bar the Big Boss and the Inhumans episode Something Inhuman This Way Comes... and co-wrote the Inhumans episode ...And Finally: Black Bolt with Rick Cleveland.

"""@en .

<http://dbkwik.webdatacommons.org/marvelcinematicuniverse.wikia.com/resource/Searching_for_Secrets> rdfs:label "Searching for Secrets"^^rdf:langString ;
    rdfs:comment """Searching for Secrets is the second episode of the web series Agents of S.H.I.E.L.D.: Double Agent.

"""@en .

<http://dbkwik.webdatacommons.org/marvelcinematicuniverse.wikia.com/resource/Sharon_Carter> rdfs:label "Sharon Carter"^^rdf:langString ;
    rdfs:comment """Sharon Carter is the great niece of legendary S.H.I.E.L.D. founder Peggy Carter. Following in her aunt's footsteps, Carter became an agent of S.H.I.E.L.D. who had briefly worked undercover as the neighbor of Steve Rogers under the direct orders of Nick Fury. She fought on the side of S.H.I.E.L.D. during the Battle at the Triskelion, facing off against Brock Rumlow to protect millions of lives. In the aftermath of the HYDRA Uprising she was forced to then leave S.H.I.E.L.D. and instead joined the CIA. She continued to have a close relationship with Rogers and sided with him when he chose to protect Bucky Barnes from the government she still worked for, indirectly being responsible for sparking the devastating Avengers Civil War.

"""@en .

<http://dbkwik.webdatacommons.org/marvelcinematicuniverse.wikia.com/resource/Shocker> rdfs:label "Shocker"^^rdf:langString ;
    rdfs:comment """Herman Schultz is a former salvage worker who had become a professional criminal and one of the key members of Adrian Toomes' Crew who had sold alien-human hybrid weaponry created by the Tinkerer. As Toomes had murdered his former crewmate Jackson Brice, who had used a modified gauntlet occasionally under the alias of Shocker, Toomes passed the gauntlet down to Schultz and then appointed him as the new Shocker. With his new title and power of the gauntlet, Schultz continued to aid Toomes with fighting Spider-Man's attempts to stop all their black market arms deals, eventually resulting in the Shocker being defeated during a fight and arrested.

"""@en .

<http://dbkwik.webdatacommons.org/marvelcinematicuniverse.wikia.com/resource/Sovereign> rdfs:label "Sovereign"^^rdf:langString ;
    rdfs:comment """The Sovereign are a highly advanced, genetically engineered galactic race who live on the collective of planets of the same name.

"""@en .

<http://dbkwik.webdatacommons.org/marvelcinematicuniverse.wikia.com/resource/Stark_Industries> rdfs:label "Stark Industries"^^rdf:langString ;
    rdfs:comment """Stark Industries is a multinational industrial company owned by Tony Stark, and is the largest tech conglomerate in the world. Founded in 1939 by Howard Stark, the elder Stark ran the company from its inception up until his death in 1991, after which Obadiah Stane was appointed interim CEO. with Tony Stark officially assuming the position shortly after at the age of 21.
"""@en .

<http://dbkwik.webdatacommons.org/marvelcinematicuniverse.wikia.com/resource/Stephen_Surjik> rdfs:label "Stephen Surjik"^^rdf:langString ;
    rdfs:comment """Stephen Surjik directed the Daredevil episodes Shadows in the Glass, Guilty as Sin and .380, the Jessica Jones episodes AKA The Sandwich Saved Me and AKA You're a Winner!, the Luke Cage episodes Take It Personal and The Creator, the Iron Fist episodes Dragon Plays with Fire in Season One and Morning of the Mindstorm in Season Two, The Defenders episode Ashes, Ashes and the The Punisher episode Memento Mori. He also directed an upcoming episode of Runaways.

"""@en .

<http://dbkwik.webdatacommons.org/marvelcinematicuniverse.wikia.com/resource/Strategic_Operations_Command_Center> rdfs:label "Strategic Operations Command Center"^^rdf:langString ;
    rdfs:comment """The Strategic Operations Command Center, or SOCC, was a special United States Army anti-Hulk Task Force under the command of then-Lieutenant general Thaddeus Ross. They battled Hulk in Brazil, and again at Culver University.

"""@en .

<http://dbkwik.webdatacommons.org/marvelcinematicuniverse.wikia.com/resource/Surtur> rdfs:label "Surtur"^^rdf:langString ;
    rdfs:comment """Surtur was the fire demon and ruler of Muspelheim. Prophesied to be the one to initiate the Asgardian doomsday known as Ragnarök, Odin successfully defeated the fire demon, stole from him the source of his power, the Eternal Flame, before banishing him and his entire race to Muspelheim. After Odin went missing following the Second Dark Elf Conflict, a weakened Surtur intended to finally start Ragnarök, only to be defeated and killed by Thor. Despite this, Thor and Loki later resurrected him using the Eternal Flame to use him to help defeat Hela. The fire demon then fulfilled the prophecy of Ragnarök by destroying Asgard along with Hela and himself in the process, unaware that the realm had already been evacuated.

"""@en .

<http://dbkwik.webdatacommons.org/marvelcinematicuniverse.wikia.com/resource/The_Asset> rdfs:label "The Asset"^^rdf:langString ;
    rdfs:comment """The Asset is the third episode of the first season of the television series Agents of S.H.I.E.L.D.

"""@en .

<http://dbkwik.webdatacommons.org/marvelcinematicuniverse.wikia.com/resource/The_Avengers_Prelude:_Fury%27s_Big_Week> rdfs:label "The Avengers Prelude: Fury's Big Week"^^rdf:langString ;
    rdfs:comment """The Avengers Prelude: Fury's Big Week, or just Fury's Big Week, is a limited series comic book which serves as a prequel to The Avengers. It was written by Christopher Yost & Eric Pearson with art duties covered by Luke Ross & Daniel HDR.

"""@en .

<http://dbkwik.webdatacommons.org/marvelcinematicuniverse.wikia.com/resource/The_Dark_at_the_End_of_the_Tunnel> rdfs:label "The Dark at the End of the Tunnel"^^rdf:langString ;
    rdfs:comment """The Dark at the End of the Tunnel is the twelfth episode of the second season of the Netflix exclusive television series Daredevil.

"""@en .

<http://dbkwik.webdatacommons.org/marvelcinematicuniverse.wikia.com/resource/The_Defenders_(episode)> rdfs:label "The Defenders (episode)"^^rdf:langString ;
    rdfs:comment """The Defenders is the eighth and final episode of the first season of The Defenders.

"""@en .

<http://dbkwik.webdatacommons.org/marvelcinematicuniverse.wikia.com/resource/The_Incredible_Hulk:_The_Big_Picture> rdfs:label "The Incredible Hulk: The Big Picture"^^rdf:langString ;
    rdfs:comment """The Incredible Hulk: The Big Picture is a motion comic included with the Walmart 2-disc set of The Incredible Hulk. The comic covers the origin of Hulk and how he found himself in South America.

"""@en .

<http://dbkwik.webdatacommons.org/marvelcinematicuniverse.wikia.com/resource/The_Iron_Ceiling> rdfs:label "The Iron Ceiling"^^rdf:langString ;
    rdfs:comment """The Iron Ceiling is the fifth episode of the first season of the television series Agent Carter.

"""@en .

<http://dbkwik.webdatacommons.org/marvelcinematicuniverse.wikia.com/resource/The_Man_in_the_Box> rdfs:label "The Man in the Box"^^rdf:langString ;
    rdfs:comment """The Man in the Box is the tenth episode of the second season of the Netflix exclusive television series Daredevil.

"""@en .

<http://dbkwik.webdatacommons.org/marvelcinematicuniverse.wikia.com/resource/The_Punisher> rdfs:label "The Punisher"^^rdf:langString ;
    rdfs:comment """Marvel's The Punisher, or simply The Punisher, is a television series based on the Marvel Comics vigilante character of the same name. It is produced by Marvel Television and streamed on Netflix.
The first season premiered on November 17, 2017.
The second season was announced on December 12, 2017.

"""@en .

<http://dbkwik.webdatacommons.org/marvelcinematicuniverse.wikia.com/resource/Theo_Broussard> rdfs:label "Theo Broussard"^^rdf:langString ;
    rdfs:comment """Doctor Theo Broussard was a psychiatrist hired by the Joint Counter Terrorist Centre to interrogate Bucky Barnes.

"""@en .

<http://dbkwik.webdatacommons.org/marvelcinematicuniverse.wikia.com/resource/Thor> rdfs:label "Thor"^^rdf:langString ;
    ns1:current <http://dbkwik.webdatacommons.org/marvelcinematicuniverse.wikia.com/resource/Thor_(film)> ;
    rdfs:comment """Thor Odinson is the current king of Asgard, a founding member of the Avengers, and the God of Thunder. When his irresponsible behavior restarted a conflict between Asgard and Jotunheim, Thor was denied the right to become king, stripped of his power, and banished by his father Odin to Earth. While exiled on Earth, Thor learned humility, finding love with Jane Foster, and helping to save his new friends from a destructive threat sent by his adoptive brother Loki. Due to his selfless act of sacrifice, Thor redeemed himself in his father's eyes and was granted his power once more, which he then used to defeat Loki's schemes of genocide.
"""@en .

<http://dbkwik.webdatacommons.org/marvelcinematicuniverse.wikia.com/resource/Thor:_The_Dark_World> rdfs:label "Thor: The Dark World"^^rdf:langString ;
    rdfs:comment """Thor: The Dark World is a 2013 superhero film, based on the Marvel Comics superhero of the same name. It is a sequel to Thor and The Avengers, and is the eighth installment in the Marvel Cinematic Universe and the second installment of Phase Two. The film was released internationally on October 30, 2013 and on November 8, 2013 in the United States.
"""@en .

<http://dbkwik.webdatacommons.org/marvelcinematicuniverse.wikia.com/resource/Tim_Roth> rdfs:label "Tim Roth"^^rdf:langString ;
    rdfs:comment """Tim Roth portrayed Emil Blonsky/Abomination in The Incredible Hulk.
Archive footage of Tim Roth from The Incredible Hulk was used in Marvel One-Shot: The Consultant.
He also voiced the character in the video game The Incredible Hulk.

"""@en .

<http://dbkwik.webdatacommons.org/marvelcinematicuniverse.wikia.com/resource/Timeline> rdfs:label "Timeline"^^rdf:langString ;
    rdfs:comment """This is a Timeline of events as depicted or mentioned in the Marvel Cinematic Universe.

"""@en .

<http://dbkwik.webdatacommons.org/marvelcinematicuniverse.wikia.com/resource/Titan> rdfs:label "Titan"^^rdf:langString ;
    rdfs:comment """Titan is the desolated homeworld of Thanos.

"""@en .

<http://dbkwik.webdatacommons.org/marvelcinematicuniverse.wikia.com/resource/Titans> rdfs:label "Titans"^^rdf:langString ;
    rdfs:comment """The Titans are a race of beings from the planet Titan who were all but destroyed by a catastrophic event.

"""@en .

<http://dbkwik.webdatacommons.org/marvelcinematicuniverse.wikia.com/resource/Tom_Shankland> rdfs:label "Tom Shankland"^^rdf:langString ;
    rdfs:comment """Tom Shankland directed the Luke Cage episode DWYCK, the Iron Fist episode Rolling Thunder Cannon Punch and The Punisher episodes 3 AM and Two Dead Men.

"""@en .

<http://dbkwik.webdatacommons.org/marvelcinematicuniverse.wikia.com/resource/Travis_Scott> rdfs:label "Travis Scott"^^rdf:langString ;
    rdfs:comment """Jacques Webster, Jr., known professionally as Travis Scott, is an American rapper, singer, songwriter, and record producer.
His collaboration with Kendrick Lamar, "Big Shot", is featured on Black Panther: The Album.

"""@en .

<http://dbkwik.webdatacommons.org/marvelcinematicuniverse.wikia.com/resource/Trevor_Slattery> rdfs:label "Trevor Slattery"^^rdf:langString ;
    rdfs:comment """Trevor Slattery was an actor with drug addictions and other legal problems until he was approached by the scientist Aldrich Killian to pose as the Mandarin, the idealized perfect terrorist. Taking responsibility for the widespread accidents caused by Killian's experiments, the Mandarin persona convinced people that he was in command of the infamous terrorist organization known as the Ten Rings, eventually becoming the most feared terrorist in the West. He was captured by Tony Stark and put in Seagate Prison, where he became something of a celebrity. There he became the subject of a documentary by Jackson Norriss, who was really an agent of the real Mandarin, and whose real purpose was to kidnap Slattery in revenge for Slattery's insult to the Mandarin.

"""@en .

<http://dbkwik.webdatacommons.org/marvelcinematicuniverse.wikia.com/resource/Two_Dead_Men> rdfs:label "Two Dead Men"^^rdf:langString ;
    rdfs:comment """Two Dead Men is the second episode of the first season of the television series The Punisher.

"""@en .

<http://dbkwik.webdatacommons.org/marvelcinematicuniverse.wikia.com/resource/Uprising_in_Attilan> rdfs:label "Uprising in Attilan"^^rdf:langString ;
    rdfs:comment """The Uprising in Attilan was a conflict orchestrated by Maximus Boltagon of Attilan, who sought to claim the throne by staging a coup d'état against the Inhuman Royal Family and overthrowing his older brother Black Bolt.

"""@en .

<http://dbkwik.webdatacommons.org/marvelcinematicuniverse.wikia.com/resource/Volstagg> rdfs:label "Volstagg"^^rdf:langString ;
    rdfs:comment """Volstagg was an Asgardian and a member of the Warriors Three. He was a good friend of Thor, Sif, and fellow members Hogun and Fandral. Alongside all his fellow warriors, Volstagg took part in a poorly considered strike against all the Frost Giants of Jotunheim, which soon resulted in King Odin deciding to directly punish Thor by banishing him to the Earth without his powers. When Loki then took the throne of Asgard during Thor's banishment, Volstagg and his allies played a key role saving Thor from the Destroyer before bringing him back to Asgard where he successfully stopped Loki from stealing the throne of Asgard and restoring the peace.
"""@en .

<http://dbkwik.webdatacommons.org/marvelcinematicuniverse.wikia.com/resource/Vulture> rdfs:label "Vulture"^^rdf:langString ;
    rdfs:comment """Adrian Toomes is the former owner of the Toomes Salvage Company, based inside New York City, who chose to be a criminal after he lost his livelihood as Damage Control, a joint venture between the federal government and Tony Stark, was created. Recruiting his co-workers and equipping himself with a flying exo-suit created from the Chitauri technology he had stolen, Toomes took on the identity of Vulture and spent the next four years stealing the advanced weaponry to sell on the black market. Toomes' activities were noticed by Spider-Man, forcing him to hunt down the young hero. During their final clash, Spider-Man defeated Vulture before saving his life, and in gratitude Toomes had refused to give up Spider-Man's true identity to his inmates, including Mac Gargan, in prison.

"""@en .

<http://dbkwik.webdatacommons.org/marvelcinematicuniverse.wikia.com/resource/War_Machine> rdfs:label "War Machine"^^rdf:langString ;
    rdfs:comment """Colonel James Rupert Rhodes, commonly known as Rhodey, is a U.S. military officer and jet pilot in the U.S. Air Force. He is the best friend of Tony Stark/Iron Man and the liaison between Stark Industries and the military in the Department of Acquisitions. When Stark was kidnapped by the Ten Rings, Rhodes led the mission to rescue his friend. He is known as War Machine when wearing his heavily-armed battlesuit but his alias was temporarily rebranded to Iron Patriot during Aldrich Killian's War.
"""@en .

<http://dbkwik.webdatacommons.org/marvelcinematicuniverse.wikia.com/resource/Winter_Soldier> rdfs:label "Winter Soldier"^^rdf:langString ;
    rdfs:comment """Sergeant James Buchanan "Bucky" Barnes was a former soldier of the 107th Infantry Regiment and the best friend of Steve Rogers, since childhood. Barnes was conscripted and assigned to the 107th in 1942. His regiment was captured by the forces of HYDRA, but Barnes along with what remained of his regiment were rescued by Rogers, who had become Captain America during Barnes' military absence. Joining forces in the continuing war, Barnes and Rogers formed the Howling Commandos to battle the Red Skull's forces. During an attempt to capture HYDRA scientist Arnim Zola, Barnes was caught in an ambush and plummeted hundreds of feet from the HYDRA train. As no body was ever recovered, he was then presumed dead, but officially listed as MIA.
"""@en .

<http://dbkwik.webdatacommons.org/marvelcinematicuniverse.wikia.com/resource/Wrigley_Fire_Department> rdfs:label "Wrigley Fire Department"^^rdf:langString ;
    rdfs:comment """The Wrigley Fire Department is the Fire Department responsible for the firefighting in Wrigley, Pennsylvania.

"""@en .

<http://marvelcinematicuniverse.wikia.com/wiki/Special:FilePath/$.jpeg?width=300> a ns3:Image ;
    dc:rights <http://marvelcinematicuniverse.wikia.com/wiki/File:$.jpeg> .

<http://marvelcinematicuniverse.wikia.com/wiki/Special:FilePath/%0A0-8-4.png?width=300> a ns3:Image ;
    dc:rights <http://marvelcinematicuniverse.wikia.com/wiki/File:%0A0-8-4.png> .

<http://dbkwik.webdatacommons.org/marvelcinematicuniverse.wikia.com/class/phase> a owl:Class ;
    rdfs:label "Phase"@en .

<http://dbkwik.webdatacommons.org/marvelcinematicuniverse.wikia.com/resource/...And_Finally:_Black_Bolt> a <http://dbkwik.webdatacommons.org/marvelcinematicuniverse.wikia.com/class/episode> ;
    rdfs:label "...And Finally: Black Bolt"^^rdf:langString ;
    ns1:director <http://dbkwik.webdatacommons.org/marvelcinematicuniverse.wikia.com/resource/Billy_Gierhart> ;
    ns1:firstAired "2017-11-10"^^xsd:date ;
    ns1:previous <http://dbkwik.webdatacommons.org/marvelcinematicuniverse.wikia.com/resource/Havoc_in_the_Hidden_Land> ;
    ns1:season 1 ;
    ns1:writer <http://dbkwik.webdatacommons.org/marvelcinematicuniverse.wikia.com/resource/Rick_Cleveland>,
        <http://dbkwik.webdatacommons.org/marvelcinematicuniverse.wikia.com/resource/Scott_Reynolds> ;
    ns3:abstract """...And Finally: Black Bolt is the eighth and final episode of the first season of the television series Inhumans.

"""@en ;
    ns3:thumbnail <http://marvelcinematicuniverse.wikia.com/wiki/Special:FilePath/...And_Finally_Black_Bolt_photo.jpg?width=300> ;
    ns3:wikiPageExternalLink <http://marvel.wikia.com/wiki/Main_Page> ;
    ns3:wikiPageWikiLink <http://dbkwik.webdatacommons.org/marvelcinematicuniverse.wikia.com/resource/Aaron_Hendry>,
        <http://dbkwik.webdatacommons.org/marvelcinematicuniverse.wikia.com/resource/Agon> ;
    ns3:wikiPageWikiLinkText "...And Finally: Black Bolt"^^rdf:langString,
        "Episode 1.08: ''...And Finally: Black Bolt"^^rdf:langString,
        "Episode 1.08: ''...And Finally: Black Bolt''"^^rdf:langString ;
    dcterms:subject <http://dbkwik.webdatacommons.org/marvelcinematicuniverse.wikia.com/resource/Category:Inhumans_(TV_series)_Episodes> ;
    rdfs:comment """...And Finally: Black Bolt is the eighth and final episode of the first season of the television series Inhumans.

"""@en ;
    skos:altLabel "...And Finally: Black Bolt"^^rdf:langString ;
    foaf:depiction <http://marvelcinematicuniverse.wikia.com/wiki/Special:FilePath/...And_Finally_Black_Bolt_photo.jpg>,
        <http://marvelcinematicuniverse.wikia.com/wiki/Special:FilePath/Daredevil-Episode-211-3-03212016.jpg> .

<http://dbkwik.webdatacommons.org/marvelcinematicuniverse.wikia.com/resource/1940s> a <http://dbkwik.webdatacommons.org/marvelcinematicuniverse.wikia.com/class/timeline> ;
    rdfs:label "1940s"^^rdf:langString ;
    rdfs:comment """This is a timeline of events that occurred during the 1940s.

"""@en .

<http://dbkwik.webdatacommons.org/marvelcinematicuniverse.wikia.com/resource/2014> rdfs:label "2014"^^rdf:langString ;
    rdfs:comment """This is a timeline of events that occurred in 2014.

"""@en .

<http://dbkwik.webdatacommons.org/marvelcinematicuniverse.wikia.com/resource/2015> rdfs:label "2015"^^rdf:langString ;
    rdfs:comment """This is a timeline of events that occurred in 2015.

"""@en .

<http://dbkwik.webdatacommons.org/marvelcinematicuniverse.wikia.com/resource/2091> a <http://dbkwik.webdatacommons.org/marvelcinematicuniverse.wikia.com/class/quote> ;
    rdfs:label "2091"^^rdf:langString ;
    rdfs:comment """This is a timeline of events that occurred in the original 2091 before Glenn Talbot was killed by Quake, preventing this future from coming to pass.

"""@en .

<http://dbkwik.webdatacommons.org/marvelcinematicuniverse.wikia.com/resource/Agents_of_S.H.I.E.L.D.:_Double_Agent> a <http://dbkwik.webdatacommons.org/marvelcinematicuniverse.wikia.com/class/web_series> ;
    rdfs:label "Agents of S.H.I.E.L.D.: Double Agent"^^rdf:langString ;
    ns1:first <http://dbkwik.webdatacommons.org/marvelcinematicuniverse.wikia.com/resource/Infiltrating_the_Set> ;
    rdfs:comment """Agents of S.H.I.E.L.D.: Double Agent is a five-part original web series designed as a behind-the-scenes feature for Agents of S.H.I.E.L.D.

"""@en .

<http://dbkwik.webdatacommons.org/marvelcinematicuniverse.wikia.com/resource/Aleta_Ogord> rdfs:label "Aleta Ogord"^^rdf:langString ;
    rdfs:comment """Aleta Ogord is a Ravager captain and the wife of the fellow Ravager captain Stakar Ogord.

"""@en .

<http://dbkwik.webdatacommons.org/marvelcinematicuniverse.wikia.com/resource/Ant-Man_(film)> a <http://dbkwik.webdatacommons.org/marvelcinematicuniverse.wikia.com/class/movie> ;
    rdfs:label "Ant-Man (film)"^^rdf:langString ;
    ns1:boxoffice "5.194E8"^^<http://dbkwik.webdatacommons.org/datatype/usDollar> ;
    ns1:producer <http://dbkwik.webdatacommons.org/marvelcinematicuniverse.wikia.com/resource/Alan_Fine>,
        <http://dbkwik.webdatacommons.org/marvelcinematicuniverse.wikia.com/resource/Brad_Winderbaum> ;
    rdfs:comment """Ant-Man is a 2015 superhero film, based on the Marvel Comics superhero of the same name. It is the twelfth installment in the Marvel Cinematic Universe and the sixth and final installment of Phase Two. The film was released on July 14, 2015 internationally and on July 17, 2015 in the United States.
"""@en .

<http://dbkwik.webdatacommons.org/marvelcinematicuniverse.wikia.com/resource/Asgard> rdfs:label "Asgard"^^rdf:langString ;
    rdfs:comment """Asgard was one of the Nine Realms and the home of the Asgardians, a powerful race recognized by the galaxy as honorable and brave peacekeepers.
Asgard was destroyed during Ragnarök when Thor ordered Loki to unleash Surtur in order to kill their sister Hela. Led by their new king, a large number of survivors fled onboard a starship, planning to relocate to Earth.

"""@en .

<http://dbkwik.webdatacommons.org/marvelcinematicuniverse.wikia.com/resource/Asgardians> a <http://dbkwik.webdatacommons.org/marvelcinematicuniverse.wikia.com/class/race> ;
    rdfs:label "Asgardians"^^rdf:langString ;
    ns1:homeplanet <http://dbkwik.webdatacommons.org/marvelcinematicuniverse.wikia.com/resource/Asgard> ;
    rdfs:comment """The Asgardians are the inhabitants of Asgard. They are a race of extraterrestrial beings similar to the human beings possessing a highly advanced form of technology resembling magic and sorcery, which their entire civilization is built on.
The Asgardians are a brave and a powerful warrior race whose passion for adventure is their religion, and their reputation as one of the mightiest races in the universe has earned them the respect and fear from other races.
"""@en .

<http://dbkwik.webdatacommons.org/marvelcinematicuniverse.wikia.com/resource/Avengers> rdfs:label "Avengers"^^rdf:langString ;
    ns1:vehicles <http://dbkwik.webdatacommons.org/marvelcinematicuniverse.wikia.com/resource/Quinjet> ;
    rdfs:comment """The Avengers, also known as the Heroes of New York, are a team of extraordinary individuals, either with superpowers or other special characteristics. Its purpose is to protect world stability from inner or extraterrestrial threats, and to work with the peaceful interests of the whole world rather than a specific country or organization. The Avengers were first assembled by S.H.I.E.L.D. when Loki invaded Earth with his Chitauri army to conquer the planet. The team defeated him and went to their separate ways.
"""@en .

<http://dbkwik.webdatacommons.org/marvelcinematicuniverse.wikia.com/resource/Billy_Russo> rdfs:label "Billy Russo"^^rdf:langString ;
    rdfs:comment "William \"Billy\" Russo is a former Special Forces Marine who had become a close friend of Frank Castle. Russo became a part of Cerberus Squad under William Rawlins' leadership, assisting in assassinations of high value targets. Upon leaving the Marines, Russo was funded by Rawlins and became the founder and CEO of Anvil Securities, training up soldiers for Rawlins' needs. Learning of Castle's return as the Punisher, Russo was recruited by Rawlins to assassinate his former friend, using Dinah Madani to learn of Castle's whereabouts which eventually exposed his own involvement in Cerberus."@en .

<http://dbkwik.webdatacommons.org/marvelcinematicuniverse.wikia.com/resource/Captain_America:_First_Vengeance> rdfs:label "Captain America: First Vengeance"^^rdf:langString ;
    ns1:editorinchief <http://dbkwik.webdatacommons.org/marvelcinematicuniverse.wikia.com/resource/Axel_Alonso> ;
    rdfs:comment """Captain America: First Vengeance is an eight part digital comic book set during the events of Captain America: The First Avenger written by Fred Van Lente.

"""@en .

<http://dbkwik.webdatacommons.org/marvelcinematicuniverse.wikia.com/resource/Captain_America:_The_First_Avenger> rdfs:label "Captain America: The First Avenger"^^rdf:langString ;
    rdfs:comment """Captain America: The First Avenger is a 2011 superhero film, based on the Marvel Comics superhero of the same name. It is the fifth installment in the Marvel Cinematic Universe and the fifth installment of Phase One.
It was directed by Joe Johnston and stars Chris Evans as Steve Rogers/Captain America, Hayley Atwell as Peggy Carter, Sebastian Stan as Bucky Barnes and Hugo Weaving as Johann Schmidt/Red Skull.
The film spawned two sequels: Captain America: The Winter Soldier in 2014 and Captain America: Civil War in 2016.

"""@en .

<http://dbkwik.webdatacommons.org/marvelcinematicuniverse.wikia.com/resource/Category:Help> rdfs:label "Help"^^rdf:langString .

<http://dbkwik.webdatacommons.org/marvelcinematicuniverse.wikia.com/resource/Doctor_Strange_(film)> rdfs:label "Doctor Strange (film)"^^rdf:langString ;
    rdfs:comment """Doctor Strange is a 2016 superhero film, based on the Marvel Comics superhero of the same name. It is the fourteenth installment in the Marvel Cinematic Universe, and the second installment of Phase Three. The film was released on October 25, 2016 internationally and on November 4, 2016 in the United States.The film is directed by Scott Derrickson and stars Benedict Cumberbatch as Stephen Strange/Doctor Strange and Dormammu, Chiwetel Ejiofor as Karl Mordo, Rachel McAdams as Christine Palmer, Benedict Wong as Wong, Mads Mikkelsen as Kaecilius and Tilda Swinton as the Ancient One.

"""@en .

<http://dbkwik.webdatacommons.org/marvelcinematicuniverse.wikia.com/resource/Earth> rdfs:label "Earth"^^rdf:langString ;
    rdfs:comment """Earth is the third planet of the Solar system, home to the humans, Inhumans, and a number of Asgardian immigrants. It is also one of the Nine Realms, a group of planetary bodies aligned by the cosmic nimbus Yggdrasil, and is also the central Realm that all the others revolve around. The various races of the Nine Realms refer to Earth as "Midgard", while those living beyond the realms call it "Terra."
Earth orbits around one single star, the Sun, and has only one permanent natural satellite, called the Moon.

"""@en .

<http://dbkwik.webdatacommons.org/marvelcinematicuniverse.wikia.com/resource/Enoch> rdfs:label "Enoch"^^rdf:langString ;
    ns1:age <http://dbkwik.webdatacommons.org/marvelcinematicuniverse.wikia.com/resource/Earth> ;
    rdfs:comment """Enoch was a Chronicom anthropologist, sent to Earth in order to study and record the history of Humans. Coming into contact with Robin Hinton, whose Inhuman power made her able to see into the future, Enoch became aware of an Extinction-Level Event that would destroy Earth itself. While helping Polly Hinton take care and raise her daughter, Enoch began to make arrangements to save humanity, including sending Phil Coulson and other agents into the future through a White Monolith, and helping Leo Fitz survive for 74 years in cryostasis to help his friends. He helped the team get back together and to the present, sacrificing himself in the process.

"""@en .

<http://dbkwik.webdatacommons.org/marvelcinematicuniverse.wikia.com/resource/Eric_Savin> rdfs:label "Eric Savin"^^rdf:langString ;
    rdfs:comment """Eric Savin was a former Lieutenant Colonel of the United States Army. He was the right-hand man of Aldrich Killian and an enemy of Iron Man, using his powers gained by injecting Extremis to seriously endanger Stark's life. He stood by Killian as he kidnapped President Matthew Ellis and took the nation hostage, only to be killed by Iron Man during the resulting battle.

"""@en .

<http://dbkwik.webdatacommons.org/marvelcinematicuniverse.wikia.com/resource/Erik_Killmonger> rdfs:label "Erik Killmonger"^^rdf:langString ;
    rdfs:comment "Erik Stevens (born N'Jadaka) was a former African-American black-ops soldier of Wakandan origin through his father, Prince N'Jobu. His savagery while serving in the U.S. black-ops unit, earned him the nickname Killmonger. Years after his uncle T'Chaka had killed his father for betraying Wakanda, Killmonger then planned to forcibly dethrone his son and heir T'Challa in order to accomplish his father's plan to seize control of the world using all of Wakanda's Vibranium technology and stop the oppression of people of African descent all across the world. Manipulating and then killing Ulysses Klaue to gain access to their city, Killmonger seemingly killed T'Challa during their ritual combat and took the throne."@en .

<http://dbkwik.webdatacommons.org/marvelcinematicuniverse.wikia.com/resource/Fred_Tatasciore> rdfs:label "Fred Tatasciore"^^rdf:langString ;
    rdfs:comment """Fred Tatasciore voiced Hulk and Abomination in The Incredible Hulk.
He also voiced Obadiah Stane/Iron Monger, A.I.M. President, Afghan Soldier and Maggia Soldier in Iron Man and Hulk in The Incredible Hulk.

"""@en .

<http://dbkwik.webdatacommons.org/marvelcinematicuniverse.wikia.com/resource/Guardians_of_the_Galaxy_Vol._2> rdfs:label "Guardians of the Galaxy Vol. 2"^^rdf:langString ;
    rdfs:comment """Guardians of the Galaxy Vol. 2 is a 2017 superhero fantasy adventure film, based on the Marvel Comics superhero team of the same name. It is the sequel to Guardians of the Galaxy and the fifteenth installment in the Marvel Cinematic Universe, as well as the third installment of Phase Three. The film was released on April 25, 2017 internationally and on May 5, 2017 in the United States.
"""@en .

<http://dbkwik.webdatacommons.org/marvelcinematicuniverse.wikia.com/resource/HYDRA_Cannon> rdfs:label "HYDRA Cannon"^^rdf:langString ;
    rdfs:comment """The HYDRA Cannon was one of the first advanced weapons that were designed by Arnim Zola when he managed to harness the power of the Tesseract by using a special battery that stores it.

"""@en .

<http://dbkwik.webdatacommons.org/marvelcinematicuniverse.wikia.com/resource/Hellfire> rdfs:label "Hellfire"^^rdf:langString ;
    rdfs:comment """JT James is an Inhuman who was taken to Afterlife under Jiaying's leadership, but was expelled from the community before undergoing Terrigenesis for trying to steal from its archives. After he finally gained his Inhuman powers with the intervention of Hive and Daisy Johnson, he started calling himself Hellfire.
"""@en .

<http://dbkwik.webdatacommons.org/marvelcinematicuniverse.wikia.com/resource/Ho_Yinsen> rdfs:label "Ho Yinsen"^^rdf:langString ;
    rdfs:comment """Ho Yinsen was a renowned scientist and surgeon, hailing from the village of Gulmira. Yinsen was held captive, alongside Tony Stark, by the Ten Rings in Afghanistan, where he was charged with attending to Stark's medical needs when Stark was brought in injured from an explosive. Having lost his family to local terrorist activity, Yinsen helped Stark escape the cave, but willingly sacrificed himself in the process.

"""@en .

<http://dbkwik.webdatacommons.org/marvelcinematicuniverse.wikia.com/resource/Iron_Fist> rdfs:label "Iron Fist"^^rdf:langString ;
    ns1:current <http://dbkwik.webdatacommons.org/marvelcinematicuniverse.wikia.com/resource/Iron_Fist> ;
    rdfs:comment "Daniel Thomas \"Danny\" Rand-K'ai is the only child of the owners of Rand Enterprises. Rand lost his parents in a plane crash which resulted with the young Rand being rescued by monks and taken to K'un-Lun where he trained and eventually took the title of the Iron Fist. Rand returned to New York City to claim back his name and soon fell into conflict against the Hand when he had learned that Madame Gao was using his company to sell her own Heroin. Rand challenged Gao and soon joined forces with his father's ally Harold Meachum and Bakuto. However, Meachum and Bakuto turned against Rand, while intending to use the power of the Iron Fist for their own purposes, forcing Rand to defeat them both."@en .

<http://dbkwik.webdatacommons.org/marvelcinematicuniverse.wikia.com/resource/Iron_Man_Armor:_Mark_II> a <http://dbkwik.webdatacommons.org/marvelcinematicuniverse.wikia.com/class/armor> ;
    rdfs:label "Iron Man Armor: Mark II"^^rdf:langString ;
    ns1:name "Prototype Flight Armor"^^rdf:langString ;
    ns1:precededBy <http://dbkwik.webdatacommons.org/marvelcinematicuniverse.wikia.com/resource/Iron_Man_Armor:_Mark_I> ;
    ns1:succeededBy <http://dbkwik.webdatacommons.org/marvelcinematicuniverse.wikia.com/resource/Iron_Man_Armor:_Mark_III> ;
    rdfs:comment """The Mark II Armor was Tony Stark's second Iron Man suit, heavily refining the bulky and rudimentary design of the previous Mark I suit, resulting in a far more articulated and sleek design.

"""@en .

<http://dbkwik.webdatacommons.org/marvelcinematicuniverse.wikia.com/resource/Iron_Man_Armor:_Mark_III> rdfs:label "Iron Man Armor: Mark III"^^rdf:langString ;
    ns1:precededBy <http://dbkwik.webdatacommons.org/marvelcinematicuniverse.wikia.com/resource/Iron_Man_Armor:_Mark_II> ;
    ns1:succeededBy <http://dbkwik.webdatacommons.org/marvelcinematicuniverse.wikia.com/resource/Iron_Man_Armor:_Mark_IV> ;
    rdfs:comment """The Mark III Armor was Tony Stark's third Iron Man suit and an upgrade from the Mark II, improving on its previous flaws. It was the first suit to integrate an advanced on-board weapons system and was the first to adopt the standard red and gold color scheme.

"""@en .

<http://dbkwik.webdatacommons.org/marvelcinematicuniverse.wikia.com/resource/Jed_Whedon> rdfs:label "Jed Whedon"^^rdf:langString ;
    rdfs:comment """Jed Whedon is co-creator and Executive Producer on Agents of S.H.I.E.L.D.
He co-wrote the Agents of S.H.I.E.L.D. episodes Pilot, 0-8-4, The Asset, Repairs, Seeds, Turn, Turn, Turn, Beginning of the End, Shadows, Aftershocks, S.O.S. Part Two, Laws of Nature, Many Heads, One Tale, The Ghost, The Return, Orientation Part One, The Real Deal, The End and Missing Pieces and wrote the episodes Ascension and Self Control.
He also directed the Agents of S.H.I.E.L.D. episodes Self Control and The End.
He also provided the voice of the Noisemaker in the episode Beginning of the End.
"""@en .

<http://dbkwik.webdatacommons.org/marvelcinematicuniverse.wikia.com/resource/Jeffrey_Bell> rdfs:label "Jeffrey Bell"^^rdf:langString ;
    rdfs:comment """Jeffrey Bell is an Executive Producer on Agents of S.H.I.E.L.D. He was also to be a showrunner of Most Wanted.
He wrote the Agents of S.H.I.E.L.D. episodes 0-8-4, Eye-Spy, T.A.H.I.T.I., Ragtag, What They Become, S.O.S. Part One, Maveth, The Good Samaritan and World's End.
He was interviewed for the documentary Marvel Studios: Assembling a Universe.

"""@en .

<http://dbkwik.webdatacommons.org/marvelcinematicuniverse.wikia.com/resource/Jiaying> rdfs:label "Jiaying"^^rdf:langString ;
    rdfs:comment """Jiaying was an Inhuman gifted with the power of life force absorption after experiencing Terrigenesis. Using her abilitiy, Jiaying retained her youthful appearance for several decades by draining the life from a number of Inhumans who had willingly sacrificed themselves for her. Thanks to this, she used her wisdom and experience to guide a number of Inhumans throughout dozens of generations, helping them to cope with their powers, and in time, harness them. She worked in a clinic in China, alongside her husband, Calvin Johnson, and had a daughter whom they named Daisy. Jiaying was captured and vivisected by the HYDRA leader Werner Reinhardt, who believed he had killed her. In truth, her body was found by her husband, who stitched her back together, allowing her healing powers to work.
"""@en .

<http://dbkwik.webdatacommons.org/marvelcinematicuniverse.wikia.com/resource/Justin_Hammer> rdfs:label "Justin Hammer"^^rdf:langString ;
    rdfs:comment """Justin Hammer is the former CEO of Hammer Industries who had formed a strong rivalry with Stark Industries. Seeking to improve his own position and attack Tony Stark, Hammer worked alongside Senator Stern and attempted to damage the public's own view of Stark, however this backfired and Hammer's own public image was highly damaged. Furious at Stark for this failure, Hammer recruited Ivan Vanko, a convicted terrorist, to attempt to replicate Stark's Arc Reactor technology, but this backfired as well when Vanko betrayed Hammer, leading into Hammer being incarcerated inside Seagate Prison for his involvement in Vanko's actions.

"""@en .

<http://dbkwik.webdatacommons.org/marvelcinematicuniverse.wikia.com/resource/Lighthouse> rdfs:label "Lighthouse"^^rdf:langString ;
    rdfs:comment """The Lighthouse is a massive bunker built in case of an apocalyptic-level event, constructed and equipped by S.H.I.E.L.D. under the command of General Rick Stoner. It is located under Lake Ontario.
In an alternate future, it was located in a chunk of the Earth's crust held together with Gravitonium. It was overruled by the Kree Watch, specifically Kasius and contained a society of subjugated Humans and Inhumans. Because of the Seer's visions, Phil Coulson and his team time-traveled there via the White Monolith and were prophesied to save humanity. Following, the return of Coulson and his fellow Agents from 2091, they began using The Lighthouse as their primary base of operations.

"""@en .

<http://dbkwik.webdatacommons.org/marvelcinematicuniverse.wikia.com/resource/List_of_Minor_Characters> rdfs:label "List of Minor Characters"^^rdf:langString ;
    rdfs:comment """This is a list of minor characters appearing across the Marvel Cinematic Universe.

"""@en .

<http://dbkwik.webdatacommons.org/marvelcinematicuniverse.wikia.com/resource/Patriot> rdfs:label "Patriot"^^rdf:langString ;
    rdfs:comment """Jeffrey Mace was the Director of S.H.I.E.L.D.. Originally working as a journalist for International Affairs, he survived Helmut Zemo's terrorist attack on the Vienna International Centre. After this, he was called upon by the government to partake in an experiment that would give him super strength under Project Patriot. Now a hero in the eyes of the public, he was considered by both Phil Coulson and President Matthew Ellis a perfect person to lead S.H.I.E.L.D. when the organization was to be legitimized again, under the guise of an Inhuman. As S.H.I.E.L.D.'s Director, Mace revealed the agency's continued existence to the world. 
"""@en .

<http://dbkwik.webdatacommons.org/marvelcinematicuniverse.wikia.com/resource/Phil_Coulson> rdfs:label "Phil Coulson"^^rdf:langString ;
    ns1:current <http://dbkwik.webdatacommons.org/marvelcinematicuniverse.wikia.com/resource/Phil_Coulson> ;
    rdfs:comment """Phillip J. "Phil" Coulson is a former Director of S.H.I.E.L.D. Prior to his appointment, he served as one of the organization's best operatives. He acted as former Director Nick Fury's right-hand man for many important missions. He was put in charge of surveillance and served as the primary operative in Fury's Avengers Initiative. Agent Coulson also ran ground interference and tactical operations in Puente Antiguo, New Mexico as part of S.H.I.E.L.D.'s investigation surrounding the incident with Thor and the Destroyer. Coulson was also the primary S.H.I.E.L.D. operative in the investigation into Stark Industries: Sector 16 and the incident on the Howard Stark Memorial Freeway.
"""@en .

<http://dbkwik.webdatacommons.org/marvelcinematicuniverse.wikia.com/resource/Pilot> rdfs:label "Pilot"^^rdf:langString ;
    rdfs:comment """Pilot is the first episode of the first season of Agents of S.H.I.E.L.D. It was shown for the first time at San Diego Comic-Con on July 18, 2013, but officially premiered on September 24, 2013.

"""@en .

<http://dbkwik.webdatacommons.org/marvelcinematicuniverse.wikia.com/resource/Randy_Vale> rdfs:label "Randy Vale"^^rdf:langString ;
    rdfs:comment """Randy Vale is a former salvage worker turned professional criminal and one of the key members of Adrian Toomes' crew who sold alien-human hybrid weaponry created by the Tinkerer.

"""@en .

<http://dbkwik.webdatacommons.org/marvelcinematicuniverse.wikia.com/resource/Runaways_(TV_series)> rdfs:label "Runaways (TV series)"^^rdf:langString ;
    rdfs:comment """Marvel's Runaways, or simply Runaways, is a television series that star the team of the same name. It is produced by Marvel Television and airs on Hulu.
On August 17, 2016, the series was officially ordered by Hulu. The first season premiered on November 21, 2017.
On January 8, 2018, the series was renewed for a second season. It will premiere on December 21, 2018.

"""@en .

<http://dbkwik.webdatacommons.org/marvelcinematicuniverse.wikia.com/resource/SZA> rdfs:label "SZA"^^rdf:langString ;
    rdfs:comment """Solána Imani Rowe, known professionally as SZA, is an American R&B singer and songwriter.
Her collaboration with Kendrick Lamar, "All the Stars", is featured on Black Panther: The Album.

"""@en .

<http://dbkwik.webdatacommons.org/marvelcinematicuniverse.wikia.com/resource/Sovereign_(Planet)> rdfs:label "Sovereign (Planet)"^^rdf:langString ;
    rdfs:comment """The Sovereign is a collective of planets and the home world of the genetically enginereed race of the same name.

"""@en .

<http://dbkwik.webdatacommons.org/marvelcinematicuniverse.wikia.com/resource/Spider-Man> rdfs:label "Spider-Man"^^rdf:langString ;
    rdfs:comment """Peter Benjamin Parker was a high school student and a superhero with spider-like abilities, fighting crime as his alter ego Spider-Man. After receiving his abilities from a spider's bite, Parker chose to protect Queens from crime with his powers, juggling all of his superhero duties and the demands of his high school life. Despite his best efforts to keep his identity secret from the world, he was found and recruited by Tony Stark in the Avengers Civil War, while gaining a new suit and technology in exchange for his help.
"""@en .

<http://dbkwik.webdatacommons.org/marvelcinematicuniverse.wikia.com/resource/T%27Chaka> rdfs:label "T'Chaka"^^rdf:langString ;
    rdfs:comment "T'Chaka was the leader of the Kingdom of Wakanda, assuming the throne and the role of Black Panther in his youth. During his time as the King, part of T'Chaka's supply of Vibranium was stolen by Ulysses Klaue, leading to T'Chaka discovering that it was in fact his own brother N'Jobu who had aided Klaue, forcing T'Chaka to kill him and leave his son behind. T'Chaka then returned home and supported his kingdom, preparing his son T'Challa to take up the throne. Following a battle involving the Avengers, T'Chaka had supported and then signed the Sokovia Accords."@en .

<http://dbkwik.webdatacommons.org/marvelcinematicuniverse.wikia.com/resource/Thor_(film)> rdfs:label "Thor (film)"^^rdf:langString ;
    rdfs:comment """Thor is a 2011 superhero film based on the Marvel Comics superhero by the same name. It is the fourth installment in the Marvel Cinematic Universe and the fourth installment of Phase One.
Though the flashback scenes take place thousands of years prior, the bulk of the film takes place during the events of The Incredible Hulk and Iron Man 2. It is directed by Kenneth Branagh and stars Chris Hemsworth, Natalie Portman, Tom Hiddleston, Idris Elba and Anthony Hopkins as Thor, Jane Foster, Loki, Heimdall and Odin.
"""@en .

<http://dbkwik.webdatacommons.org/marvelcinematicuniverse.wikia.com/resource/WHiH_Newsfront_(web_series)> a <http://dbkwik.webdatacommons.org/marvelcinematicuniverse.wikia.com/class/web_series> ;
    rdfs:label "WHiH Newsfront (web series)"^^rdf:langString ;
    rdfs:comment """WHiH Newsfront is an American web series, based on an online news program with the same name supported by the television network WHiH World News. It airs on Youtube and is part of the promotional campaigns for the movies Ant-Man and Captain America: Civil War. It aired on July 2, 2015 and was renewed in April 22, 2016.

"""@en .

<http://dbkwik.webdatacommons.org/marvelcinematicuniverse.wikia.com/resource/War_on_HYDRA> rdfs:label "War on HYDRA"^^rdf:langString ;
    rdfs:comment "The War on HYDRA was a conflict between the terrorist organization HYDRA and all world governments and security organizations after the revelation of HYDRA's continued existence. At first, HYDRA had the upper hand over S.H.I.E.L.D., because S.H.I.E.L.D. was reduced to only a shadow of its former strength, and the HYDRA leader Daniel Whitehall used that to retrieve the mysterious Obelisk. However, once S.H.I.E.L.D. was redeemed in the eyes of the law, they turned the tables on HYDRA, who lost the battle for the ancient Kree City, and many of its leaders, including Whitehall, in rapid succession. Though Baron von Strucker and Doctor List continued HYDRA's experiments on enhanced people, their efforts were rendered null when their HYDRA cell was destroyed by S.H.I.E.L.D."@en .

<http://dbkwik.webdatacommons.org/marvelcinematicuniverse.wikia.com/resource/Wendell_Rand> rdfs:label "Wendell Rand"^^rdf:langString ;
    ns1:years <http://dbkwik.webdatacommons.org/marvelcinematicuniverse.wikia.com/resource/2000s> ;
    rdfs:comment """Wendell Rand was the CEO of Rand Enterprises and father of Danny Rand.

"""@en .

<http://dbkwik.webdatacommons.org/marvelcinematicuniverse.wikia.com/class/cancelled> a owl:Class ;
    rdfs:label "Cancelled"@en .

<http://dbkwik.webdatacommons.org/marvelcinematicuniverse.wikia.com/class/documentary> a owl:Class ;
    rdfs:label "Documentary"@en .

<http://dbkwik.webdatacommons.org/marvelcinematicuniverse.wikia.com/class/youtube> a owl:Class ;
    rdfs:label "YouTube"@en .

<http://dbkwik.webdatacommons.org/marvelcinematicuniverse.wikia.com/resource/2000s> rdfs:label "2000s"^^rdf:langString ;
    rdfs:comment """This is a timeline of events that occurred during the 2000s.

"""@en .

<http://dbkwik.webdatacommons.org/marvelcinematicuniverse.wikia.com/resource/Ant-Man_and_the_Wasp> a <http://dbkwik.webdatacommons.org/marvelcinematicuniverse.wikia.com/class/movie> ;
    rdfs:label "Ant-Man and the Wasp"^^rdf:langString ;
    ns1:boxoffice "6.215E8"^^<http://dbkwik.webdatacommons.org/datatype/usDollar> ;
    ns1:producer <http://dbkwik.webdatacommons.org/marvelcinematicuniverse.wikia.com/resource/Charles_Newirth> ;
    rdfs:comment """Ant-Man and the Wasp is a 2018 superhero film based on the Marvel Comics superheroes of the same names. It is a sequel to Ant-Man and Captain America: Civil War and the twentieth installment in the Marvel Cinematic Universe, while also being the eighth installment of Phase Three. The movie was released on July 6, 2018.
"""@en .

<http://dbkwik.webdatacommons.org/marvelcinematicuniverse.wikia.com/resource/Avengers:_Infinity_War> a <http://dbkwik.webdatacommons.org/marvelcinematicuniverse.wikia.com/class/movie> ;
    rdfs:label "Avengers: Infinity War"^^rdf:langString ;
    ns1:boxoffice "2.047E9"^^<http://dbkwik.webdatacommons.org/datatype/usDollar> ;
    rdfs:comment """Avengers: Infinity War is a 2018 superhero film, based on the Marvel Comics superhero team of the same name. It is a sequel to The Avengers and Avengers: Age of Ultron and a crossover between/sequel to Captain America: Civil War, Doctor Strange, Guardians of the Galaxy Vol. 2, Spider-Man: Homecoming, Thor: Ragnarok and Black Panther. The film is the nineteenth main installment in the Marvel Cinematic Universe as well as the seventh in Phase Three. The movie was released on April 27, 2018.
"""@en .

<http://dbkwik.webdatacommons.org/marvelcinematicuniverse.wikia.com/resource/Bear_McCreary> rdfs:label "Bear McCreary"^^rdf:langString ;
    rdfs:comment """Bear McCreary scored Agents of S.H.I.E.L.D. and Agents of S.H.I.E.L.D.: Slingshot.

"""@en .

<http://dbkwik.webdatacommons.org/marvelcinematicuniverse.wikia.com/resource/Category:Galleries> rdfs:label "Galleries"^^rdf:langString .

<http://dbkwik.webdatacommons.org/marvelcinematicuniverse.wikia.com/resource/Hand> rdfs:label "Hand"^^rdf:langString ;
    rdfs:comment "The Yami no te (闇の手), referred to as the Hand, was an ancient and powerful ninja clan with the ultimate goal to gain immortality. The Hand originated in K'un-Lun, when the five founders were banished from the city and have since lived on in the shadows for centuries, promoting their goal through wars and influence on powerful people. When the Hand came to New York City, the branch leader Nobu Yoshioka used Wilson Fisk in order to bring to the city Black Sky. However, his plan was interrupted by the vigilante Daredevil, and eventually, they had to stop their operation after Yoshioka's death. By the power of resurrection the Hand had obtained, Yoshioka returned to lead the Hand in New York City in order to find a new Black Sky for their war against the Chaste."@en .

<http://dbkwik.webdatacommons.org/marvelcinematicuniverse.wikia.com/resource/Harold_Meachum> rdfs:label "Harold Meachum"^^rdf:langString ;
    rdfs:comment "Harold Meachum was a ruthless businessman who built up Rand Enterprises with his dear friend Wendell Rand. However Meachum's greed led him to make a deal with Madame Gao to have the Rands murdered, and when he was diagnosed with cancer, he agreed to help the Hand in exchange for his life. Meachum was brought back from the dead and forced to live in hiding, controlling his former company through his own son Ward Meachum. Upon the return of Danny Rand, who was now the Iron Fist, Meachum saw a chance to return to his old life and manipulated Iron Fist into fighting the Hand for him, allowing him to kill Bakuto and have Gao disappear while Meachum returned to New York City and betrayed Rand."@en .

<http://dbkwik.webdatacommons.org/marvelcinematicuniverse.wikia.com/resource/Jackson_Brice> rdfs:label "Jackson Brice"^^rdf:langString ;
    rdfs:comment """Jackson Brice was a member of Adrian Toomes' criminal group who used modified weaponry, including a gauntlet, to showcase and sell alien-human hybrid weaponry under the alias of Shocker. Having jeopardized the group by recklessly and repeatedly firing an Ultron Blaster Gun publicly and threatening to expose Toomes' criminal lifestyle, he was killed by Toomes in retaliation.

"""@en .

<http://dbkwik.webdatacommons.org/marvelcinematicuniverse.wikia.com/resource/Marvel_One-Shot:_All_Hail_the_King> a <http://dbkwik.webdatacommons.org/marvelcinematicuniverse.wikia.com/class/one-shot> ;
    rdfs:label "Marvel One-Shot: All Hail the King"^^rdf:langString ;
    rdfs:comment """All Hail the King is the fifth Marvel One-Shot and was released on the Thor: The Dark World Blu-ray. It takes place after the events of Iron Man 3.

"""@en .

<http://dbkwik.webdatacommons.org/marvelcinematicuniverse.wikia.com/resource/New_York_City> rdfs:label "New York City"^^rdf:langString ;
    rdfs:comment """New York City is the largest city in the state of New York and the city with the largest metropolitan area in the United States of America.

"""@en .

<http://dbkwik.webdatacommons.org/marvelcinematicuniverse.wikia.com/resource/S.H.I.E.L.D.> rdfs:label "S.H.I.E.L.D."^^rdf:langString ;
    rdfs:comment "The Strategic Homeland Intervention, Enforcement and Logistics Division, better known by its acronym S.H.I.E.L.D., is an American extra-governmental military counter-terrorism and intelligence agency, tasked with maintaining both national and global security. Founded in the wake of the Allied victory over the Axis powers and HYDRA in World War II, S.H.I.E.L.D. was organized to protect the United States from all possible threats. With its advanced weapons and extraordinary agents, S.H.I.E.L.D. was maybe the greatest military power on Earth. Run by Nick Fury and the World Security Council in the modern age, S.H.I.E.L.D. had to deal with the significant rise in enhanced individuals, dangerous advanced technology, and alien contact. But all the problems S.H.I.E.L.D."@en .

<http://dbkwik.webdatacommons.org/marvelcinematicuniverse.wikia.com/class/clear> a owl:Class ;
    rdfs:label "Clear"@en .

<http://dbkwik.webdatacommons.org/marvelcinematicuniverse.wikia.com/class/game> a owl:Class ;
    rdfs:label "Game"@en .

<http://dbkwik.webdatacommons.org/marvelcinematicuniverse.wikia.com/class/stub> a owl:Class ;
    rdfs:label "Stub"@en .

<http://dbkwik.webdatacommons.org/marvelcinematicuniverse.wikia.com/resource/Daredevil> rdfs:label "Daredevil"^^rdf:langString ;
    rdfs:comment """Matthew Michael "Matt" Murdock is a man who was blinded as a young boy by a radioactive substance that fell from a crashed vehicle, and even though he lost his sight, his other four senses were heightened to a superhuman level. After his father was murdered by mobsters, Murdock dedicated his life to fight injustice in New York City as a lawyer by day with his law firm Nelson and Murdock, and by night as a vigilante known as Daredevil. His actions as a crime fighter put Murdock into conflict with a crime lord named Wilson Fisk. Murdock used his skills to expose Fisk's criminal activities and have him taken to prison.
"""@en .

<http://dbkwik.webdatacommons.org/marvelcinematicuniverse.wikia.com/resource/Hulk> rdfs:label "Hulk"^^rdf:langString ;
    rdfs:comment """Robert Bruce Banner, M.D., Ph.D. is a renowned scientist who was highly respected for all his work in the fields of Biochemistry, Nuclear Physics, and Gamma Radiation. As part of a program commissioned by General Thaddeus Ross to recreate the Super Soldier Serum which created Captain America, Banner conducted an experiment with Gamma Radiation. However, when an exposure to high levels of Gamma Radiation instead of Vita Radiation went awry, the mild-mannered scientist had found that when angered or provoked, he would transform into the huge, rage-fueled, nearly mindless and green-skinned monster known as Hulk.
"""@en .

<http://dbkwik.webdatacommons.org/marvelcinematicuniverse.wikia.com/resource/Humans> rdfs:label "Humans"^^rdf:langString ;
    rdfs:comment """Humans (Homo sapiens) are the intelligent inhabitants of Earth. The races of the Nine Realms refer to Humans as Mortals, while the various alien cultures living beyond the realms use the term Terrans. Their population used to consist of 7.5 billion inhabitants but after Thanos snapped half of the universe away their population decreased to about 3.75 billion.

"""@en .

<http://dbkwik.webdatacommons.org/marvelcinematicuniverse.wikia.com/resource/Iron_Man_2_(video_game)> rdfs:label "Iron Man 2 (video game)"^^rdf:langString ;
    ns1:developers "', '"^^rdf:langString ;
    rdfs:comment """Iron Man 2 is a 2010 video game loosely based on the film of the same name. It was released on May 4, 2010, days after the film's international release and days before the film's domestic release. The game was published by Sega and developed by Secret Level (Xbox 360 & PlayStation 3), High Voltage Software (Wii & PlayStation Portable) and Gameloft (Wireless).
"""@en .

<http://dbkwik.webdatacommons.org/marvelcinematicuniverse.wikia.com/resource/Kendrick_Lamar> rdfs:label "Kendrick Lamar"^^rdf:langString ;
    rdfs:comment """Kendrick Lamar Duckworth, professionally known as Kendrick Lamar, is an American hip hop recording artist.
He produced Black Panther: The Album with Top Dawg and featured on the songs "Black Panther", "All the Stars", "King's Dead", "Big Shot" and "Pray for Me".
His song "Backseat Freestyle" is featured in the Jessica Jones episode AKA You're a Winner!.

"""@en .

<http://dbkwik.webdatacommons.org/marvelcinematicuniverse.wikia.com/resource/Luke_Cage_(TV_series)> rdfs:label "Luke Cage (TV series)"^^rdf:langString ;
    rdfs:comment """Marvel's Luke Cage, or simply Luke Cage, is a television series that stars the superhero character of the same name.
The first season premiered on September 30, 2016.
The second season premiered on June 22, 2018.

"""@en .

<http://dbkwik.webdatacommons.org/marvelcinematicuniverse.wikia.com/resource/Marvel_Studios:_Assembling_a_Universe> a <http://dbkwik.webdatacommons.org/marvelcinematicuniverse.wikia.com/class/documentary> ;
    rdfs:label "Marvel Studios: Assembling a Universe"^^rdf:langString ;
    rdfs:comment """Marvel Studios: Assembling a Universe is a one-hour special documentary that aired on ABC on March 18, 2014. The documentary showed exclusive looks at all the previous films and one-shots as well as sneak peeks of Captain America: The Winter Soldier, Guardians of the Galaxy, Avengers: Age of Ultron and future episodes of Agents of S.H.I.E.L.D..

"""@en .

<http://dbkwik.webdatacommons.org/marvelcinematicuniverse.wikia.com/resource/Mike_del_Mundo> rdfs:label "Mike del Mundo"^^rdf:langString ;
    rdfs:comment "Mike del Munro was an artist for Guidebook to the Marvel Cinematic Universe - Iron Man, Guidebook to the Marvel Cinematic Universe - The Incredible Hulk, Guidebook to the Marvel Cinematic Universe - Iron Man 2, Guidebook to the Marvel Cinematic Universe - Captain America: The First Avenger, Guidebook to the Marvel Cinematic Universe - The Avengers, Guidebook to the Marvel Cinematic Universe - Captain America: The Winter Soldier, Guidebook to the Marvel Cinematic Universe - Ant-Man, Guidebook to the Marvel Cinematic Universe - Marvel's Agents of S.H.I.E.L.D. Season One, Guidebook to the Marvel Cinematic Universe - Guardians of the Galaxy, Guidebook to the Marvel Cinematic Universe - Avengers: Age of Ultron, Guidebook to the Marvel Cinematic Universe - Marvel's Agents of S.H.I.E.L.D."@en .

<http://dbkwik.webdatacommons.org/marvelcinematicuniverse.wikia.com/resource/Troy_Benjamin> rdfs:label "Troy Benjamin"^^rdf:langString ;
    rdfs:comment "Troy Benjamin wrote Agents of S.H.I.E.L.D.: Season One Declassified, Agents of S.H.I.E.L.D.: Season Two Declassified, and Guidebook to the Marvel Cinematic Universe."@en .

<http://dbkwik.webdatacommons.org/marvelcinematicuniverse.wikia.com/resource/United_States_of_America> rdfs:label "United States of America"^^rdf:langString ;
    rdfs:comment """The United States of America, commonly referred to as the United States, America or simply the States, is a federal nation consisting of 50 American states.

"""@en .

<http://dbkwik.webdatacommons.org/marvelcinematicuniverse.wikia.com/resource/Will_Corona_Pilgrim> rdfs:label "Will Corona Pilgrim"^^rdf:langString ;
    rdfs:comment """Will Corona Pilgrim is the Creative Research Manager for Marvel Studios.
He co-wrote the comics Iron Man 3 Prelude, The Avengers Adaptation, Guardians of the Galaxy: Galaxy's Most Wanted, Avengers: Age of Ultron Prelude, Avengers: Operation HYDRA, Avengers: Age of Ultron Prelude - This Scepter'd Isle, Ant-Man Prelude, Ant-Man - Scott Lang: Small Time, Ant-Man: Larger Than Life, Captain America: Civil War Prelude, Doctor Strange Prelude, Guardians of the Galaxy Vol. 2 Prelude, Spider-Man: Homecoming Prelude, Thor: Ragnarok Prelude, Black Panther Prelude, Avengers: Infinity War Prelude and Ant-Man and the Wasp Prelude.

"""@en .

<http://dbkwik.webdatacommons.org/marvelcinematicuniverse.wikia.com/class/actor> a owl:Class ;
    rdfs:label "Actor"@en .

<http://dbkwik.webdatacommons.org/marvelcinematicuniverse.wikia.com/class/armor> a owl:Class ;
    rdfs:label "Armor"@en .

<http://dbkwik.webdatacommons.org/marvelcinematicuniverse.wikia.com/class/book> a owl:Class ;
    rdfs:label "Book"@en .

<http://dbkwik.webdatacommons.org/marvelcinematicuniverse.wikia.com/class/box> a owl:Class ;
    rdfs:label "Box"@en .

<http://dbkwik.webdatacommons.org/marvelcinematicuniverse.wikia.com/class/character> a owl:Class ;
    rdfs:label "Character"@en .

<http://dbkwik.webdatacommons.org/marvelcinematicuniverse.wikia.com/class/comic> a owl:Class ;
    rdfs:label "Comic"@en .

<http://dbkwik.webdatacommons.org/marvelcinematicuniverse.wikia.com/class/conflict> a owl:Class ;
    rdfs:label "Conflict"@en .

<http://dbkwik.webdatacommons.org/marvelcinematicuniverse.wikia.com/class/disambig> a owl:Class ;
    rdfs:label "Disambig"@en .

<http://dbkwik.webdatacommons.org/marvelcinematicuniverse.wikia.com/class/dvd> a owl:Class ;
    rdfs:label "DVD"@en .

<http://dbkwik.webdatacommons.org/marvelcinematicuniverse.wikia.com/class/episode> a owl:Class ;
    rdfs:label "Episode"@en .

<http://dbkwik.webdatacommons.org/marvelcinematicuniverse.wikia.com/class/event> a owl:Class ;
    rdfs:label "Event"@en .

<http://dbkwik.webdatacommons.org/marvelcinematicuniverse.wikia.com/class/filmmaker> a owl:Class ;
    rdfs:label "Filmmaker"@en .

<http://dbkwik.webdatacommons.org/marvelcinematicuniverse.wikia.com/class/google+> a owl:Class ;
    rdfs:label "Google+"@en .

<http://dbkwik.webdatacommons.org/marvelcinematicuniverse.wikia.com/class/guidebook> a owl:Class ;
    rdfs:label "Guidebook"@en .

<http://dbkwik.webdatacommons.org/marvelcinematicuniverse.wikia.com/class/imdb> a owl:Class ;
    rdfs:label "IMDb"@en .

<http://dbkwik.webdatacommons.org/marvelcinematicuniverse.wikia.com/class/item> a owl:Class ;
    rdfs:label "Item"@en .

<http://dbkwik.webdatacommons.org/marvelcinematicuniverse.wikia.com/class/linkedin> a owl:Class ;
    rdfs:label "Linkedin"@en .

<http://dbkwik.webdatacommons.org/marvelcinematicuniverse.wikia.com/class/location> a owl:Class ;
    rdfs:label "Location"@en .

<http://dbkwik.webdatacommons.org/marvelcinematicuniverse.wikia.com/class/marvel> a owl:Class ;
    rdfs:label "Marvel"@en .

<http://dbkwik.webdatacommons.org/marvelcinematicuniverse.wikia.com/class/movie> a owl:Class ;
    rdfs:label "Movie"@en .

<http://dbkwik.webdatacommons.org/marvelcinematicuniverse.wikia.com/class/music> a owl:Class ;
    rdfs:label "Music"@en .

<http://dbkwik.webdatacommons.org/marvelcinematicuniverse.wikia.com/class/one-shot> a owl:Class ;
    rdfs:label "One-Shot"@en .

<http://dbkwik.webdatacommons.org/marvelcinematicuniverse.wikia.com/class/organization> a owl:Class ;
    rdfs:label "Organization"@en .

<http://dbkwik.webdatacommons.org/marvelcinematicuniverse.wikia.com/class/project> a owl:Class ;
    rdfs:label "Project"@en .

<http://dbkwik.webdatacommons.org/marvelcinematicuniverse.wikia.com/class/quote> a owl:Class ;
    rdfs:label "Quote"@en .

<http://dbkwik.webdatacommons.org/marvelcinematicuniverse.wikia.com/class/race> a owl:Class ;
    rdfs:label "Race"@en .

<http://dbkwik.webdatacommons.org/marvelcinematicuniverse.wikia.com/class/reflist> a owl:Class ;
    rdfs:label "Reflist"@en .

<http://dbkwik.webdatacommons.org/marvelcinematicuniverse.wikia.com/class/season> a owl:Class ;
    rdfs:label "Season"@en .

<http://dbkwik.webdatacommons.org/marvelcinematicuniverse.wikia.com/class/song> a owl:Class ;
    rdfs:label "Song"@en .

<http://dbkwik.webdatacommons.org/marvelcinematicuniverse.wikia.com/class/soundtrack> a owl:Class ;
    rdfs:label "Soundtrack"@en .

<http://dbkwik.webdatacommons.org/marvelcinematicuniverse.wikia.com/class/tv> a owl:Class ;
    rdfs:label "TV"@en .

<http://dbkwik.webdatacommons.org/marvelcinematicuniverse.wikia.com/class/vehicle> a owl:Class ;
    rdfs:label "Vehicle"@en .

<http://dbkwik.webdatacommons.org/marvelcinematicuniverse.wikia.com/class/war> a owl:Class ;
    rdfs:label "War"@en .

<http://dbkwik.webdatacommons.org/marvelcinematicuniverse.wikia.com/class/web_series> a owl:Class ;
    rdfs:label "Web Series"@en .

<http://dbkwik.webdatacommons.org/marvelcinematicuniverse.wikia.com/class/wp> a owl:Class ;
    rdfs:label "WP"@en .

<http://dbkwik.webdatacommons.org/marvelcinematicuniverse.wikia.com/class/wps> a owl:Class ;
    rdfs:label "WPS"@en .

<http://dbkwik.webdatacommons.org/marvelcinematicuniverse.wikia.com/resource/Agent_Carter_(TV_series)> a <http://dbkwik.webdatacommons.org/marvelcinematicuniverse.wikia.com/class/tv> ;
    rdfs:label "Agent Carter (TV series)"^^rdf:langString ;
    ns1:channel <http://dbkwik.webdatacommons.org/marvelcinematicuniverse.wikia.com/resource/American_Broadcasting_Company> ;
    ns1:composer <http://dbkwik.webdatacommons.org/marvelcinematicuniverse.wikia.com/resource/Christopher_Lennertz> ;
    ns1:dates "--01-06"^^xsd:gMonthDay ;
    ns1:first <http://dbkwik.webdatacommons.org/marvelcinematicuniverse.wikia.com/resource/Now_is_Not_the_End> ;
    ns1:last <http://dbkwik.webdatacommons.org/marvelcinematicuniverse.wikia.com/resource/Hollywood_Ending> ;
    ns1:prev <http://dbkwik.webdatacommons.org/marvelcinematicuniverse.wikia.com/resource/Agents_of_S.H.I.E.L.D.> ;
    ns1:showrunners <http://dbkwik.webdatacommons.org/marvelcinematicuniverse.wikia.com/resource/Chris_Dingess>,
        <http://dbkwik.webdatacommons.org/marvelcinematicuniverse.wikia.com/resource/Michele_Fazekas> ;
    rdfs:comment "Agent Carter was an American television series based on Marvel Comics character Peggy Carter. It was produced by Marvel Television and aired on the ABC network, and has been set in the Marvel Cinematic Universe. It occurs after the events of Captain America: The First Avenger and before Marvel One-Shot: Agent Carter with Hayley Atwell reprising her role as Carter. Reaper creators Tara Butters and Michele Fazekas will be writing and executive producing the show as well as serving as the showrunners for the series. On May 8, 2014 Marvel Entertainment announced that ABC has picked up Agent Carter to series. The series premiered in January 2015. On May 15, 2014, Hayley Atwell stated that the show would run for 8 episodes."@en .

<http://dbkwik.webdatacommons.org/marvelcinematicuniverse.wikia.com/resource/Agents_of_S.H.I.E.L.D.> a <http://dbkwik.webdatacommons.org/marvelcinematicuniverse.wikia.com/class/tv> ;
    rdfs:label "Agents of S.H.I.E.L.D."^^rdf:langString ;
    ns1:channel <http://dbkwik.webdatacommons.org/marvelcinematicuniverse.wikia.com/resource/American_Broadcasting_Company> ;
    ns1:composer <http://dbkwik.webdatacommons.org/marvelcinematicuniverse.wikia.com/resource/Bear_McCreary> ;
    ns1:dates "--09-24"^^xsd:gMonthDay ;
    ns1:first <http://dbkwik.webdatacommons.org/marvelcinematicuniverse.wikia.com/resource/Pilot> ;
    ns1:showrunners <http://dbkwik.webdatacommons.org/marvelcinematicuniverse.wikia.com/resource/Jed_Whedon>,
        <http://dbkwik.webdatacommons.org/marvelcinematicuniverse.wikia.com/resource/Jeffrey_Bell> ;
    rdfs:comment """Agents of S.H.I.E.L.D. is an American television series, based on the famous Marvel Comics organization. It is produced by Marvel Television and airs on the ABC network, and is set in the Marvel Cinematic Universe, sharing continuity with the films in that franchise. The pilot, which was written by Joss Whedon, Jed Whedon, and Maurissa Tancharoen and directed by Joss Whedon, reached an audience of almost 12 million viewers.
"""@en .

<http://dbkwik.webdatacommons.org/marvelcinematicuniverse.wikia.com/resource/Aldrich_Killian> rdfs:label "Aldrich Killian"^^rdf:langString ;
    ns1:oneshot <http://dbkwik.webdatacommons.org/marvelcinematicuniverse.wikia.com/resource/Marvel_One-Shot:_All_Hail_the_King> ;
    rdfs:comment "Aldrich Killian was the founder and chief executive officer of Advanced Idea Mechanics. When Tony Stark refused to join him in his research, Killian participated in the development of Extremis thereby amassing a group of Extremis-enhanced soldiers under his command. To mask his illegal activities as a terrorist attacks he created the idealized terrorist persona known as the \"Mandarin\" portrayed by the British actor Trevor Slattery to serve as his proxy, unaware that the Mandarin truly existed. He also conspired with Vice President Rodriguez in an attempt to take control over both the United States of America and the War on Terror, manipulating them for his own profit."@en .

<http://dbkwik.webdatacommons.org/marvelcinematicuniverse.wikia.com/resource/American_Broadcasting_Company> a <http://dbkwik.webdatacommons.org/marvelcinematicuniverse.wikia.com/class/linkedin> ;
    rdfs:label "American Broadcasting Company"^^rdf:langString ;
    rdfs:comment """The American Broadcasting Company (ABC) is an American commercial broadcast television network viewed in the United States and Canada. It is a sister channel of Freeform.
It has aired the first, second, third, fourth and fifth seasons of Agents of S.H.I.E.L.D., the first and second seasons of the series Agent Carter and the series Inhumans, which is co-produced with the IMAX Corporation.

"""@en .

<http://dbkwik.webdatacommons.org/marvelcinematicuniverse.wikia.com/resource/Axel_Alonso> rdfs:label "Axel Alonso"^^rdf:langString ;
    rdfs:comment """Axel Alonso is the editor-in-chief of Marvel Comics.
He was interviewed for the documentaries Marvel Studios: Assembling a Universe, Marvel 75 Years: From Pulp to Pop and Captain America: 75 Heroic Years.

"""@en .

<http://dbkwik.webdatacommons.org/marvelcinematicuniverse.wikia.com/resource/Before_20th_Century> rdfs:label "Before 20th Century"^^rdf:langString ;
    ns1:before <http://dbkwik.webdatacommons.org/marvelcinematicuniverse.wikia.com/resource/Timeline> ;
    ns1:current <http://dbkwik.webdatacommons.org/marvelcinematicuniverse.wikia.com/resource/Before_20th_Century> ;
    rdfs:comment """This is a timeline of events that occurred before the 20th century.

"""@en .

<http://dbkwik.webdatacommons.org/marvelcinematicuniverse.wikia.com/resource/Clearance_Level> rdfs:label "Clearance Level"^^rdf:langString ;
    rdfs:comment """Clearance Levels were used by S.H.I.E.L.D. to keep order in their system and protect information that is protected by S.H.I.E.L.D.

"""@en .

<http://dbkwik.webdatacommons.org/marvelcinematicuniverse.wikia.com/resource/Iron_Man_(film)> rdfs:label "Iron Man (film)"^^rdf:langString ;
    rdfs:comment """Iron Man is a 2008 superhero film, based on the Marvel Comics superhero of the same name. It is the first installment in the Marvel Cinematic Universe and the first installment of Phase One.
It was directed by Jon Favreau and stars Robert Downey, Jr. as Tony Stark, Terrence Howard as Lt. Colonel James "Rhodey" Rhodes, Gwyneth Paltrow as Pepper Potts and Jeff Bridges as Obadiah Stane. The film spawned two sequels: Iron Man 2 in 2010 and Iron Man 3 in 2013.

"""@en .

<http://dbkwik.webdatacommons.org/marvelcinematicuniverse.wikia.com/resource/New_York> rdfs:label "New York"^^rdf:langString ;
    rdfs:comment """New York is a state located in the northeastern and mid-Atlantic regions of the United States of America.

"""@en .

<http://dbkwik.webdatacommons.org/marvelcinematicuniverse.wikia.com/resource/North_America> rdfs:label "North America"^^rdf:langString ;
    rdfs:comment """North America is one of the seven continents. United States of America is located in North America.

"""@en .

<http://dbkwik.webdatacommons.org/marvelcinematicuniverse.wikia.com/resource/2016> rdfs:label "2016"^^rdf:langString ;
    rdfs:comment """This is a timeline of events that occurred in 2016.

"""@en .

<http://dbkwik.webdatacommons.org/marvelcinematicuniverse.wikia.com/resource/A.I.M.> a <http://dbkwik.webdatacommons.org/marvelcinematicuniverse.wikia.com/class/organization> ;
    rdfs:label "A.I.M."^^rdf:langString ;
    ns1:comic <http://dbkwik.webdatacommons.org/marvelcinematicuniverse.wikia.com/resource/Captain_America:_Civil_War_Prelude>,
        <http://dbkwik.webdatacommons.org/marvelcinematicuniverse.wikia.com/resource/Iron_Man:_The_Price_of_Doing_Business> ;
    ns1:formerleaders <http://dbkwik.webdatacommons.org/marvelcinematicuniverse.wikia.com/resource/Aldrich_Killian> ;
    ns1:formermembers <http://dbkwik.webdatacommons.org/marvelcinematicuniverse.wikia.com/resource/Ellen_Brandt>,
        <http://dbkwik.webdatacommons.org/marvelcinematicuniverse.wikia.com/resource/Eric_Savin> ;
    ns1:founder <http://dbkwik.webdatacommons.org/marvelcinematicuniverse.wikia.com/resource/Aldrich_Killian> ;
    ns1:game <http://dbkwik.webdatacommons.org/marvelcinematicuniverse.wikia.com/resource/Iron_Man_(video_game)>,
        <http://dbkwik.webdatacommons.org/marvelcinematicuniverse.wikia.com/resource/Iron_Man_2_(video_game)> ;
    ns1:members <http://dbkwik.webdatacommons.org/marvelcinematicuniverse.wikia.com/resource/Rodriguez>,
        <http://dbkwik.webdatacommons.org/marvelcinematicuniverse.wikia.com/resource/Trevor_Slattery> ;
    ns1:movie <http://dbkwik.webdatacommons.org/marvelcinematicuniverse.wikia.com/resource/Iron_Man_3> ;
    rdfs:comment """Advanced Idea Mechanics, better known by its acronym A.I.M., was a scientific research and development agency founded by Aldrich Killian and funded by the United States government. 

"""@en .

<http://dbkwik.webdatacommons.org/marvelcinematicuniverse.wikia.com/resource/Iron_Man> rdfs:label "Iron Man"^^rdf:langString ;
    rdfs:comment """Anthony Edward "Tony" Stark is a genius, billionaire, philanthropist and the former head of Stark Industries. Using his own great wealth and exceptional technical knowledge, Stark enjoyed the playboy lifestyle for many years until he was kidnapped by the Ten Rings. With his life on the line, Stark created an armored suit which he used to escape his captors, returning home and becoming the superhero known as Iron Man, battling against terrorists as well as his former business partner Obadiah Stane. Stark enjoyed the fame that came with his new secret identity and decided to share it with the world, publicly announcing himself as Iron Man.
"""@en .

<http://dbkwik.webdatacommons.org/marvelcinematicuniverse.wikia.com/class/timeline> a owl:Class ;
    rdfs:label "Timeline"@en .

<http://dbkwik.webdatacommons.org/marvelcinematicuniverse.wikia.com/resource/2017> rdfs:label "2017"^^rdf:langString ;
    rdfs:comment """This is a timeline of events that occurred in 2017.

"""@en .

